<?xml version="1.0" encoding="UTF-8"?>
<rdf:RDF
	xmlns:rdf="http://www.w3.org/1999/02/22-rdf-syntax-ns#"
	xmlns:rdfs="http://www.w3.org/2000/01/rdf-schema#"
	xmlns:skos="http://www.w3.org/2004/02/skos/core#"
	xmlns:skosxl="http://www.w3.org/2008/05/skos-xl#"
	xmlns:owl="http://www.w3.org/2002/07/owl#"
	xmlns:dc="http://purl.org/dc/elements/1.1/"
	xmlns:dcterms="http://purl.org/dc/terms/"
	xmlns:csw="http://semantic-web.at/ontologies/csw.owl#"
	xmlns:ctag="http://commontag.org/ns#"
	xmlns:opencyc="http://sw.opencyc.org/concept/"
	xmlns:freebase="http://rdf.freebase.com/ns/"
	xmlns:xsd="http://www.w3.org/2001/XMLSchema#"
	xmlns:tags="http://www.holygoat.co.uk/owl/redwood/0.1/tags/"
	xmlns:foaf="http://xmlns.com/foaf/0.1/"
	xmlns:cyc="http://sw.cyc.com/concept/"
	xmlns:cycAnnot="http://sw.cyc.com/CycAnnotations_v1#"
	xmlns:dbpedia="http://dbpedia.org/resource/">

<rdf:Description rdf:about="https://resource.geosphere.at/thes/lith/2">
	<skos:narrower rdf:resource="https://resource.geosphere.at/thes/lith/3"/>
	<skos:prefLabel xml:lang="en">Pyroclastics</skos:prefLabel>
	<dcterms:created rdf:datatype="http://www.w3.org/2001/XMLSchema#dateTime">2012-03-12T16:42:56.000Z</dcterms:created>
	<skos:definition xml:lang="en">Pyroclastics are formed by fragmentation as a result of explosive volcanic eruptions or processes. Pyroclastic deposits are assemblages, either unconsolidated or consolidated, that contain &gt;75% vol. of pyroclasts (Le Maitre et al., 2005).</skos:definition>
	<dcterms:references rdf:resource="https://resource.geosphere.at/thes/citation/477"/>
	<skos:scopeNote xml:lang="en">The classification of pyroclastics is purely descriptive and based on the average pyroclast size.</skos:scopeNote>
	<colourHexCode xmlns="http://dbpedia.org/ontology/">#A64DBF</colourHexCode>
</rdf:Description>

<rdf:Description rdf:about="https://resource.geosphere.at/thes/lith/1">
	<dcterms:date rdf:datatype="http://www.w3.org/2001/XMLSchema#dateTime">2011-03-15T15:22:10Z</dcterms:date>
	<dcterms:hasVersion rdf:datatype="http://www.w3.org/2001/XMLSchema#int">16</dcterms:hasVersion>
	<rdf:type rdf:resource="http://www.w3.org/2004/02/skos/core#Concept"/>
	<skos:prefLabel xml:lang="en">Igneous material</skos:prefLabel>
	<dcterms:references rdf:resource="https://resource.geosphere.at/thes/citation/545"/>
	<skos:exactMatch rdf:resource="http://resource.geosciml.org/classifier/cgi/lithology/igneous_material"/>
	<colourHexCode xmlns="http://dbpedia.org/ontology/">#9900D9</colourHexCode>
	<dcterms:created rdf:datatype="http://www.w3.org/2001/XMLSchema#dateTime">2012-03-12T13:50:38.000Z</dcterms:created>
	<skos:definition xml:lang="de">Natürlich vorkommendes (un-)verfestigtes Material, welches aus (teilweise) geschmolzenem Material (Magma) oder als Resultat eines magmatischen Prozesses wie Intrusion und Abkühlung von Magma oder einer vulkanischen Eruption entsteht (Neuendorf et al., 2005).</skos:definition>
	<skos:exactMatch rdf:resource="http://inspire.ec.europa.eu/codelist/LithologyValue/igneousMaterial"/>
	<skos:prefLabel xml:lang="de">Magmatisches Material</skos:prefLabel>
	<skos:narrower rdf:resource="https://resource.geosphere.at/thes/lith/2"/>
	<skos:definition xml:lang="en">A naturally-occurring solidified or unsolidified material formed from molten or partially molten material (magma) as the result of an igneous process such as intrusion and cooling of magma, or volcanic eruption (Neuendorf et al., 2005).</skos:definition>
</rdf:Description>

<rdf:Description rdf:about="https://resource.geosphere.at/thes/lith/6">
	<skos:exactMatch rdf:resource="http://www.wikidata.org/entity/Q108689"/>
	<dcterms:references rdf:resource="https://resource.geosphere.at/thes/citation/477"/>
	<skos:related rdf:resource="https://resource.geosphere.at/thes/lith/5"/>
	<rdf:type rdf:resource="http://www.w3.org/2004/02/skos/core#Concept"/>
	<dcterms:date rdf:datatype="http://www.w3.org/2001/XMLSchema#dateTime">2011-03-15T15:22:10Z</dcterms:date>
	<skos:broadMatch rdf:resource="http://inspire.ec.europa.eu/codelist/LithologyValue/igneousRock"/>
	<skos:narrower rdf:resource="https://resource.geosphere.at/thes/lith/254"/>
	<skos:exactMatch rdf:resource="http://resource.geosciml.org/classifier/cgi/lithology/fine_grained_igneous_rock"/>
	<skos:exactMatch rdf:resource="http://dbpedia.org/resource/Volcanic_rock"/>
	<dcterms:created rdf:datatype="http://www.w3.org/2001/XMLSchema#dateTime">2012-03-12T16:37:14.000Z</dcterms:created>
	<skos:narrower rdf:resource="https://resource.geosphere.at/thes/lith/96"/>
	<skos:definition xml:lang="en">An igneous rock that can be associated with volcanism and has a relatively fine-grained texture in which most of the individual crystals can not be seen with the unaided eye. The term also includes subvolcanic (hypabyssal) rocks (Le Maitre et al., 2005).</skos:definition>
	<skos:narrower rdf:resource="https://resource.geosphere.at/thes/lith/69"/>
	<skos:narrower rdf:resource="https://resource.geosphere.at/thes/lith/66"/>
	<skos:narrower rdf:resource="https://resource.geosphere.at/thes/lith/67"/>
	<skos:narrower rdf:resource="https://resource.geosphere.at/thes/lith/68"/>
	<skos:narrower rdf:resource="https://resource.geosphere.at/thes/lith/64"/>
	<skos:narrower rdf:resource="https://resource.geosphere.at/thes/lith/65"/>
	<skos:narrower rdf:resource="https://resource.geosphere.at/thes/lith/62"/>
	<skos:narrower rdf:resource="https://resource.geosphere.at/thes/lith/63"/>
	<dcterms:hasVersion rdf:datatype="http://www.w3.org/2001/XMLSchema#int">6</dcterms:hasVersion>
	<skos:definition xml:lang="de">Magmatisches Gestein, welches mit Vulkanismus assoziiert ist und eine sehr feinkörnige Textur besitzt. Die meisten Kristallindividuen sind mit freiem Auge nicht sichtbar. Das Konzept beinhaltet auch subvulkanische Gesteine (Le Maitre et al., 2005).</skos:definition>
	<colourHexCode xmlns="http://dbpedia.org/ontology/">#B300CC</colourHexCode>
</rdf:Description>

<rdf:Description rdf:about="https://resource.geosphere.at/thes/lith/68">
	<dcterms:date rdf:datatype="http://www.w3.org/2001/XMLSchema#dateTime">2011-03-15T15:22:10Z</dcterms:date>
	<dcterms:references rdf:resource="https://resource.geosphere.at/thes/citation/477"/>
	<dcterms:created rdf:datatype="http://www.w3.org/2001/XMLSchema#dateTime">2012-03-12T16:30:47.000Z</dcterms:created>
	<dcterms:references rdf:resource="https://resource.geosphere.at/thes/citation/802"/>
	<skos:exactMatch rdf:resource="http://resource.geosciml.org/classifier/cgi/lithology/tephritoid"/>
	<skos:prefLabel xml:lang="en">Tephritic rock</skos:prefLabel>
	<skos:exactMatch rdf:resource="http://inspire.ec.europa.eu/codelist/LithologyValue/tephritoid"/>
	<skos:definition xml:lang="de">Gestein, welches der QAPF-Gelände-Klassifikation für vulkanische Gesteine entspricht (Streckeisen, 1978) und als Tephrit identifiziert wurde. Modal definiert in QAPF-Feldern 13-14 (Le Maitre et al., 2005).</skos:definition>
	<skos:altLabel xml:lang="de">Tephritoid</skos:altLabel>
	<skos:altLabel xml:lang="en">Tephritoid</skos:altLabel>
	<skos:prefLabel xml:lang="de">Tephritisches Gestein</skos:prefLabel>
	<dcterms:hasVersion rdf:datatype="http://www.w3.org/2001/XMLSchema#int">10</dcterms:hasVersion>
	<colourHexCode xmlns="http://dbpedia.org/ontology/">#7359F2</colourHexCode>
	<skos:definition xml:lang="en">A rock that corresponds to the QAPF 'field' classification for volcanic rocks (Streckeisen 1978) identified as tephrite. QAPF-fields 13-14 (Le Maitre et al., 2005).</skos:definition>
	<rdf:type rdf:resource="http://www.w3.org/2004/02/skos/core#Concept"/>
	<skos:narrower rdf:resource="https://resource.geosphere.at/thes/lith/88"/>
	<skos:narrower rdf:resource="https://resource.geosphere.at/thes/lith/89"/>
	<skos:narrower rdf:resource="https://resource.geosphere.at/thes/lith/86"/>
	<skos:narrower rdf:resource="https://resource.geosphere.at/thes/lith/87"/>
</rdf:Description>

<rdf:Description rdf:about="https://resource.geosphere.at/thes/lith/88">
	<skos:exactMatch rdf:resource="http://inspire.ec.europa.eu/codelist/LithologyValue/basanite"/>
	<skos:prefLabel xml:lang="en">Basanite</skos:prefLabel>
	<skos:related rdf:resource="https://resource.geosphere.at/thes/lith/57"/>
	<dcterms:date rdf:datatype="http://www.w3.org/2001/XMLSchema#dateTime">2011-03-15T15:22:10Z</dcterms:date>
	<dcterms:references rdf:resource="https://resource.geosphere.at/thes/citation/477"/>
	<colourHexCode xmlns="http://dbpedia.org/ontology/">#8080F2</colourHexCode>
	<skos:prefLabel xml:lang="de">Basanit</skos:prefLabel>
	<skos:exactMatch rdf:resource="http://data.bgs.ac.uk/id/EarthMaterialClass/RockName/BSN"/>
	<skos:exactMatch rdf:resource="http://dbpedia.org/resource/Basanite"/>
	<rdf:type rdf:resource="http://www.w3.org/2004/02/skos/core#Concept"/>
	<skos:exactMatch rdf:resource="http://resource.geosciml.org/classifier/cgi/lithology/basanite"/>
	<dcterms:hasVersion rdf:datatype="http://www.w3.org/2001/XMLSchema#int">10</dcterms:hasVersion>
	<skos:exactMatch rdf:resource="http://www.wikidata.org/entity/Q32805"/>
	<dcterms:created rdf:datatype="http://www.w3.org/2001/XMLSchema#dateTime">2012-05-07T08:31:28.000Z</dcterms:created>
</rdf:Description>

<rdf:Description rdf:about="https://resource.geosphere.at/thes/lith/89">
	<skos:exactMatch rdf:resource="http://inspire.ec.europa.eu/codelist/LithologyValue/tephrite"/>
	<colourHexCode xmlns="http://dbpedia.org/ontology/">#7373F2</colourHexCode>
	<skos:exactMatch rdf:resource="http://data.bgs.ac.uk/id/EarthMaterialClass/RockName/TEP"/>
	<skos:exactMatch rdf:resource="http://resource.geosciml.org/classifier/cgi/lithology/tephrite"/>
	<skos:exactMatch rdf:resource="http://dbpedia.org/resource/Tephrite"/>
	<dcterms:references rdf:resource="https://resource.geosphere.at/thes/citation/477"/>
	<skos:related rdf:resource="https://resource.geosphere.at/thes/lith/58"/>
	<skos:prefLabel xml:lang="de">Tephrit</skos:prefLabel>
	<dcterms:date rdf:datatype="http://www.w3.org/2001/XMLSchema#dateTime">2011-03-15T15:22:10Z</dcterms:date>
	<rdf:type rdf:resource="http://www.w3.org/2004/02/skos/core#Concept"/>
	<skos:prefLabel xml:lang="en">Tephrite</skos:prefLabel>
	<dcterms:created rdf:datatype="http://www.w3.org/2001/XMLSchema#dateTime">2012-03-12T16:29:46.000Z</dcterms:created>
	<dcterms:hasVersion rdf:datatype="http://www.w3.org/2001/XMLSchema#int">11</dcterms:hasVersion>
</rdf:Description>

<rdf:Description rdf:about="https://resource.geosphere.at/thes/lith/86">
	<dcterms:created rdf:datatype="http://www.w3.org/2001/XMLSchema#dateTime">2012-03-12T15:54:32.000Z</dcterms:created>
	<skos:related rdf:resource="https://resource.geosphere.at/thes/lith/56"/>
	<rdf:type rdf:resource="http://www.w3.org/2004/02/skos/core#Concept"/>
	<skos:prefLabel xml:lang="de">Phonolithischer Basanit</skos:prefLabel>
	<skos:exactMatch rdf:resource="http://inspire.ec.europa.eu/codelist/LithologyValue/phonoliticBasanite"/>
	<skos:exactMatch rdf:resource="http://resource.geosciml.org/classifier/cgi/lithology/phonolitic_basanite"/>
	<dcterms:hasVersion rdf:datatype="http://www.w3.org/2001/XMLSchema#int">9</dcterms:hasVersion>
	<dcterms:date rdf:datatype="http://www.w3.org/2001/XMLSchema#dateTime">2011-03-15T15:22:10Z</dcterms:date>
	<skos:prefLabel xml:lang="en">Phonolitic basanite</skos:prefLabel>
	<dcterms:references rdf:resource="https://resource.geosphere.at/thes/citation/477"/>
</rdf:Description>

<rdf:Description rdf:about="https://resource.geosphere.at/thes/lith/87">
	<skos:prefLabel xml:lang="de">Phonolithischer Tephrit</skos:prefLabel>
	<dcterms:date rdf:datatype="http://www.w3.org/2001/XMLSchema#dateTime">2011-03-15T15:22:10Z</dcterms:date>
	<dcterms:references rdf:resource="https://resource.geosphere.at/thes/citation/477"/>
	<skos:exactMatch rdf:resource="http://inspire.ec.europa.eu/codelist/LithologyValue/phonoliticTephrite"/>
	<dcterms:hasVersion rdf:datatype="http://www.w3.org/2001/XMLSchema#int">13</dcterms:hasVersion>
	<rdf:type rdf:resource="http://www.w3.org/2004/02/skos/core#Concept"/>
	<skos:exactMatch rdf:resource="http://resource.geosciml.org/classifier/cgi/lithology/phonolitic_tephrite"/>
	<dcterms:created rdf:datatype="http://www.w3.org/2001/XMLSchema#dateTime">2012-03-12T15:55:25.000Z</dcterms:created>
	<skos:related rdf:resource="https://resource.geosphere.at/thes/lith/55"/>
	<skos:prefLabel xml:lang="en">Phonolitic tephrite</skos:prefLabel>
</rdf:Description>

<rdf:Description rdf:about="https://resource.geosphere.at/thes/lith/69">
	<skos:altLabel xml:lang="de">Foiditoid</skos:altLabel>
	<skos:altLabel xml:lang="en">Foiditoid</skos:altLabel>
	<dcterms:hasVersion rdf:datatype="http://www.w3.org/2001/XMLSchema#int">11</dcterms:hasVersion>
	<dcterms:references rdf:resource="https://resource.geosphere.at/thes/citation/477"/>
	<skos:exactMatch rdf:resource="http://inspire.ec.europa.eu/codelist/LithologyValue/foidGabbroid"/>
	<dcterms:date rdf:datatype="http://www.w3.org/2001/XMLSchema#dateTime">2011-03-15T15:22:10Z</dcterms:date>
	<dcterms:references rdf:resource="https://resource.geosphere.at/thes/citation/802"/>
	<rdf:type rdf:resource="http://www.w3.org/2004/02/skos/core#Concept"/>
	<skos:exactMatch rdf:resource="http://resource.geosciml.org/classifier/cgi/lithology/foiditoid"/>
	<skos:prefLabel xml:lang="de">Foiditisches Gestein</skos:prefLabel>
	<skos:narrower rdf:resource="https://resource.geosphere.at/thes/lith/91"/>
	<skos:narrower rdf:resource="https://resource.geosphere.at/thes/lith/90"/>
	<skos:prefLabel xml:lang="en">Foiditic rock</skos:prefLabel>
	<dcterms:created rdf:datatype="http://www.w3.org/2001/XMLSchema#dateTime">2012-03-12T13:23:55.000Z</dcterms:created>
	<colourHexCode xmlns="http://dbpedia.org/ontology/">#F273BF</colourHexCode>
</rdf:Description>

<rdf:Description rdf:about="https://resource.geosphere.at/thes/lith/91">
	<dcterms:created rdf:datatype="http://www.w3.org/2001/XMLSchema#dateTime">2012-03-12T16:30:03.000Z</dcterms:created>
	<skos:definition xml:lang="de">Foiditisches Gestein, welches in der QAPF-Klassifikation durch einen F kleiner als 90 Vol.-% und einem Plagioklasfaktor größer als 50 charakterisiert ist. Der normative Olivinbestand ist kleiner als 10 Vol.-%.(Le Maitre et al., 2005)</skos:definition>
	<skos:exactMatch rdf:resource="http://resource.geosciml.org/classifier/cgi/lithology/tephritic_foidite"/>
	<skos:exactMatch rdf:resource="http://inspire.ec.europa.eu/codelist/LithologyValue/tephriticFoidite"/>
	<skos:prefLabel xml:lang="de">Tephritischer Foidit</skos:prefLabel>
	<dcterms:date rdf:datatype="http://www.w3.org/2001/XMLSchema#dateTime">2011-03-15T15:22:10Z</dcterms:date>
	<dcterms:references rdf:resource="https://resource.geosphere.at/thes/citation/477"/>
	<skos:prefLabel xml:lang="en">Tephritic foidite</skos:prefLabel>
	<rdf:type rdf:resource="http://www.w3.org/2004/02/skos/core#Concept"/>
	<dcterms:hasVersion rdf:datatype="http://www.w3.org/2001/XMLSchema#int">8</dcterms:hasVersion>
</rdf:Description>

<rdf:Description rdf:about="https://resource.geosphere.at/thes/lith/90">
	<skos:prefLabel xml:lang="de">Phonolithischer Foidit</skos:prefLabel>
	<skos:exactMatch rdf:resource="http://inspire.ec.europa.eu/codelist/LithologyValue/phonoliticFoidite"/>
	<skos:exactMatch rdf:resource="http://resource.geosciml.org/classifier/cgi/lithology/phonolitic_foidite"/>
	<dcterms:references rdf:resource="https://resource.geosphere.at/thes/citation/477"/>
	<dcterms:date rdf:datatype="http://www.w3.org/2001/XMLSchema#dateTime">2011-03-15T15:22:10Z</dcterms:date>
	<rdf:type rdf:resource="http://www.w3.org/2004/02/skos/core#Concept"/>
	<dcterms:created rdf:datatype="http://www.w3.org/2001/XMLSchema#dateTime">2012-03-12T15:54:49.000Z</dcterms:created>
	<skos:prefLabel xml:lang="en">Phonolitic foidite</skos:prefLabel>
	<dcterms:hasVersion rdf:datatype="http://www.w3.org/2001/XMLSchema#int">10</dcterms:hasVersion>
</rdf:Description>

<rdf:Description rdf:about="https://resource.geosphere.at/thes/lith/66">
	<skos:prefLabel xml:lang="de">Basaltisches Gestein</skos:prefLabel>
	<skos:narrower rdf:resource="https://resource.geosphere.at/thes/lith/82"/>
	<skos:exactMatch rdf:resource="http://inspire.ec.europa.eu/codelist/LithologyValue/basalt"/>
	<skos:prefLabel xml:lang="en">Basaltic rock</skos:prefLabel>
	<skos:narrowMatch rdf:resource="http://resource.geosciml.org/classifier/cgi/lithology/basalt"/>
	<dcterms:date rdf:datatype="http://www.w3.org/2001/XMLSchema#dateTime">2011-03-15T15:22:10Z</dcterms:date>
	<skos:related rdf:resource="https://resource.geosphere.at/thes/lith/20"/>
	<dcterms:created rdf:datatype="http://www.w3.org/2001/XMLSchema#dateTime">2012-01-25T12:22:13.000Z</dcterms:created>
	<dcterms:references rdf:resource="https://resource.geosphere.at/thes/citation/477"/>
	<skos:altLabel xml:lang="de">Basaltoid</skos:altLabel>
	<skos:altLabel xml:lang="en">Basaltoid</skos:altLabel>
	<dcterms:hasVersion rdf:datatype="http://www.w3.org/2001/XMLSchema#int">10</dcterms:hasVersion>
	<dcterms:references rdf:resource="https://resource.geosphere.at/thes/citation/802"/>
	<rdf:type rdf:resource="http://www.w3.org/2004/02/skos/core#Concept"/>
</rdf:Description>

<rdf:Description rdf:about="https://resource.geosphere.at/thes/lith/82">
	<skos:exactMatch rdf:resource="http://www.wikidata.org/entity/Q43338"/>
	<foaf:depiction rdf:resource="https://resource.geosphere.at/img/thes/Basalt.jpg"/>
	<skos:exactMatch rdf:resource="http://data.bgs.ac.uk/id/EarthMaterialClass/RockName/BA"/>
	<dcterms:hasVersion rdf:datatype="http://www.w3.org/2001/XMLSchema#int">11</dcterms:hasVersion>
	<skos:prefLabel xml:lang="de">Basalt</skos:prefLabel>
	<skos:prefLabel xml:lang="en">Basalt</skos:prefLabel>
	<skos:related rdf:resource="https://resource.geosphere.at/thes/lith/48"/>
	<dcterms:references rdf:resource="https://resource.geosphere.at/thes/citation/477"/>
	<dcterms:date rdf:datatype="http://www.w3.org/2001/XMLSchema#dateTime">2011-03-15T15:22:10Z</dcterms:date>
	<colourHexCode xmlns="http://dbpedia.org/ontology/">#6600FF</colourHexCode>
	<rdf:type rdf:resource="http://www.w3.org/2004/02/skos/core#Concept"/>
	<skos:exactMatch rdf:resource="http://resource.geosciml.org/classifier/cgi/lithology/basalt"/>
	<skos:related rdf:resource="https://resource.geosphere.at/thes/lith/144"/>
	<skos:exactMatch rdf:resource="http://dbpedia.org/resource/Basalt"/>
	<dcterms:created rdf:datatype="http://www.w3.org/2001/XMLSchema#dateTime">2015-02-25T08:15:21.000Z</dcterms:created>
	<skos:exactMatch rdf:resource="http://inspire.ec.europa.eu/codelist/LithologyValue/basalt"/>
	<skos:related rdf:resource="https://resource.geosphere.at/thes/lith/96"/>
</rdf:Description>

<rdf:Description rdf:about="https://resource.geosphere.at/thes/lith/67">
	<colourHexCode xmlns="http://dbpedia.org/ontology/">#5926F2</colourHexCode>
	<skos:definition xml:lang="en">A rock that corresponds to the QAPF 'field' classification for volcanic rocks (Streckeisen 1978) identified as phonolite. QAPF-fields 11-12 (Le Maitre et al., 2005).</skos:definition>
	<dcterms:references rdf:resource="https://resource.geosphere.at/thes/citation/802"/>
	<skos:altLabel xml:lang="en">Phonolitoid</skos:altLabel>
	<skos:narrower rdf:resource="https://resource.geosphere.at/thes/lith/85"/>
	<skos:narrower rdf:resource="https://resource.geosphere.at/thes/lith/84"/>
	<rdf:type rdf:resource="http://www.w3.org/2004/02/skos/core#Concept"/>
	<skos:exactMatch rdf:resource="http://inspire.ec.europa.eu/codelist/LithologyValue/phonolitoid"/>
	<skos:altLabel xml:lang="de">Phonolithoid</skos:altLabel>
	<skos:prefLabel xml:lang="de">Phonolithisches Gestein</skos:prefLabel>
	<skos:exactMatch rdf:resource="http://resource.geosciml.org/classifier/cgi/lithology/phonolitoid"/>
	<dcterms:hasVersion rdf:datatype="http://www.w3.org/2001/XMLSchema#int">12</dcterms:hasVersion>
	<skos:definition xml:lang="de">Ein Gestein, welches der QAPF-Gelände-Klassifikation für vulkanische Gesteine entspricht (Streckeisen, 1978) und als Phonolith identifiziert wurde. Modal definiert in QAPF-Feldern 11-12 (Le Maitre et al., 2005).</skos:definition>
	<skos:prefLabel xml:lang="en">Phonolitic rock</skos:prefLabel>
	<dcterms:created rdf:datatype="http://www.w3.org/2001/XMLSchema#dateTime">2012-03-12T15:55:09.000Z</dcterms:created>
	<dcterms:references rdf:resource="https://resource.geosphere.at/thes/citation/477"/>
	<dcterms:date rdf:datatype="http://www.w3.org/2001/XMLSchema#dateTime">2011-03-15T15:22:10Z</dcterms:date>
	<skos:related rdf:resource="https://resource.geosphere.at/thes/lith/22"/>
</rdf:Description>

<rdf:Description rdf:about="https://resource.geosphere.at/thes/lith/84">
	<dcterms:created rdf:datatype="http://www.w3.org/2001/XMLSchema#dateTime">2012-03-12T15:54:16.000Z</dcterms:created>
	<rdf:type rdf:resource="http://www.w3.org/2004/02/skos/core#Concept"/>
	<skos:exactMatch rdf:resource="http://resource.geosciml.org/classifier/cgi/lithology/phonolilte"/>
	<skos:definition xml:lang="de">Vulkanisches Gestein, welches hauptsächlich aus Alkalifeldspat und Feldspatvertretern besteht. Modal definiert in QAPF-Feld 11 (Le Maitre et al., 2005).</skos:definition>
	<skos:exactMatch rdf:resource="http://inspire.ec.europa.eu/codelist/LithologyValue/phonolite"/>
	<skos:related rdf:resource="https://resource.geosphere.at/thes/lith/53"/>
	<skos:prefLabel xml:lang="de">Phonolith</skos:prefLabel>
	<colourHexCode xmlns="http://dbpedia.org/ontology/">#594DF2</colourHexCode>
	<dcterms:references rdf:resource="https://resource.geosphere.at/thes/citation/477"/>
	<skos:exactMatch rdf:resource="http://www.wikidata.org/entity/Q1257550"/>
	<dcterms:date rdf:datatype="http://www.w3.org/2001/XMLSchema#dateTime">2011-03-15T15:22:10Z</dcterms:date>
	<skos:definition xml:lang="en">A volcanic rock consisting essentially of alkali feldspar and foids. Defined modally in QAPF-field 11 (Le Maitre et al., 2005).</skos:definition>
	<skos:prefLabel xml:lang="en">Phonolite</skos:prefLabel>
	<skos:exactMatch rdf:resource="http://data.bgs.ac.uk/id/EarthMaterialClass/RockName/PN"/>
	<skos:exactMatch rdf:resource="http://dbpedia.org/resource/Phonolite"/>
	<dcterms:hasVersion rdf:datatype="http://www.w3.org/2001/XMLSchema#int">9</dcterms:hasVersion>
</rdf:Description>

<rdf:Description rdf:about="https://resource.geosphere.at/thes/lith/85">
	<skos:definition xml:lang="en">An alkaline volcanic rock consisting of alkali feldspar, plagioclase, feldspathoids, and various mafic minerals. Defined modally in QAPF-field 12 (Le Maitre et al., 2005).</skos:definition>
	<skos:exactMatch rdf:resource="http://inspire.ec.europa.eu/codelist/LithologyValue/tephriticPhonolite"/>
	<skos:prefLabel xml:lang="en">Tephritic phonolite</skos:prefLabel>
	<skos:definition xml:lang="de">Alkalisches vulkanisches Gestein, welches aus Alkalifeldspat, Plagioklas, Feldspatvertretern und verschiedenen mafischen Mineralen besteht. Modal definiert in QAPF-Feld 12 (Le Maitre et al., 2005).</skos:definition>
	<skos:related rdf:resource="https://resource.geosphere.at/thes/lith/54"/>
	<dcterms:hasVersion rdf:datatype="http://www.w3.org/2001/XMLSchema#int">8</dcterms:hasVersion>
	<dcterms:references rdf:resource="https://resource.geosphere.at/thes/citation/477"/>
	<dcterms:date rdf:datatype="http://www.w3.org/2001/XMLSchema#dateTime">2011-03-15T15:22:10Z</dcterms:date>
	<rdf:type rdf:resource="http://www.w3.org/2004/02/skos/core#Concept"/>
	<skos:prefLabel xml:lang="de">Tephritischer Phonolit</skos:prefLabel>
	<dcterms:created rdf:datatype="http://www.w3.org/2001/XMLSchema#dateTime">2012-03-12T16:30:29.000Z</dcterms:created>
	<skos:exactMatch rdf:resource="http://resource.geosciml.org/classifier/cgi/lithology/tephritic_phonolite"/>
</rdf:Description>

<rdf:Description rdf:about="https://resource.geosphere.at/thes/lith/64">
	<skos:prefLabel xml:lang="en">Trachytic rock</skos:prefLabel>
	<skos:prefLabel xml:lang="de">Trachytisches Gestein</skos:prefLabel>
	<skos:altLabel xml:lang="de">Trachytoid</skos:altLabel>
	<skos:altLabel xml:lang="en">Trachytoid</skos:altLabel>
	<skos:exactMatch rdf:resource="http://inspire.ec.europa.eu/codelist/LithologyValue/trachyticRock"/>
	<dcterms:date rdf:datatype="http://www.w3.org/2001/XMLSchema#dateTime">2011-03-15T15:22:10Z</dcterms:date>
	<dcterms:references rdf:resource="https://resource.geosphere.at/thes/citation/477"/>
	<skos:related rdf:resource="https://resource.geosphere.at/thes/lith/19"/>
	<dcterms:references rdf:resource="https://resource.geosphere.at/thes/citation/802"/>
	<skos:narrower rdf:resource="https://resource.geosphere.at/thes/lith/80"/>
	<skos:narrower rdf:resource="https://resource.geosphere.at/thes/lith/81"/>
	<skos:narrower rdf:resource="https://resource.geosphere.at/thes/lith/78"/>
	<skos:narrower rdf:resource="https://resource.geosphere.at/thes/lith/79"/>
	<skos:narrower rdf:resource="https://resource.geosphere.at/thes/lith/76"/>
	<skos:narrower rdf:resource="https://resource.geosphere.at/thes/lith/77"/>
	<skos:narrower rdf:resource="https://resource.geosphere.at/thes/lith/74"/>
	<skos:narrower rdf:resource="https://resource.geosphere.at/thes/lith/75"/>
	<skos:narrower rdf:resource="https://resource.geosphere.at/thes/lith/73"/>
	<rdf:type rdf:resource="http://www.w3.org/2004/02/skos/core#Concept"/>
	<skos:definition xml:lang="de">Gestein, welches der QAPF-Gelände-Klassifikation für vulkanische Gesteine entspricht (Streckeisen, 1978) und als Trachyt identifiziert wurde. Modal definiert in QAPF-Feldern 6-8 (Le Maitre et al., 2005).</skos:definition>
	<skos:definition xml:lang="en">A rock that corresponds to the QAPF 'field' classification for volcanic rocks (Streckeisen 1978) identified as trachyte. QAPF-fields 6-8 (Le Maitre et al., 2005).</skos:definition>
	<skos:exactMatch rdf:resource="http://resource.geosciml.org/classifier/cgi/lithology/trachytoid"/>
	<dcterms:created rdf:datatype="http://www.w3.org/2001/XMLSchema#dateTime">2012-03-12T16:32:12.000Z</dcterms:created>
	<colourHexCode xmlns="http://dbpedia.org/ontology/">#A17AED</colourHexCode>
	<dcterms:hasVersion rdf:datatype="http://www.w3.org/2001/XMLSchema#int">11</dcterms:hasVersion>
</rdf:Description>

<rdf:Description rdf:about="https://resource.geosphere.at/thes/lith/79">
	<dcterms:created rdf:datatype="http://www.w3.org/2001/XMLSchema#dateTime">2012-03-12T16:07:11.000Z</dcterms:created>
	<skos:prefLabel xml:lang="en">Quartz latite</skos:prefLabel>
	<skos:prefLabel xml:lang="de">Quarz-Latit</skos:prefLabel>
	<rdf:type rdf:resource="http://www.w3.org/2004/02/skos/core#Concept"/>
	<skos:definition xml:lang="en">A volcanic rock consisting of approximately equal amounts of plagioclase and alkali feldspar, with quartz between 5-20% of felsic mineral content, and mafic minerals. Defined modally in QAPF-field 8* (Le Maitre et al., 2005).</skos:definition>
	<skos:definition xml:lang="de">Vulkanisches Gestein, welches zu gleichen Anteilen aus Plagioklas und Alkalifeldspat, Quarz (5–20 % der felsischen Minerale) und mafischen Mineralen besteht. Modal definiert in QAPF-Feld 8* (Le Maitre et al., 2005).</skos:definition>
	<dcterms:hasVersion rdf:datatype="http://www.w3.org/2001/XMLSchema#int">10</dcterms:hasVersion>
	<skos:exactMatch rdf:resource="http://inspire.ec.europa.eu/codelist/LithologyValue/quartzLatite"/>
	<skos:exactMatch rdf:resource="http://resource.geosciml.org/classifier/cgi/lithology/quartz_latite"/>
	<skos:related rdf:resource="https://resource.geosphere.at/thes/lith/81"/>
	<skos:related rdf:resource="https://resource.geosphere.at/thes/lith/80"/>
	<dcterms:references rdf:resource="https://resource.geosphere.at/thes/citation/477"/>
	<dcterms:date rdf:datatype="http://www.w3.org/2001/XMLSchema#dateTime">2011-03-15T15:22:10Z</dcterms:date>
	<skos:related rdf:resource="https://resource.geosphere.at/thes/lith/35"/>
</rdf:Description>

<rdf:Description rdf:about="https://resource.geosphere.at/thes/lith/77">
	<dcterms:hasVersion rdf:datatype="http://www.w3.org/2001/XMLSchema#int">8</dcterms:hasVersion>
	<dcterms:created rdf:datatype="http://www.w3.org/2001/XMLSchema#dateTime">2012-03-12T16:31:59.000Z</dcterms:created>
	<skos:exactMatch rdf:resource="http://dbpedia.org/resource/Trachyte"/>
	<skos:related rdf:resource="https://resource.geosphere.at/thes/lith/78"/>
	<skos:related rdf:resource="https://resource.geosphere.at/thes/lith/76"/>
	<skos:related rdf:resource="https://resource.geosphere.at/thes/lith/33"/>
	<skos:exactMatch rdf:resource="http://data.bgs.ac.uk/id/EarthMaterialClass/RockName/TR"/>
	<dcterms:references rdf:resource="https://resource.geosphere.at/thes/citation/477"/>
	<skos:prefLabel xml:lang="en">Trachyte</skos:prefLabel>
	<dcterms:date rdf:datatype="http://www.w3.org/2001/XMLSchema#dateTime">2011-03-15T15:22:10Z</dcterms:date>
	<skos:exactMatch rdf:resource="http://resource.geosciml.org/classifier/cgi/lithology/trachyte"/>
	<skos:exactMatch rdf:resource="http://inspire.ec.europa.eu/codelist/LithologyValue/trachyte"/>
	<rdf:type rdf:resource="http://www.w3.org/2004/02/skos/core#Concept"/>
	<skos:exactMatch rdf:resource="http://www.wikidata.org/entity/Q332748"/>
	<colourHexCode xmlns="http://dbpedia.org/ontology/">#A17AED</colourHexCode>
	<skos:prefLabel xml:lang="de">Trachyt</skos:prefLabel>
</rdf:Description>

<rdf:Description rdf:about="https://resource.geosphere.at/thes/lith/78">
	<dcterms:created rdf:datatype="http://www.w3.org/2001/XMLSchema#dateTime">2012-03-12T13:22:54.000Z</dcterms:created>
	<skos:definition xml:lang="de">Vulkanisches Gestein mit Trachyt-Zusammensetzung, welches kleine Mengen von Feldspatvertretern beinhaltet (&lt; 10 % der felsischen Minerale). Modal definiert in QAPF-Feld 7' (Le Maitre et al., 2005).</skos:definition>
	<skos:exactMatch rdf:resource="http://inspire.ec.europa.eu/codelist/LithologyValue/foidBearingTrachyte"/>
	<skos:related rdf:resource="https://resource.geosphere.at/thes/lith/76"/>
	<skos:related rdf:resource="https://resource.geosphere.at/thes/lith/77"/>
	<dcterms:date rdf:datatype="http://www.w3.org/2001/XMLSchema#dateTime">2011-03-15T15:22:10Z</dcterms:date>
	<skos:prefLabel xml:lang="de">Foidführender Trachyt</skos:prefLabel>
	<skos:related rdf:resource="https://resource.geosphere.at/thes/lith/34"/>
	<dcterms:references rdf:resource="https://resource.geosphere.at/thes/citation/477"/>
	<skos:definition xml:lang="en">A volcanic rock with the composition of a trachyte, containing small quantities of feldspathoids (&lt; 10% of the felsic minerals). Defined modally in QAPF-field 7' (Le Maitre et al., 2005).</skos:definition>
	<skos:prefLabel xml:lang="en">Foid-bearing trachyte</skos:prefLabel>
	<dcterms:hasVersion rdf:datatype="http://www.w3.org/2001/XMLSchema#int">10</dcterms:hasVersion>
	<rdf:type rdf:resource="http://www.w3.org/2004/02/skos/core#Concept"/>
	<skos:exactMatch rdf:resource="http://resource.geosciml.org/classifier/cgi/lithology/foid_bearing_trachyte"/>
</rdf:Description>

<rdf:Description rdf:about="https://resource.geosphere.at/thes/lith/75">
	<skos:exactMatch rdf:resource="http://resource.geosciml.org/classifier/cgi/lithology/foid_bearing_alkali_feldspar_trachyte"/>
	<dcterms:references rdf:resource="https://resource.geosphere.at/thes/citation/477"/>
	<dcterms:date rdf:datatype="http://www.w3.org/2001/XMLSchema#dateTime">2011-03-15T15:22:10Z</dcterms:date>
	<skos:related rdf:resource="https://resource.geosphere.at/thes/lith/31"/>
	<skos:definition xml:lang="en">A volcanic rock with the composition of an alkali feldspar trachyte, containing small quantities of feldspathoids (&lt; 10% of the felsic minerals). Defined modally in QAPF-field 6' (Le Maitre et al., 2005).</skos:definition>
	<skos:prefLabel xml:lang="en">Foid-bearing alkali feldspar trachyte</skos:prefLabel>
	<dcterms:hasVersion rdf:datatype="http://www.w3.org/2001/XMLSchema#int">9</dcterms:hasVersion>
	<rdf:type rdf:resource="http://www.w3.org/2004/02/skos/core#Concept"/>
	<skos:prefLabel xml:lang="de">Foidführender Alkalifeldspat-Trachyt</skos:prefLabel>
	<skos:definition xml:lang="de">Vulkanisches Gestein mit Alkalifeldspat-Trachyt-Zusammensetzung, welches kleine Mengen von Feldspatvertretern beinhaltet (&lt; 10 % der felsischen Minerale). Modal definiert in QAPF-Feld 6' (Le Maitre et al., 2005).</skos:definition>
	<dcterms:created rdf:datatype="http://www.w3.org/2001/XMLSchema#dateTime">2012-03-12T13:17:27.000Z</dcterms:created>
	<skos:related rdf:resource="https://resource.geosphere.at/thes/lith/73"/>
	<skos:related rdf:resource="https://resource.geosphere.at/thes/lith/74"/>
	<skos:exactMatch rdf:resource="http://inspire.ec.europa.eu/codelist/LithologyValue/foidBearingAlkaliFeldsparTrachyte"/>
</rdf:Description>

<rdf:Description rdf:about="https://resource.geosphere.at/thes/lith/76">
	<dcterms:date rdf:datatype="http://www.w3.org/2001/XMLSchema#dateTime">2011-03-15T15:22:10Z</dcterms:date>
	<dcterms:references rdf:resource="https://resource.geosphere.at/thes/citation/477"/>
	<skos:related rdf:resource="https://resource.geosphere.at/thes/lith/78"/>
	<skos:related rdf:resource="https://resource.geosphere.at/thes/lith/77"/>
	<dcterms:hasVersion rdf:datatype="http://www.w3.org/2001/XMLSchema#int">9</dcterms:hasVersion>
	<skos:prefLabel xml:lang="de">Quarz-Trachyt</skos:prefLabel>
	<skos:definition xml:lang="en">A volcanic rock consisting of phenocrysts of alkali feldspar and quartz in a cryptocrystalline or glassy matrix. Quartz trachyte is the volcanic equivalent of quartz syenite. Defined modally in QAPF-field 7* (Le Maitre et al., 2005).</skos:definition>
	<skos:related rdf:resource="https://resource.geosphere.at/thes/lith/32"/>
	<skos:prefLabel xml:lang="en">Quartz trachyte</skos:prefLabel>
	<skos:exactMatch rdf:resource="http://resource.geosciml.org/classifier/cgi/lithology/quartz_trachyte"/>
	<dcterms:created rdf:datatype="http://www.w3.org/2001/XMLSchema#dateTime">2012-03-12T16:10:41.000Z</dcterms:created>
	<skos:definition xml:lang="de">Vulkanisches Gestein, welches aus Phenokristallen von Alkalifeldspat und Quarz in einer kryptokristallinen oder glasigen Matrix besteht. Vulkanisches Äquivalent von Quarz-Syenit. Modal definiert in QAPF-Feld 7* (Le Maitre et al., 2005).</skos:definition>
	<skos:exactMatch rdf:resource="http://inspire.ec.europa.eu/codelist/LithologyValue/quartzTrachyte"/>
	<rdf:type rdf:resource="http://www.w3.org/2004/02/skos/core#Concept"/>
</rdf:Description>

<rdf:Description rdf:about="https://resource.geosphere.at/thes/lith/73">
	<skos:related rdf:resource="https://resource.geosphere.at/thes/lith/29"/>
	<skos:exactMatch rdf:resource="http://resource.geosciml.org/classifier/cgi/lithology/quartz_alkali_feldspar_trachyte"/>
	<skos:definition xml:lang="en">A felsic volcanic rock consisting essentially of alkali feldspar, quartz, and mafic minerals. Defined modally in QAPF-field 6* (Le Maitre et al., 2005).</skos:definition>
	<skos:prefLabel xml:lang="en">Quartz alkali feldspar trachyte</skos:prefLabel>
	<skos:exactMatch rdf:resource="http://inspire.ec.europa.eu/codelist/LithologyValue/quartzAlkaliFeldsparTrachyte"/>
	<dcterms:date rdf:datatype="http://www.w3.org/2001/XMLSchema#dateTime">2011-03-15T15:22:10Z</dcterms:date>
	<dcterms:created rdf:datatype="http://www.w3.org/2001/XMLSchema#dateTime">2012-03-12T16:01:59.000Z</dcterms:created>
	<dcterms:hasVersion rdf:datatype="http://www.w3.org/2001/XMLSchema#int">9</dcterms:hasVersion>
	<skos:related rdf:resource="https://resource.geosphere.at/thes/lith/75"/>
	<skos:related rdf:resource="https://resource.geosphere.at/thes/lith/74"/>
	<skos:definition xml:lang="de">Felsisches vulkanisches Gestein, welches aus überwiegend Alkalifeldspat, Quarz und mafischen Mineralen besteht. Modal definiert in QAPF-Feld 6* (Le Maitre et al., 2005).</skos:definition>
	<dcterms:references rdf:resource="https://resource.geosphere.at/thes/citation/477"/>
	<rdf:type rdf:resource="http://www.w3.org/2004/02/skos/core#Concept"/>
	<skos:prefLabel xml:lang="de">Quarz-Alkalifeldspat-Trachyt</skos:prefLabel>
</rdf:Description>

<rdf:Description rdf:about="https://resource.geosphere.at/thes/lith/74">
	<rdf:type rdf:resource="http://www.w3.org/2004/02/skos/core#Concept"/>
	<skos:exactMatch rdf:resource="http://resource.geosciml.org/classifier/cgi/lithology/alkali_feldspar_trachyte"/>
	<dcterms:hasVersion rdf:datatype="http://www.w3.org/2001/XMLSchema#int">10</dcterms:hasVersion>
	<skos:exactMatch rdf:resource="http://inspire.ec.europa.eu/codelist/LithologyValue/alkaliFeldsparTrachyte"/>
	<skos:related rdf:resource="https://resource.geosphere.at/thes/lith/73"/>
	<skos:related rdf:resource="https://resource.geosphere.at/thes/lith/75"/>
	<skos:definition xml:lang="en">A volcanic rock and variety of trachyte in which plagioclase comprises &lt; 10% of the total feldspar. Defined modally in QAPF-field 6 (Le Maitre et al., 2005).</skos:definition>
	<dcterms:created rdf:datatype="http://www.w3.org/2001/XMLSchema#dateTime">2012-03-08T09:32:51.000Z</dcterms:created>
	<skos:definition xml:lang="de">Vulkanisches Gestein und Varietät von Trachyt mit &lt; 10 % Plagioklasanteil am Gesamtfeldspat. Modal definiert in QAPF-Feld 6 (Le Maitre et al., 2005).</skos:definition>
	<skos:prefLabel xml:lang="de">Alkalifeldspat-Trachyt</skos:prefLabel>
	<dcterms:date rdf:datatype="http://www.w3.org/2001/XMLSchema#dateTime">2011-03-15T15:22:10Z</dcterms:date>
	<skos:related rdf:resource="https://resource.geosphere.at/thes/lith/30"/>
	<skos:prefLabel xml:lang="en">Alkali feldspar trachyte</skos:prefLabel>
	<dcterms:references rdf:resource="https://resource.geosphere.at/thes/citation/477"/>
</rdf:Description>

<rdf:Description rdf:about="https://resource.geosphere.at/thes/lith/80">
	<skos:exactMatch rdf:resource="http://inspire.ec.europa.eu/codelist/LithologyValue/latite"/>
	<dcterms:created rdf:datatype="http://www.w3.org/2001/XMLSchema#dateTime">2012-03-12T13:58:10.000Z</dcterms:created>
	<skos:exactMatch rdf:resource="http://resource.geosciml.org/classifier/cgi/lithology/latite"/>
	<rdf:type rdf:resource="http://www.w3.org/2004/02/skos/core#Concept"/>
	<skos:definition xml:lang="en">A volcanic rock consisting of approximately equal amounts of sodic plagioclase and alkali feldspar. Volcanic equivalent of monzonite. Defined modally in QAPF-field 8 (Le Maitre et al., 2005).</skos:definition>
	<skos:prefLabel xml:lang="de">Latit</skos:prefLabel>
	<skos:exactMatch rdf:resource="http://data.bgs.ac.uk/id/EarthMaterialClass/RockName/LA"/>
	<skos:exactMatch rdf:resource="http://dbpedia.org/resource/Latite"/>
	<skos:prefLabel xml:lang="en">Latite</skos:prefLabel>
	<colourHexCode xmlns="http://dbpedia.org/ontology/">#AD8CF2</colourHexCode>
	<dcterms:hasVersion rdf:datatype="http://www.w3.org/2001/XMLSchema#int">8</dcterms:hasVersion>
	<skos:exactMatch rdf:resource="http://www.wikidata.org/entity/Q666363"/>
	<skos:related rdf:resource="https://resource.geosphere.at/thes/lith/79"/>
	<skos:related rdf:resource="https://resource.geosphere.at/thes/lith/81"/>
	<dcterms:references rdf:resource="https://resource.geosphere.at/thes/citation/477"/>
	<dcterms:date rdf:datatype="http://www.w3.org/2001/XMLSchema#dateTime">2011-03-15T15:22:10Z</dcterms:date>
	<skos:definition xml:lang="de">Vulkanisches Gestein, welches zu gleichen Anteilen aus Natrium-Plagioklas und Alkalifeldspat besteht. Vulkanisches Äquivalent zu Monzonit. Modal definiert in QAPF-Feld 8 (Le Maitre et al., 2005).</skos:definition>
	<skos:related rdf:resource="https://resource.geosphere.at/thes/lith/36"/>
</rdf:Description>

<rdf:Description rdf:about="https://resource.geosphere.at/thes/lith/81">
	<dcterms:date rdf:datatype="http://www.w3.org/2001/XMLSchema#dateTime">2011-03-15T15:22:10Z</dcterms:date>
	<skos:related rdf:resource="https://resource.geosphere.at/thes/lith/79"/>
	<dcterms:created rdf:datatype="http://www.w3.org/2001/XMLSchema#dateTime">2012-03-12T13:20:20.000Z</dcterms:created>
	<dcterms:references rdf:resource="https://resource.geosphere.at/thes/citation/477"/>
	<skos:exactMatch rdf:resource="http://resource.geosciml.org/classifier/cgi/lithology/foid_bearing_latite"/>
	<skos:related rdf:resource="https://resource.geosphere.at/thes/lith/37"/>
	<dcterms:hasVersion rdf:datatype="http://www.w3.org/2001/XMLSchema#int">9</dcterms:hasVersion>
	<rdf:type rdf:resource="http://www.w3.org/2004/02/skos/core#Concept"/>
	<skos:exactMatch rdf:resource="http://inspire.ec.europa.eu/codelist/LithologyValue/foidBearingLatite"/>
	<skos:related rdf:resource="https://resource.geosphere.at/thes/lith/80"/>
	<skos:prefLabel xml:lang="en">Foid-bearing latite</skos:prefLabel>
	<skos:prefLabel xml:lang="de">Foidführender Latit</skos:prefLabel>
	<skos:definition xml:lang="en">A volcanic rock with the composition of a latite, containing small quantities of feldspathoids (&lt; 10% of the felsic minerals). Defined modally in QAPF-field 8', (Le Maitre et al., 2005).</skos:definition>
	<skos:definition xml:lang="de">Vulkanisches Gestein mit Latit-Zusammensetzung, welches kleine Mengen von Feldspatvertretern beinhaltet (&lt; 10 % der felsischen Minerale). Modal definiert in QAPF-Feld 8' (Le Maitre et al., 2005).</skos:definition>
</rdf:Description>

<rdf:Description rdf:about="https://resource.geosphere.at/thes/lith/65">
	<skos:exactMatch rdf:resource="http://inspire.ec.europa.eu/codelist/LithologyValue/andesite"/>
	<skos:narrower rdf:resource="https://resource.geosphere.at/thes/lith/83"/>
	<skos:altLabel xml:lang="de">Andesitoid</skos:altLabel>
	<skos:altLabel xml:lang="en">Andesitoid</skos:altLabel>
	<dcterms:references rdf:resource="https://resource.geosphere.at/thes/citation/477"/>
	<dcterms:date rdf:datatype="http://www.w3.org/2001/XMLSchema#dateTime">2011-03-15T15:22:10Z</dcterms:date>
	<skos:closeMatch rdf:resource="http://resource.geosciml.org/classifier/cgi/lithology/high_magnesium_fine_grained_igneous_rocks"/>
	<rdf:type rdf:resource="http://www.w3.org/2004/02/skos/core#Concept"/>
	<dcterms:references rdf:resource="https://resource.geosphere.at/thes/citation/802"/>
	<skos:related rdf:resource="https://resource.geosphere.at/thes/lith/157"/>
	<skos:prefLabel xml:lang="en">Andesitic rock</skos:prefLabel>
	<skos:related rdf:resource="https://resource.geosphere.at/thes/lith/20"/>
	<dcterms:hasVersion rdf:datatype="http://www.w3.org/2001/XMLSchema#int">11</dcterms:hasVersion>
	<dcterms:created rdf:datatype="http://www.w3.org/2001/XMLSchema#dateTime">2012-03-08T09:38:52.000Z</dcterms:created>
	<skos:prefLabel xml:lang="de">Andesitisches Gestein</skos:prefLabel>
</rdf:Description>

<rdf:Description rdf:about="https://resource.geosphere.at/thes/lith/83">
	<dcterms:created rdf:datatype="http://www.w3.org/2001/XMLSchema#dateTime">2012-03-08T09:36:31.000Z</dcterms:created>
	<dcterms:hasVersion rdf:datatype="http://www.w3.org/2001/XMLSchema#int">14</dcterms:hasVersion>
	<skos:exactMatch rdf:resource="http://www.wikidata.org/entity/Q181908"/>
	<colourHexCode xmlns="http://dbpedia.org/ontology/">#9145EB</colourHexCode>
	<skos:exactMatch rdf:resource="http://resource.geosciml.org/classifier/cgi/lithology/andesite"/>
	<skos:exactMatch rdf:resource="http://dbpedia.org/resource/Andesite"/>
	<dcterms:date rdf:datatype="http://www.w3.org/2001/XMLSchema#dateTime">2011-03-15T15:22:10Z</dcterms:date>
	<dcterms:references rdf:resource="https://resource.geosphere.at/thes/citation/477"/>
	<skos:prefLabel xml:lang="en">Andesite</skos:prefLabel>
	<skos:related rdf:resource="https://resource.geosphere.at/thes/lith/45"/>
	<rdf:type rdf:resource="http://www.w3.org/2004/02/skos/core#Concept"/>
	<skos:exactMatch rdf:resource="http://inspire.ec.europa.eu/codelist/LithologyValue/andesite"/>
	<skos:prefLabel xml:lang="de">Andesit</skos:prefLabel>
	<skos:exactMatch rdf:resource="http://data.bgs.ac.uk/id/EarthMaterialClass/RockName/AND"/>
</rdf:Description>

<rdf:Description rdf:about="https://resource.geosphere.at/thes/lith/62">
	<dcterms:date rdf:datatype="http://www.w3.org/2001/XMLSchema#dateTime">2011-03-15T15:22:10Z</dcterms:date>
	<skos:definition xml:lang="en">A rock that corresponds to the QAPF 'field' classification for volcanic rocks (Streckeisen 1978) identified as rhyolite. QAPF-fields 2-3 (Le Maitre et al., 2005).</skos:definition>
	<rdf:type rdf:resource="http://www.w3.org/2004/02/skos/core#Concept"/>
	<dcterms:references rdf:resource="https://resource.geosphere.at/thes/citation/802"/>
	<skos:related rdf:resource="https://resource.geosphere.at/thes/lith/18"/>
	<dcterms:hasVersion rdf:datatype="http://www.w3.org/2001/XMLSchema#int">10</dcterms:hasVersion>
	<skos:definition xml:lang="de">Gestein, welches der QAPF-Gelände-Klassifikation für vulkanische Gesteine entspricht (Streckeisen, 1978) und als Rhyolith identifiziert wurde. Modal definiert in QAPF-Feldern 2-3 (Le Maitre et al., 2005).</skos:definition>
	<skos:narrower rdf:resource="https://resource.geosphere.at/thes/lith/70"/>
	<skos:narrower rdf:resource="https://resource.geosphere.at/thes/lith/71"/>
	<skos:exactMatch rdf:resource="http://inspire.ec.europa.eu/codelist/LithologyValue/rhyolitoid"/>
	<skos:prefLabel xml:lang="en">Rhyolithic rock</skos:prefLabel>
	<skos:altLabel xml:lang="de">Rhyolithoid</skos:altLabel>
	<skos:altLabel xml:lang="en">Rhyolithoid</skos:altLabel>
	<dcterms:created rdf:datatype="http://www.w3.org/2001/XMLSchema#dateTime">2012-03-12T16:12:44.000Z</dcterms:created>
	<skos:prefLabel xml:lang="de">Rhyolitisches Gestein</skos:prefLabel>
	<colourHexCode xmlns="http://dbpedia.org/ontology/">#BF8CF2</colourHexCode>
	<dcterms:references rdf:resource="https://resource.geosphere.at/thes/citation/477"/>
	<skos:exactMatch rdf:resource="http://resource.geosciml.org/classifier/cgi/lithology/rhyolitoid"/>
</rdf:Description>

<rdf:Description rdf:about="https://resource.geosphere.at/thes/lith/71">
	<dcterms:hasVersion rdf:datatype="http://www.w3.org/2001/XMLSchema#int">8</dcterms:hasVersion>
	<skos:exactMatch rdf:resource="http://inspire.ec.europa.eu/codelist/LithologyValue/rhyolite"/>
	<skos:prefLabel xml:lang="de">Rhyolith</skos:prefLabel>
	<skos:prefLabel xml:lang="en">Rhyolite</skos:prefLabel>
	<skos:exactMatch rdf:resource="http://resource.geosciml.org/classifier/cgi/lithology/rhyolite"/>
	<skos:exactMatch rdf:resource="http://data.bgs.ac.uk/id/EarthMaterialClass/RockName/RY"/>
	<dcterms:date rdf:datatype="http://www.w3.org/2001/XMLSchema#dateTime">2011-03-15T15:22:10Z</dcterms:date>
	<dcterms:references rdf:resource="https://resource.geosphere.at/thes/citation/477"/>
	<skos:exactMatch rdf:resource="http://dbpedia.org/resource/Rhyolite"/>
	<rdf:type rdf:resource="http://www.w3.org/2004/02/skos/core#Concept"/>
	<colourHexCode xmlns="http://dbpedia.org/ontology/">#C799F2</colourHexCode>
	<skos:exactMatch rdf:resource="http://www.wikidata.org/entity/Q190727"/>
	<dcterms:created rdf:datatype="http://www.w3.org/2001/XMLSchema#dateTime">2012-03-12T16:12:29.000Z</dcterms:created>
</rdf:Description>

<rdf:Description rdf:about="https://resource.geosphere.at/thes/lith/70">
	<skos:exactMatch rdf:resource="http://resource.geosciml.org/classifier/cgi/lithology/alkali_feldspar_rhyolite"/>
	<skos:prefLabel xml:lang="en">Alkali feldspar rhyolite</skos:prefLabel>
	<dcterms:references rdf:resource="https://resource.geosphere.at/thes/citation/477"/>
	<dcterms:hasVersion rdf:datatype="http://www.w3.org/2001/XMLSchema#int">9</dcterms:hasVersion>
	<dcterms:date rdf:datatype="http://www.w3.org/2001/XMLSchema#dateTime">2011-03-15T15:22:10Z</dcterms:date>
	<rdf:type rdf:resource="http://www.w3.org/2004/02/skos/core#Concept"/>
	<skos:definition xml:lang="en">A volcanic rock and variety of rhyolite in which plagioclase comprises &lt; 10% of the total feldspar. Defined modally in QAPF-field 2 (Le Maitre et al., 2005).</skos:definition>
	<skos:prefLabel xml:lang="de">Alkalifeldspat-Rhyolith</skos:prefLabel>
	<skos:related rdf:resource="https://resource.geosphere.at/thes/lith/25"/>
	<skos:definition xml:lang="de">Vulkanisches Gestein und Varietät von Rhyolith mit &lt; 10 % Plagioklasanteil am Gesamtfeldspat. Modal definiert in QAPF-Feld 2 (Le Maitre et al., 2005).</skos:definition>
	<dcterms:created rdf:datatype="http://www.w3.org/2001/XMLSchema#dateTime">2012-03-08T09:32:05.000Z</dcterms:created>
	<colourHexCode xmlns="http://dbpedia.org/ontology/">#CCA6F2</colourHexCode>
	<skos:exactMatch rdf:resource="http://inspire.ec.europa.eu/codelist/LithologyValue/alkaliFeldsparRhyolite"/>
</rdf:Description>

<rdf:Description rdf:about="https://resource.geosphere.at/thes/lith/96">
	<skos:exactMatch rdf:resource="http://inspire.ec.europa.eu/codelist/LithologyValue/doleriticRock"/>
	<rdf:type rdf:resource="http://www.w3.org/2004/02/skos/core#Concept"/>
	<skos:altLabel xml:lang="en">Diabase</skos:altLabel>
	<skos:scopeNote xml:lang="de">Dieses subvulkanische Gestein tritt überwiegend in Form von Gängen und Lagergängen (Sills) auf. Der Begriff Diabas wird in (älterer) deutschsprachiger Literatur oft für alterierte /schwach metamorphe, mittelkörnige Basalte von präkänozoischem Ursprung verwendet.</skos:scopeNote>
	<skos:prefLabel xml:lang="de">Dolerit</skos:prefLabel>
	<skos:prefLabel xml:lang="en">Dolerite</skos:prefLabel>
	<skos:scopeNote xml:lang="en">This sub-volcanic rock occurs in form of dykes and sills. The term Diabase is used in (older) German literature for medium-grained Basalts that are alterated or show a low metamorphic grade and formed in pre-cenozoic times.</skos:scopeNote>
	<skos:related rdf:resource="https://resource.geosphere.at/thes/lith/48"/>
	<skos:closeMatch rdf:resource="http://resource.geosciml.org/classifier/cgi/lithology/doleritic_rock"/>
	<skos:altLabel xml:lang="de">Mikrogabbro</skos:altLabel>
	<skos:related rdf:resource="https://resource.geosphere.at/thes/lith/82"/>
	<colourHexCode xmlns="http://dbpedia.org/ontology/">#8019CC</colourHexCode>
	<dcterms:references rdf:resource="https://resource.geosphere.at/thes/citation/477"/>
	<dcterms:date rdf:datatype="http://www.w3.org/2001/XMLSchema#dateTime">2011-03-15T15:22:10Z</dcterms:date>
	<skos:altLabel xml:lang="de">Diabas</skos:altLabel>
	<dcterms:hasVersion rdf:datatype="http://www.w3.org/2001/XMLSchema#int">14</dcterms:hasVersion>
	<skos:altLabel xml:lang="en">Microgabbro</skos:altLabel>
	<dcterms:created rdf:datatype="http://www.w3.org/2001/XMLSchema#dateTime">2012-09-04T11:19:48.000Z</dcterms:created>
</rdf:Description>

<rdf:Description rdf:about="https://resource.geosphere.at/thes/lith/63">
	<skos:altLabel xml:lang="de">Dazitoid</skos:altLabel>
	<dcterms:references rdf:resource="https://resource.geosphere.at/thes/citation/477"/>
	<skos:related rdf:resource="https://resource.geosphere.at/thes/lith/18"/>
	<skos:narrowMatch rdf:resource="http://resource.geosciml.org/classifier/cgi/lithology/dacite"/>
	<dcterms:date rdf:datatype="http://www.w3.org/2001/XMLSchema#dateTime">2011-03-15T15:22:10Z</dcterms:date>
	<skos:altLabel xml:lang="en">Dacitoid</skos:altLabel>
	<skos:prefLabel xml:lang="de">Dazitisches Gestein</skos:prefLabel>
	<dcterms:references rdf:resource="https://resource.geosphere.at/thes/citation/802"/>
	<dcterms:hasVersion rdf:datatype="http://www.w3.org/2001/XMLSchema#int">10</dcterms:hasVersion>
	<skos:narrower rdf:resource="https://resource.geosphere.at/thes/lith/72"/>
	<rdf:type rdf:resource="http://www.w3.org/2004/02/skos/core#Concept"/>
	<skos:exactMatch rdf:resource="http://inspire.ec.europa.eu/codelist/LithologyValue/dacite"/>
	<dcterms:created rdf:datatype="http://www.w3.org/2001/XMLSchema#dateTime">2012-01-25T12:23:18.000Z</dcterms:created>
	<skos:prefLabel xml:lang="en">Dacitic rock</skos:prefLabel>
</rdf:Description>

<rdf:Description rdf:about="https://resource.geosphere.at/thes/lith/72">
	<skos:exactMatch rdf:resource="http://inspire.ec.europa.eu/codelist/LithologyValue/dacite"/>
	<rdf:type rdf:resource="http://www.w3.org/2004/02/skos/core#Concept"/>
	<colourHexCode xmlns="http://dbpedia.org/ontology/">#B373F2</colourHexCode>
	<skos:prefLabel xml:lang="en">Dacite</skos:prefLabel>
	<skos:altLabel xml:lang="de">Dacit</skos:altLabel>
	<skos:exactMatch rdf:resource="http://data.bgs.ac.uk/id/EarthMaterialClass/RockName/DA"/>
	<dcterms:references rdf:resource="https://resource.geosphere.at/thes/citation/477"/>
	<skos:exactMatch rdf:resource="http://dbpedia.org/resource/Dacite"/>
	<skos:exactMatch rdf:resource="http://www.wikidata.org/entity/Q466481"/>
	<dcterms:date rdf:datatype="http://www.w3.org/2001/XMLSchema#dateTime">2011-03-15T15:22:10Z</dcterms:date>
	<skos:prefLabel xml:lang="de">Dazit</skos:prefLabel>
	<skos:exactMatch rdf:resource="http://resource.geosciml.org/classifier/cgi/lithology/dacite"/>
	<skos:related rdf:resource="https://resource.geosphere.at/thes/lith/27"/>
	<skos:related rdf:resource="https://resource.geosphere.at/thes/lith/28"/>
	<dcterms:hasVersion rdf:datatype="http://www.w3.org/2001/XMLSchema#int">8</dcterms:hasVersion>
	<dcterms:created rdf:datatype="http://www.w3.org/2001/XMLSchema#dateTime">2012-03-12T12:33:09.000Z</dcterms:created>
</rdf:Description>

<rdf:Description rdf:about="https://resource.geosphere.at/thes/lith/92">
	<skos:exactMatch rdf:resource="http://resource.geosciml.org/classifier/cgi/lithology/foidite"/>
	<rdf:type rdf:resource="http://www.w3.org/2004/02/skos/core#Concept"/>
	<skos:exactMatch rdf:resource="http://inspire.ec.europa.eu/codelist/LithologyValue/foidite"/>
	<dcterms:hasVersion rdf:datatype="http://www.w3.org/2001/XMLSchema#int">10</dcterms:hasVersion>
	<skos:related rdf:resource="https://resource.geosphere.at/thes/lith/59"/>
	<skos:prefLabel xml:lang="de">Foidit</skos:prefLabel>
	<colourHexCode xmlns="http://dbpedia.org/ontology/">#804DE6</colourHexCode>
	<skos:exactMatch rdf:resource="http://data.bgs.ac.uk/id/EarthMaterialClass/RockName/FDI"/>
	<dcterms:references rdf:resource="https://resource.geosphere.at/thes/citation/477"/>
	<skos:prefLabel xml:lang="en">Foidite</skos:prefLabel>
	<dcterms:created rdf:datatype="http://www.w3.org/2001/XMLSchema#dateTime">2012-03-12T13:23:30.000Z</dcterms:created>
	<dcterms:date rdf:datatype="http://www.w3.org/2001/XMLSchema#dateTime">2011-03-15T15:22:10Z</dcterms:date>
</rdf:Description>

<rdf:Description rdf:about="https://resource.geosphere.at/thes/lith/254">
	<skos:definition xml:lang="en">Metamorphosed volcanic rocks of usually acid to intermediate chemistry (ignimbrite, tuff, tuffite) with porphyroblasts in a fine-grained groudmass. (Heinisch, 1981; Neuendorf et al., 2005: 509)</skos:definition>
	<dcterms:created rdf:datatype="http://www.w3.org/2001/XMLSchema#dateTime">2017-01-27T17:00:43.000Z</dcterms:created>
	<skos:scopeNote xml:lang="de">Verwendung vor allem in schwach metamorph überprägten, paläozoischen Schichtverbänden des Ordoviziums. Der Begriff Porphyroid kann auch auf Feldspat führende Metasedimente mit porphyrischer Textur angewandt werden.</skos:scopeNote>
	<status xmlns="https://resource.geosphere.at/schema/thes#" rdf:datatype="http://www.w3.org/2001/XMLSchema#integer">1</status>
	<dcterms:references rdf:resource="https://resource.geosphere.at/thes/citation/292"/>
	<skos:example xml:lang="en">Blasseneck Porphyroid</skos:example>
	<skos:prefLabel xml:lang="de">Porphyroid</skos:prefLabel>
	<skos:prefLabel xml:lang="en">Porphyroid</skos:prefLabel>
	<skos:definition xml:lang="de">Metamorph überprägte, saure bis intermediäre Vulkanite (Ignimbrite, Tuffe, Tuffite), mit porphyroblastischer Textur. (Heinisch, 1981; Neuendorf et al., 2005: 509) </skos:definition>
	<dcterms:source rdf:resource="https://www.mineralienatlas.de/lexikon/index.php/Porphyroid"/>
	<rdf:type rdf:resource="http://www.w3.org/2004/02/skos/core#Concept"/>
	<skos:example xml:lang="de">Blasseneck-Porphyroid</skos:example>
	<dcterms:references rdf:resource="https://resource.geosphere.at/thes/citation/545"/>
	<skos:broadMatch rdf:resource="http://inspire.ec.europa.eu/codelist/LithologyValue/acidicIgneousMaterial"/>
	<skos:broadMatch rdf:resource="http://resource.geosciml.org/classifier/cgi/lithology/acidic_igneous_material"/>
</rdf:Description>

<rdf:Description rdf:about="https://resource.geosphere.at/thes/lith/7">
	<dcterms:created rdf:datatype="http://www.w3.org/2001/XMLSchema#dateTime">2012-05-08T11:01:16.000Z</dcterms:created>
	<skos:exactMatch rdf:resource="http://resource.geosciml.org/classifier/cgi/lithology/ultramafic_igneous_rock"/>
	<dcterms:hasVersion rdf:datatype="http://www.w3.org/2001/XMLSchema#int">8</dcterms:hasVersion>
	<skos:narrower rdf:resource="https://resource.geosphere.at/thes/lith/61"/>
	<skos:narrower rdf:resource="https://resource.geosphere.at/thes/lith/60"/>
	<rdf:type rdf:resource="http://www.w3.org/2004/02/skos/core#Concept"/>
	<skos:exactMatch rdf:resource="http://inspire.ec.europa.eu/codelist/LithologyValue/ultramaficIgneousRock"/>
	<skos:exactMatch rdf:resource="http://dbpedia.org/resource/Ultramafic_rock"/>
	<skos:definition xml:lang="en">An igneous rock with a colour index M &gt; 90%. The index is equivalent to the quantity of mafic minerals such as olivine, orthopyroxene, clinopyroxene, hornblende, and sometimes biotite. This rock type includes ultramafite (ultramafic plutonic rock) and ultramafitite (ultramafic volcanic rock). The use of these terms is not recommended by the IUGS (Le Maitre et al., 2005).</skos:definition>
	<skos:exactMatch rdf:resource="http://www.wikidata.org/entity/Q1143398"/>
	<colourHexCode xmlns="http://dbpedia.org/ontology/">#CC008C</colourHexCode>
	<skos:prefLabel xml:lang="de">Ultramafisches Gestein</skos:prefLabel>
	<dcterms:references rdf:resource="https://resource.geosphere.at/thes/citation/477"/>
	<dcterms:date rdf:datatype="http://www.w3.org/2001/XMLSchema#dateTime">2011-03-15T15:22:10Z</dcterms:date>
	<skos:prefLabel xml:lang="en">Ultramafic rock</skos:prefLabel>
</rdf:Description>

<rdf:Description rdf:about="https://resource.geosphere.at/thes/lith/60">
	<dcterms:created rdf:datatype="http://www.w3.org/2001/XMLSchema#dateTime">2012-07-18T09:11:55.000Z</dcterms:created>
	<rdf:type rdf:resource="http://www.w3.org/2004/02/skos/core#Concept"/>
	<skos:exactMatch rdf:resource="http://resource.geosciml.org/classifier/cgi/lithology/peridotite"/>
	<skos:exactMatch rdf:resource="http://www.wikidata.org/entity/Q239918"/>
	<skos:exactMatch rdf:resource="http://inspire.ec.europa.eu/codelist/LithologyValue/peridotite"/>
	<skos:exactMatch rdf:resource="http://data.bgs.ac.uk/id/EarthMaterialClass/RockName/PDT"/>
	<skos:prefLabel xml:lang="de">Peridotit</skos:prefLabel>
	<colourHexCode xmlns="http://dbpedia.org/ontology/">#D90D99</colourHexCode>
	<dcterms:references rdf:resource="https://resource.geosphere.at/thes/citation/477"/>
	<skos:prefLabel xml:lang="en">Peridotite</skos:prefLabel>
	<dcterms:date rdf:datatype="http://www.w3.org/2001/XMLSchema#dateTime">2011-03-15T15:22:10Z</dcterms:date>
	<dcterms:hasVersion rdf:datatype="http://www.w3.org/2001/XMLSchema#int">9</dcterms:hasVersion>
</rdf:Description>

<rdf:Description rdf:about="https://resource.geosphere.at/thes/lith/61">
	<skos:definition xml:lang="de">Ultramafisches Gestein, welches sich fast gänzlich aus einem oder mehreren Pyroxenmineralien und gelegentlich Biotit, Hornblende und Olivin zusammensetzt (Le Maitre et al., 2005).</skos:definition>
	<skos:exactMatch rdf:resource="http://dbpedia.org/resource/Pyroxenite"/>
	<skos:prefLabel xml:lang="de">Pyroxenit</skos:prefLabel>
	<skos:prefLabel xml:lang="en">Pyroxenite</skos:prefLabel>
	<skos:definition xml:lang="en">Ultramafic rock composed almost entirely of one or more pyroxenes and occasionally biotite, hornblende, or olivine (Le Maitre et al., 2005).</skos:definition>
	<skos:exactMatch rdf:resource="http://data.bgs.ac.uk/id/EarthMaterialClass/RockName/PXT"/>
	<skos:exactMatch rdf:resource="http://resource.geosciml.org/classifier/cgi/lithology/pyroxenite"/>
	<colourHexCode xmlns="http://dbpedia.org/ontology/">#E626A6</colourHexCode>
	<dcterms:date rdf:datatype="http://www.w3.org/2001/XMLSchema#dateTime">2011-03-15T15:22:10Z</dcterms:date>
	<dcterms:references rdf:resource="https://resource.geosphere.at/thes/citation/477"/>
	<dcterms:hasVersion rdf:datatype="http://www.w3.org/2001/XMLSchema#int">7</dcterms:hasVersion>
	<dcterms:created rdf:datatype="http://www.w3.org/2001/XMLSchema#dateTime">2012-03-12T16:01:10.000Z</dcterms:created>
	<skos:exactMatch rdf:resource="http://inspire.ec.europa.eu/codelist/LithologyValue/pyroxenite"/>
	<rdf:type rdf:resource="http://www.w3.org/2004/02/skos/core#Concept"/>
	<skos:exactMatch rdf:resource="http://www.wikidata.org/entity/Q648913"/>
</rdf:Description>

<rdf:Description rdf:about="https://resource.geosphere.at/thes/lith/5">
	<rdf:type rdf:resource="http://www.w3.org/2004/02/skos/core#Concept"/>
	<skos:narrower rdf:resource="https://resource.geosphere.at/thes/lith/18"/>
	<skos:narrower rdf:resource="https://resource.geosphere.at/thes/lith/19"/>
	<skos:narrower rdf:resource="https://resource.geosphere.at/thes/lith/23"/>
	<skos:narrower rdf:resource="https://resource.geosphere.at/thes/lith/24"/>
	<skos:narrower rdf:resource="https://resource.geosphere.at/thes/lith/21"/>
	<skos:narrower rdf:resource="https://resource.geosphere.at/thes/lith/22"/>
	<skos:narrower rdf:resource="https://resource.geosphere.at/thes/lith/20"/>
	<skos:prefLabel xml:lang="en">Plutonic rock</skos:prefLabel>
	<skos:exactMatch rdf:resource="http://resource.geosciml.org/classifier/cgi/lithology/phaneritic_igneous_rock"/>
	<skos:broadMatch rdf:resource="http://inspire.ec.europa.eu/codelist/LithologyValue/igneousRock"/>
	<skos:narrower rdf:resource="https://resource.geosphere.at/thes/lith/251"/>
	<dcterms:date rdf:datatype="http://www.w3.org/2001/XMLSchema#dateTime">2011-03-15T15:22:10Z</dcterms:date>
	<skos:narrower rdf:resource="https://resource.geosphere.at/thes/lith/93"/>
	<skos:narrower rdf:resource="https://resource.geosphere.at/thes/lith/94"/>
	<dcterms:references rdf:resource="https://resource.geosphere.at/thes/citation/477"/>
	<skos:related rdf:resource="https://resource.geosphere.at/thes/lith/6"/>
	<dcterms:created rdf:datatype="http://www.w3.org/2001/XMLSchema#dateTime">2012-01-25T09:32:40.000Z</dcterms:created>
	<skos:narrower rdf:resource="https://resource.geosphere.at/thes/lith/59"/>
	<dcterms:hasVersion rdf:datatype="http://www.w3.org/2001/XMLSchema#int">12</dcterms:hasVersion>
	<skos:narrower rdf:resource="https://resource.geosphere.at/thes/lith/157"/>
	<colourHexCode xmlns="http://dbpedia.org/ontology/">#B300CC</colourHexCode>
</rdf:Description>

<rdf:Description rdf:about="https://resource.geosphere.at/thes/lith/59">
	<rdf:type rdf:resource="http://www.w3.org/2004/02/skos/core#Concept"/>
	<skos:definition xml:lang="en">A plutonic rock consisting of feldspathoids (&gt;60% of the felsic minerals). Defined modally in QAPF-field 15 (Le Maitre et al., 2005).</skos:definition>
	<skos:related rdf:resource="https://resource.geosphere.at/thes/lith/92"/>
	<skos:definition xml:lang="de">Plutonisches Gestein, welches aus Feldspatvertretern (&gt; 60 % der felsischen Minerale) besteht. Modal definiert in QAPF-Feld 15 (Le Maitre et al., 2005).</skos:definition>
	<skos:exactMatch rdf:resource="http://inspire.ec.europa.eu/codelist/LithologyValue/foidolite"/>
	<skos:exactMatch rdf:resource="http://resource.geosciml.org/classifier/cgi/lithology/foidolite"/>
	<skos:prefLabel xml:lang="de">Foidolit</skos:prefLabel>
	<skos:exactMatch rdf:resource="http://data.bgs.ac.uk/id/EarthMaterialClass/RockName/FDO"/>
	<dcterms:references rdf:resource="https://resource.geosphere.at/thes/citation/477"/>
	<skos:prefLabel xml:lang="en">Foidolite</skos:prefLabel>
	<dcterms:date rdf:datatype="http://www.w3.org/2001/XMLSchema#dateTime">2011-03-15T15:22:10Z</dcterms:date>
	<skos:exactMatch rdf:resource="http://dbpedia.org/resource/Foidolite"/>
	<colourHexCode xmlns="http://dbpedia.org/ontology/">#E633B3</colourHexCode>
	<dcterms:hasVersion rdf:datatype="http://www.w3.org/2001/XMLSchema#int">7</dcterms:hasVersion>
	<skos:exactMatch rdf:resource="http://www.wikidata.org/entity/Q2351327"/>
	<dcterms:created rdf:datatype="http://www.w3.org/2001/XMLSchema#dateTime">2012-03-12T13:24:48.000Z</dcterms:created>
</rdf:Description>

<rdf:Description rdf:about="https://resource.geosphere.at/thes/lith/157">
	<skos:related rdf:resource="https://resource.geosphere.at/thes/lith/20"/>
	<skos:definition xml:lang="en">A rock that corresponds to the QAPF 'field' classification for plutonic rocks (Streckeisen, 1976) identified as anorthosite QAPF-field 10 (Le Maitre et al., 2005).</skos:definition>
	<skos:exactMatch rdf:resource="http://inspire.ec.europa.eu/codelist/LithologyValue/anorthositicRock"/>
	<skos:exactMatch rdf:resource="http://resource.geosciml.org/classifier/cgi/lithology/anorthositic_rock"/>
	<skos:related rdf:resource="https://resource.geosphere.at/thes/lith/65"/>
	<dcterms:hasVersion rdf:datatype="http://www.w3.org/2001/XMLSchema#int">24</dcterms:hasVersion>
	<skos:prefLabel xml:lang="de">Anorthositisches Gestein</skos:prefLabel>
	<skos:prefLabel xml:lang="en">Anorthositic rock</skos:prefLabel>
	<dcterms:references rdf:resource="https://resource.geosphere.at/thes/citation/801"/>
	<dcterms:references rdf:resource="https://resource.geosphere.at/thes/citation/477"/>
	<rdf:type rdf:resource="http://www.w3.org/2004/02/skos/core#Concept"/>
	<dcterms:created rdf:datatype="http://www.w3.org/2001/XMLSchema#dateTime">2012-03-12T09:26:34.000Z</dcterms:created>
	<dcterms:date rdf:datatype="http://www.w3.org/2001/XMLSchema#dateTime">2011-03-21T11:53:24Z</dcterms:date>
	<colourHexCode xmlns="http://dbpedia.org/ontology/">#F7ABC4</colourHexCode>
	<skos:narrower rdf:resource="https://resource.geosphere.at/thes/lith/52"/>
	<skos:narrower rdf:resource="https://resource.geosphere.at/thes/lith/50"/>
	<skos:narrower rdf:resource="https://resource.geosphere.at/thes/lith/51"/>
	<skos:definition xml:lang="de">Gestein, welches der QAPF-Gelände-Klassifikation für plutonische Gesteine entspricht (Streckeisen, 1976) und als Anorthosit identifiziert wurde. Modal definiert in QAPF-Feld 10 (Le Maitre et al., 2005).</skos:definition>
</rdf:Description>

<rdf:Description rdf:about="https://resource.geosphere.at/thes/lith/51">
	<skos:exactMatch rdf:resource="http://resource.geosciml.org/classifier/cgi/lithology/anorthosite"/>
	<dcterms:date rdf:datatype="http://www.w3.org/2001/XMLSchema#dateTime">2011-03-15T15:22:10Z</dcterms:date>
	<dcterms:references rdf:resource="https://resource.geosphere.at/thes/citation/477"/>
	<skos:prefLabel xml:lang="de">Anorthosit</skos:prefLabel>
	<dcterms:hasVersion rdf:datatype="http://www.w3.org/2001/XMLSchema#int">10</dcterms:hasVersion>
	<skos:related rdf:resource="https://resource.geosphere.at/thes/lith/50"/>
	<skos:related rdf:resource="https://resource.geosphere.at/thes/lith/52"/>
	<rdf:type rdf:resource="http://www.w3.org/2004/02/skos/core#Concept"/>
	<skos:definition xml:lang="en">A leucocratic plutonic rock consisting essentially of calcic plagioclase, often with small amounts of pyroxene. Defined modally in QAPF-field 10 (Le Maitre et al., 2005).</skos:definition>
	<skos:exactMatch rdf:resource="http://inspire.ec.europa.eu/codelist/LithologyValue/anorthosite"/>
	<skos:prefLabel xml:lang="en">Anorthosite</skos:prefLabel>
	<skos:exactMatch rdf:resource="http://data.bgs.ac.uk/id/EarthMaterialClass/RockName/ANO"/>
	<skos:definition xml:lang="de">Leukokrates plutonisches Gestein, welches hauptsächlich aus Kalzium-Plagioklas und oft kleinen Mengen von Pyroxen besteht. Modal definiert in QAPF-Feld 10 (Le Maitre et al., 2005).</skos:definition>
	<dcterms:created rdf:datatype="http://www.w3.org/2001/XMLSchema#dateTime">2012-03-08T09:41:13.000Z</dcterms:created>
	<colourHexCode xmlns="http://dbpedia.org/ontology/">#FFA3B9</colourHexCode>
</rdf:Description>

<rdf:Description rdf:about="https://resource.geosphere.at/thes/lith/52">
	<skos:related rdf:resource="https://resource.geosphere.at/thes/lith/50"/>
	<skos:related rdf:resource="https://resource.geosphere.at/thes/lith/51"/>
	<dcterms:date rdf:datatype="http://www.w3.org/2001/XMLSchema#dateTime">2011-03-15T15:22:10Z</dcterms:date>
	<skos:definition xml:lang="en">A plutonic rock with the composition of an anorthosite, containing small quantities of feldspathoids (&lt; 10% of the felsic minerals). Defined modally in QAPF-field 10' (Le Maitre et al., 2005).</skos:definition>
	<skos:prefLabel xml:lang="de">Foidführender Anorthosit</skos:prefLabel>
	<dcterms:references rdf:resource="https://resource.geosphere.at/thes/citation/477"/>
	<skos:exactMatch rdf:resource="http://inspire.ec.europa.eu/codelist/LithologyValue/foidBearingAnorthosite"/>
	<skos:exactMatch rdf:resource="http://resource.geosciml.org/classifier/cgi/lithology/foid_bearing_anorthosite"/>
	<skos:definition xml:lang="de">Plutonisches Gestein mit Anorthosit-Zusammensetzung, welches kleine Mengen von Feldspatvertretern beinhaltet (&lt; 10 % der felsischen Minerale). Modal definiert in QAPF-Feld 10' (Le Maitre et al., 2005).</skos:definition>
	<skos:prefLabel xml:lang="en">Foid-bearing anorthosite</skos:prefLabel>
	<rdf:type rdf:resource="http://www.w3.org/2004/02/skos/core#Concept"/>
	<dcterms:created rdf:datatype="http://www.w3.org/2001/XMLSchema#dateTime">2012-03-12T13:18:28.000Z</dcterms:created>
	<dcterms:hasVersion rdf:datatype="http://www.w3.org/2001/XMLSchema#int">10</dcterms:hasVersion>
</rdf:Description>

<rdf:Description rdf:about="https://resource.geosphere.at/thes/lith/50">
	<dcterms:created rdf:datatype="http://www.w3.org/2001/XMLSchema#dateTime">2012-03-12T16:02:15.000Z</dcterms:created>
	<dcterms:date rdf:datatype="http://www.w3.org/2001/XMLSchema#dateTime">2011-03-15T15:22:10Z</dcterms:date>
	<skos:exactMatch rdf:resource="http://resource.geosciml.org/classifier/cgi/lithology/quartz_anorthosite"/>
	<rdf:type rdf:resource="http://www.w3.org/2004/02/skos/core#Concept"/>
	<skos:exactMatch rdf:resource="http://inspire.ec.europa.eu/codelist/LithologyValue/quartzAnorthosite"/>
	<skos:definition xml:lang="en">A leucocratic plutonic rock consisting essentially of calcic plagioclase, quartz, and small amounts of pyroxene. Defined modally in QAPF-field 10* (Le Maitre et al., 2005).</skos:definition>
	<skos:prefLabel xml:lang="de">Quarz-Anorthosit</skos:prefLabel>
	<dcterms:hasVersion rdf:datatype="http://www.w3.org/2001/XMLSchema#int">9</dcterms:hasVersion>
	<skos:definition xml:lang="de">Leukokrates plutonisches Gestein, welches hauptsächlich aus Kalzium-Plagioklas, Quarz und kleinen Mengen Pyroxen besteht. Modal definiert in QAPF-Feld 10* (Le Maitre et al., 2005).</skos:definition>
	<skos:prefLabel xml:lang="en">Quartz anorthosite</skos:prefLabel>
	<skos:related rdf:resource="https://resource.geosphere.at/thes/lith/51"/>
	<skos:related rdf:resource="https://resource.geosphere.at/thes/lith/52"/>
	<dcterms:references rdf:resource="https://resource.geosphere.at/thes/citation/477"/>
</rdf:Description>

<rdf:Description rdf:about="https://resource.geosphere.at/thes/lith/24">
	<skos:definition xml:lang="de">Gestein, welches der QAPF-Gelände-Klassifikation für plutonische Gesteine entspricht (Streckeisen 1976). Es enthält einen wesentlichen Anteil an Foiden; Plagioklas (Anorthitgehalt 50–100 %) überwiegt gegenüber Alkalifeldspat. Modal definiert in QAPF-Feldern 13-14 (Le Maitre et al., 2005).</skos:definition>
	<dcterms:created rdf:datatype="http://www.w3.org/2001/XMLSchema#dateTime">2012-03-12T13:07:25.000Z</dcterms:created>
	<skos:prefLabel xml:lang="en">Foid gabbroic rock</skos:prefLabel>
	<skos:definition xml:lang="en">A rock that corresponds to the QAPF 'field' classification for plutonic rocks (Streckeisen 1976) that contain essential foids and in which plagioclase (anorthite 50-100%) is more abundant than alkali feldspar. QAPF-fields 13-14 (Le Maitre et al., 2005).</skos:definition>
	<rdf:type rdf:resource="http://www.w3.org/2004/02/skos/core#Concept"/>
	<skos:altLabel xml:lang="en">Foid gabbroid</skos:altLabel>
	<skos:altLabel xml:lang="de">Foid-Gabbroid</skos:altLabel>
	<skos:narrower rdf:resource="https://resource.geosphere.at/thes/lith/58"/>
	<skos:narrower rdf:resource="https://resource.geosphere.at/thes/lith/55"/>
	<dcterms:hasVersion rdf:datatype="http://www.w3.org/2001/XMLSchema#int">10</dcterms:hasVersion>
	<skos:exactMatch rdf:resource="http://inspire.ec.europa.eu/codelist/LithologyValue/foidGabbroid"/>
	<dcterms:date rdf:datatype="http://www.w3.org/2001/XMLSchema#dateTime">2011-03-15T15:22:10Z</dcterms:date>
	<colourHexCode xmlns="http://dbpedia.org/ontology/">#F273BF</colourHexCode>
	<dcterms:references rdf:resource="https://resource.geosphere.at/thes/citation/477"/>
	<skos:exactMatch rdf:resource="http://resource.geosciml.org/classifier/cgi/lithology/foid_gabbroid"/>
	<dcterms:references rdf:resource="https://resource.geosphere.at/thes/citation/801"/>
</rdf:Description>

<rdf:Description rdf:about="https://resource.geosphere.at/thes/lith/58">
	<dcterms:hasVersion rdf:datatype="http://www.w3.org/2001/XMLSchema#int">11</dcterms:hasVersion>
	<skos:definition xml:lang="en">An alkaline plutonic rock consisting of feldspathoids (10-60% of the felsic minerals), calcic plagioclase, and large quantities of mafic minerals. Defined modally in QAPF-field 14 (Le Maitre et al., 2005).</skos:definition>
	<skos:related rdf:resource="https://resource.geosphere.at/thes/lith/89"/>
	<skos:definition xml:lang="de">Alkalisches plutonisches Gestein, welches aus Feldspatvertretern (10–60% der felsischen Minerale), Kalzium-Plagioklas und großen Mengen mafischer Minerale besteht. Modal definiert in QAPF-Feld 14 (Le Maitre et al., 2005).</skos:definition>
	<dcterms:date rdf:datatype="http://www.w3.org/2001/XMLSchema#dateTime">2011-03-15T15:22:10Z</dcterms:date>
	<dcterms:references rdf:resource="https://resource.geosphere.at/thes/citation/477"/>
	<skos:exactMatch rdf:resource="http://inspire.ec.europa.eu/codelist/LithologyValue/foidGabbro"/>
	<skos:prefLabel xml:lang="en">Foid gabbro</skos:prefLabel>
	<skos:prefLabel xml:lang="de">Foid-Gabbro</skos:prefLabel>
	<rdf:type rdf:resource="http://www.w3.org/2004/02/skos/core#Concept"/>
	<skos:exactMatch rdf:resource="http://resource.geosciml.org/classifier/cgi/lithology/foid_gabbro"/>
	<dcterms:created rdf:datatype="http://www.w3.org/2001/XMLSchema#dateTime">2012-03-12T13:06:29.000Z</dcterms:created>
	<colourHexCode xmlns="http://dbpedia.org/ontology/">#CE929F</colourHexCode>
</rdf:Description>

<rdf:Description rdf:about="https://resource.geosphere.at/thes/lith/55">
	<skos:exactMatch rdf:resource="http://inspire.ec.europa.eu/codelist/LithologyValue/foidMonzogabbro"/>
	<rdf:type rdf:resource="http://www.w3.org/2004/02/skos/core#Concept"/>
	<skos:definition xml:lang="de">Alkalisches plutonisches Gestein, welches aus Feldspatvertretern (10–60 % der felsischen Minerale), Kalzium-Plagioklas, untergeordnet Alkalifeldspat und großen Mengen mafischer Minerale besteht. Modal definiert in QAPF-Feld 13 (Le Maitre et al., 2005).</skos:definition>
	<skos:prefLabel xml:lang="de">Foid-Monzogabbro</skos:prefLabel>
	<skos:prefLabel xml:lang="en">Foid monzogabbro</skos:prefLabel>
	<skos:definition xml:lang="en">An alkaline plutonic rock consisting of feldspathoids (10-60% of the felsic minerals), calcic plagioclase, subordinate alkali feldspar, and large quantities of mafic minerals. Defined modally in QAPF-field 13 (Le Maitre et al., 2005).</skos:definition>
	<dcterms:hasVersion rdf:datatype="http://www.w3.org/2001/XMLSchema#int">10</dcterms:hasVersion>
	<dcterms:created rdf:datatype="http://www.w3.org/2001/XMLSchema#dateTime">2012-03-12T13:08:26.000Z</dcterms:created>
	<skos:related rdf:resource="https://resource.geosphere.at/thes/lith/87"/>
	<skos:exactMatch rdf:resource="http://resource.geosciml.org/classifier/cgi/lithology/foid_monzogabbro"/>
	<dcterms:references rdf:resource="https://resource.geosphere.at/thes/citation/477"/>
	<dcterms:date rdf:datatype="http://www.w3.org/2001/XMLSchema#dateTime">2011-03-15T15:22:10Z</dcterms:date>
</rdf:Description>

<rdf:Description rdf:about="https://resource.geosphere.at/thes/lith/22">
	<skos:altLabel xml:lang="en">Foid syenitoid</skos:altLabel>
	<dcterms:hasVersion rdf:datatype="http://www.w3.org/2001/XMLSchema#int">11</dcterms:hasVersion>
	<skos:related rdf:resource="https://resource.geosphere.at/thes/lith/67"/>
	<skos:prefLabel xml:lang="de">Foid-syenitisches Gestein</skos:prefLabel>
	<skos:definition xml:lang="en">A rock that corresponds to the QAPF 'field' classification for plutonic rocks (Streckeisen 1976) that contain essential foids and in which alkali feldspar is more abundant than plagioclase. QAPF-fields 11-12 (Le Maitre et al., 2005).</skos:definition>
	<skos:narrower rdf:resource="https://resource.geosphere.at/thes/lith/54"/>
	<skos:narrower rdf:resource="https://resource.geosphere.at/thes/lith/53"/>
	<dcterms:date rdf:datatype="http://www.w3.org/2001/XMLSchema#dateTime">2011-03-15T15:22:10Z</dcterms:date>
	<skos:definition xml:lang="de">Gestein, welches der QAPF-Gelände-Klassifikation für plutonische Gesteine entspricht (Streckeisen, 1976). Es enthält einen wesentlichen Anteil an Foiden; Alkalifeldspat überwiegt gegenüber Plagioklas. Modal definiert in QAPF-Feldern 11-12 (Le Maitre et al., 2005).</skos:definition>
	<dcterms:references rdf:resource="https://resource.geosphere.at/thes/citation/477"/>
	<skos:prefLabel xml:lang="en">Foid syenitic rock</skos:prefLabel>
	<dcterms:references rdf:resource="https://resource.geosphere.at/thes/citation/801"/>
	<skos:exactMatch rdf:resource="http://inspire.ec.europa.eu/codelist/LithologyValue/foidSyenitoid"/>
	<rdf:type rdf:resource="http://www.w3.org/2004/02/skos/core#Concept"/>
	<colourHexCode xmlns="http://dbpedia.org/ontology/">#ED54BA</colourHexCode>
	<skos:altLabel xml:lang="de">Foid-Syenitoid</skos:altLabel>
	<dcterms:created rdf:datatype="http://www.w3.org/2001/XMLSchema#dateTime">2012-03-12T13:10:12.000Z</dcterms:created>
	<skos:exactMatch rdf:resource="http://resource.geosciml.org/classifier/cgi/lithology/foid_syenitoid"/>
</rdf:Description>

<rdf:Description rdf:about="https://resource.geosphere.at/thes/lith/53">
	<dcterms:hasVersion rdf:datatype="http://www.w3.org/2001/XMLSchema#int">8</dcterms:hasVersion>
	<skos:exactMatch rdf:resource="http://inspire.ec.europa.eu/codelist/LithologyValue/foidSyenite"/>
	<skos:definition xml:lang="de">Leukokrates, alkalisches, plutonisches Gestein, welches aus Feldspatvertretern (10–60 % der felsischen Minerale), Alkalifeldspat und mafischen Mineralen besteht. Modal definiert in QAPF-Feld 11 (Le Maitre et al., 2005).</skos:definition>
	<skos:related rdf:resource="https://resource.geosphere.at/thes/lith/84"/>
	<skos:prefLabel xml:lang="en">Foid syenite</skos:prefLabel>
	<dcterms:references rdf:resource="https://resource.geosphere.at/thes/citation/477"/>
	<skos:exactMatch rdf:resource="http://resource.geosciml.org/classifier/cgi/lithology/foid_syenite"/>
	<dcterms:date rdf:datatype="http://www.w3.org/2001/XMLSchema#dateTime">2011-03-15T15:22:10Z</dcterms:date>
	<rdf:type rdf:resource="http://www.w3.org/2004/02/skos/core#Concept"/>
	<dcterms:created rdf:datatype="http://www.w3.org/2001/XMLSchema#dateTime">2012-03-12T13:09:43.000Z</dcterms:created>
	<skos:prefLabel xml:lang="de">Foid-Syenit</skos:prefLabel>
	<skos:definition xml:lang="en">A leucocratic alkaline plutonic rock consisting of feldspathoids (10-60% of the felsic minerals), alkali feldspar, and mafic minerals. Defined modally in QAPF-field 11 (Le Maitre et al., 2005).</skos:definition>
	<colourHexCode xmlns="http://dbpedia.org/ontology/">#FF9EBE</colourHexCode>
</rdf:Description>

<rdf:Description rdf:about="https://resource.geosphere.at/thes/lith/54">
	<dcterms:created rdf:datatype="http://www.w3.org/2001/XMLSchema#dateTime">2012-03-12T13:09:00.000Z</dcterms:created>
	<skos:definition xml:lang="de">Seltenes alkalisches plutonisches Gestein, welches aus Feldspatvertretern, Alkalifeldspat, Plagioklas und mafischen Mineralen besteht. Modal definiert in QAPF-Feld 12 (Le Maitre et al., 2005).</skos:definition>
	<skos:related rdf:resource="https://resource.geosphere.at/thes/lith/85"/>
	<skos:prefLabel xml:lang="en">Foid monzosyenite</skos:prefLabel>
	<dcterms:hasVersion rdf:datatype="http://www.w3.org/2001/XMLSchema#int">10</dcterms:hasVersion>
	<dcterms:date rdf:datatype="http://www.w3.org/2001/XMLSchema#dateTime">2011-03-15T15:22:10Z</dcterms:date>
	<skos:exactMatch rdf:resource="http://resource.geosciml.org/classifier/cgi/lithology/foid_monzosyenite"/>
	<dcterms:references rdf:resource="https://resource.geosphere.at/thes/citation/477"/>
	<skos:exactMatch rdf:resource="http://inspire.ec.europa.eu/codelist/LithologyValue/foidMonzosyenite"/>
	<skos:definition xml:lang="en">A rare alkaline plutonic rock consisting of feldspathoids, alkali feldspar, plagioclase, and mafic minerals. Defined modally in QAPF-field 12 (Le Maitre et al., 2005).</skos:definition>
	<rdf:type rdf:resource="http://www.w3.org/2004/02/skos/core#Concept"/>
	<skos:prefLabel xml:lang="de">Foid-Monzosyenit</skos:prefLabel>
</rdf:Description>

<rdf:Description rdf:about="https://resource.geosphere.at/thes/lith/23">
	<dcterms:created rdf:datatype="http://www.w3.org/2001/XMLSchema#dateTime">2012-03-12T13:05:35.000Z</dcterms:created>
	<skos:altLabel xml:lang="de">Foid-Dioritoid</skos:altLabel>
	<colourHexCode xmlns="http://dbpedia.org/ontology/">#F791C4</colourHexCode>
	<skos:prefLabel xml:lang="en">Foid dioritic rock</skos:prefLabel>
	<skos:exactMatch rdf:resource="http://resource.geosciml.org/classifier/cgi/lithology/foid_dioritoid"/>
	<skos:altLabel xml:lang="en">Foid dioritoid</skos:altLabel>
	<skos:exactMatch rdf:resource="http://inspire.ec.europa.eu/codelist/LithologyValue/foidDioritoid"/>
	<dcterms:references rdf:resource="https://resource.geosphere.at/thes/citation/477"/>
	<dcterms:date rdf:datatype="http://www.w3.org/2001/XMLSchema#dateTime">2011-03-15T15:22:10Z</dcterms:date>
	<dcterms:hasVersion rdf:datatype="http://www.w3.org/2001/XMLSchema#int">12</dcterms:hasVersion>
	<dcterms:references rdf:resource="https://resource.geosphere.at/thes/citation/801"/>
	<skos:definition xml:lang="en">A rock that corresponds to the QAPF 'field' classification for plutonic rocks (Streckeisen 1976) that contain essential foids and in which plagioclase (anorthite 0-50%) is more abundant than alkali feldspar. QAPF-fields 13-14 (Le Maitre et al., 2005).</skos:definition>
	<skos:prefLabel xml:lang="de">Foid-dioritisches Gestein</skos:prefLabel>
	<skos:narrower rdf:resource="https://resource.geosphere.at/thes/lith/56"/>
	<skos:narrower rdf:resource="https://resource.geosphere.at/thes/lith/57"/>
	<skos:definition xml:lang="de">Gestein, welches der QAPF-Gelände-Klassifikation für plutonische Gesteine entspricht (Streckeisen, 1976). Es enthält einen wesentlichen Anteil an Foiden; Plagioklas (Anorthitgehalt 0–50 %) überwiegt gegenüber Alkalifeldspat. Modal definiert in QAPF-Feldern 13-14 (Le Maitre et al., 2005).</skos:definition>
	<rdf:type rdf:resource="http://www.w3.org/2004/02/skos/core#Concept"/>
</rdf:Description>

<rdf:Description rdf:about="https://resource.geosphere.at/thes/lith/57">
	<skos:definition xml:lang="en">An alkaline plutonic rock consisting of feldspathoids (10-60% of the felsic minerals), intermediate plagioclase, and large quantities of mafic minerals. Defined modally in QAPF-field 14 (Le Maitre et al., 2005).</skos:definition>
	<dcterms:created rdf:datatype="http://www.w3.org/2001/XMLSchema#dateTime">2012-03-12T13:05:04.000Z</dcterms:created>
	<dcterms:references rdf:resource="https://resource.geosphere.at/thes/citation/477"/>
	<dcterms:hasVersion rdf:datatype="http://www.w3.org/2001/XMLSchema#int">20</dcterms:hasVersion>
	<dcterms:date rdf:datatype="http://www.w3.org/2001/XMLSchema#dateTime">2011-03-15T15:22:10Z</dcterms:date>
	<skos:exactMatch rdf:resource="http://resource.geosciml.org/classifier/cgi/lithology/foid_diorite"/>
	<rdf:type rdf:resource="http://www.w3.org/2004/02/skos/core#Concept"/>
	<skos:prefLabel xml:lang="en">Foid diorite</skos:prefLabel>
	<skos:definition xml:lang="de">Alkalisches plutonisches Gestein welches aus Feldspatvertretern (10-60% der felsischen Minerale), intermediärem Plagioklas und großen Mengen mafischer Minerale besteht. Modal definiert in QAPF-Feld 14. (Le Maitre et al. 2005)</skos:definition>
	<skos:prefLabel xml:lang="de">Foid-Diorit</skos:prefLabel>
	<skos:related rdf:resource="https://resource.geosphere.at/thes/lith/88"/>
	<skos:exactMatch rdf:resource="http://inspire.ec.europa.eu/codelist/LithologyValue/foidDiorite"/>
	<skos:definition xml:lang="de">Alkalisches plutonisches Gestein, welches aus Feldspatvertretern (10–60% der felsischen Minerale), Kalzium-Plagioklas und großen Mengen mafischer Minerale besteht. Modal definiert in QAPF-Feld 14 (Le Maitre et al., 2005).</skos:definition>
	<colourHexCode xmlns="http://dbpedia.org/ontology/">#E88CA0</colourHexCode>
</rdf:Description>

<rdf:Description rdf:about="https://resource.geosphere.at/thes/lith/56">
	<dcterms:references rdf:resource="https://resource.geosphere.at/thes/citation/477"/>
	<dcterms:hasVersion rdf:datatype="http://www.w3.org/2001/XMLSchema#int">11</dcterms:hasVersion>
	<skos:definition xml:lang="de">Alkalisches plutonisches Gestein, welches aus Feldspatvertretern (10–60 % der felsischen Minerale), intermediärem Plagioklas, untergeordnet Alkalifeldspat und großen Mengen mafischer Minerale besteht. Modal definiert in QAPF-Feld 13 (Le Maitre et al., 2005).</skos:definition>
	<rdf:type rdf:resource="http://www.w3.org/2004/02/skos/core#Concept"/>
	<skos:related rdf:resource="https://resource.geosphere.at/thes/lith/86"/>
	<skos:exactMatch rdf:resource="http://resource.geosciml.org/classifier/cgi/lithology/foid_monzodiorite"/>
	<skos:definition xml:lang="en">An alkaline plutonic rock consisting of feldspathoids (10-60% of the felsic minerals), intermediate plagioclase, subordinate alkali feldspar, and large quantities of mafic minerals. Defined modally in QAPF-field 13 (Le Maitre et al., 2005).</skos:definition>
	<skos:prefLabel xml:lang="en">Foid monzodiorite</skos:prefLabel>
	<skos:exactMatch rdf:resource="http://inspire.ec.europa.eu/codelist/LithologyValue/foidMonzodiorite"/>
	<skos:prefLabel xml:lang="de">Foid-Monzodiorit</skos:prefLabel>
	<dcterms:created rdf:datatype="http://www.w3.org/2001/XMLSchema#dateTime">2012-03-12T13:07:55.000Z</dcterms:created>
	<dcterms:date rdf:datatype="http://www.w3.org/2001/XMLSchema#dateTime">2011-03-15T15:22:10Z</dcterms:date>
</rdf:Description>

<rdf:Description rdf:about="https://resource.geosphere.at/thes/lith/20">
	<skos:related rdf:resource="https://resource.geosphere.at/thes/lith/65"/>
	<skos:related rdf:resource="https://resource.geosphere.at/thes/lith/66"/>
	<dcterms:references rdf:resource="https://resource.geosphere.at/thes/citation/477"/>
	<skos:related rdf:resource="https://resource.geosphere.at/thes/lith/157"/>
	<dcterms:references rdf:resource="https://resource.geosphere.at/thes/citation/801"/>
	<skos:related rdf:resource="https://resource.geosphere.at/thes/lith/21"/>
	<colourHexCode xmlns="http://dbpedia.org/ontology/">#D959A1</colourHexCode>
	<skos:narrower rdf:resource="https://resource.geosphere.at/thes/lith/45"/>
	<skos:narrower rdf:resource="https://resource.geosphere.at/thes/lith/44"/>
	<skos:narrower rdf:resource="https://resource.geosphere.at/thes/lith/46"/>
	<skos:narrower rdf:resource="https://resource.geosphere.at/thes/lith/40"/>
	<dcterms:hasVersion rdf:datatype="http://www.w3.org/2001/XMLSchema#int">16</dcterms:hasVersion>
	<skos:prefLabel xml:lang="de">Dioritisches Gestein</skos:prefLabel>
	<skos:narrower rdf:resource="https://resource.geosphere.at/thes/lith/39"/>
	<skos:narrower rdf:resource="https://resource.geosphere.at/thes/lith/38"/>
	<skos:prefLabel xml:lang="en">Dioritic rock</skos:prefLabel>
	<rdf:type rdf:resource="http://www.w3.org/2004/02/skos/core#Concept"/>
	<skos:exactMatch rdf:resource="http://resource.geosciml.org/classifier/cgi/lithology/dioritic_rock"/>
	<skos:definition xml:lang="de">Gestein, welches der QAPF-Gelände-Klassifikation für plutonische Gesteine entspricht (Streckeisen, 1976) und als Diorit oder Monzodiorit identifiziert wurde. Modal definiert in QAPF-Feldern 9-10 (Le Maitre et al., 2005).</skos:definition>
	<skos:altLabel xml:lang="de">Dioritoid</skos:altLabel>
	<skos:altLabel xml:lang="en">Dioritoid</skos:altLabel>
	<dcterms:created rdf:datatype="http://www.w3.org/2001/XMLSchema#dateTime">2012-03-12T12:44:17.000Z</dcterms:created>
	<skos:definition xml:lang="en">A rock that corresponds to the QAPF 'field' classification for plutonic rocks (Streckeisen 1976) identified as diorite or monzodiorite. QAPF-fields 9-10 (Le Maitre et al., 2005).</skos:definition>
	<skos:exactMatch rdf:resource="http://inspire.ec.europa.eu/codelist/LithologyValue/dioriticRock"/>
	<dcterms:date rdf:datatype="http://www.w3.org/2001/XMLSchema#dateTime">2011-03-15T15:22:10Z</dcterms:date>
</rdf:Description>

<rdf:Description rdf:about="https://resource.geosphere.at/thes/lith/38">
	<dcterms:date rdf:datatype="http://www.w3.org/2001/XMLSchema#dateTime">2011-03-15T15:22:10Z</dcterms:date>
	<dcterms:references rdf:resource="https://resource.geosphere.at/thes/citation/477"/>
	<skos:related rdf:resource="https://resource.geosphere.at/thes/lith/40"/>
	<skos:related rdf:resource="https://resource.geosphere.at/thes/lith/39"/>
	<dcterms:hasVersion rdf:datatype="http://www.w3.org/2001/XMLSchema#int">10</dcterms:hasVersion>
	<skos:prefLabel xml:lang="en">Quartz monzodiorite</skos:prefLabel>
	<skos:definition xml:lang="de">Plutonisches Gestein, welches aus Kalzium-Plagioklas, Alkalifeldspat Quarz und mafischen Mineralen besteht. Modal definiert in QAPF-Feld 9* (Le Maitre et al., 2005).</skos:definition>
	<rdf:type rdf:resource="http://www.w3.org/2004/02/skos/core#Concept"/>
	<skos:prefLabel xml:lang="de">Quarz-Monzodiorit</skos:prefLabel>
	<skos:definition xml:lang="en">A plutonic rock consisting essentially of calcic plagioclase, alkali feldspar, quartz, and mafic minerals. Defined modally in QAPF-field 9* (Le Maitre et al., 2005).</skos:definition>
	<skos:exactMatch rdf:resource="http://resource.geosciml.org/classifier/cgi/lithology/quartz_monzodiorite"/>
	<skos:exactMatch rdf:resource="http://inspire.ec.europa.eu/codelist/LithologyValue/quartzMonzodiorite"/>
	<dcterms:created rdf:datatype="http://www.w3.org/2001/XMLSchema#dateTime">2012-03-12T16:08:38.000Z</dcterms:created>
</rdf:Description>

<rdf:Description rdf:about="https://resource.geosphere.at/thes/lith/46">
	<skos:definition xml:lang="de">Plutonisches Gestein mit Diorit-Zusammensetzung, welches kleine Mengen von Feldspatvertretern beinhaltet (&lt; 10 % der felsischen Minerale). Modal definiert in QAPF-Feld 10' (Le Maitre et al., 2005).</skos:definition>
	<dcterms:created rdf:datatype="http://www.w3.org/2001/XMLSchema#dateTime">2012-03-12T13:19:00.000Z</dcterms:created>
	<skos:prefLabel xml:lang="de">Foidführender Diorit</skos:prefLabel>
	<dcterms:hasVersion rdf:datatype="http://www.w3.org/2001/XMLSchema#int">13</dcterms:hasVersion>
	<skos:prefLabel xml:lang="en">Foid-bearing diorite</skos:prefLabel>
	<skos:exactMatch rdf:resource="http://resource.geosciml.org/classifier/cgi/lithology/foid_bearing_diorite"/>
	<skos:exactMatch rdf:resource="http://inspire.ec.europa.eu/codelist/LithologyValue/foidBearingDiorite"/>
	<dcterms:date rdf:datatype="http://www.w3.org/2001/XMLSchema#dateTime">2011-03-15T15:22:10Z</dcterms:date>
	<dcterms:references rdf:resource="https://resource.geosphere.at/thes/citation/477"/>
	<skos:related rdf:resource="https://resource.geosphere.at/thes/lith/45"/>
	<skos:related rdf:resource="https://resource.geosphere.at/thes/lith/44"/>
	<skos:definition xml:lang="en">A plutonic rock with the composition of a diorite, containing small quantities of feldspathoids (&lt; 10% of the felsic minerals). Defined modally in QAPF-field 10' (Le Maitre et al., 2005).</skos:definition>
	<rdf:type rdf:resource="http://www.w3.org/2004/02/skos/core#Concept"/>
</rdf:Description>

<rdf:Description rdf:about="https://resource.geosphere.at/thes/lith/44">
	<dcterms:references rdf:resource="https://resource.geosphere.at/thes/citation/477"/>
	<skos:definition xml:lang="de">Plutonisches Gestein, welches aus Plagioklas, Quarz und mafischen Mineralen besteht. Modal definiert in QAPF-Feld 10* (Le Maitre et al., 2005).</skos:definition>
	<skos:definition xml:lang="en">A plutonic rock consisting essentially of plagioclase, quartz, and mafic minerals. Defined modally in QAPF-field 10* (Le Maitre et al., 2005).</skos:definition>
	<skos:exactMatch rdf:resource="http://inspire.ec.europa.eu/codelist/LithologyValue/quartzDiorite"/>
	<dcterms:hasVersion rdf:datatype="http://www.w3.org/2001/XMLSchema#int">7</dcterms:hasVersion>
	<rdf:type rdf:resource="http://www.w3.org/2004/02/skos/core#Concept"/>
	<colourHexCode xmlns="http://dbpedia.org/ontology/">#E066A1</colourHexCode>
	<skos:prefLabel xml:lang="en">Quartz diorite</skos:prefLabel>
	<dcterms:created rdf:datatype="http://www.w3.org/2001/XMLSchema#dateTime">2012-03-12T16:04:11.000Z</dcterms:created>
	<skos:related rdf:resource="https://resource.geosphere.at/thes/lith/46"/>
	<skos:exactMatch rdf:resource="http://resource.geosciml.org/classifier/cgi/lithology/quartz_diorite"/>
	<skos:prefLabel xml:lang="de">Quarz-Diorit</skos:prefLabel>
	<skos:related rdf:resource="https://resource.geosphere.at/thes/lith/45"/>
	<dcterms:date rdf:datatype="http://www.w3.org/2001/XMLSchema#dateTime">2011-03-15T15:22:10Z</dcterms:date>
</rdf:Description>

<rdf:Description rdf:about="https://resource.geosphere.at/thes/lith/45">
	<dcterms:created rdf:datatype="http://www.w3.org/2001/XMLSchema#dateTime">2012-03-12T12:42:09.000Z</dcterms:created>
	<skos:related rdf:resource="https://resource.geosphere.at/thes/lith/46"/>
	<skos:related rdf:resource="https://resource.geosphere.at/thes/lith/44"/>
	<dcterms:hasVersion rdf:datatype="http://www.w3.org/2001/XMLSchema#int">15</dcterms:hasVersion>
	<skos:exactMatch rdf:resource="http://data.bgs.ac.uk/id/EarthMaterialClass/RockName/DI"/>
	<skos:definition xml:lang="en">A plutonic rock consisting of intermediate plagioclase, commonly with hornblende, biotite, and augite. Defined modally in QAPF-field 10 (Le Maitre et al., 2005).</skos:definition>
	<dcterms:references rdf:resource="https://resource.geosphere.at/thes/citation/477"/>
	<skos:exactMatch rdf:resource="http://resource.geosciml.org/classifier/cgi/lithology/diorite"/>
	<skos:exactMatch rdf:resource="http://dbpedia.org/resource/Diorite"/>
	<dcterms:date rdf:datatype="http://www.w3.org/2001/XMLSchema#dateTime">2011-03-15T15:22:10Z</dcterms:date>
	<rdf:type rdf:resource="http://www.w3.org/2004/02/skos/core#Concept"/>
	<skos:related rdf:resource="https://resource.geosphere.at/thes/lith/134"/>
	<skos:exactMatch rdf:resource="http://inspire.ec.europa.eu/codelist/LithologyValue/diorite"/>
	<skos:prefLabel xml:lang="de">Diorit</skos:prefLabel>
	<colourHexCode xmlns="http://dbpedia.org/ontology/">#E673A6</colourHexCode>
	<skos:definition xml:lang="de">Plutonisches Gestein, welches aus intermediärem Plagioklas und gewöhnlich Hornblende, oft mit Biotit und Augit besteht. Modal definiert in QAPF-Feld 10 (Le Maitre et al., 2005).</skos:definition>
	<skos:exactMatch rdf:resource="http://www.wikidata.org/entity/Q187408"/>
	<skos:prefLabel xml:lang="en">Diorite</skos:prefLabel>
	<skos:related rdf:resource="https://resource.geosphere.at/thes/lith/83"/>
</rdf:Description>

<rdf:Description rdf:about="https://resource.geosphere.at/thes/lith/40">
	<skos:definition xml:lang="de">Plutonisches Gestein mit Monzodiorit-Zusammensetzung, welches kleine Mengen von Feldspatvertretern beinhaltet (&lt; 10 % der felsischen Minerale). Modal definiert in QAPF-Feld 9' (Le Maitre et al., 2005).</skos:definition>
	<skos:prefLabel xml:lang="de">Foidführender Monzodiorit</skos:prefLabel>
	<dcterms:date rdf:datatype="http://www.w3.org/2001/XMLSchema#dateTime">2011-03-15T15:22:10Z</dcterms:date>
	<dcterms:references rdf:resource="https://resource.geosphere.at/thes/citation/477"/>
	<skos:prefLabel xml:lang="en">Foid-bearing monzodiorite</skos:prefLabel>
	<skos:exactMatch rdf:resource="http://inspire.ec.europa.eu/codelist/LithologyValue/foidBearingMonzodiorite"/>
	<skos:related rdf:resource="https://resource.geosphere.at/thes/lith/39"/>
	<skos:related rdf:resource="https://resource.geosphere.at/thes/lith/38"/>
	<skos:definition xml:lang="en">A plutonic rock with the composition of a monzodiorite, containing small quantities of feldspathoids (&lt; 10% of the felsic minerals). Defined modally in QAPF-field 9' (Le Maitre et al., 2005).</skos:definition>
	<rdf:type rdf:resource="http://www.w3.org/2004/02/skos/core#Concept"/>
	<dcterms:created rdf:datatype="http://www.w3.org/2001/XMLSchema#dateTime">2012-03-12T13:20:46.000Z</dcterms:created>
	<skos:exactMatch rdf:resource="http://resource.geosciml.org/classifier/cgi/lithology/foid_bearing_monzodiorite"/>
	<dcterms:hasVersion rdf:datatype="http://www.w3.org/2001/XMLSchema#int">10</dcterms:hasVersion>
</rdf:Description>

<rdf:Description rdf:about="https://resource.geosphere.at/thes/lith/39">
	<skos:definition xml:lang="de">Plutonisches Gestein mit einer intermediären Zusammensetzung zwischen Monzonit und Diorit. Modal definiert in QAPF-Feld 9 (Le Maitre et al., 2005).</skos:definition>
	<dcterms:date rdf:datatype="http://www.w3.org/2001/XMLSchema#dateTime">2011-03-15T15:22:10Z</dcterms:date>
	<dcterms:references rdf:resource="https://resource.geosphere.at/thes/citation/477"/>
	<skos:definition xml:lang="en">A plutonic rock of gabbroic appearance that contains minor but essential orthoclase, as well as calcic plagioclase. Defined modally in QAPF-field 9 (Le Maitre et al., 2005).</skos:definition>
	<skos:exactMatch rdf:resource="http://resource.geosciml.org/classifier/cgi/lithology/monzodiorite"/>
	<skos:prefLabel xml:lang="de">Monzodiorit</skos:prefLabel>
	<skos:exactMatch rdf:resource="http://data.bgs.ac.uk/id/EarthMaterialClass/RockName/MZDI"/>
	<skos:related rdf:resource="https://resource.geosphere.at/thes/lith/40"/>
	<skos:prefLabel xml:lang="en">Monzodiorite</skos:prefLabel>
	<skos:related rdf:resource="https://resource.geosphere.at/thes/lith/38"/>
	<dcterms:created rdf:datatype="http://www.w3.org/2001/XMLSchema#dateTime">2012-03-12T14:34:41.000Z</dcterms:created>
	<colourHexCode xmlns="http://dbpedia.org/ontology/">#DB61AD</colourHexCode>
	<rdf:type rdf:resource="http://www.w3.org/2004/02/skos/core#Concept"/>
	<skos:exactMatch rdf:resource="http://inspire.ec.europa.eu/codelist/LithologyValue/monzodiorite"/>
	<dcterms:hasVersion rdf:datatype="http://www.w3.org/2001/XMLSchema#int">11</dcterms:hasVersion>
</rdf:Description>

<rdf:Description rdf:about="https://resource.geosphere.at/thes/lith/21">
	<skos:definition xml:lang="en">A rock that corresponds to the QAPF 'field' classification for plutonic rocks (Streckeisen 1976) identified as gabbro or monzogabbro. QAPF-fields 9-10 (Le Maitre et al., 2005).</skos:definition>
	<skos:definition xml:lang="de">Gestein, welches der QAPF-Gelände-Klassifikation für plutonische Gesteine entspricht (Streckeisen, 1976) und als Gabbro oder Monzogabbro identifiziert wurde. Modal definiert in QAPF-Feldern 9-10 (Le Maitre et al., 2005).</skos:definition>
	<dcterms:hasVersion rdf:datatype="http://www.w3.org/2001/XMLSchema#int">15</dcterms:hasVersion>
	<skos:narrower rdf:resource="https://resource.geosphere.at/thes/lith/49"/>
	<skos:narrower rdf:resource="https://resource.geosphere.at/thes/lith/48"/>
	<skos:narrower rdf:resource="https://resource.geosphere.at/thes/lith/47"/>
	<skos:narrower rdf:resource="https://resource.geosphere.at/thes/lith/42"/>
	<skos:narrower rdf:resource="https://resource.geosphere.at/thes/lith/41"/>
	<skos:narrower rdf:resource="https://resource.geosphere.at/thes/lith/43"/>
	<dcterms:references rdf:resource="https://resource.geosphere.at/thes/citation/477"/>
	<skos:prefLabel xml:lang="en">Gabbroic rock</skos:prefLabel>
	<skos:altLabel xml:lang="de">Gabbroid</skos:altLabel>
	<skos:altLabel xml:lang="en">Gabbroid</skos:altLabel>
	<dcterms:date rdf:datatype="http://www.w3.org/2001/XMLSchema#dateTime">2011-03-15T15:22:10Z</dcterms:date>
	<rdf:type rdf:resource="http://www.w3.org/2004/02/skos/core#Concept"/>
	<dcterms:references rdf:resource="https://resource.geosphere.at/thes/citation/801"/>
	<colourHexCode xmlns="http://dbpedia.org/ontology/">#F24073</colourHexCode>
	<skos:exactMatch rdf:resource="http://inspire.ec.europa.eu/codelist/LithologyValue/gabbroicRock"/>
	<skos:related rdf:resource="https://resource.geosphere.at/thes/lith/20"/>
	<dcterms:created rdf:datatype="http://www.w3.org/2001/XMLSchema#dateTime">2012-03-12T13:29:25.000Z</dcterms:created>
	<skos:exactMatch rdf:resource="http://resource.geosciml.org/classifier/cgi/lithology/gabbroid"/>
</rdf:Description>

<rdf:Description rdf:about="https://resource.geosphere.at/thes/lith/48">
	<skos:definition xml:lang="en">A coarse-grained plutonic rock composed essentially of calcic plagioclase, pyroxene, and iron oxides. If olivine is an essential constituent it is an olivine gabbro. Defined modally in QAPF-field 10 (Le Maitre et al., 2005).</skos:definition>
	<skos:exactMatch rdf:resource="http://inspire.ec.europa.eu/codelist/LithologyValue/gabbro"/>
	<skos:related rdf:resource="https://resource.geosphere.at/thes/lith/82"/>
	<skos:related rdf:resource="https://resource.geosphere.at/thes/lith/96"/>
	<skos:definition xml:lang="de">Grobkörniges plutonisches Gestein, welches sich aus Kalzium-Plagioklas, Pyroxen und Eisenoxid zusammensetzt. Bei erheblicher Anwesenheit von Olivin spricht man von Olivin-Gabbro. Modal definiert in QAPF-Feld 10 (Le Maitre et al., 2005).</skos:definition>
	<skos:prefLabel xml:lang="de">Gabbro</skos:prefLabel>
	<skos:prefLabel xml:lang="en">Gabbro</skos:prefLabel>
	<skos:exactMatch rdf:resource="http://data.bgs.ac.uk/id/EarthMaterialClass/RockName/GB"/>
	<skos:exactMatch rdf:resource="http://www.wikidata.org/entity/Q46947"/>
	<dcterms:hasVersion rdf:datatype="http://www.w3.org/2001/XMLSchema#int">13</dcterms:hasVersion>
	<skos:exactMatch rdf:resource="http://dbpedia.org/resource/Gabbro"/>
	<dcterms:date rdf:datatype="http://www.w3.org/2001/XMLSchema#dateTime">2011-03-15T15:22:10Z</dcterms:date>
	<dcterms:references rdf:resource="https://resource.geosphere.at/thes/citation/477"/>
	<rdf:type rdf:resource="http://www.w3.org/2004/02/skos/core#Concept"/>
	<skos:related rdf:resource="https://resource.geosphere.at/thes/lith/142"/>
	<dcterms:created rdf:datatype="http://www.w3.org/2001/XMLSchema#dateTime">2012-09-19T09:47:52.000Z</dcterms:created>
	<colourHexCode xmlns="http://dbpedia.org/ontology/">#F24073</colourHexCode>
	<skos:exactMatch rdf:resource="http://resource.geosciml.org/classifier/cgi/lithology/gabbro"/>
	<foaf:depiction rdf:resource="https://resource.geosphere.at/img/thes/gabbro.jpg"/>
</rdf:Description>

<rdf:Description rdf:about="https://resource.geosphere.at/thes/lith/49">
	<skos:exactMatch rdf:resource="http://inspire.ec.europa.eu/codelist/LithologyValue/foidBearingGabbro"/>
	<skos:prefLabel xml:lang="de">Foidführender Gabbro</skos:prefLabel>
	<dcterms:date rdf:datatype="http://www.w3.org/2001/XMLSchema#dateTime">2011-03-15T15:22:10Z</dcterms:date>
	<rdf:type rdf:resource="http://www.w3.org/2004/02/skos/core#Concept"/>
	<skos:exactMatch rdf:resource="http://resource.geosciml.org/classifier/cgi/lithology/foid_bearing_gabbro"/>
	<dcterms:hasVersion rdf:datatype="http://www.w3.org/2001/XMLSchema#int">7</dcterms:hasVersion>
	<skos:prefLabel xml:lang="en">Foid-bearing gabbro</skos:prefLabel>
	<dcterms:created rdf:datatype="http://www.w3.org/2001/XMLSchema#dateTime">2012-03-12T13:19:38.000Z</dcterms:created>
	<skos:definition xml:lang="en">A plutonic rock with the composition of a gabbro, containing small quantities of feldspathoids (&lt; 10% of the felsic minerals). Defined modally in QAPF-field 10' (Le Maitre et al., 2005).</skos:definition>
	<skos:definition xml:lang="de">Plutonisches Gestein mit Gabbro-Zusammensetzung, welches kleine Mengen von Feldspatvertretern beinhaltet (&lt; 10 % der felsischen Minerale). Modal definiert in QAPF-Feld 10' (Le Maitre et al., 2005).</skos:definition>
	<dcterms:references rdf:resource="https://resource.geosphere.at/thes/citation/477"/>
</rdf:Description>

<rdf:Description rdf:about="https://resource.geosphere.at/thes/lith/47">
	<rdf:type rdf:resource="http://www.w3.org/2004/02/skos/core#Concept"/>
	<skos:prefLabel xml:lang="en">Quartz gabbro</skos:prefLabel>
	<skos:definition xml:lang="de">Plutonisches Gestein, welches aus Kalzium-Plagioklas, Klinopyroxen und Quarz besteht. Modal definiert in QAPF-Feld 10* (Le Maitre et al., 2005).</skos:definition>
	<skos:prefLabel xml:lang="de">Quarz-Gabbro</skos:prefLabel>
	<skos:exactMatch rdf:resource="http://resource.geosciml.org/classifier/cgi/lithology/quartz_gabbro"/>
	<dcterms:references rdf:resource="https://resource.geosphere.at/thes/citation/477"/>
	<dcterms:date rdf:datatype="http://www.w3.org/2001/XMLSchema#dateTime">2011-03-15T15:22:10Z</dcterms:date>
	<dcterms:created rdf:datatype="http://www.w3.org/2001/XMLSchema#dateTime">2012-03-12T16:04:28.000Z</dcterms:created>
	<dcterms:hasVersion rdf:datatype="http://www.w3.org/2001/XMLSchema#int">7</dcterms:hasVersion>
	<skos:exactMatch rdf:resource="http://inspire.ec.europa.eu/codelist/LithologyValue/quartzGabbro"/>
	<skos:definition xml:lang="en">A plutonic rock composed mainly of calcic plagioclase, clinopyroxene, and quartz. Defined modally in QAPF-field 10* (Le Maitre et al., 2005).</skos:definition>
</rdf:Description>

<rdf:Description rdf:about="https://resource.geosphere.at/thes/lith/42">
	<colourHexCode xmlns="http://dbpedia.org/ontology/">#E64073</colourHexCode>
	<skos:prefLabel xml:lang="de">Monzogabbro</skos:prefLabel>
	<skos:prefLabel xml:lang="en">Monzogabbro</skos:prefLabel>
	<skos:exactMatch rdf:resource="http://inspire.ec.europa.eu/codelist/LithologyValue/monzogabbro"/>
	<dcterms:date rdf:datatype="http://www.w3.org/2001/XMLSchema#dateTime">2011-03-15T15:22:10Z</dcterms:date>
	<skos:exactMatch rdf:resource="http://data.bgs.ac.uk/id/EarthMaterialClass/RockName/MZGAB"/>
	<dcterms:created rdf:datatype="http://www.w3.org/2001/XMLSchema#dateTime">2012-01-25T11:51:22.000Z</dcterms:created>
	<skos:exactMatch rdf:resource="http://resource.geosciml.org/classifier/cgi/lithology/monzogabbro"/>
	<skos:definition xml:lang="de">Plutonisches Gestein mit gabbroidem Erscheinungsbild, welches geringfügig Orthoklas und Kalzium-Plagioklas enthält. Modal definiert in QAPF-Feld 9 (Le Maitre et al., 2005).</skos:definition>
	<dcterms:references rdf:resource="https://resource.geosphere.at/thes/citation/477"/>
	<skos:definition xml:lang="en">A plutonic rock of gabbroic aspect that contains minor but essential orthoclase as well as calcic plagioclase. Defined modally in QAPF-field 9 (Le Maitre et al., 2005).</skos:definition>
	<dcterms:hasVersion rdf:datatype="http://www.w3.org/2001/XMLSchema#int">8</dcterms:hasVersion>
	<rdf:type rdf:resource="http://www.w3.org/2004/02/skos/core#Concept"/>
</rdf:Description>

<rdf:Description rdf:about="https://resource.geosphere.at/thes/lith/43">
	<skos:exactMatch rdf:resource="http://resource.geosciml.org/classifier/cgi/lithology/foid_bearing_monzogabbro"/>
	<rdf:type rdf:resource="http://www.w3.org/2004/02/skos/core#Concept"/>
	<skos:exactMatch rdf:resource="http://inspire.ec.europa.eu/codelist/LithologyValue/foidBearingMonzogabbro"/>
	<dcterms:hasVersion rdf:datatype="http://www.w3.org/2001/XMLSchema#int">7</dcterms:hasVersion>
	<skos:definition xml:lang="en">A plutonic rock with the composition of a monzogabbro, containing small quantities of feldspathoids (&lt; 10% of the felsic minerals). Defined modally in QAPF-field 9' (Le Maitre et al., 2005).</skos:definition>
	<skos:prefLabel xml:lang="de">Foidführender Monzogabbro</skos:prefLabel>
	<skos:prefLabel xml:lang="en">Foid-bearing monzogabbro</skos:prefLabel>
	<dcterms:created rdf:datatype="http://www.w3.org/2001/XMLSchema#dateTime">2012-03-12T13:21:19.000Z</dcterms:created>
	<skos:definition xml:lang="de">Plutonisches Gestein mit Monzogabbro-Zusammensetzung, welches kleine Mengen von Feldspatvertretern beinhaltet (&lt; 10 % der felsischen Minerale). Modal definiert in QAPF-Feld 9' (Le Maitre et al., 2005).</skos:definition>
	<dcterms:references rdf:resource="https://resource.geosphere.at/thes/citation/477"/>
	<dcterms:date rdf:datatype="http://www.w3.org/2001/XMLSchema#dateTime">2011-03-15T15:22:10Z</dcterms:date>
</rdf:Description>

<rdf:Description rdf:about="https://resource.geosphere.at/thes/lith/41">
	<dcterms:hasVersion rdf:datatype="http://www.w3.org/2001/XMLSchema#int">8</dcterms:hasVersion>
	<skos:prefLabel xml:lang="de">Quarz-Monzogabbro</skos:prefLabel>
	<skos:definition xml:lang="en">A plutonic rock consisting essentially of calcic plagioclase, alkali feldspar, mafic minerals and quartz. Defined modally in QAPF-field 9* (Le Maitre et al., 2005).</skos:definition>
	<dcterms:date rdf:datatype="http://www.w3.org/2001/XMLSchema#dateTime">2011-03-15T15:22:10Z</dcterms:date>
	<dcterms:references rdf:resource="https://resource.geosphere.at/thes/citation/477"/>
	<skos:exactMatch rdf:resource="http://inspire.ec.europa.eu/codelist/LithologyValue/quartzMonzogabbro"/>
	<rdf:type rdf:resource="http://www.w3.org/2004/02/skos/core#Concept"/>
	<skos:definition xml:lang="de">Plutonisches Gestein, welches aus Kalzium-Plagioklas, Alkalifeldspat, mafischen Mineralen und Quarz besteht. Modal definiert in QAPF-Feld 9* (Le Maitre et al., 2005).</skos:definition>
	<dcterms:created rdf:datatype="http://www.w3.org/2001/XMLSchema#dateTime">2012-03-12T16:09:00.000Z</dcterms:created>
	<skos:exactMatch rdf:resource="http://resource.geosciml.org/classifier/cgi/lithology/quartz_monzogabbro"/>
	<skos:prefLabel xml:lang="en">Quartz monzogabbro</skos:prefLabel>
</rdf:Description>

<rdf:Description rdf:about="https://resource.geosphere.at/thes/lith/19">
	<skos:related rdf:resource="https://resource.geosphere.at/thes/lith/64"/>
	<dcterms:references rdf:resource="https://resource.geosphere.at/thes/citation/477"/>
	<skos:exactMatch rdf:resource="http://inspire.ec.europa.eu/codelist/LithologyValue/syeniticRock"/>
	<colourHexCode xmlns="http://dbpedia.org/ontology/">#FF4DCC</colourHexCode>
	<skos:exactMatch rdf:resource="http://resource.geosciml.org/classifier/cgi/lithology/syenitoid"/>
	<dcterms:references rdf:resource="https://resource.geosphere.at/thes/citation/801"/>
	<dcterms:hasVersion rdf:datatype="http://www.w3.org/2001/XMLSchema#int">11</dcterms:hasVersion>
	<skos:prefLabel xml:lang="en">Syenitic rock</skos:prefLabel>
	<skos:prefLabel xml:lang="de">Syenitisches Gestein</skos:prefLabel>
	<skos:narrower rdf:resource="https://resource.geosphere.at/thes/lith/29"/>
	<skos:narrower rdf:resource="https://resource.geosphere.at/thes/lith/37"/>
	<skos:narrower rdf:resource="https://resource.geosphere.at/thes/lith/33"/>
	<skos:narrower rdf:resource="https://resource.geosphere.at/thes/lith/34"/>
	<skos:narrower rdf:resource="https://resource.geosphere.at/thes/lith/35"/>
	<skos:narrower rdf:resource="https://resource.geosphere.at/thes/lith/36"/>
	<skos:definition xml:lang="en">A rock that corresponds to the QAPF 'field' classification for plutonic rocks (Streckeisen 1976) identified as syenite or monzonite QAPF-fields 6-8 (Le Maitre et al., 2005).</skos:definition>
	<skos:narrower rdf:resource="https://resource.geosphere.at/thes/lith/30"/>
	<rdf:type rdf:resource="http://www.w3.org/2004/02/skos/core#Concept"/>
	<skos:narrower rdf:resource="https://resource.geosphere.at/thes/lith/31"/>
	<skos:narrower rdf:resource="https://resource.geosphere.at/thes/lith/32"/>
	<skos:altLabel xml:lang="de">Syenitoid</skos:altLabel>
	<skos:altLabel xml:lang="en">Syenitoid</skos:altLabel>
	<skos:definition xml:lang="de">Gestein, welches der QAPF-Gelände-Klassifikation für plutonische Gesteine entspricht (Streckeisen, 1976) und als Syenit oder Monzonit identifiziert wurde. Modal definiert in QAPF-Feldern 6-8 (Le Maitre et al., 2005).</skos:definition>
	<dcterms:created rdf:datatype="http://www.w3.org/2001/XMLSchema#dateTime">2012-03-12T16:27:52.000Z</dcterms:created>
	<dcterms:date rdf:datatype="http://www.w3.org/2001/XMLSchema#dateTime">2011-03-15T15:22:10Z</dcterms:date>
</rdf:Description>

<rdf:Description rdf:about="https://resource.geosphere.at/thes/lith/37">
	<dcterms:date rdf:datatype="http://www.w3.org/2001/XMLSchema#dateTime">2011-03-15T15:22:10Z</dcterms:date>
	<skos:exactMatch rdf:resource="http://inspire.ec.europa.eu/codelist/LithologyValue/foidBearingMonzonite"/>
	<skos:prefLabel xml:lang="de">Foidführender Monzonit</skos:prefLabel>
	<rdf:type rdf:resource="http://www.w3.org/2004/02/skos/core#Concept"/>
	<skos:exactMatch rdf:resource="http://resource.geosciml.org/classifier/cgi/lithology/foid_bearing_monzonite"/>
	<dcterms:hasVersion rdf:datatype="http://www.w3.org/2001/XMLSchema#int">10</dcterms:hasVersion>
	<skos:prefLabel xml:lang="en">Foid-bearing monzonite</skos:prefLabel>
	<skos:related rdf:resource="https://resource.geosphere.at/thes/lith/81"/>
	<skos:definition xml:lang="de">Plutonisches Gestein mit Monzonit-Zusammensetzung, welches kleine Mengen von Feldspatvertretern beinhaltet (&lt; 10 % der felsischen Minerale). Modal definiert in QAPF-Feld 8' (Le Maitre et al., 2005).</skos:definition>
	<skos:related rdf:resource="https://resource.geosphere.at/thes/lith/36"/>
	<skos:related rdf:resource="https://resource.geosphere.at/thes/lith/35"/>
	<skos:definition xml:lang="en">A plutonic rock with the composition of a monzonite, containing small quantities of feldspathoids (&lt; 10% of the felsic minerals). Defined modally in QAPF-field 8' (Le Maitre et al., 2005).</skos:definition>
	<dcterms:created rdf:datatype="http://www.w3.org/2001/XMLSchema#dateTime">2012-03-12T13:21:54.000Z</dcterms:created>
	<dcterms:references rdf:resource="https://resource.geosphere.at/thes/citation/477"/>
</rdf:Description>

<rdf:Description rdf:about="https://resource.geosphere.at/thes/lith/35">
	<rdf:type rdf:resource="http://www.w3.org/2004/02/skos/core#Concept"/>
	<dcterms:created rdf:datatype="http://www.w3.org/2001/XMLSchema#dateTime">2012-03-12T16:09:49.000Z</dcterms:created>
	<skos:prefLabel xml:lang="en">Quartz monzonite</skos:prefLabel>
	<skos:related rdf:resource="https://resource.geosphere.at/thes/lith/79"/>
	<skos:prefLabel xml:lang="de">Quarz-Monzonit</skos:prefLabel>
	<skos:definition xml:lang="en">A plutonic rock consisting of approximately equal quantities of plagioclase and alkali feldspar, together with essential quartz (between 5-20% of the felsic mineral content) . Defined modally in QAPF-field 8* (Le Maitre et al., 2005).</skos:definition>
	<skos:definition xml:lang="de">Plutonisches Gestein, welches zu gleichen Anteilen aus Plagioklas und Alkalifeldspat und erheblichen Anteilen Quarz (5–20 % der felsischen Minerale) besteht. Modal definiert in QAPF-Feld 8* (Le Maitre et al., 2005).</skos:definition>
	<dcterms:references rdf:resource="https://resource.geosphere.at/thes/citation/477"/>
	<skos:exactMatch rdf:resource="http://resource.geosciml.org/classifier/cgi/lithology/quartz_monzonite"/>
	<dcterms:date rdf:datatype="http://www.w3.org/2001/XMLSchema#dateTime">2011-03-15T15:22:10Z</dcterms:date>
	<skos:related rdf:resource="https://resource.geosphere.at/thes/lith/36"/>
	<skos:related rdf:resource="https://resource.geosphere.at/thes/lith/37"/>
	<skos:exactMatch rdf:resource="http://inspire.ec.europa.eu/codelist/LithologyValue/quartzMonzonite"/>
	<colourHexCode xmlns="http://dbpedia.org/ontology/">#F24DCC</colourHexCode>
	<dcterms:hasVersion rdf:datatype="http://www.w3.org/2001/XMLSchema#int">9</dcterms:hasVersion>
</rdf:Description>

<rdf:Description rdf:about="https://resource.geosphere.at/thes/lith/36">
	<skos:exactMatch rdf:resource="http://inspire.ec.europa.eu/codelist/LithologyValue/monzonite"/>
	<skos:definition xml:lang="en">A plutonic rock consisting of approximately equal amounts of plagioclase and alkali feldspar, with minor amphibole and/or pyroxene. Defined modally in QAPF-field 8 (Le Maitre et al., 2005).</skos:definition>
	<skos:related rdf:resource="https://resource.geosphere.at/thes/lith/35"/>
	<skos:related rdf:resource="https://resource.geosphere.at/thes/lith/37"/>
	<skos:exactMatch rdf:resource="http://dbpedia.org/resource/Monzonite"/>
	<skos:exactMatch rdf:resource="http://resource.geosciml.org/classifier/cgi/lithology/monzonite"/>
	<skos:related rdf:resource="https://resource.geosphere.at/thes/lith/80"/>
	<colourHexCode xmlns="http://dbpedia.org/ontology/">#F259D4</colourHexCode>
	<skos:exactMatch rdf:resource="http://www.wikidata.org/entity/Q1130233"/>
	<dcterms:created rdf:datatype="http://www.w3.org/2001/XMLSchema#dateTime">2012-03-12T14:35:34.000Z</dcterms:created>
	<skos:definition xml:lang="de">Plutonisches Gestein, welches zu gleichen Anteilen aus Plagioklas und Alkalifeldspat mit wenig Amphibol und/oder Pyroxen besteht. Modal definiert in QAPF-Feld 8 (Le Maitre et al., 2005).</skos:definition>
	<skos:prefLabel xml:lang="de">Monzonit</skos:prefLabel>
	<dcterms:date rdf:datatype="http://www.w3.org/2001/XMLSchema#dateTime">2011-03-15T15:22:10Z</dcterms:date>
	<dcterms:references rdf:resource="https://resource.geosphere.at/thes/citation/477"/>
	<dcterms:hasVersion rdf:datatype="http://www.w3.org/2001/XMLSchema#int">8</dcterms:hasVersion>
	<skos:prefLabel xml:lang="en">Monzonite</skos:prefLabel>
	<rdf:type rdf:resource="http://www.w3.org/2004/02/skos/core#Concept"/>
	<skos:exactMatch rdf:resource="http://data.bgs.ac.uk/id/EarthMaterialClass/RockName/MZ"/>
</rdf:Description>

<rdf:Description rdf:about="https://resource.geosphere.at/thes/lith/33">
	<skos:related rdf:resource="https://resource.geosphere.at/thes/lith/32"/>
	<dcterms:hasVersion rdf:datatype="http://www.w3.org/2001/XMLSchema#int">11</dcterms:hasVersion>
	<skos:related rdf:resource="https://resource.geosphere.at/thes/lith/34"/>
	<skos:exactMatch rdf:resource="http://data.bgs.ac.uk/id/EarthMaterialClass/RockName/SY"/>
	<foaf:depiction rdf:resource="https://resource.geosphere.at/img/thes/AKL_Museum_Syenite.jpg"/>
	<dcterms:references rdf:resource="https://resource.geosphere.at/thes/citation/477"/>
	<dcterms:date rdf:datatype="http://www.w3.org/2001/XMLSchema#dateTime">2011-03-15T15:22:10Z</dcterms:date>
	<skos:exactMatch rdf:resource="http://inspire.ec.europa.eu/codelist/LithologyValue/syenite"/>
	<rdf:type rdf:resource="http://www.w3.org/2004/02/skos/core#Concept"/>
	<skos:definition xml:lang="de">Plutonisches Gestein, welches aus überwiegend Alkalifeldspat und untergeordnet Natrium-Plagioklas, Biotit, Pyroxen, Amphibol manchmal Fayalit besteht. Quarz und Nephelin können als Bestandteile vorkommen. Modal definiert in QAPF-Feld 7 (Le Maitre et al., 2005).</skos:definition>
	<skos:exactMatch rdf:resource="http://dbpedia.org/resource/Syenite"/>
	<skos:prefLabel xml:lang="en">Syenite</skos:prefLabel>
	<skos:definition xml:lang="en">A plutonic rock consisting mainly of alkali feldspar with subordinate sodic plagioclase, biotite, pyroxene, amphibole, and occasionally fayalite. Minor quartz and or nepheline may be present. Defined modally in QAPF-field 7 (Le Maitre et al., 2005).</skos:definition>
	<dcterms:created rdf:datatype="http://www.w3.org/2001/XMLSchema#dateTime">2013-07-12T11:10:48.000Z</dcterms:created>
	<skos:prefLabel xml:lang="de">Syenit</skos:prefLabel>
	<colourHexCode xmlns="http://dbpedia.org/ontology/">#FF66E6</colourHexCode>
	<skos:exactMatch rdf:resource="http://resource.geosciml.org/classifier/cgi/lithology/syenite"/>
	<skos:related rdf:resource="https://resource.geosphere.at/thes/lith/77"/>
</rdf:Description>

<rdf:Description rdf:about="https://resource.geosphere.at/thes/lith/34">
	<dcterms:created rdf:datatype="http://www.w3.org/2001/XMLSchema#dateTime">2012-03-12T13:22:29.000Z</dcterms:created>
	<skos:exactMatch rdf:resource="http://inspire.ec.europa.eu/codelist/LithologyValue/foidBearingSyenite"/>
	<skos:related rdf:resource="https://resource.geosphere.at/thes/lith/78"/>
	<dcterms:hasVersion rdf:datatype="http://www.w3.org/2001/XMLSchema#int">9</dcterms:hasVersion>
	<skos:definition xml:lang="de">Plutonisches Gestein mit Syenit-Zusammensetzung, welches kleine Mengen von Feldspatvertretern beinhaltet (&lt; 10 % der felsischen Minerale). Modal definiert in QAPF-Feld 7' (Le Maitre et al., 2005).</skos:definition>
	<dcterms:date rdf:datatype="http://www.w3.org/2001/XMLSchema#dateTime">2011-03-15T15:22:10Z</dcterms:date>
	<skos:related rdf:resource="https://resource.geosphere.at/thes/lith/33"/>
	<skos:related rdf:resource="https://resource.geosphere.at/thes/lith/32"/>
	<dcterms:references rdf:resource="https://resource.geosphere.at/thes/citation/477"/>
	<skos:prefLabel xml:lang="en">Foid-bearing syenite</skos:prefLabel>
	<rdf:type rdf:resource="http://www.w3.org/2004/02/skos/core#Concept"/>
	<skos:exactMatch rdf:resource="http://resource.geosciml.org/classifier/cgi/lithology/foid_bearing_syenite"/>
	<skos:definition xml:lang="en">A plutonic rock with the composition of a syenite, containing small quantities of feldspathoids (&lt; 10% of the felsic minerals). Defined modally in QAPF-field 7' (Le Maitre et al., 2005).</skos:definition>
	<skos:prefLabel xml:lang="de">Foidführender Syenit</skos:prefLabel>
	<colourHexCode xmlns="http://dbpedia.org/ontology/">#FF73F2</colourHexCode>
</rdf:Description>

<rdf:Description rdf:about="https://resource.geosphere.at/thes/lith/31">
	<skos:related rdf:resource="https://resource.geosphere.at/thes/lith/30"/>
	<skos:exactMatch rdf:resource="http://resource.geosciml.org/classifier/cgi/lithology/foid_bearing_alkali_feldspar_syenite"/>
	<skos:prefLabel xml:lang="de">Foidführender Alkalifeldspat-Syenit</skos:prefLabel>
	<skos:definition xml:lang="en">A plutonic rock with the composition of an alkali feldspar syenite, containing small quantities of feldspathoids (&lt; 10% of the felsic minerals). Defined modally in QAPF-field 6' (Le Maitre et al., 2005).</skos:definition>
	<rdf:type rdf:resource="http://www.w3.org/2004/02/skos/core#Concept"/>
	<dcterms:hasVersion rdf:datatype="http://www.w3.org/2001/XMLSchema#int">8</dcterms:hasVersion>
	<dcterms:created rdf:datatype="http://www.w3.org/2001/XMLSchema#dateTime">2012-03-12T13:16:24.000Z</dcterms:created>
	<skos:related rdf:resource="https://resource.geosphere.at/thes/lith/75"/>
	<skos:exactMatch rdf:resource="http://inspire.ec.europa.eu/codelist/LithologyValue/foidBearingAlkaliFeldsparSyenite"/>
	<dcterms:references rdf:resource="https://resource.geosphere.at/thes/citation/477"/>
	<skos:related rdf:resource="https://resource.geosphere.at/thes/lith/29"/>
	<dcterms:date rdf:datatype="http://www.w3.org/2001/XMLSchema#dateTime">2011-03-15T15:22:10Z</dcterms:date>
	<skos:prefLabel xml:lang="en">Foid-bearing alkali feldspar syenite</skos:prefLabel>
	<skos:definition xml:lang="de">Plutonisches Gestein mit Alkalifeldspat-Syenit-Zusammensetzung, welches kleine Mengen von Feldspatvertretern beinhaltet (&lt; 10 % der felsischen Minerale). Modal definiert in QAPF-Feld 6' (Le Maitre et al., 2005).</skos:definition>
</rdf:Description>

<rdf:Description rdf:about="https://resource.geosphere.at/thes/lith/32">
	<dcterms:references rdf:resource="https://resource.geosphere.at/thes/citation/477"/>
	<skos:related rdf:resource="https://resource.geosphere.at/thes/lith/76"/>
	<skos:related rdf:resource="https://resource.geosphere.at/thes/lith/33"/>
	<skos:related rdf:resource="https://resource.geosphere.at/thes/lith/34"/>
	<skos:definition xml:lang="de">Plutonisches Gestein, welches aus Alkalifeldspat, Quarz und mafischen Mineralen besteht. Modal definiert in QAPF-Feld 7* (Le Maitre et al., 2005).</skos:definition>
	<colourHexCode xmlns="http://dbpedia.org/ontology/">#FF59D9</colourHexCode>
	<dcterms:hasVersion rdf:datatype="http://www.w3.org/2001/XMLSchema#int">8</dcterms:hasVersion>
	<skos:exactMatch rdf:resource="http://resource.geosciml.org/classifier/cgi/lithology/quartz_syenite"/>
	<rdf:type rdf:resource="http://www.w3.org/2004/02/skos/core#Concept"/>
	<skos:prefLabel xml:lang="de">Quarz-Syenit</skos:prefLabel>
	<skos:definition xml:lang="en">A plutonic rock consisting essentially of alkali feldspar, quartz and mafic minerals. Defined modally in QAPF-field 7*. (Le Maitre et al., 2005).</skos:definition>
	<skos:exactMatch rdf:resource="http://inspire.ec.europa.eu/codelist/LithologyValue/quartzSyenite"/>
	<dcterms:created rdf:datatype="http://www.w3.org/2001/XMLSchema#dateTime">2012-03-12T16:10:22.000Z</dcterms:created>
	<skos:prefLabel xml:lang="en">Quartz syenite</skos:prefLabel>
	<dcterms:date rdf:datatype="http://www.w3.org/2001/XMLSchema#dateTime">2011-03-15T15:22:10Z</dcterms:date>
</rdf:Description>

<rdf:Description rdf:about="https://resource.geosphere.at/thes/lith/30">
	<skos:definition xml:lang="en">A plutonic rock and variety of syenite in which plagioclase comprises &lt; 10% of the total feldspar. Defined modally in QAPF-field 6 (Le Maitre et al., 2005).</skos:definition>
	<skos:prefLabel xml:lang="de">Alkalifeldspat-Syenit</skos:prefLabel>
	<skos:exactMatch rdf:resource="http://resource.geosciml.org/classifier/cgi/lithology/alkali_feldspar_syenite"/>
	<skos:related rdf:resource="https://resource.geosphere.at/thes/lith/74"/>
	<skos:prefLabel xml:lang="en">Alkali feldspar syenite</skos:prefLabel>
	<dcterms:date rdf:datatype="http://www.w3.org/2001/XMLSchema#dateTime">2011-03-15T15:22:10Z</dcterms:date>
	<skos:related rdf:resource="https://resource.geosphere.at/thes/lith/29"/>
	<skos:related rdf:resource="https://resource.geosphere.at/thes/lith/31"/>
	<dcterms:references rdf:resource="https://resource.geosphere.at/thes/citation/477"/>
	<dcterms:created rdf:datatype="http://www.w3.org/2001/XMLSchema#dateTime">2012-03-08T09:32:22.000Z</dcterms:created>
	<skos:definition xml:lang="de">Plutonisches Gestein und Varietät von Syenit mit &lt; 10 % Plagioklasanteil am Gesamtfeldspat. Modal definiert in QAPF-Feld 6 (Le Maitre et al., 2005).</skos:definition>
	<skos:exactMatch rdf:resource="http://inspire.ec.europa.eu/codelist/LithologyValue/alkaliFeldsparSyenite"/>
	<rdf:type rdf:resource="http://www.w3.org/2004/02/skos/core#Concept"/>
	<dcterms:hasVersion rdf:datatype="http://www.w3.org/2001/XMLSchema#int">9</dcterms:hasVersion>
</rdf:Description>

<rdf:Description rdf:about="https://resource.geosphere.at/thes/lith/29">
	<skos:prefLabel xml:lang="de">Quarz-Alkalifeldspat-Syenit</skos:prefLabel>
	<skos:definition xml:lang="en">A felsic plutonic rock consisting essentially of alkali feldspar, quartz, and mafic minerals. Defined modally in QAPF-field 6* (Le Maitre et al., 2005).</skos:definition>
	<skos:related rdf:resource="https://resource.geosphere.at/thes/lith/73"/>
	<skos:prefLabel xml:lang="en">Quartz alkali feldspar syenite</skos:prefLabel>
	<skos:exactMatch rdf:resource="http://resource.geosciml.org/classifier/cgi/lithology/quartz_alkali_feldspar_syenite"/>
	<dcterms:date rdf:datatype="http://www.w3.org/2001/XMLSchema#dateTime">2011-03-15T15:22:10Z</dcterms:date>
	<skos:related rdf:resource="https://resource.geosphere.at/thes/lith/30"/>
	<skos:related rdf:resource="https://resource.geosphere.at/thes/lith/31"/>
	<dcterms:references rdf:resource="https://resource.geosphere.at/thes/citation/477"/>
	<dcterms:created rdf:datatype="http://www.w3.org/2001/XMLSchema#dateTime">2012-03-12T16:01:44.000Z</dcterms:created>
	<skos:exactMatch rdf:resource="http://inspire.ec.europa.eu/codelist/LithologyValue/quartzAlkaliFeldsparSyenite"/>
	<rdf:type rdf:resource="http://www.w3.org/2004/02/skos/core#Concept"/>
	<skos:definition xml:lang="de">Felsisches plutonisches Gestein, welches aus Alkalifeldspat, Quarz und mafischen Mineralen besteht. Modal definiert in QAPF-Feld 6* (Le Maitre et al., 2005).</skos:definition>
	<dcterms:hasVersion rdf:datatype="http://www.w3.org/2001/XMLSchema#int">8</dcterms:hasVersion>
</rdf:Description>

<rdf:Description rdf:about="https://resource.geosphere.at/thes/lith/18">
	<colourHexCode xmlns="http://dbpedia.org/ontology/">#FF3333</colourHexCode>
	<dcterms:created rdf:datatype="http://www.w3.org/2001/XMLSchema#dateTime">2013-05-28T14:04:06.000Z</dcterms:created>
	<dcterms:references rdf:resource="https://resource.geosphere.at/thes/citation/801"/>
	<skos:altLabel xml:lang="de">Granitoid</skos:altLabel>
	<skos:altLabel xml:lang="en">Granitoid</skos:altLabel>
	<status xmlns="https://resource.geosphere.at/schema/thes#" rdf:datatype="http://www.w3.org/2001/XMLSchema#integer">1</status>
	<rdf:type rdf:resource="http://www.w3.org/2004/02/skos/core#Concept"/>
	<skos:definition xml:lang="en">A rock that corresponds to the QAPF 'field' classification for plutonic rocks (Streckeisen 1976) identified as granite, granodiorite, or tonalite. QAPF-fields 2– 5. (Le Maitre et al., 2005)</skos:definition>
	<skos:prefLabel xml:lang="de">Granitisches Gestein</skos:prefLabel>
	<foaf:depiction rdf:resource="https://resource.geosphere.at/img/thes/Granit.jpg"/>
	<skos:narrower rdf:resource="https://resource.geosphere.at/thes/lith/28"/>
	<skos:narrower rdf:resource="https://resource.geosphere.at/thes/lith/25"/>
	<skos:narrower rdf:resource="https://resource.geosphere.at/thes/lith/26"/>
	<skos:narrower rdf:resource="https://resource.geosphere.at/thes/lith/27"/>
	<dcterms:hasVersion rdf:datatype="http://www.w3.org/2001/XMLSchema#int">15</dcterms:hasVersion>
	<skos:prefLabel xml:lang="en">Granitic rock</skos:prefLabel>
	<skos:exactMatch rdf:resource="http://resource.geosciml.org/classifier/cgi/lithology/granitoid"/>
	<skos:related rdf:resource="https://resource.geosphere.at/thes/lith/62"/>
	<skos:related rdf:resource="https://resource.geosphere.at/thes/lith/63"/>
	<skos:exactMatch rdf:resource="http://inspire.ec.europa.eu/codelist/LithologyValue/granitoid"/>
	<skos:definition xml:lang="de">Gestein, welches der QAPF-Gelände-Klassifikation für plutonische Gesteine entspricht (Streckeisen, 1976) und als Granit, Granodiorit oder Tonalit identifiziert wurde. Modal definiert in QAPF-Feldern 2– 5. (Le Maitre et al., 2005)</skos:definition>
	<dcterms:references rdf:resource="https://resource.geosphere.at/thes/citation/477"/>
	<dcterms:date rdf:datatype="http://www.w3.org/2001/XMLSchema#dateTime">2011-03-15T15:22:10Z</dcterms:date>
</rdf:Description>

<rdf:Description rdf:about="https://resource.geosphere.at/thes/lith/26">
	<skos:exactMatch rdf:resource="http://inspire.ec.europa.eu/codelist/LithologyValue/granite"/>
	<foaf:depiction rdf:resource="https://resource.geosphere.at/img/thes/Granit.jpg"/>
	<colourHexCode xmlns="http://dbpedia.org/ontology/">#FF4D4D</colourHexCode>
	<skos:definition xml:lang="en">A plutonic rock consisting essentially of quartz, alkali feldspar, and sodic plagioclase in various proportions, usually with biotite and/or hornblende. Defined modally in QAPF-field 3 (Le Maitre et al., 2005).</skos:definition>
	<dcterms:references rdf:resource="https://resource.geosphere.at/thes/citation/477"/>
	<skos:exactMatch rdf:resource="http://dbpedia.org/resource/Granite"/>
	<dcterms:date rdf:datatype="http://www.w3.org/2001/XMLSchema#dateTime">2011-03-15T15:22:10Z</dcterms:date>
	<skos:exactMatch rdf:resource="http://resource.geosciml.org/classifier/cgi/lithology/granite"/>
	<dcterms:hasVersion rdf:datatype="http://www.w3.org/2001/XMLSchema#int">40</dcterms:hasVersion>
	<rdf:type rdf:resource="http://www.w3.org/2004/02/skos/core#Concept"/>
	<skos:related rdf:resource="https://resource.geosphere.at/thes/lith/143"/>
	<skos:prefLabel xml:lang="de">Granit</skos:prefLabel>
	<skos:exactMatch rdf:resource="http://data.bgs.ac.uk/id/EarthMaterialClass/RockName/GN"/>
	<skos:prefLabel xml:lang="en">Granite</skos:prefLabel>
	<skos:definition xml:lang="de">Plutonisches Gestein, welches aus Quarz, Alkalifeldspat und Natrium-Plagioklas in unterschiedlichen Anteilen besteht, gewöhnlich mit Biotit und/oder Hornblende. Modal definiert in QAPF-Feld 3 (Le Maitre et al., 2005).</skos:definition>
	<skos:exactMatch rdf:resource="http://www.wikidata.org/entity/Q41177"/>
	<dcterms:created rdf:datatype="http://www.w3.org/2001/XMLSchema#dateTime">2013-10-21T07:09:51.000Z</dcterms:created>
</rdf:Description>

<rdf:Description rdf:about="https://resource.geosphere.at/thes/lith/27">
	<skos:exactMatch rdf:resource="http://resource.geosciml.org/classifier/cgi/lithology/granodiorite"/>
	<skos:exactMatch rdf:resource="http://data.bgs.ac.uk/id/EarthMaterialClass/RockName/GD"/>
	<skos:definition xml:lang="en">A plutonic rock consisting essentially of quartz, sodic plagioclase, and smaller quantities of alkali feldspar, together with minor biotite and hornblende. Defined modally in QAPF-field 4 (Le Maitre et al., 2005).</skos:definition>
	<dcterms:hasVersion rdf:datatype="http://www.w3.org/2001/XMLSchema#int">8</dcterms:hasVersion>
	<skos:related rdf:resource="https://resource.geosphere.at/thes/lith/72"/>
	<skos:exactMatch rdf:resource="http://dbpedia.org/resource/Granodiorite"/>
	<dcterms:references rdf:resource="https://resource.geosphere.at/thes/citation/477"/>
	<dcterms:date rdf:datatype="http://www.w3.org/2001/XMLSchema#dateTime">2011-03-15T15:22:10Z</dcterms:date>
	<colourHexCode xmlns="http://dbpedia.org/ontology/">#FF8080</colourHexCode>
	<skos:definition xml:lang="de">Plutonisches Gestein, welches aus Quarz, Natrium-Plagioklas, geringeren Anteilen Alkalifeldspat und untergeordnet Biotit und Hornblende besteht. Modal definiert in QAPF-Feld 4 (Le Maitre et al., 2005).</skos:definition>
	<skos:prefLabel xml:lang="de">Granodiorit</skos:prefLabel>
	<skos:exactMatch rdf:resource="http://inspire.ec.europa.eu/codelist/LithologyValue/granodiorite"/>
	<rdf:type rdf:resource="http://www.w3.org/2004/02/skos/core#Concept"/>
	<skos:exactMatch rdf:resource="http://www.wikidata.org/entity/Q215690"/>
	<dcterms:created rdf:datatype="http://www.w3.org/2001/XMLSchema#dateTime">2012-03-12T13:39:34.000Z</dcterms:created>
	<skos:prefLabel xml:lang="en">Granodiorite</skos:prefLabel>
</rdf:Description>

<rdf:Description rdf:about="https://resource.geosphere.at/thes/lith/25">
	<skos:definition xml:lang="en">A plutonic rock and a variety of granite in which plagioclase comprises &lt; 10% of the total feldspar. Defined modally in QAPF-field 2 (Le Maitre et al., 2005).</skos:definition>
	<dcterms:date rdf:datatype="http://www.w3.org/2001/XMLSchema#dateTime">2011-03-15T15:22:10Z</dcterms:date>
	<skos:exactMatch rdf:resource="http://inspire.ec.europa.eu/codelist/LithologyValue/alkaliFeldsparGranite"/>
	<rdf:type rdf:resource="http://www.w3.org/2004/02/skos/core#Concept"/>
	<skos:definition xml:lang="de">Plutonisches Gestein und Varietät von Granit mit &lt; 10 % Plagioklasanteil am Gesamtfeldspat. Modal definiert in QAPF-Feld 2 (Le Maitre et al., 2005).</skos:definition>
	<skos:prefLabel xml:lang="en">Alkali feldspar granite</skos:prefLabel>
	<dcterms:hasVersion rdf:datatype="http://www.w3.org/2001/XMLSchema#int">8</dcterms:hasVersion>
	<skos:related rdf:resource="https://resource.geosphere.at/thes/lith/70"/>
	<dcterms:created rdf:datatype="http://www.w3.org/2001/XMLSchema#dateTime">2012-03-08T09:31:37.000Z</dcterms:created>
	<skos:exactMatch rdf:resource="http://resource.geosciml.org/classifier/cgi/lithology/alkali_feldspar_granite"/>
	<skos:prefLabel xml:lang="de">Alkalifeldspat-Granit</skos:prefLabel>
	<dcterms:references rdf:resource="https://resource.geosphere.at/thes/citation/477"/>
</rdf:Description>

<rdf:Description rdf:about="https://resource.geosphere.at/thes/lith/28">
	<dcterms:hasVersion rdf:datatype="http://www.w3.org/2001/XMLSchema#int">7</dcterms:hasVersion>
	<colourHexCode xmlns="http://dbpedia.org/ontology/">#FF6666</colourHexCode>
	<skos:exactMatch rdf:resource="http://resource.geosciml.org/classifier/cgi/lithology/tonalite"/>
	<skos:exactMatch rdf:resource="http://data.bgs.ac.uk/id/EarthMaterialClass/RockName/TO"/>
	<skos:exactMatch rdf:resource="http://inspire.ec.europa.eu/codelist/LithologyValue/tonalite"/>
	<dcterms:references rdf:resource="https://resource.geosphere.at/thes/citation/477"/>
	<dcterms:date rdf:datatype="http://www.w3.org/2001/XMLSchema#dateTime">2011-03-15T15:22:10Z</dcterms:date>
	<skos:related rdf:resource="https://resource.geosphere.at/thes/lith/72"/>
	<rdf:type rdf:resource="http://www.w3.org/2004/02/skos/core#Concept"/>
	<skos:definition xml:lang="en">A plutonic rock consisting essentially of quartz, intermediate plagioclase, and usually biotite and amphibole. Defined modally in QAPF-field 5 (Le Maitre et al., 2005).</skos:definition>
	<skos:related rdf:resource="https://resource.geosphere.at/thes/lith/135"/>
	<skos:definition xml:lang="de">Plutonisches Gestein, welches aus Quarz, intermediärem Plagioklas und gewöhnlich Biotit und Amphibol besteht. Modal definiert in QAPF-Feld 5 (Le Maitre et al., 2005).</skos:definition>
	<skos:prefLabel xml:lang="de">Tonalit</skos:prefLabel>
	<skos:prefLabel xml:lang="en">Tonalite</skos:prefLabel>
	<dcterms:created rdf:datatype="http://www.w3.org/2001/XMLSchema#dateTime">2012-03-12T16:31:07.000Z</dcterms:created>
	<skos:exactMatch rdf:resource="http://dbpedia.org/resource/Tonalite"/>
</rdf:Description>

<rdf:Description rdf:about="https://resource.geosphere.at/thes/lith/95">
	<dcterms:hasVersion rdf:datatype="http://www.w3.org/2001/XMLSchema#int">13</dcterms:hasVersion>
	<skos:prefLabel xml:lang="de">Lamprophyr</skos:prefLabel>
	<skos:exactMatch rdf:resource="http://www.wikidata.org/entity/Q774790"/>
	<skos:exactMatch rdf:resource="http://dbpedia.org/resource/Lamprophyre"/>
	<dcterms:date rdf:datatype="http://www.w3.org/2001/XMLSchema#dateTime">2011-03-15T15:22:10Z</dcterms:date>
	<dcterms:references rdf:resource="https://resource.geosphere.at/thes/citation/477"/>
	<skos:broadMatch rdf:resource="http://resource.geosciml.org/classifier/cgi/lithology/exotic_alkaline_rock"/>
	<rdf:type rdf:resource="http://www.w3.org/2004/02/skos/core#Concept"/>
	<skos:prefLabel xml:lang="en">Lamprophyre</skos:prefLabel>
	<skos:broadMatch rdf:resource="http://inspire.ec.europa.eu/codelist/LithologyValue/exoticAlkalineRock"/>
	<dcterms:created rdf:datatype="http://www.w3.org/2001/XMLSchema#dateTime">2012-03-12T13:54:32.000Z</dcterms:created>
	<colourHexCode xmlns="http://dbpedia.org/ontology/">#B300B3</colourHexCode>
</rdf:Description>

<rdf:Description rdf:about="https://resource.geosphere.at/thes/lith/93">
	<dcterms:date rdf:datatype="http://www.w3.org/2001/XMLSchema#dateTime">2011-03-15T15:22:10Z</dcterms:date>
	<skos:exactMatch rdf:resource="http://inspire.ec.europa.eu/codelist/LithologyValue/aplite"/>
	<colourHexCode xmlns="http://dbpedia.org/ontology/">#FFCC33</colourHexCode>
	<skos:definition xml:lang="de">Helles (leukokrates) plutonisches Gestein, welches durch eine feinkörnige, allotriomorphe, granulare Textur gekennzeichnet ist. Besitzt üblicherweise granitische Zusammensetzung mit Quarz, Alkalifeldspat und Natrium-Plagioklas (Neuendorf et al., 2005).</skos:definition>
	<dcterms:references rdf:resource="https://resource.geosphere.at/thes/citation/545"/>
	<dcterms:hasVersion rdf:datatype="http://www.w3.org/2001/XMLSchema#int">10</dcterms:hasVersion>
	<skos:prefLabel xml:lang="en">Aplite</skos:prefLabel>
	<rdf:type rdf:resource="http://www.w3.org/2004/02/skos/core#Concept"/>
	<skos:prefLabel xml:lang="de">Aplit</skos:prefLabel>
	<skos:exactMatch rdf:resource="http://resource.geosciml.org/classifier/cgi/lithology/aplite"/>
	<skos:definition xml:lang="en">A light coloured (leucocratic) igneous rock characterised by a fine-grained allotriomorphic-granular texture, usually with a granitic composition consisting of quartz, alkali feldspar, and sodic plagioclase (Neuendorf et al., 2005).</skos:definition>
	<skos:exactMatch rdf:resource="http://dbpedia.org/resource/Aplite"/>
	<dcterms:created rdf:datatype="http://www.w3.org/2001/XMLSchema#dateTime">2012-03-12T09:28:53.000Z</dcterms:created>
</rdf:Description>

<rdf:Description rdf:about="https://resource.geosphere.at/thes/lith/94">
	<dcterms:hasVersion rdf:datatype="http://www.w3.org/2001/XMLSchema#int">10</dcterms:hasVersion>
	<skos:exactMatch rdf:resource="http://data.bgs.ac.uk/id/EarthMaterialClass/RockName/PEG"/>
	<skos:prefLabel xml:lang="de">Pegmatit</skos:prefLabel>
	<dcterms:date rdf:datatype="http://www.w3.org/2001/XMLSchema#dateTime">2011-03-15T15:22:10Z</dcterms:date>
	<rdf:type rdf:resource="http://www.w3.org/2004/02/skos/core#Concept"/>
	<skos:definition xml:lang="en">An exceptionally coarse-grained igneous rock with interlocking crystals, most of which are &gt; 1cm in diameter. The composition of pegmatites is usually granitic but can also be similar to other igneous rock types. Pegmatites usually occur as irregular dykes, lenses, or veins associated with plutons or batholiths (Neuendorf et al., 2005).</skos:definition>
	<skos:prefLabel xml:lang="en">Pegmatite</skos:prefLabel>
	<dcterms:references rdf:resource="https://resource.geosphere.at/thes/citation/545"/>
	<skos:exactMatch rdf:resource="http://resource.geosciml.org/classifier/cgi/lithology/pegmatite"/>
	<colourHexCode xmlns="http://dbpedia.org/ontology/">#FFB219</colourHexCode>
	<dcterms:created rdf:datatype="http://www.w3.org/2001/XMLSchema#dateTime">2012-03-12T15:53:37.000Z</dcterms:created>
	<skos:exactMatch rdf:resource="http://dbpedia.org/resource/Pegmatite"/>
	<skos:definition xml:lang="de">Außergewöhnlich grobkörniges plutonisches Gestein mit ineinander verzahnten Kristallen, die meistens einen Durchmesser &gt; 1 cm haben. Pegmatite besitzen typischerweise eine granitische Zusammensetzung, der Begriff kann sich jedoch auch auf grobkörnige plutonische Gesteine mit anderer Zusammensetzung beziehen. Pegmatite kommen in Form von Dykes, Linsen oder Adern vor, die mit Plutonen oder Batholiten assoziiert sind (Neuendorf et al., 2005).</skos:definition>
	<skos:exactMatch rdf:resource="http://inspire.ec.europa.eu/codelist/LithologyValue/pegmatite"/>
	<skos:exactMatch rdf:resource="http://www.wikidata.org/entity/Q105630"/>
</rdf:Description>

<rdf:Description rdf:about="https://resource.geosphere.at/thes/lith/251">
	<rdf:type rdf:resource="http://www.w3.org/2004/02/skos/core#Concept"/>
	<dcterms:references rdf:resource="https://resource.geosphere.at/thes/citation/477"/>
	<skos:broadMatch rdf:resource="http://inspire.ec.europa.eu/codelist/LithologyValue/acidicIgneousRock"/>
	<skos:definition xml:lang="en">A collective term for plutonic rocks in which the quartz content is more than 90% of the felsic minerals. Now defined modally in QAPF (Streckeisen, 1973) field 1a (Le Maitre et al., 2005). </skos:definition>
	<skos:definition xml:lang="de">Ein Sammelbegriff für plutonische Gesteine, in welchen der Quarzgehalt &gt;90% der felsischen Mineralien ist. Definiert im QAPF (Streckeisen, 1973) - Feld 1a (Le Maitre et al., 2005).</skos:definition>
	<skos:prefLabel xml:lang="de">Quarzolith</skos:prefLabel>
	<skos:prefLabel xml:lang="en">Quartzolite</skos:prefLabel>
	<dcterms:created rdf:datatype="http://www.w3.org/2001/XMLSchema#dateTime">2015-08-19T11:25:45.000Z</dcterms:created>
	<skos:broadMatch rdf:resource="http://resource.geosciml.org/classifier/cgi/lithology/quartz_rich_igneous_rock"/>
</rdf:Description>

<rdf:Description rdf:about="https://resource.geosphere.at/thes/lith/97">
	<skos:related rdf:resource="https://resource.geosphere.at/thes/lith/158"/>
	<skos:prefLabel xml:lang="en">Composite genesis material</skos:prefLabel>
	<dcterms:references rdf:resource="https://resource.geosphere.at/thes/citation/546"/>
	<skos:narrower rdf:resource="https://resource.geosphere.at/thes/lith/146"/>
	<skos:exactMatch rdf:resource="http://inspire.ec.europa.eu/codelist/LithologyValue/compositeGenesisMaterial"/>
	<skos:prefLabel xml:lang="de">Polygenetisches Material</skos:prefLabel>
	<dcterms:date rdf:datatype="http://www.w3.org/2001/XMLSchema#dateTime">2011-03-16T09:19:05Z</dcterms:date>
	<dcterms:hasVersion rdf:datatype="http://www.w3.org/2001/XMLSchema#int">10</dcterms:hasVersion>
	<skos:exactMatch rdf:resource="http://resource.geosciml.org/classifier/cgi/lithology/composite_genesis_material"/>
	<rdf:type rdf:resource="http://www.w3.org/2004/02/skos/core#Concept"/>
	<skos:narrower rdf:resource="https://resource.geosphere.at/thes/lith/155"/>
	<skos:narrower rdf:resource="https://resource.geosphere.at/thes/lith/156"/>
	<skos:narrower rdf:resource="https://resource.geosphere.at/thes/lith/98"/>
	<colourHexCode xmlns="http://dbpedia.org/ontology/">#A6D9CC</colourHexCode>
	<dcterms:created rdf:datatype="http://www.w3.org/2001/XMLSchema#dateTime">2012-03-12T12:18:50.000Z</dcterms:created>
</rdf:Description>

<rdf:Description rdf:about="https://resource.geosphere.at/thes/lith/146">
	<skos:definition xml:lang="en">Material formed by mechanical (brittle and/or ductile) deformation in faults (Heitzmann, 1985).</skos:definition>
	<dcterms:hasVersion rdf:datatype="http://www.w3.org/2001/XMLSchema#int">9</dcterms:hasVersion>
	<skos:exactMatch rdf:resource="http://inspire.ec.europa.eu/codelist/LithologyValue/faultRelatedMaterial"/>
	<skos:prefLabel xml:lang="en">Fault-related material</skos:prefLabel>
	<colourHexCode xmlns="http://dbpedia.org/ontology/">#E6E600</colourHexCode>
	<skos:narrower rdf:resource="https://resource.geosphere.at/thes/lith/147"/>
	<dcterms:references rdf:resource="https://resource.geosphere.at/thes/citation/271"/>
	<skos:narrower rdf:resource="https://resource.geosphere.at/thes/lith/154"/>
	<skos:narrower rdf:resource="https://resource.geosphere.at/thes/lith/153"/>
	<skos:narrower rdf:resource="https://resource.geosphere.at/thes/lith/152"/>
	<rdf:type rdf:resource="http://www.w3.org/2004/02/skos/core#Concept"/>
	<skos:definition xml:lang="de">Material, welches durch überwiegend mechanische (spröde und/oder duktile) Deformation in Störungen gebildet wird (Heitzmann, 1985).</skos:definition>
	<skos:exactMatch rdf:resource="http://resource.geosciml.org/classifier/cgi/lithology/fault_related_material"/>
	<dcterms:created rdf:datatype="http://www.w3.org/2001/XMLSchema#dateTime">2012-03-12T12:58:58.000Z</dcterms:created>
	<skos:prefLabel xml:lang="de">Störungsmaterial</skos:prefLabel>
	<dcterms:date rdf:datatype="http://www.w3.org/2001/XMLSchema#dateTime">2011-03-16T09:19:05Z</dcterms:date>
</rdf:Description>

<rdf:Description rdf:about="https://resource.geosphere.at/thes/lith/147">
	<dcterms:created rdf:datatype="http://www.w3.org/2001/XMLSchema#dateTime">2012-01-25T13:44:36.000Z</dcterms:created>
	<skos:prefLabel xml:lang="de">Störungsgestein</skos:prefLabel>
	<skos:prefLabel xml:lang="en">Fault rock</skos:prefLabel>
	<skos:narrower rdf:resource="https://resource.geosphere.at/thes/lith/243"/>
	<skos:broadMatch rdf:resource="http://resource.geosciml.org/classifier/cgi/lithology/fault_related_material"/>
	<skos:closeMatch rdf:resource="http://dbpedia.org/resource/Fault_block"/>
	<skos:narrower rdf:resource="https://resource.geosphere.at/thes/lith/151"/>
	<skos:narrower rdf:resource="https://resource.geosphere.at/thes/lith/150"/>
	<rdf:type rdf:resource="http://www.w3.org/2004/02/skos/core#Concept"/>
	<skos:exactMatch rdf:resource="http://inspire.ec.europa.eu/codelist/LithologyValue/faultRelatedMaterial"/>
	<skos:narrower rdf:resource="https://resource.geosphere.at/thes/lith/148"/>
	<skos:definition xml:lang="en">A rock formed as a result of deformation in a fault zone (Fettes &amp; Desmons, 2007).</skos:definition>
	<dcterms:hasVersion rdf:datatype="http://www.w3.org/2001/XMLSchema#int">8</dcterms:hasVersion>
	<dcterms:date rdf:datatype="http://www.w3.org/2001/XMLSchema#dateTime">2011-03-16T09:19:05Z</dcterms:date>
	<dcterms:references rdf:resource="https://resource.geosphere.at/thes/citation/216"/>
	<skos:definition xml:lang="de">Gestein, welches durch Deformation in einer Störungszone entsteht (Fettes &amp; Desmons, 2007).</skos:definition>
</rdf:Description>

<rdf:Description rdf:about="https://resource.geosphere.at/thes/lith/148">
	<skos:definition xml:lang="en">A fault rock which is cohesive and characterised by a well-developed schistosity resulting from a tectonic reduction in grain size within a ductile shear-zone, and which commonly contains rounded porphyroclasts and lithic fragments of similar composition to the minerals in the matrix (Fettes &amp; Desmons, 2007; Passchier &amp; Trouw, 1996).</skos:definition>
	<skos:prefLabel xml:lang="en">Mylonite</skos:prefLabel>
	<skos:narrower rdf:resource="https://resource.geosphere.at/thes/lith/149"/>
	<skos:exactMatch rdf:resource="http://resource.geosciml.org/classifier/cgi/lithology/mylonitic_rock"/>
	<dcterms:references rdf:resource="https://resource.geosphere.at/thes/citation/216"/>
	<rdf:type rdf:resource="http://www.w3.org/2004/02/skos/core#Concept"/>
	<dcterms:date rdf:datatype="http://www.w3.org/2001/XMLSchema#dateTime">2011-03-16T09:19:05Z</dcterms:date>
	<dcterms:references rdf:resource="https://resource.geosphere.at/thes/citation/557"/>
	<skos:exactMatch rdf:resource="http://inspire.ec.europa.eu/codelist/LithologyValue/myloniticRock"/>
	<skos:definition xml:lang="de">Kohäsives Störungsgestein, charakterisiert durch eine gut entwickelte Schieferung, welche durch tektonische Korngrößenverkleinerung in einer duktilen Scherzone entsteht. Zeigt typischerweise gerundete Porphyroklasten und lithische Fragmente mit einer ähnlichen Zusammensetzung wie die Matrixminerale (Fettes &amp; Desmons, 2007; Passchier &amp; Trouw, 1996).</skos:definition>
	<skos:prefLabel xml:lang="de">Mylonit</skos:prefLabel>
	<skos:exactMatch rdf:resource="http://data.bgs.ac.uk/id/EarthMaterialClass/RockName/MYLO"/>
	<colourHexCode xmlns="http://dbpedia.org/ontology/">#E6E600</colourHexCode>
	<dcterms:created rdf:datatype="http://www.w3.org/2001/XMLSchema#dateTime">2012-03-12T14:35:54.000Z</dcterms:created>
	<dcterms:hasVersion rdf:datatype="http://www.w3.org/2001/XMLSchema#int">11</dcterms:hasVersion>
</rdf:Description>

<rdf:Description rdf:about="https://resource.geosphere.at/thes/lith/149">
	<dcterms:date rdf:datatype="http://www.w3.org/2001/XMLSchema#dateTime">2011-03-16T09:19:05Z</dcterms:date>
	<dcterms:references rdf:resource="https://resource.geosphere.at/thes/citation/216"/>
	<skos:definition xml:lang="en">A phyllosillicate-rich mylonite that has the lustrous sheen of a phyllite (Fettes &amp; Desmons, 2007).</skos:definition>
	<skos:exactMatch rdf:resource="http://resource.geosciml.org/classifier/cgi/lithology/phyllonite"/>
	<skos:exactMatch rdf:resource="http://inspire.ec.europa.eu/codelist/LithologyValue/phyllonite"/>
	<skos:definition xml:lang="de">Phyllosilikatreicher Mylonit, welcher den schimmernden Glanz (Seidenglanz) von Phyllit zeigt (Fettes &amp; Desmons, 2007).</skos:definition>
	<skos:prefLabel xml:lang="de">Phyllonit</skos:prefLabel>
	<foaf:depiction rdf:resource="https://resource.geosphere.at/img/thes/Phyllonit.jpg"/>
	<skos:exactMatch rdf:resource="http://data.bgs.ac.uk/id/EarthMaterialClass/RockName/PHY"/>
	<skos:prefLabel xml:lang="en">Phyllonite</skos:prefLabel>
	<dcterms:created rdf:datatype="http://www.w3.org/2001/XMLSchema#dateTime">2013-04-05T09:37:04.000Z</dcterms:created>
	<dcterms:hasVersion rdf:datatype="http://www.w3.org/2001/XMLSchema#int">7</dcterms:hasVersion>
	<rdf:type rdf:resource="http://www.w3.org/2004/02/skos/core#Concept"/>
	<colourHexCode xmlns="http://dbpedia.org/ontology/">#339966</colourHexCode>
</rdf:Description>

<rdf:Description rdf:about="https://resource.geosphere.at/thes/lith/151">
	<skos:definition xml:lang="en">A fault rock which is cohesive with a poorly-developed or absent schistosity, or which is incohesive, characterised by generally angular porphyroclasts and lithic fragments in a finer-grained matrix of similar composition. Brittle deformation mechanisms are predominant but plastic deformation may also be involved (modified from Fettes &amp; Desmons 2007).</skos:definition>
	<dcterms:hasVersion rdf:datatype="http://www.w3.org/2001/XMLSchema#int">7</dcterms:hasVersion>
	<skos:definition xml:lang="de">Ein kohäsives Störungsgestein mit einer schlecht entwickelten oder fehlenden Schieferung. Charakterisiert durch überwiegend eckige Porphyroklasten und lithische Fragmente in einer feinkörnigen Matrix mit ähnlicher Zusammensetzung. Spröde Deformationsmechanismen sind vorherrschend obwohl auch plastische Deformation vorkommen kann (verändert nach Fettes &amp; Desmons 2007).</skos:definition>
	<skos:prefLabel xml:lang="de">Kataklasit</skos:prefLabel>
	<skos:prefLabel xml:lang="en">Cataclasite</skos:prefLabel>
	<dcterms:date rdf:datatype="http://www.w3.org/2001/XMLSchema#dateTime">2011-03-16T09:19:05Z</dcterms:date>
	<dcterms:references rdf:resource="https://resource.geosphere.at/thes/citation/216"/>
	<skos:exactMatch rdf:resource="http://data.bgs.ac.uk/id/EarthMaterialClass/RockName/CAT"/>
	<skos:exactMatch rdf:resource="http://resource.geosciml.org/classifier/cgi/lithology/cataclasite_series"/>
	<skos:exactMatch rdf:resource="http://inspire.ec.europa.eu/codelist/LithologyValue/cataclasiteSeries"/>
	<foaf:depiction rdf:resource="https://resource.geosphere.at/img/thes/Kataklasit.jpg"/>
	<skos:exactMatch rdf:resource="http://dbpedia.org/resource/Cataclasite"/>
	<rdf:type rdf:resource="http://www.w3.org/2004/02/skos/core#Concept"/>
	<dcterms:created rdf:datatype="http://www.w3.org/2001/XMLSchema#dateTime">2013-04-05T09:32:14.000Z</dcterms:created>
	<colourHexCode xmlns="http://dbpedia.org/ontology/">#F4FFD5</colourHexCode>
</rdf:Description>

<rdf:Description rdf:about="https://resource.geosphere.at/thes/lith/150">
	<rdf:type rdf:resource="http://www.w3.org/2004/02/skos/core#Concept"/>
	<skos:prefLabel xml:lang="en">Pseudotachylite</skos:prefLabel>
	<dcterms:hasVersion rdf:datatype="http://www.w3.org/2001/XMLSchema#int">10</dcterms:hasVersion>
	<skos:definition xml:lang="en">An ultrafine-grained vitreous-looking material, usually black and flinty in appearance, occurring as thin planar veins, injection veins or as a matrix to pseudo-conglomerates or breccias, which infills dilation fractures in the host rock. Formed by local melting due to brittle faulting in response to seismic activity and local generation of frictional heat (Fettes &amp; Desmons, 2007; Passchier &amp; Trouw, 1996).</skos:definition>
	<dcterms:references rdf:resource="https://resource.geosphere.at/thes/citation/216"/>
	<skos:broadMatch rdf:resource="http://resource.geosciml.org/classifier/cgi/lithology/fault_related_material"/>
	<skos:exactMatch rdf:resource="http://dbpedia.org/resource/Pseudotachylite"/>
	<skos:prefLabel xml:lang="de">Pseudotachylit</skos:prefLabel>
	<dcterms:date rdf:datatype="http://www.w3.org/2001/XMLSchema#dateTime">2011-03-16T09:19:05Z</dcterms:date>
	<skos:exactMatch rdf:resource="http://data.bgs.ac.uk/id/EarthMaterialClass/RockName/PSTACH"/>
	<skos:broadMatch rdf:resource="http://inspire.ec.europa.eu/codelist/LithologyValue/faultRelatedMaterial"/>
	<dcterms:created rdf:datatype="http://www.w3.org/2001/XMLSchema#dateTime">2012-03-12T15:58:16.000Z</dcterms:created>
	<dcterms:references rdf:resource="https://resource.geosphere.at/thes/citation/557"/>
	<skos:definition xml:lang="de">Ultrafeinkörniges, glasiges Material mit typischerweise schwarzem und kieseligem Erscheinungsbild, das als planare Adern, Injektionsadern oder als Matrix von Pseudo-Konglomeraten oder Brekzien vorkommt, welche die durch Störungen verursachten Hohlräume füllen. Entsteht aus lokaler Schmelze während spröder Deformation auf Grund von seismischer Aktivität und damit einhergehender lokaler Reibungswärme (Fettes &amp; Desmons, 2007; Passchier &amp; Trouw, 1996).</skos:definition>
</rdf:Description>

<rdf:Description rdf:about="https://resource.geosphere.at/thes/lith/153">
	<dcterms:created rdf:datatype="http://www.w3.org/2001/XMLSchema#dateTime">2013-04-05T09:42:59.000Z</dcterms:created>
	<skos:prefLabel xml:lang="en">Tectonic breccia</skos:prefLabel>
	<skos:definition xml:lang="de">Inkohäsives Störungsgestein mit ≥ 90 % eckigen Porphyroklasten und lithischen Fragmenten in einer feinkörnigen Matrix mit ähnlicher Zusammensetzung (Fettes &amp; Desmons, 2007; Heitzmann, 1985).</skos:definition>
	<dcterms:references rdf:resource="https://resource.geosphere.at/thes/citation/271"/>
	<rdf:type rdf:resource="http://www.w3.org/2004/02/skos/core#Concept"/>
	<skos:related rdf:resource="https://resource.geosphere.at/thes/lith/182"/>
	<dcterms:hasVersion rdf:datatype="http://www.w3.org/2001/XMLSchema#int">14</dcterms:hasVersion>
	<dcterms:date rdf:datatype="http://www.w3.org/2001/XMLSchema#dateTime">2011-03-16T09:19:05Z</dcterms:date>
	<skos:closeMatch rdf:resource="http://inspire.ec.europa.eu/codelist/LithologyValue/brecciaGougeSeries"/>
	<foaf:depiction rdf:resource="https://resource.geosphere.at/img/thes/Tektonische_Brekzie.jpg"/>
	<skos:closeMatch rdf:resource="http://resource.geosciml.org/classifier/cgi/lithology/breccia_gouge_series"/>
	<skos:definition xml:lang="en">A fault rock which is incohesive rock material with ≥ 90% generally angular porphyroclasts and lithic fragments in a finer-grained matrix of similar composition (Fettes &amp; Desmons, 2007; Heitzmann, 1985).</skos:definition>
	<skos:prefLabel xml:lang="de">Tektonische Brekzie</skos:prefLabel>
	<dcterms:references rdf:resource="https://resource.geosphere.at/thes/citation/216"/>
</rdf:Description>

<rdf:Description rdf:about="https://resource.geosphere.at/thes/lith/152">
	<skos:prefLabel xml:lang="en">Kakirite</skos:prefLabel>
	<skos:broadMatch rdf:resource="http://inspire.ec.europa.eu/codelist/LithologyValue/faultRelatedMaterial"/>
	<skos:closeMatch rdf:resource="http://resource.geosciml.org/classifier/cgi/lithology/breccia_gouge_series"/>
	<skos:prefLabel xml:lang="de">Kakirit</skos:prefLabel>
	<dcterms:hasVersion rdf:datatype="http://www.w3.org/2001/XMLSchema#int">11</dcterms:hasVersion>
	<dcterms:references rdf:resource="https://resource.geosphere.at/thes/citation/271"/>
	<foaf:depiction rdf:resource="https://resource.geosphere.at/img/thes/Kakirit.jpg"/>
	<skos:definition xml:lang="en">A fault rock that is incohesive and has only poorly-developed schistosity, if any. Kalkirite is characterised by generally angular porphyroclasts and lithic fragments in a finer-grained matrix of similar composition.It is formed by brittle deformation mechanisms such as cataclastic flow (Fettes &amp; Desmons, 2007; Heitzmann, 1985).</skos:definition>
	<skos:definition xml:lang="de">Inkohäsives Störungsgestein mit einer schlecht entwickelten oder fehlenden Schieferung. Charakterisiert durch überwiegend eckige Porphyroklasten und lithische Fragmente in einer feinkörnigen Matrix mit ähnlicher Zusammensetzung. Spröde Deformationsmechanismen (Kataklase) sind vorherrschend (Fettes &amp; Desmons, 2007; Heitzmann, 1985).</skos:definition>
	<rdf:type rdf:resource="http://www.w3.org/2004/02/skos/core#Concept"/>
	<dcterms:created rdf:datatype="http://www.w3.org/2001/XMLSchema#dateTime">2013-04-05T09:30:42.000Z</dcterms:created>
	<dcterms:references rdf:resource="https://resource.geosphere.at/thes/citation/216"/>
	<dcterms:date rdf:datatype="http://www.w3.org/2001/XMLSchema#dateTime">2011-03-16T09:19:05Z</dcterms:date>
</rdf:Description>

<rdf:Description rdf:about="https://resource.geosphere.at/thes/lith/154">
	<skos:closeMatch rdf:resource="http://resource.geosciml.org/classifier/cgi/lithology/breccia_gouge_series"/>
	<rdf:type rdf:resource="http://www.w3.org/2004/02/skos/core#Concept"/>
	<skos:prefLabel xml:lang="en">Fault gouge</skos:prefLabel>
	<skos:prefLabel xml:lang="de">Gesteinsmehl</skos:prefLabel>
	<skos:definition xml:lang="en">An incohesive, clay-rich, fine- to ultrafine-grained fault rock, which may possess a schistosity and containing &lt; 30% visible fragments. Lithic clasts may be present (Fettes &amp; Desmons, 2007; Heitzmann, 1985).</skos:definition>
	<skos:altLabel xml:lang="de">Störungsletten</skos:altLabel>
	<skos:exactMatch rdf:resource="http://dbpedia.org/resource/Fault_gouge"/>
	<skos:definition xml:lang="de">Inkohäsives, toniges, fein- bis ultrafeinkörniges Störungsgestein, welches eine Schieferung besitzen kann und &lt; 30 % sichtbare Fragmente aufweist. Kann lithische Klasten führen (Fettes &amp; Desmons, 2007; Heitzmann, 1985).</skos:definition>
	<dcterms:references rdf:resource="https://resource.geosphere.at/thes/citation/271"/>
	<dcterms:created rdf:datatype="http://www.w3.org/2001/XMLSchema#dateTime">2012-03-12T12:55:41.000Z</dcterms:created>
	<dcterms:date rdf:datatype="http://www.w3.org/2001/XMLSchema#dateTime">2011-03-16T09:19:05Z</dcterms:date>
	<skos:closeMatch rdf:resource="http://inspire.ec.europa.eu/codelist/LithologyValue/brecciaGougeSeries"/>
	<dcterms:hasVersion rdf:datatype="http://www.w3.org/2001/XMLSchema#int">11</dcterms:hasVersion>
	<dcterms:references rdf:resource="https://resource.geosphere.at/thes/citation/216"/>
</rdf:Description>

<rdf:Description rdf:about="https://resource.geosphere.at/thes/lith/156">
	<colourHexCode xmlns="http://dbpedia.org/ontology/">#A6D9CC</colourHexCode>
	<skos:exactMatch rdf:resource="http://inspire.ec.europa.eu/codelist/LithologyValue/materialFormedInSurficialEnvironment"/>
	<dcterms:date rdf:datatype="http://www.w3.org/2001/XMLSchema#dateTime">2011-03-16T09:19:05Z</dcterms:date>
	<skos:definition xml:lang="de">Material, das als Verwitterungsprodukt gebildet wurde und nach der Alteration des Ausgangsprodukts durch chemische oder physikalische Verwitterung in situ an der Erdoberfläche blieb. Der Begriff umfasst auch Bauxit (McMillan &amp; Powell, 1999).</skos:definition>
	<dcterms:hasVersion rdf:datatype="http://www.w3.org/2001/XMLSchema#int">10</dcterms:hasVersion>
	<skos:prefLabel xml:lang="de">Oberflächenbildungen</skos:prefLabel>
	<dcterms:references rdf:resource="https://resource.geosphere.at/thes/citation/485"/>
	<skos:prefLabel xml:lang="en">Surficially formed material</skos:prefLabel>
	<skos:definition xml:lang="en">Material formed as a product of weathering that has remained in situ following alteration of the parent material by the action of chemical and/or physical weathering processes operating on the Earth's surface. The term includes bauxite (McMillan &amp; Powell, 2004).</skos:definition>
	<skos:exactMatch rdf:resource="http://resource.geosciml.org/classifier/cgi/lithology/material_formed_in_surficial_environment"/>
	<rdf:type rdf:resource="http://www.w3.org/2004/02/skos/core#Concept"/>
	<dcterms:created rdf:datatype="http://www.w3.org/2001/XMLSchema#dateTime">2012-03-12T16:27:12.000Z</dcterms:created>
</rdf:Description>

<rdf:Description rdf:about="https://resource.geosphere.at/thes/lith/98">
	<dcterms:date rdf:datatype="http://www.w3.org/2001/XMLSchema#dateTime">2011-03-16T09:19:05Z</dcterms:date>
	<rdf:type rdf:resource="http://www.w3.org/2004/02/skos/core#Concept"/>
	<colourHexCode xmlns="http://dbpedia.org/ontology/">#3D8A3D</colourHexCode>
	<skos:narrower rdf:resource="https://resource.geosphere.at/thes/lith/142"/>
	<skos:narrower rdf:resource="https://resource.geosphere.at/thes/lith/144"/>
	<skos:narrower rdf:resource="https://resource.geosphere.at/thes/lith/143"/>
	<skos:narrower rdf:resource="https://resource.geosphere.at/thes/lith/145"/>
	<dcterms:references rdf:resource="https://resource.geosphere.at/thes/citation/545"/>
	<skos:altLabel xml:lang="de">Metamorphes Gestein</skos:altLabel>
	<skos:exactMatch rdf:resource="http://www.wikidata.org/entity/Q47069"/>
	<skos:narrower rdf:resource="https://resource.geosphere.at/thes/lith/108"/>
	<skos:narrower rdf:resource="https://resource.geosphere.at/thes/lith/104"/>
	<skos:altLabel xml:lang="en">Metamorphite</skos:altLabel>
	<skos:narrower rdf:resource="https://resource.geosphere.at/thes/lith/119"/>
	<skos:narrower rdf:resource="https://resource.geosphere.at/thes/lith/118"/>
	<skos:exactMatch rdf:resource="http://dbpedia.org/resource/Metamorphic_rock"/>
	<skos:exactMatch rdf:resource="http://resource.geosciml.org/classifier/cgi/lithology/metamorphic_rock"/>
	<skos:narrower rdf:resource="https://resource.geosphere.at/thes/lith/123"/>
	<skos:narrower rdf:resource="https://resource.geosphere.at/thes/lith/120"/>
	<skos:definition xml:lang="de">Gestein, welches durch mineralogische, chemische oder strukturelle Veränderungen im überwiegend festen Zustand aus präexistierenden Gesteinen auf Grund von Änderungen in Temperatur, Druck, Scherstress und chemischer Umgebung entsteht (Neuendorf et al., 2005).</skos:definition>
	<skos:narrower rdf:resource="https://resource.geosphere.at/thes/lith/126"/>
	<skos:narrower rdf:resource="https://resource.geosphere.at/thes/lith/129"/>
	<skos:narrower rdf:resource="https://resource.geosphere.at/thes/lith/128"/>
	<skos:narrower rdf:resource="https://resource.geosphere.at/thes/lith/127"/>
	<skos:narrower rdf:resource="https://resource.geosphere.at/thes/lith/136"/>
	<skos:prefLabel xml:lang="de">Metamorphit</skos:prefLabel>
	<dcterms:hasVersion rdf:datatype="http://www.w3.org/2001/XMLSchema#int">9</dcterms:hasVersion>
	<skos:prefLabel xml:lang="en">Metamorphic rock</skos:prefLabel>
	<skos:exactMatch rdf:resource="http://data.bgs.ac.uk/id/EarthMaterialClass/RockName/METR"/>
	<skos:exactMatch rdf:resource="http://inspire.ec.europa.eu/codelist/LithologyValue/metamorphicRock"/>
	<dcterms:created rdf:datatype="http://www.w3.org/2001/XMLSchema#dateTime">2012-03-12T14:29:37.000Z</dcterms:created>
	<skos:definition xml:lang="en">A rock derived from pre-existing rocks by mineralogical, chemical, or structural changes that have taken place essentially in a solid state, in response to marked changes in temperature, pressure, and shearing stress and chemical environment (in any combination), generally at depth in the Earth's crust (Neuendorf et al., 2005).</skos:definition>
	<skos:narrower rdf:resource="https://resource.geosphere.at/thes/lith/99"/>
	<skos:narrower rdf:resource="https://resource.geosphere.at/thes/lith/250"/>
	<skos:narrower rdf:resource="https://resource.geosphere.at/thes/lith/255"/>
	<skos:narrower rdf:resource="https://resource.geosphere.at/thes/lith/258"/>
</rdf:Description>

<rdf:Description rdf:about="https://resource.geosphere.at/thes/lith/145">
	<dcterms:created rdf:datatype="http://www.w3.org/2001/XMLSchema#dateTime">2012-03-12T16:26:36.000Z</dcterms:created>
	<skos:prefLabel xml:lang="de">Spilit</skos:prefLabel>
	<dcterms:hasVersion rdf:datatype="http://www.w3.org/2001/XMLSchema#int">8</dcterms:hasVersion>
	<skos:definition xml:lang="de">Verändertes, basisches bis intermediäres, (sub-)vulkanisches Gestein, dessen Feldspat teilweise oder komplett durch Albit repräsentiert wird und von Chlorit, Calcit, Quarz, Epidot und Prehnit begleitet wird. Die Erhaltung von eruptiven Merkmalen ist ein wichtiges Charakteristikum von Spiliten (Fettes &amp; Desmons, 2007).</skos:definition>
	<skos:definition xml:lang="en">An altered basic to intermediate hypabyssal to volcanic rock in which the feldspar is partially or completely composed of albite and is typically accompanied by chlorite, calcite, quartz, epidote, and prehnite. The preservation of eruptive features is an important characteristic of spilites (Fettes &amp; Desmons, 2007).</skos:definition>
	<skos:exactMatch rdf:resource="http://inspire.ec.europa.eu/codelist/LithologyValue/spilite"/>
	<skos:exactMatch rdf:resource="http://dbpedia.org/resource/Spilite"/>
	<skos:related rdf:resource="https://resource.geosphere.at/thes/lith/120"/>
	<dcterms:references rdf:resource="https://resource.geosphere.at/thes/citation/216"/>
	<rdf:type rdf:resource="http://www.w3.org/2004/02/skos/core#Concept"/>
	<skos:exactMatch rdf:resource="http://resource.geosciml.org/classifier/cgi/lithology/spilite"/>
	<colourHexCode xmlns="http://dbpedia.org/ontology/">#A6E666</colourHexCode>
	<dcterms:date rdf:datatype="http://www.w3.org/2001/XMLSchema#dateTime">2011-03-16T09:19:05Z</dcterms:date>
	<skos:prefLabel xml:lang="en">Spilite</skos:prefLabel>
</rdf:Description>

<rdf:Description rdf:about="https://resource.geosphere.at/thes/lith/123">
	<skos:definition xml:lang="de">Gestein, das durch eine Metamorphose lokaler Ausdehnung entsteht, welche die Umgebungsgesteine von Magmenkörpern beeinflusst. Diese Magmen können in einer Vielzahl von Milieus wirken, als oberflächennahe Vulkanite bis zu Magmenkörpern im oberen Mantel in kontinentalen oder ozeanischen Settings (Fettes &amp; Desmons, 2007).</skos:definition>
	<skos:broadMatch rdf:resource="http://resource.geosciml.org/classifier/cgi/lithology/metamorphic_rock"/>
	<skos:narrower rdf:resource="https://resource.geosphere.at/thes/lith/124"/>
	<skos:prefLabel xml:lang="de">Kontaktmetamorphes Gestein</skos:prefLabel>
	<rdf:type rdf:resource="http://www.w3.org/2004/02/skos/core#Concept"/>
	<dcterms:hasVersion rdf:datatype="http://www.w3.org/2001/XMLSchema#int">9</dcterms:hasVersion>
	<skos:broadMatch rdf:resource="http://inspire.ec.europa.eu/codelist/LithologyValue/metamorphicRock"/>
	<dcterms:date rdf:datatype="http://www.w3.org/2001/XMLSchema#dateTime">2011-03-16T09:19:05Z</dcterms:date>
	<dcterms:created rdf:datatype="http://www.w3.org/2001/XMLSchema#dateTime">2012-03-12T12:22:08.000Z</dcterms:created>
	<skos:definition xml:lang="en">A rock that originates from a type of (thermal) metamorphism of local extent, that affects the country rocks around magma bodies emplaced in a variety of environments, from volcanic to upper mantle depth, in both continental and oceanic settings (Fettes &amp; Desmons, 2007).</skos:definition>
	<dcterms:references rdf:resource="https://resource.geosphere.at/thes/citation/216"/>
	<skos:prefLabel xml:lang="en">Contact-metamorphic rock</skos:prefLabel>
</rdf:Description>

<rdf:Description rdf:about="https://resource.geosphere.at/thes/lith/124">
	<skos:prefLabel xml:lang="de">Hornfels</skos:prefLabel>
	<skos:prefLabel xml:lang="en">Hornfels</skos:prefLabel>
	<skos:definition xml:lang="de">Hartes, kompaktes, kontaktmetamorphes Gestein unbestimmter Korngröße, vornehmlich aus Silikat- und Oxidmineralen in veränderlichen Verhältnissen mit hornartigem Aussehen und einem subconchoidalen (muscheligen) bis gezackten Bruch. Es kann einige vom Protolith ererbte strukturelle Kennzeichen wie Schichtung, sedimentäre Lamination oder metamorphen Lagenbau enthalten. Hornfelse kommen meist (aber nicht ausschließlich) im innersten Teil von Kontaktaureolen vor (Fettes &amp; Desmons, 2007).</skos:definition>
	<colourHexCode xmlns="http://dbpedia.org/ontology/">#8CBF8C</colourHexCode>
	<skos:definition xml:lang="en">A hard, compact, contact-metamorphic rock of any grain size , predominantly composed of silicate and oxide minerals in varying proportions, with a horny appearance and a subconchoidal to jagged fracture. A hornfels may retain some of the structural features inherited from its protolith, such as bedding, sedimentary lamination, or metamorphic layering. Hornfels occur mostly, but not exclusively, in the innermost parts of contact aureoles (Fettes &amp; Desmons, 2007).</skos:definition>
	<dcterms:references rdf:resource="https://resource.geosphere.at/thes/citation/216"/>
	<rdf:type rdf:resource="http://www.w3.org/2004/02/skos/core#Concept"/>
	<dcterms:date rdf:datatype="http://www.w3.org/2001/XMLSchema#dateTime">2011-03-16T09:19:05Z</dcterms:date>
	<skos:exactMatch rdf:resource="http://data.bgs.ac.uk/id/EarthMaterialClass/RockName/HNFELS"/>
	<skos:exactMatch rdf:resource="http://inspire.ec.europa.eu/codelist/LithologyValue/hornfels"/>
	<skos:exactMatch rdf:resource="http://resource.geosciml.org/classifier/cgi/lithology/hornfels"/>
	<dcterms:created rdf:datatype="http://www.w3.org/2001/XMLSchema#dateTime">2012-03-12T14:35:07.000Z</dcterms:created>
	<dcterms:hasVersion rdf:datatype="http://www.w3.org/2001/XMLSchema#int">7</dcterms:hasVersion>
	<skos:exactMatch rdf:resource="http://dbpedia.org/resource/Hornfels"/>
</rdf:Description>

<rdf:Description rdf:about="https://resource.geosphere.at/thes/lith/255">
	<skos:broadMatch rdf:resource="http://inspire.ec.europa.eu/codelist/LithologyValue/metamorphicRock"/>
	<rdf:type rdf:resource="http://www.w3.org/2004/02/skos/core#Concept"/>
	<skos:prefLabel xml:lang="de">Metasiliziklastisches Gestein</skos:prefLabel>
	<dcterms:created rdf:datatype="http://www.w3.org/2001/XMLSchema#dateTime">2019-06-07T15:29:08.301Z</dcterms:created>
	<skos:prefLabel xml:lang="en">Metasiliciclastic sedimentary rock</skos:prefLabel>
	<skos:definition xml:lang="de">Ein Begriff für siliziklastische Gesteine, die Anzeichen einer metamorphen Überprägung aufweisen. (modifiziert nach Neuendorf et al., 2005).</skos:definition>
	<skos:definition xml:lang="en">A term for siliciclastic rocks, that show evidence of having been subjected to metamorphism. (modified after Neuendorf et al., 2005).</skos:definition>
	<dcterms:references rdf:resource="https://resource.geosphere.at/thes/citation/545"/>
	<dcterms:source rdf:resource="https://www.mindat.org/min-51363.html"/>
	<skos:broadMatch rdf:resource="http://resource.geosciml.org/classifier/cgi/lithology/metamorphic_rock"/>
	<skos:scopeNote xml:lang="en">The use of 'meta' together with the protolith names for metamorphic rocks focuses on their geological histories, not on their metamorphic grades.</skos:scopeNote>
	<skos:scopeNote xml:lang="de">Beim Benutzen des Präfixes 'Meta,' in Kombination mit dem Protolithnamen zur Benennung von Metamorphiten, liegt der Fokus auf der Veranschaulichung der geologischen Entwicklung, jedoch nicht auf dem Grad der Metamorphose.</skos:scopeNote>
</rdf:Description>

<rdf:Description rdf:about="https://resource.geosphere.at/thes/lith/104">
	<skos:prefLabel xml:lang="de">Migmatisches Gestein</skos:prefLabel>
	<skos:narrower rdf:resource="https://resource.geosphere.at/thes/lith/107"/>
	<skos:narrowMatch rdf:resource="http://resource.geosciml.org/classifier/cgi/lithology/migmatite"/>
	<skos:narrower rdf:resource="https://resource.geosphere.at/thes/lith/106"/>
	<skos:narrower rdf:resource="https://resource.geosphere.at/thes/lith/105"/>
	<skos:narrowMatch rdf:resource="http://inspire.ec.europa.eu/codelist/LithologyValue/migmatite"/>
	<skos:definition xml:lang="de">Gestein, das durch Anatexis (Aufschmelzen von Gestein) entsteht, unabhängig vom Anteil der Schmelze oder dem Prozess der Aufschmelzung (verändert nach Fettes &amp; Desmons, 2007).</skos:definition>
	<dcterms:hasVersion rdf:datatype="http://www.w3.org/2001/XMLSchema#int">8</dcterms:hasVersion>
	<rdf:type rdf:resource="http://www.w3.org/2004/02/skos/core#Concept"/>
	<dcterms:date rdf:datatype="http://www.w3.org/2001/XMLSchema#dateTime">2011-03-16T09:19:05Z</dcterms:date>
	<dcterms:created rdf:datatype="http://www.w3.org/2001/XMLSchema#dateTime">2012-03-12T14:33:06.000Z</dcterms:created>
	<skos:definition xml:lang="en">Any rock formed by anatexis (i.e. melting of a rock), irrespective of the proportion of the melt or the process of melting (modified from Fettes &amp; Desmons, 2007).</skos:definition>
	<skos:prefLabel xml:lang="en">Migmatic rock</skos:prefLabel>
	<dcterms:references rdf:resource="https://resource.geosphere.at/thes/citation/216"/>
</rdf:Description>

<rdf:Description rdf:about="https://resource.geosphere.at/thes/lith/106">
	<dcterms:references rdf:resource="https://resource.geosphere.at/thes/citation/216"/>
	<rdf:type rdf:resource="http://www.w3.org/2004/02/skos/core#Concept"/>
	<skos:prefLabel xml:lang="de">Metatexit</skos:prefLabel>
	<skos:broadMatch rdf:resource="http://inspire.ec.europa.eu/codelist/LithologyValue/migmatite"/>
	<dcterms:date rdf:datatype="http://www.w3.org/2001/XMLSchema#dateTime">2011-03-16T09:19:05Z</dcterms:date>
	<skos:definition xml:lang="de">Varietät von Migmatit mit diskretem Leukosom, Mesosom und Melanosom. Das Gestein markiert initiale Stadien der Anatexis (Fettes &amp; Desmons, 2007).</skos:definition>
	<dcterms:created rdf:datatype="http://www.w3.org/2001/XMLSchema#dateTime">2012-03-12T14:31:29.000Z</dcterms:created>
	<dcterms:hasVersion rdf:datatype="http://www.w3.org/2001/XMLSchema#int">8</dcterms:hasVersion>
	<skos:definition xml:lang="en">A variety of migmatite with discrete leucosomes, mesosomes, and melanosomes. Rocks formed in the initial stages of anatexis (Fettes &amp; Desmons, 2007).</skos:definition>
	<skos:prefLabel xml:lang="en">Metatexite</skos:prefLabel>
	<skos:closeMatch rdf:resource="http://resource.geosciml.org/classifier/cgi/lithology/migmatite"/>
</rdf:Description>

<rdf:Description rdf:about="https://resource.geosphere.at/thes/lith/105">
	<skos:altLabel xml:lang="en">Anatexite</skos:altLabel>
	<skos:exactMatch rdf:resource="http://resource.geosciml.org/classifier/cgi/lithology/migmatite"/>
	<skos:definition xml:lang="de">Silikatisches metamorphes Gestein, welches im meso- bis megaskopischen Maßstab durchgehend heterogen ist und typischerweise aus dunklen und hellen Anteilen besteht. Die dunkleren Teile (Melanosom oder Paleosom) zeigen üblicherweise Charakteristika von metamorphen Gesteinen, dagegen zeigen die hellen Teile (Leukosom oder Neosom) eine magmatisches Erscheinungsbild (Fettes &amp; Desmons, 2007).</skos:definition>
	<skos:prefLabel xml:lang="en">Migmatite</skos:prefLabel>
	<rdf:type rdf:resource="http://www.w3.org/2004/02/skos/core#Concept"/>
	<skos:exactMatch rdf:resource="http://dbpedia.org/resource/Migmatite"/>
	<colourHexCode xmlns="http://dbpedia.org/ontology/">#19BF66</colourHexCode>
	<skos:exactMatch rdf:resource="http://www.wikidata.org/entity/Q744630"/>
	<skos:altLabel xml:lang="de">Anatexit</skos:altLabel>
	<skos:exactMatch rdf:resource="http://inspire.ec.europa.eu/codelist/LithologyValue/migmatite"/>
	<dcterms:created rdf:datatype="http://www.w3.org/2001/XMLSchema#dateTime">2012-03-12T14:33:42.000Z</dcterms:created>
	<dcterms:hasVersion rdf:datatype="http://www.w3.org/2001/XMLSchema#int">7</dcterms:hasVersion>
	<skos:prefLabel xml:lang="de">Migmatit</skos:prefLabel>
	<dcterms:date rdf:datatype="http://www.w3.org/2001/XMLSchema#dateTime">2011-03-16T09:19:05Z</dcterms:date>
	<skos:definition xml:lang="en">A composite silicate metamorphic rock, pervasively heterogeneous on a meso- to megascopic scale. It typically consists of darker and lighter parts: the darker parts (melanosomes or paleosomes) usually exhibit features of metamorphic rocks whereas the lighter parts (leucosomes or neosomes) are of igneous appearance (Fettes &amp; Desmons, 2007).</skos:definition>
	<dcterms:references rdf:resource="https://resource.geosphere.at/thes/citation/216"/>
</rdf:Description>

<rdf:Description rdf:about="https://resource.geosphere.at/thes/lith/107">
	<dcterms:hasVersion rdf:datatype="http://www.w3.org/2001/XMLSchema#int">7</dcterms:hasVersion>
	<skos:prefLabel xml:lang="de">Diatexit</skos:prefLabel>
	<dcterms:date rdf:datatype="http://www.w3.org/2001/XMLSchema#dateTime">2011-03-16T09:19:05Z</dcterms:date>
	<skos:definition xml:lang="en">A type of migmatite where the darker and the lighter parts form schlieren and nebulitic structures that merge into one another (Fettes &amp; Desmons, 2007).</skos:definition>
	<skos:prefLabel xml:lang="en">Diatexite</skos:prefLabel>
	<skos:definition xml:lang="de">Migmatit, bei dem die dunklen und hellen Anteile Schlieren und nebulitische Strukturen bilden, die ineinander übergehen (Fettes &amp; Desmons, 2007).</skos:definition>
	<skos:broadMatch rdf:resource="http://inspire.ec.europa.eu/codelist/LithologyValue/migmatite"/>
	<dcterms:references rdf:resource="https://resource.geosphere.at/thes/citation/216"/>
	<skos:closeMatch rdf:resource="http://resource.geosciml.org/classifier/cgi/lithology/migmatite"/>
	<dcterms:created rdf:datatype="http://www.w3.org/2001/XMLSchema#dateTime">2012-03-12T12:40:16.000Z</dcterms:created>
	<rdf:type rdf:resource="http://www.w3.org/2004/02/skos/core#Concept"/>
</rdf:Description>

<rdf:Description rdf:about="https://resource.geosphere.at/thes/lith/126">
	<skos:definition xml:lang="en">A schistose or gneissose metamorphic rock consisting predominantly of actinolite, ocellar albite, and epidote, possibly with chlorite and titanite (Fettes &amp; Desmons, 2007).</skos:definition>
	<skos:prefLabel xml:lang="en">Prasinite</skos:prefLabel>
	<skos:exactMatch rdf:resource="http://inspire.ec.europa.eu/codelist/LithologyValue/chloriteActinoliteEpidoteMetamorphicRock"/>
	<dcterms:date rdf:datatype="http://www.w3.org/2001/XMLSchema#dateTime">2011-03-16T09:19:05Z</dcterms:date>
	<dcterms:hasVersion rdf:datatype="http://www.w3.org/2001/XMLSchema#int">11</dcterms:hasVersion>
	<dcterms:references rdf:resource="https://resource.geosphere.at/thes/citation/216"/>
	<skos:exactMatch rdf:resource="http://resource.geosciml.org/classifier/cgi/lithology/chlorite_actinolite_epidote_metamorphic_rock"/>
	<skos:prefLabel xml:lang="de">Prasinit</skos:prefLabel>
	<skos:related rdf:resource="https://resource.geosphere.at/thes/lith/125"/>
	<skos:definition xml:lang="de">Geschiefertes oder massiges metamorphes Gestein mit vorwiegend Aktinolith, Albit und Epidot und mitunter Chlorit und Titanit (Fettes &amp; Desmons, 2007).</skos:definition>
	<dcterms:created rdf:datatype="http://www.w3.org/2001/XMLSchema#dateTime">2014-06-26T12:56:16.000Z</dcterms:created>
	<rdf:type rdf:resource="http://www.w3.org/2004/02/skos/core#Concept"/>
	<foaf:depiction rdf:resource="https://resource.geosphere.at/img/thes/prasinit.jpg"/>
	<colourHexCode xmlns="http://dbpedia.org/ontology/">#26994D</colourHexCode>
</rdf:Description>

<rdf:Description rdf:about="https://resource.geosphere.at/thes/lith/258">
	<skos:exactMatch rdf:resource="http://dbpedia.org/resource/Metavolcanic_rock"/>
	<skos:scopeNote xml:lang="en">The use of 'meta' together with the protolith names for metamorphic rocks focuses on their geological histories, not on their metamorphic grades.</skos:scopeNote>
	<skos:broadMatch rdf:resource="http://resource.geosciml.org/classifier/cgi/lithology/metamorphic_rock"/>
	<skos:broadMatch rdf:resource="http://inspire.ec.europa.eu/codelist/LithologyValue/metamorphicRock"/>
	<skos:scopeNote xml:lang="de">Beim Benutzen des Präfixes 'Meta,' in Kombination mit dem Protolithnamen zur Benennung von Metamorphiten, liegt der Fokus auf der Veranschaulichung der geologischen Entwicklung, jedoch nicht auf dem Grad der Metamorphose.</skos:scopeNote>
	<skos:exactMatch rdf:resource="https://www.wikidata.org/wiki/Q6823306"/>
	<rdf:type rdf:resource="http://www.w3.org/2004/02/skos/core#Concept"/>
	<dcterms:created rdf:datatype="http://www.w3.org/2001/XMLSchema#dateTime">2020-01-21T11:04:54.475Z</dcterms:created>
	<skos:prefLabel xml:lang="de">Metavulkanit</skos:prefLabel>
	<skos:prefLabel xml:lang="en">Metavolcanic rock</skos:prefLabel>
	<skos:altLabel xml:lang="de">Metavulkanisches Gestein</skos:altLabel>
	<skos:definition xml:lang="en">An informal term for volcanic rocks that show evidence of having been subjected to metamorphism. (Neuendorf et al., 2005)</skos:definition>
	<skos:definition xml:lang="de">Ein meist informell verwendeter Begriff für vulkanische Gesteine, welche Anzeichen einer metamorphen Überprägung aufweisen. (Neuendorf et al., 2005)</skos:definition>
	<dcterms:references rdf:resource="https://resource.geosphere.at/thes/citation/545"/>
</rdf:Description>

<rdf:Description rdf:about="https://resource.geosphere.at/thes/lith/136">
	<skos:prefLabel xml:lang="de">Schiefer</skos:prefLabel>
	<skos:narrower rdf:resource="https://resource.geosphere.at/thes/lith/125"/>
	<dcterms:created rdf:datatype="http://www.w3.org/2001/XMLSchema#dateTime">2012-03-12T16:41:36.000Z</dcterms:created>
	<skos:narrower rdf:resource="https://resource.geosphere.at/thes/lith/139"/>
	<skos:narrower rdf:resource="https://resource.geosphere.at/thes/lith/141"/>
	<skos:definition xml:lang="de">Metamorphes Gestein mit einer schiefrigen Struktur (einer Foliation, die entweder gut entwickelt ist oder in regelmäßigen Abständen vorkommt, so dass das Gestein eine Spaltbarkeit von ≤ 1 cm zeigt; mineralogischer und/oder lithologischer Lagenbau ist gewöhnlich vorhanden), wobei &lt; 20 % Feldspatgehalt die Zusammensetzungsgrenze zu Gneis markiert (Fettes &amp; Desmons, 2007; Neuendorf et al., 2005).</skos:definition>
	<skos:narrower rdf:resource="https://resource.geosphere.at/thes/lith/137"/>
	<skos:exactMatch rdf:resource="http://www.wikidata.org/entity/Q15315"/>
	<dcterms:references rdf:resource="https://resource.geosphere.at/thes/citation/216"/>
	<rdf:type rdf:resource="http://www.w3.org/2004/02/skos/core#Concept"/>
	<dcterms:date rdf:datatype="http://www.w3.org/2001/XMLSchema#dateTime">2011-03-16T09:19:05Z</dcterms:date>
	<skos:exactMatch rdf:resource="http://inspire.ec.europa.eu/codelist/LithologyValue/schist"/>
	<dcterms:references rdf:resource="https://resource.geosphere.at/thes/citation/545"/>
	<skos:prefLabel xml:lang="en">Schist</skos:prefLabel>
	<skos:closeMatch rdf:resource="http://resource.geosciml.org/classifier/cgi/lithology/schist"/>
	<colourHexCode xmlns="http://dbpedia.org/ontology/">#33A666</colourHexCode>
	<dcterms:hasVersion rdf:datatype="http://www.w3.org/2001/XMLSchema#int">17</dcterms:hasVersion>
	<skos:exactMatch rdf:resource="http://data.bgs.ac.uk/id/EarthMaterialClass/RockName/SCH"/>
	<skos:definition xml:lang="en">A metamorphic rock with a schistose structure (a foliation that is either well developed or a continuous foliation so that the rock will split in on a scale of ≤ 1 cm; mineralogical and/or lithological layering is commonly present). Schist is distinguished from gneiss by a composition of &lt; 20% feldspar (and &gt;50% mica) (Fettes &amp; Desmons, 2007; Neuendorf et al., 2005).</skos:definition>
</rdf:Description>

<rdf:Description rdf:about="https://resource.geosphere.at/thes/lith/137">
	<rdf:type rdf:resource="http://www.w3.org/2004/02/skos/core#Concept"/>
	<skos:definition xml:lang="de">Ultrafeines oder sehr feinkörniges metamorphes Gestein, das eine durchgehende Foliation aufweist (Schieferspaltbarkeit) und dessen einzelne Körner zu klein sind, um sie mit freiem Auge zu erkennen. Tonschiefer zeigt normalerweise sehr niedrigmetamorphe Bedingungen an, obwohl er auch unter niedrigmetamorphen Bedingungen vorkommen kann. Ist das metamorphe Äquivalent von Schieferton (Fettes &amp; Desmons, 2007).</skos:definition>
	<skos:related rdf:resource="https://resource.geosphere.at/thes/lith/172"/>
	<dcterms:date rdf:datatype="http://www.w3.org/2001/XMLSchema#dateTime">2011-03-16T09:19:05Z</dcterms:date>
	<colourHexCode xmlns="http://dbpedia.org/ontology/">#80F299</colourHexCode>
	<skos:prefLabel xml:lang="en">Slate</skos:prefLabel>
	<skos:exactMatch rdf:resource="http://inspire.ec.europa.eu/codelist/LithologyValue/slate"/>
	<dcterms:references rdf:resource="https://resource.geosphere.at/thes/citation/216"/>
	<dcterms:created rdf:datatype="http://www.w3.org/2001/XMLSchema#dateTime">2012-03-12T16:25:03.000Z</dcterms:created>
	<skos:exactMatch rdf:resource="http://resource.geosciml.org/classifier/cgi/lithology/slate"/>
	<skos:definition xml:lang="en">An ultrafine- or very fine-grained metamorphic rock displaying a continuous foliation in which the individual grains are too small to be seen by the unaided eye (slaty cleavage). Slate is usually of very low metamorphic grade, although it may also occur under low-grade conditions; it is the metamorphic equivalent of shale (Fettes &amp; Desmons, 2007).</skos:definition>
	<skos:exactMatch rdf:resource="http://www.wikidata.org/entity/Q207079"/>
	<skos:prefLabel xml:lang="de">Tonschiefer</skos:prefLabel>
	<skos:exactMatch rdf:resource="http://data.bgs.ac.uk/id/EarthMaterialClass/RockName/SLTE"/>
	<dcterms:hasVersion rdf:datatype="http://www.w3.org/2001/XMLSchema#int">7</dcterms:hasVersion>
</rdf:Description>

<rdf:Description rdf:about="https://resource.geosphere.at/thes/lith/125">
	<rdf:type rdf:resource="http://www.w3.org/2004/02/skos/core#Concept"/>
	<skos:narrower rdf:resource="https://resource.geosphere.at/thes/lith/140"/>
	<skos:exactMatch rdf:resource="http://inspire.ec.europa.eu/codelist/LithologyValue/chloriteActinoliteEpidoteMetamorphicRock"/>
	<dcterms:hasVersion rdf:datatype="http://www.w3.org/2001/XMLSchema#int">10</dcterms:hasVersion>
	<dcterms:date rdf:datatype="http://www.w3.org/2001/XMLSchema#dateTime">2011-03-16T09:19:05Z</dcterms:date>
	<skos:definition xml:lang="de">Schiefer, dessen grünliche Farbe sich von Mineralen wie Aktinolith, Chlorit und Epidot ableitet (Fettes &amp; Desmons, 2007).</skos:definition>
	<dcterms:references rdf:resource="https://resource.geosphere.at/thes/citation/216"/>
	<skos:definition xml:lang="en">A greenish schist in which the colour is due to the presence of minerals such as actinolite, chlorite, and epidote (Fettes &amp; Desmons, 2007).</skos:definition>
	<skos:exactMatch rdf:resource="http://resource.geosciml.org/classifier/cgi/lithology/chlorite_actinolite_epidote_metamorphic_rock"/>
	<skos:prefLabel xml:lang="en">Greenschist</skos:prefLabel>
	<skos:related rdf:resource="https://resource.geosphere.at/thes/lith/126"/>
	<skos:exactMatch rdf:resource="http://dbpedia.org/resource/Greenschist"/>
	<skos:prefLabel xml:lang="de">Grünschiefer</skos:prefLabel>
	<dcterms:created rdf:datatype="http://www.w3.org/2001/XMLSchema#dateTime">2014-01-21T13:23:32.000Z</dcterms:created>
	<colourHexCode xmlns="http://dbpedia.org/ontology/">#26994D</colourHexCode>
</rdf:Description>

<rdf:Description rdf:about="https://resource.geosphere.at/thes/lith/140">
	<skos:definition xml:lang="de">Schiefer, dessen Hauptbestandteil Chlorit ist, der durch parallele Anordnung dem Gestein die Schieferung verleiht. Quarz, Epidot, Magnetit und Granat können vorkommen (Neuendorf et al., 2005).</skos:definition>
	<skos:broadMatch rdf:resource="http://resource.geosciml.org/classifier/cgi/lithology/chlorite_actinolite_epidote_metamorphic_rock"/>
	<dcterms:hasVersion rdf:datatype="http://www.w3.org/2001/XMLSchema#int">10</dcterms:hasVersion>
	<skos:prefLabel xml:lang="en">Chlorite schist</skos:prefLabel>
	<rdf:type rdf:resource="http://www.w3.org/2004/02/skos/core#Concept"/>
	<skos:definition xml:lang="en">A schist in which the main constituent is chlorite, which imparts schistosity by its parallel alignment. Quartz, epidote, magnetite and garnet may be present (Neuendorf et al., 2005).</skos:definition>
	<dcterms:created rdf:datatype="http://www.w3.org/2001/XMLSchema#dateTime">2012-03-12T12:01:13.000Z</dcterms:created>
	<skos:prefLabel xml:lang="de">Chloritschiefer</skos:prefLabel>
	<dcterms:date rdf:datatype="http://www.w3.org/2001/XMLSchema#dateTime">2011-03-16T09:19:05Z</dcterms:date>
	<dcterms:references rdf:resource="https://resource.geosphere.at/thes/citation/545"/>
	<skos:closeMatch rdf:resource="http://inspire.ec.europa.eu/codelist/LithologyValue/chloriteActinoliteEpidoteMetamorphicRock"/>
	<colourHexCode xmlns="http://dbpedia.org/ontology/">#26994D</colourHexCode>
</rdf:Description>

<rdf:Description rdf:about="https://resource.geosphere.at/thes/lith/139">
	<skos:definition xml:lang="de">Unterart von Schiefer mit Glimmer als einzigem Hauptbestandteil und untergeordnet Quarz sowie &lt; 20 % Feldspat (verändert nach Fettes &amp; Desmons, 2007).</skos:definition>
	<skos:prefLabel xml:lang="en">Mica schist</skos:prefLabel>
	<skos:definition xml:lang="en">A variety of schist with mica as the only major constituent, subordinate quartz, and &lt; 20% feldspar (modified from Fettes &amp; Desmons, 2007).</skos:definition>
	<skos:exactMatch rdf:resource="http://inspire.ec.europa.eu/codelist/LithologyValue/micaSchist"/>
	<skos:exactMatch rdf:resource="http://www.wikidata.org/entity/Q3856092"/>
	<skos:narrower rdf:resource="https://resource.geosphere.at/thes/lith/246"/>
	<skos:narrower rdf:resource="https://resource.geosphere.at/thes/lith/245"/>
	<skos:narrower rdf:resource="https://resource.geosphere.at/thes/lith/244"/>
	<skos:narrower rdf:resource="https://resource.geosphere.at/thes/lith/247"/>
	<dcterms:hasVersion rdf:datatype="http://www.w3.org/2001/XMLSchema#int">14</dcterms:hasVersion>
	<skos:narrower rdf:resource="https://resource.geosphere.at/thes/lith/138"/>
	<skos:prefLabel xml:lang="de">Glimmerschiefer</skos:prefLabel>
	<colourHexCode xmlns="http://dbpedia.org/ontology/">#4DBF80</colourHexCode>
	<rdf:type rdf:resource="http://www.w3.org/2004/02/skos/core#Concept"/>
	<dcterms:created rdf:datatype="http://www.w3.org/2001/XMLSchema#dateTime">2014-06-04T12:41:03.000Z</dcterms:created>
	<skos:exactMatch rdf:resource="http://resource.geosciml.org/classifier/cgi/lithology/mica_schist"/>
	<dcterms:references rdf:resource="https://resource.geosphere.at/thes/citation/216"/>
	<dcterms:date rdf:datatype="http://www.w3.org/2001/XMLSchema#dateTime">2011-03-16T09:19:05Z</dcterms:date>
</rdf:Description>

<rdf:Description rdf:about="https://resource.geosphere.at/thes/lith/245">
	<skos:prefLabel xml:lang="de">Staurolith-Glimmerschiefer</skos:prefLabel>
	<skos:broadMatch rdf:resource="http://resource.geosciml.org/classifier/cgi/lithology/mica_schist"/>
	<rdf:type rdf:resource="http://www.w3.org/2004/02/skos/core#Concept"/>
	<skos:definition xml:lang="de">Glimmerschiefer der Staurolith führt.</skos:definition>
	<skos:broadMatch rdf:resource="http://inspire.ec.europa.eu/codelist/LithologyValue/micaSchist"/>
	<skos:prefLabel xml:lang="en">Staurolite-mica schist</skos:prefLabel>
	<dcterms:created rdf:datatype="http://www.w3.org/2001/XMLSchema#dateTime">2012-01-20T15:03:32.000Z</dcterms:created>
	<skos:definition xml:lang="en">A mica-schist that contains Staurolite.</skos:definition>
	<dcterms:hasVersion rdf:datatype="http://www.w3.org/2001/XMLSchema#int">10</dcterms:hasVersion>
</rdf:Description>

<rdf:Description rdf:about="https://resource.geosphere.at/thes/lith/244">
	<dcterms:created rdf:datatype="http://www.w3.org/2001/XMLSchema#dateTime">2012-01-20T14:51:35.000Z</dcterms:created>
	<skos:prefLabel xml:lang="en">Garnet-mica schist</skos:prefLabel>
	<foaf:depiction rdf:resource="https://resource.geosphere.at/img/thes/Glimmerschiefer_1.jpg"/>
	<skos:broadMatch rdf:resource="http://resource.geosciml.org/classifier/cgi/lithology/mica_schist"/>
	<skos:definition xml:lang="en">A mica-schist that contains garnet.</skos:definition>
	<rdf:type rdf:resource="http://www.w3.org/2004/02/skos/core#Concept"/>
	<skos:broadMatch rdf:resource="http://inspire.ec.europa.eu/codelist/LithologyValue/micaSchist"/>
	<dcterms:hasVersion rdf:datatype="http://www.w3.org/2001/XMLSchema#int">8</dcterms:hasVersion>
	<skos:prefLabel xml:lang="de">Granat-Glimmerschiefer</skos:prefLabel>
	<skos:definition xml:lang="de">Glimmerschiefer der Granat führt.</skos:definition>
</rdf:Description>

<rdf:Description rdf:about="https://resource.geosphere.at/thes/lith/247">
	<skos:broadMatch rdf:resource="http://inspire.ec.europa.eu/codelist/LithologyValue/micaSchist"/>
	<skos:prefLabel xml:lang="de">Andalusit-Glimmerschiefer</skos:prefLabel>
	<skos:definition xml:lang="de">Glimmerschiefer der Andalusit führt.</skos:definition>
	<dcterms:hasVersion rdf:datatype="http://www.w3.org/2001/XMLSchema#int">13</dcterms:hasVersion>
	<rdf:type rdf:resource="http://www.w3.org/2004/02/skos/core#Concept"/>
	<dcterms:created rdf:datatype="http://www.w3.org/2001/XMLSchema#dateTime">2012-01-20T15:17:51.000Z</dcterms:created>
	<skos:prefLabel xml:lang="en">Andalusite-mica schist</skos:prefLabel>
	<skos:broadMatch rdf:resource="http://resource.geosciml.org/classifier/cgi/lithology/mica_schist"/>
	<skos:definition xml:lang="en">A mica-schist that contains andalusite.</skos:definition>
</rdf:Description>

<rdf:Description rdf:about="https://resource.geosphere.at/thes/lith/246">
	<dcterms:hasVersion rdf:datatype="http://www.w3.org/2001/XMLSchema#int">9</dcterms:hasVersion>
	<skos:prefLabel xml:lang="de">Disthen-Glimmerschiefer</skos:prefLabel>
	<skos:prefLabel xml:lang="en">Kyanite-mica schist</skos:prefLabel>
	<skos:broadMatch rdf:resource="http://inspire.ec.europa.eu/codelist/LithologyValue/micaSchist"/>
	<skos:definition xml:lang="de">Glimmerschiefer der Disthen führt.</skos:definition>
	<skos:altLabel xml:lang="de">Kyanit-Glimmerschiefer</skos:altLabel>
	<skos:definition xml:lang="en">A mica-schist that contains kyanite.</skos:definition>
	<dcterms:created rdf:datatype="http://www.w3.org/2001/XMLSchema#dateTime">2012-01-20T15:11:17.000Z</dcterms:created>
	<rdf:type rdf:resource="http://www.w3.org/2004/02/skos/core#Concept"/>
	<skos:broadMatch rdf:resource="http://resource.geosciml.org/classifier/cgi/lithology/mica_schist"/>
</rdf:Description>

<rdf:Description rdf:about="https://resource.geosphere.at/thes/lith/138">
	<colourHexCode xmlns="http://dbpedia.org/ontology/">#73F28C</colourHexCode>
	<dcterms:hasVersion rdf:datatype="http://www.w3.org/2001/XMLSchema#int">8</dcterms:hasVersion>
	<skos:exactMatch rdf:resource="http://inspire.ec.europa.eu/codelist/LithologyValue/phyllite"/>
	<dcterms:date rdf:datatype="http://www.w3.org/2001/XMLSchema#dateTime">2011-03-16T09:19:05Z</dcterms:date>
	<skos:prefLabel xml:lang="de">Phyllit</skos:prefLabel>
	<dcterms:references rdf:resource="https://resource.geosphere.at/thes/citation/216"/>
	<skos:definition xml:lang="en">A fine to medium-grained metamorphic rock characterised by well developed continuous schistosity resulting from the parallel arrangement of phyllosilicates. Phyllite is usually of low metamorphic grade, and is intermediate between slate and mica-schist (Fettes &amp; Desmons, 2007).</skos:definition>
	<skos:definition xml:lang="de">Fein- bis mittelkörniges metamorphes Gestein, das infolge paralleler Anordnung von Phyllosilikaten eine durchgehende Schieferung aufweist. Phyllit wird bei niedrigmetamorphen Bedingungen gebildet und liegt im Übergangsbereich zwischen Tonschiefer und Glimmerschiefer (Fettes &amp; Desmons, 2007).</skos:definition>
	<skos:exactMatch rdf:resource="http://www.wikidata.org/entity/Q731880"/>
	<skos:prefLabel xml:lang="en">Phyllite</skos:prefLabel>
	<dcterms:created rdf:datatype="http://www.w3.org/2001/XMLSchema#dateTime">2012-03-12T15:56:22.000Z</dcterms:created>
	<rdf:type rdf:resource="http://www.w3.org/2004/02/skos/core#Concept"/>
	<skos:exactMatch rdf:resource="http://resource.geosciml.org/classifier/cgi/lithology/phyllite"/>
</rdf:Description>

<rdf:Description rdf:about="https://resource.geosphere.at/thes/lith/141">
	<dcterms:references rdf:resource="https://resource.geosphere.at/thes/citation/545"/>
	<skos:broadMatch rdf:resource="http://inspire.ec.europa.eu/codelist/LithologyValue/schist"/>
	<skos:broadMatch rdf:resource="http://resource.geosciml.org/classifier/cgi/lithology/schist"/>
	<skos:prefLabel xml:lang="de">Grafitschiefer</skos:prefLabel>
	<dcterms:hasVersion rdf:datatype="http://www.w3.org/2001/XMLSchema#int">8</dcterms:hasVersion>
	<rdf:type rdf:resource="http://www.w3.org/2004/02/skos/core#Concept"/>
	<skos:definition xml:lang="en">A schist in which graphite is the main constituent, imparting schistosity by its parallel alignment (Neuendorf et al., 2005).</skos:definition>
	<skos:prefLabel xml:lang="en">Graphite schist</skos:prefLabel>
	<skos:altLabel xml:lang="de">Graphitschiefer</skos:altLabel>
	<skos:definition xml:lang="de">Schiefer, dessen Hauptbestandteil Graphit ist und dessen parallele Anordnung dem Gestein die Schieferung verleiht (Neuendorf et al., 2005).</skos:definition>
	<dcterms:date rdf:datatype="http://www.w3.org/2001/XMLSchema#dateTime">2011-03-16T09:19:05Z</dcterms:date>
	<dcterms:created rdf:datatype="http://www.w3.org/2001/XMLSchema#dateTime">2014-06-04T12:41:14.000Z</dcterms:created>
</rdf:Description>

<rdf:Description rdf:about="https://resource.geosphere.at/thes/lith/128">
	<dcterms:references rdf:resource="https://resource.geosphere.at/thes/citation/545"/>
	<skos:definition xml:lang="de">Granoblastisches metamorphes Gestein, welches überwiegend aus Quarz besteht und durch Rekristallisation von Sandstein oder Kieselgestein während regionaler oder thermischer Metamorphose entsteht (Neuendorf et al., 2005).</skos:definition>
	<skos:definition xml:lang="en">A granoblastic metamorphic rock consisting mainly of quartz and formed by recrystallisation of sandstone or chert, by either regional or thermal metamorphism (Neuendorf et al., 2005).</skos:definition>
	<skos:prefLabel xml:lang="en">Quartzite</skos:prefLabel>
	<colourHexCode xmlns="http://dbpedia.org/ontology/">#E6F259</colourHexCode>
	<skos:exactMatch rdf:resource="http://data.bgs.ac.uk/id/EarthMaterialClass/RockName/QZITE"/>
	<dcterms:hasVersion rdf:datatype="http://www.w3.org/2001/XMLSchema#int">7</dcterms:hasVersion>
	<rdf:type rdf:resource="http://www.w3.org/2004/02/skos/core#Concept"/>
	<skos:exactMatch rdf:resource="http://inspire.ec.europa.eu/codelist/LithologyValue/quartzite"/>
	<dcterms:date rdf:datatype="http://www.w3.org/2001/XMLSchema#dateTime">2011-03-16T09:19:05Z</dcterms:date>
	<dcterms:created rdf:datatype="http://www.w3.org/2001/XMLSchema#dateTime">2012-03-12T16:11:14.000Z</dcterms:created>
	<skos:prefLabel xml:lang="de">Quarzit</skos:prefLabel>
	<skos:exactMatch rdf:resource="http://resource.geosciml.org/classifier/cgi/lithology/quartzite"/>
</rdf:Description>

<rdf:Description rdf:about="https://resource.geosphere.at/thes/lith/99">
	<skos:definition xml:lang="en">A rock characterised by the pressure-dominated metamorphic conditions that comprise the glaucophane-schist and eclogite facies (Fettes &amp; Desmons, 2007).</skos:definition>
	<skos:prefLabel xml:lang="de">Hochdruckmetamorphes Gestein</skos:prefLabel>
	<dcterms:date rdf:datatype="http://www.w3.org/2001/XMLSchema#dateTime">2011-03-16T09:19:05Z</dcterms:date>
	<dcterms:references rdf:resource="https://resource.geosphere.at/thes/citation/216"/>
	<dcterms:hasVersion rdf:datatype="http://www.w3.org/2001/XMLSchema#int">8</dcterms:hasVersion>
	<rdf:type rdf:resource="http://www.w3.org/2004/02/skos/core#Concept"/>
	<skos:broadMatch rdf:resource="http://resource.geosciml.org/classifier/cgi/lithology/metamorphic_rock"/>
	<skos:definition xml:lang="de">Gestein, das durch eine druckbetonte Metamorphose charakterisiert ist. Die Metamorphosebedingungen liegen dabei im Bereich der Glaukophanschiefer- bzw. Eklogit-Fazies (Fettes &amp; Desmons, 2007).</skos:definition>
	<skos:narrower rdf:resource="https://resource.geosphere.at/thes/lith/103"/>
	<skos:narrower rdf:resource="https://resource.geosphere.at/thes/lith/101"/>
	<skos:narrower rdf:resource="https://resource.geosphere.at/thes/lith/100"/>
	<skos:prefLabel xml:lang="en">High-pressure metamorphic rock</skos:prefLabel>
	<dcterms:created rdf:datatype="http://www.w3.org/2001/XMLSchema#dateTime">2012-03-12T13:46:52.000Z</dcterms:created>
	<skos:broadMatch rdf:resource="http://inspire.ec.europa.eu/codelist/LithologyValue/metamorphicRock"/>
</rdf:Description>

<rdf:Description rdf:about="https://resource.geosphere.at/thes/lith/101">
	<rdf:type rdf:resource="http://www.w3.org/2004/02/skos/core#Concept"/>
	<skos:definition xml:lang="de">Metamorphes Gestein, dessen blaue Farbe durch die Anwesenheit von Natrium-Amphibol (z.B. Glaukophan, Crossit) und Lawsonit gekennzeichnet ist (Fettes &amp; Desmons, 2007; Neuendorf et al., 2005).</skos:definition>
</rdf:Description>

<rdf:Description rdf:about="https://resource.geosphere.at/thes/lith/0">
	<dcterms:title xml:lang="de">Lithologische Beschreibungen und Gesteinsklassifikation</dcterms:title>
	<dcterms:title xml:lang="en">Lithological Descriptions and Rock Classification</dcterms:title>
</rdf:Description>

<rdf:Description rdf:about="https://resource.geosphere.at/thes/lith/adms/0.1">
	<dcterms:modified rdf:datatype="http://www.w3.org/2001/XMLSchema#dateTime">2025-02-24T10:38:10.827Z</dcterms:modified>
</rdf:Description>

<rdf:Description rdf:about="https://resource.geosphere.at/thes/lith/2">
	<dcterms:hasVersion rdf:datatype="http://www.w3.org/2001/XMLSchema#int">13</dcterms:hasVersion>
	<skos:narrower rdf:resource="https://resource.geosphere.at/thes/lith/4"/>
</rdf:Description>

<rdf:Description rdf:about="https://resource.geosphere.at/thes/lith/101">
	<dcterms:hasVersion rdf:datatype="http://www.w3.org/2001/XMLSchema#int">10</dcterms:hasVersion>
	<dcterms:date rdf:datatype="http://www.w3.org/2001/XMLSchema#dateTime">2011-03-16T09:19:05Z</dcterms:date>
	<skos:exactMatch rdf:resource="http://inspire.ec.europa.eu/codelist/LithologyValue/glaucophaneLawsoniteEpidoteMetamorphicRock"/>
	<skos:prefLabel xml:lang="en">Blueschist</skos:prefLabel>
	<dcterms:references rdf:resource="https://resource.geosphere.at/thes/citation/216"/>
	<colourHexCode xmlns="http://dbpedia.org/ontology/">#73B380</colourHexCode>
	<dcterms:created rdf:datatype="http://www.w3.org/2001/XMLSchema#dateTime">2012-03-12T10:31:26.000Z</dcterms:created>
	<dcterms:references rdf:resource="https://resource.geosphere.at/thes/citation/545"/>
	<skos:prefLabel xml:lang="de">Blauschiefer</skos:prefLabel>
	<skos:narrower rdf:resource="https://resource.geosphere.at/thes/lith/102"/>
	<skos:exactMatch rdf:resource="http://dbpedia.org/resource/Blueschist"/>
	<skos:definition xml:lang="en">A metamorphic rock (schist) with a bluish colour that is due to the presence of sodic amphibole (e.g., glaucophane, crossite) and lawsonite (Fettes &amp; Desmons, 2007; Neuendorf et al., 2005).</skos:definition>
	<skos:exactMatch rdf:resource="http://resource.geosciml.org/classifier/cgi/lithology/glaucophane_lawsonite_epidote_metamorphic_rock"/>
</rdf:Description>

<rdf:Description rdf:about="https://resource.geosphere.at/thes/lith/102">
	<skos:definition xml:lang="en">A schist with a bluish colour due to the presence of glaucophane (Fettes &amp; Desmons, 2007).</skos:definition>
	<skos:prefLabel xml:lang="en">Glaucophane-schist</skos:prefLabel>
	<dcterms:hasVersion rdf:datatype="http://www.w3.org/2001/XMLSchema#int">8</dcterms:hasVersion>
	<dcterms:date rdf:datatype="http://www.w3.org/2001/XMLSchema#dateTime">2011-03-16T09:19:05Z</dcterms:date>
	<skos:definition xml:lang="de">Schiefer, dessen blaue Farbe durch die Anwesenheit von Glaukophan hervorgerufen wird (Fettes &amp; Desmons, 2007).</skos:definition>
	<skos:prefLabel xml:lang="de">Glaukophan-Schiefer</skos:prefLabel>
	<dcterms:references rdf:resource="https://resource.geosphere.at/thes/citation/216"/>
	<skos:exactMatch rdf:resource="http://inspire.ec.europa.eu/codelist/LithologyValue/glaucophaneLawsoniteEpidoteMetamorphicRock"/>
	<skos:exactMatch rdf:resource="http://resource.geosciml.org/classifier/cgi/lithology/glaucophane_lawsonite_epidote_metamorphic_rock"/>
	<rdf:type rdf:resource="http://www.w3.org/2004/02/skos/core#Concept"/>
	<dcterms:created rdf:datatype="http://www.w3.org/2001/XMLSchema#dateTime">2012-03-12T13:31:41.000Z</dcterms:created>
	<colourHexCode xmlns="http://dbpedia.org/ontology/">#73B380</colourHexCode>
</rdf:Description>

<rdf:Description rdf:about="https://resource.geosphere.at/thes/lith/103">
	<dcterms:date rdf:datatype="http://www.w3.org/2001/XMLSchema#dateTime">2011-03-16T09:19:05Z</dcterms:date>
	<skos:prefLabel xml:lang="de">Weißschiefer</skos:prefLabel>
	<skos:definition xml:lang="de">Heller Schiefer, der Kyanit (Disthen) und Talk enthält. Weißschiefer sind Al-Mg-reiche Gesteine, welche unter eklogitfaziellen Bedingungen gebildet wurden (Fettes &amp; Desmons, 2007).</skos:definition>
	<dcterms:hasVersion rdf:datatype="http://www.w3.org/2001/XMLSchema#int">7</dcterms:hasVersion>
	<skos:broadMatch rdf:resource="http://inspire.ec.europa.eu/codelist/LithologyValue/metamorphicRock"/>
	<skos:broadMatch rdf:resource="http://resource.geosciml.org/classifier/cgi/lithology/metamorphic_rock"/>
	<dcterms:references rdf:resource="https://resource.geosphere.at/thes/citation/216"/>
	<rdf:type rdf:resource="http://www.w3.org/2004/02/skos/core#Concept"/>
	<skos:definition xml:lang="en">A light-coloured schist containing kyanite and talc. Whiteschists represent Al-Mg-rich rocks metamorphosed under eclogite facies conditions (Fettes &amp; Desmons, 2007).</skos:definition>
	<dcterms:created rdf:datatype="http://www.w3.org/2001/XMLSchema#dateTime">2012-03-12T16:39:27.000Z</dcterms:created>
	<skos:prefLabel xml:lang="en">Whiteschist</skos:prefLabel>
</rdf:Description>

<rdf:Description rdf:about="https://resource.geosphere.at/thes/lith/100">
	<dcterms:created rdf:datatype="http://www.w3.org/2001/XMLSchema#dateTime">2012-03-12T12:52:10.000Z</dcterms:created>
	<skos:exactMatch rdf:resource="http://dbpedia.org/resource/Eclogite"/>
	<rdf:type rdf:resource="http://www.w3.org/2004/02/skos/core#Concept"/>
	<skos:prefLabel xml:lang="de">Eklogit</skos:prefLabel>
	<dcterms:references rdf:resource="https://resource.geosphere.at/thes/citation/216"/>
	<dcterms:date rdf:datatype="http://www.w3.org/2001/XMLSchema#dateTime">2011-03-16T09:19:05Z</dcterms:date>
	<colourHexCode xmlns="http://dbpedia.org/ontology/">#33CC59</colourHexCode>
	<skos:prefLabel xml:lang="en">Eclogite</skos:prefLabel>
	<skos:exactMatch rdf:resource="http://inspire.ec.europa.eu/codelist/LithologyValue/eclogite"/>
	<skos:definition xml:lang="en">A plagioclase-free metamorphic rock composed of ≥ 75% vol. omphacite and garnet, both of which are present as major constituents but of neither of which forms &gt; 75% vol. (Fettes &amp; Desmons, 2007).</skos:definition>
	<skos:definition xml:lang="de">Plagioklasfreies metamorphes Gestein, das aus ≥ 75 % Omphazit und Granat zusammengesetzt ist. Beide Minerale sind Hauptbestandteile, wobei keines der beiden &gt; 75 % einnimmt (Fettes &amp; Desmons, 2007).</skos:definition>
	<skos:exactMatch rdf:resource="http://www.wikidata.org/entity/Q729546"/>
	<dcterms:hasVersion rdf:datatype="http://www.w3.org/2001/XMLSchema#int">9</dcterms:hasVersion>
	<skos:exactMatch rdf:resource="http://resource.geosciml.org/classifier/cgi/lithology/eclogite"/>
	<skos:exactMatch rdf:resource="http://data.bgs.ac.uk/id/EarthMaterialClass/RockName/ECLOG"/>
</rdf:Description>

<rdf:Description rdf:about="https://resource.geosphere.at/thes/lith/127">
	<skos:exactMatch rdf:resource="http://dbpedia.org/resource/Serpentinite"/>
	<skos:prefLabel xml:lang="en">Serpentinite</skos:prefLabel>
	<skos:exactMatch rdf:resource="http://www.wikidata.org/entity/Q737339"/>
	<dcterms:hasVersion rdf:datatype="http://www.w3.org/2001/XMLSchema#int">8</dcterms:hasVersion>
	<skos:exactMatch rdf:resource="http://resource.geosciml.org/classifier/cgi/lithology/serpentinite"/>
	<skos:definition xml:lang="en">A metamorphic rock with &gt; 75% vol. minerals of the serpentine group (Fettes &amp; Desmons, 2007).</skos:definition>
	<foaf:depiction rdf:resource="https://resource.geosphere.at/img/thes/Serpentinit.jpg"/>
	<skos:exactMatch rdf:resource="http://data.bgs.ac.uk/id/EarthMaterialClass/RockName/SEPITE"/>
	<skos:definition xml:lang="de">Metamorphes Gestein, welches zu &gt; 75 Vol.-% aus Mineralen der Serpentin-Gruppe besteht (Fettes &amp; Desmons, 2007).</skos:definition>
	<rdf:type rdf:resource="http://www.w3.org/2004/02/skos/core#Concept"/>
	<colourHexCode xmlns="http://dbpedia.org/ontology/">#8CBF80</colourHexCode>
	<dcterms:created rdf:datatype="http://www.w3.org/2001/XMLSchema#dateTime">2013-04-05T09:40:15.000Z</dcterms:created>
	<skos:exactMatch rdf:resource="http://inspire.ec.europa.eu/codelist/LithologyValue/serpentinite"/>
	<dcterms:references rdf:resource="https://resource.geosphere.at/thes/citation/216"/>
	<dcterms:date rdf:datatype="http://www.w3.org/2001/XMLSchema#dateTime">2011-03-16T09:19:05Z</dcterms:date>
	<skos:prefLabel xml:lang="de">Serpentinit</skos:prefLabel>
</rdf:Description>

<rdf:Description rdf:about="https://resource.geosphere.at/thes/lith/108">
	<skos:definition xml:lang="de">Metamorphes (metasomatisches) Karbonat- und/oder karbonatführendes und/oder Kalksilikatgestein, welches im Fall von Kalksilikaten auch karbonatfrei sein kann. Der Begriff umfasst Marmor, Karbonat-Silikatgestein, Kalksilikatgestein und karbonatführende Silikatgesteine (Fettes &amp; Desmons, 2007).</skos:definition>
	<skos:prefLabel xml:lang="de">Metakarbonatisches Gestein</skos:prefLabel>
	<dcterms:hasVersion rdf:datatype="http://www.w3.org/2001/XMLSchema#int">7</dcterms:hasVersion>
	<skos:exactMatch rdf:resource="http://resource.geosciml.org/classifier/cgi/lithology/metamorphic_rock"/>
	<skos:narrower rdf:resource="https://resource.geosphere.at/thes/lith/116"/>
	<skos:narrower rdf:resource="https://resource.geosphere.at/thes/lith/113"/>
	<skos:narrower rdf:resource="https://resource.geosphere.at/thes/lith/112"/>
	<skos:narrower rdf:resource="https://resource.geosphere.at/thes/lith/109"/>
	<skos:definition xml:lang="en">A metamorphic (metasomatic) carbonate and/or carbonate-bearing and/or calc-silicate rock which, in the case of calc-silicate rocks, can be carbonate-free. The term includes marble, carbonate-silicate rocks, calc-silicate rocks, and carbonate-bearing silicate rocks (Fettes &amp; Desmons, 2007).</skos:definition>
	<skos:broadMatch rdf:resource="http://inspire.ec.europa.eu/codelist/LithologyValue/metasomaticRock"/>
	<skos:prefLabel xml:lang="en">Metacarbonatic rock</skos:prefLabel>
	<dcterms:references rdf:resource="https://resource.geosphere.at/thes/citation/216"/>
	<rdf:type rdf:resource="http://www.w3.org/2004/02/skos/core#Concept"/>
	<dcterms:created rdf:datatype="http://www.w3.org/2001/XMLSchema#dateTime">2012-03-12T14:27:51.000Z</dcterms:created>
	<dcterms:date rdf:datatype="http://www.w3.org/2001/XMLSchema#dateTime">2011-03-16T09:19:05Z</dcterms:date>
	<skos:scopeNote xml:lang="de">Beim Benutzen des Präfixes 'Meta,' in Kombination mit dem Protolithnamen zur Benennung von Metamorphiten, liegt der Fokus auf der Veranschaulichung der geologischen Entwicklung, jedoch nicht auf dem Grad der Metamorphose.</skos:scopeNote>
</rdf:Description>

<rdf:Description rdf:about="https://resource.geosphere.at/thes/lith/113">
	<rdf:type rdf:resource="http://www.w3.org/2004/02/skos/core#Concept"/>
	<dcterms:hasVersion rdf:datatype="http://www.w3.org/2001/XMLSchema#int">7</dcterms:hasVersion>
	<dcterms:date rdf:datatype="http://www.w3.org/2001/XMLSchema#dateTime">2011-03-16T09:19:05Z</dcterms:date>
	<skos:broadMatch rdf:resource="http://inspire.ec.europa.eu/codelist/LithologyValue/metamorphicRock"/>
	<skos:definition xml:lang="de">Metamorphes Gestein, welches hauptsächlich aus Kalksilikatmineralen und &lt; 5 % Karbonatmineralen (Calcit und/oder Aragonit und/oder Dolomit) besteht (Fettes &amp; Desmons, 2007).</skos:definition>
	<skos:definition xml:lang="en">A metamorphic rock mainly composed of calc-silicate minerals containing &lt; 5% vol. of carbonate minerals (calcite and/or aragonite and/or dolomite) (Fettes &amp; Desmons, 2007).</skos:definition>
	<dcterms:references rdf:resource="https://resource.geosphere.at/thes/citation/216"/>
	<skos:prefLabel xml:lang="en">Calc-silicate rock</skos:prefLabel>
	<skos:broadMatch rdf:resource="http://resource.geosciml.org/classifier/cgi/lithology/metamorphic_rock"/>
	<dcterms:created rdf:datatype="http://www.w3.org/2001/XMLSchema#dateTime">2012-01-25T15:02:56.000Z</dcterms:created>
	<skos:prefLabel xml:lang="de">Kalksilikatgestein</skos:prefLabel>
</rdf:Description>

<rdf:Description rdf:about="https://resource.geosphere.at/thes/lith/112">
	<skos:prefLabel xml:lang="de">Karbonat-Silikatgestein</skos:prefLabel>
	<skos:narrower rdf:resource="https://resource.geosphere.at/thes/lith/115"/>
	<skos:definition xml:lang="en">Metamorphic rock mainly composed of silicate minerals (including calc-silicate minerals) containing between 5 and 50% vol. of carbonate minerals (calcite and/or aragonite and/or dolomite) (Fettes &amp; Desmons, 2007).</skos:definition>
	<dcterms:references rdf:resource="https://resource.geosphere.at/thes/citation/216"/>
	<rdf:type rdf:resource="http://www.w3.org/2004/02/skos/core#Concept"/>
	<skos:prefLabel xml:lang="en">Carbonate-silicate rock</skos:prefLabel>
	<dcterms:date rdf:datatype="http://www.w3.org/2001/XMLSchema#dateTime">2011-03-16T09:19:05Z</dcterms:date>
	<skos:definition xml:lang="de">Metamorphes Gestein, welches hauptsächlich aus Silikaten (einschließlich der Kalksilikatminerale) und 5–50 % Karbonatmineralen (Calcit und/oder Aragonit und/oder Dolomit) besteht (Fettes &amp; Desmons, 2007).</skos:definition>
	<dcterms:hasVersion rdf:datatype="http://www.w3.org/2001/XMLSchema#int">8</dcterms:hasVersion>
	<dcterms:created rdf:datatype="http://www.w3.org/2001/XMLSchema#dateTime">2012-03-12T10:54:46.000Z</dcterms:created>
	<skos:broadMatch rdf:resource="http://inspire.ec.europa.eu/codelist/LithologyValue/metamorphicRock"/>
	<skos:broadMatch rdf:resource="http://resource.geosciml.org/classifier/cgi/lithology/metamorphic_rock"/>
</rdf:Description>

<rdf:Description rdf:about="https://resource.geosphere.at/thes/lith/115">
	<dcterms:date rdf:datatype="http://www.w3.org/2001/XMLSchema#dateTime">2011-03-16T09:19:05Z</dcterms:date>
	<skos:closeMatch rdf:resource="http://resource.geosciml.org/classifier/cgi/lithology/mica_schist"/>
	<skos:definition xml:lang="en">A metacarbonate rock with a schistose structure and composed of calcite oriented mica and quartz (Fettes &amp; Desmons, 2007).</skos:definition>
	<skos:broadMatch rdf:resource="http://inspire.ec.europa.eu/codelist/LithologyValue/micaSchist"/>
	<skos:prefLabel xml:lang="en">Calc-mica schist</skos:prefLabel>
	<dcterms:hasVersion rdf:datatype="http://www.w3.org/2001/XMLSchema#int">7</dcterms:hasVersion>
	<rdf:type rdf:resource="http://www.w3.org/2004/02/skos/core#Concept"/>
	<dcterms:references rdf:resource="https://resource.geosphere.at/thes/citation/216"/>
	<skos:definition xml:lang="de">Metakarbonatisches Gestein mit einer schiefrigen Struktur, welches sich aus Calcit, orientiertem Glimmer und Quarz zusammensetzt (Fettes &amp; Desmons, 2007).</skos:definition>
	<skos:prefLabel xml:lang="de">Kalkglimmerschiefer</skos:prefLabel>
	<dcterms:created rdf:datatype="http://www.w3.org/2001/XMLSchema#dateTime">2012-01-25T15:03:38.000Z</dcterms:created>
</rdf:Description>

<rdf:Description rdf:about="https://resource.geosphere.at/thes/lith/116">
	<skos:prefLabel xml:lang="en">Ophicarbonate</skos:prefLabel>
	<skos:definition xml:lang="en">A rock consisting of serpentinite and carbonate minerals. The serpentinite is commonly fragmented or brecciated, veined, and impregnated by the carbonate material (calcite, dolomite, or magnesite) (Fettes &amp; Desmons, 2007).</skos:definition>
	<skos:broadMatch rdf:resource="http://resource.geosciml.org/classifier/cgi/lithology/metamorphic_rock"/>
	<skos:narrower rdf:resource="https://resource.geosphere.at/thes/lith/117"/>
	<skos:prefLabel xml:lang="de">Ophikarbonat</skos:prefLabel>
	<dcterms:hasVersion rdf:datatype="http://www.w3.org/2001/XMLSchema#int">7</dcterms:hasVersion>
	<rdf:type rdf:resource="http://www.w3.org/2004/02/skos/core#Concept"/>
	<skos:broadMatch rdf:resource="http://inspire.ec.europa.eu/codelist/LithologyValue/metamorphicRock"/>
	<dcterms:date rdf:datatype="http://www.w3.org/2001/XMLSchema#dateTime">2011-03-16T09:19:05Z</dcterms:date>
	<skos:definition xml:lang="de">Gestein, welches aus Serpentinit und Karbonatmineralen besteht. Der Serpentinit ist typischerweise fragmentiert oder brekziert, von Adern durchzogen und mit karbonatischem Material (Calcit, Dolomit oder Magnesit) imprägniert (Fettes &amp; Desmons, 2007).</skos:definition>
	<dcterms:created rdf:datatype="http://www.w3.org/2001/XMLSchema#dateTime">2012-03-12T15:50:13.000Z</dcterms:created>
	<dcterms:references rdf:resource="https://resource.geosphere.at/thes/citation/216"/>
</rdf:Description>

<rdf:Description rdf:about="https://resource.geosphere.at/thes/lith/117">
	<skos:definition xml:lang="de">Ophikarbonat, in dem Calcit das überwiegende Karbonatmineral darstellt (Fettes &amp; Desmons, 2007).</skos:definition>
	<dcterms:created rdf:datatype="http://www.w3.org/2001/XMLSchema#dateTime">2012-01-25T15:04:34.000Z</dcterms:created>
	<skos:broadMatch rdf:resource="http://inspire.ec.europa.eu/codelist/LithologyValue/metamorphicRock"/>
	<rdf:type rdf:resource="http://www.w3.org/2004/02/skos/core#Concept"/>
	<skos:prefLabel xml:lang="en">Ophicalcite</skos:prefLabel>
	<dcterms:hasVersion rdf:datatype="http://www.w3.org/2001/XMLSchema#int">6</dcterms:hasVersion>
	<skos:prefLabel xml:lang="de">Ophicalcit</skos:prefLabel>
	<dcterms:date rdf:datatype="http://www.w3.org/2001/XMLSchema#dateTime">2011-03-16T09:19:05Z</dcterms:date>
	<skos:broadMatch rdf:resource="http://resource.geosciml.org/classifier/cgi/lithology/metamorphic_rock"/>
	<dcterms:references rdf:resource="https://resource.geosphere.at/thes/citation/216"/>
	<skos:definition xml:lang="en">A variety of ophicarbonate in which calcite is the predominant carbonate mineral (Fettes &amp; Desmons, 2007).</skos:definition>
	<colourHexCode xmlns="http://dbpedia.org/ontology/">#3D8A3D</colourHexCode>
</rdf:Description>

<rdf:Description rdf:about="https://resource.geosphere.at/thes/lith/109">
	<dcterms:date rdf:datatype="http://www.w3.org/2001/XMLSchema#dateTime">2011-03-16T09:19:05Z</dcterms:date>
	<skos:exactMatch rdf:resource="http://www.wikidata.org/entity/Q40861"/>
	<skos:prefLabel xml:lang="en">Marble</skos:prefLabel>
	<skos:narrower rdf:resource="https://resource.geosphere.at/thes/lith/241"/>
	<skos:narrower rdf:resource="https://resource.geosphere.at/thes/lith/242"/>
	<dcterms:hasVersion rdf:datatype="http://www.w3.org/2001/XMLSchema#int">9</dcterms:hasVersion>
	<skos:definition xml:lang="en">A metamorphic rock containing &gt; 50% vol. of carbonate minerals (calcite and/or aragonite and/or dolomite) (Fettes &amp; Desmons, 2007).</skos:definition>
	<skos:prefLabel xml:lang="de">Marmor</skos:prefLabel>
	<skos:narrower rdf:resource="https://resource.geosphere.at/thes/lith/110"/>
	<skos:narrower rdf:resource="https://resource.geosphere.at/thes/lith/111"/>
	<rdf:type rdf:resource="http://www.w3.org/2004/02/skos/core#Concept"/>
	<skos:exactMatch rdf:resource="http://data.bgs.ac.uk/id/EarthMaterialClass/RockName/MARBLE"/>
	<skos:exactMatch rdf:resource="http://resource.geosciml.org/classifier/cgi/lithology/marble"/>
	<dcterms:created rdf:datatype="http://www.w3.org/2001/XMLSchema#dateTime">2013-04-05T09:34:23.000Z</dcterms:created>
	<colourHexCode xmlns="http://dbpedia.org/ontology/">#33B3E6</colourHexCode>
	<dcterms:references rdf:resource="https://resource.geosphere.at/thes/citation/216"/>
	<skos:exactMatch rdf:resource="http://dbpedia.org/resource/Marble"/>
	<skos:definition xml:lang="de">Metamorphes Gestein, welches &gt; 50 % Karbonatminerale (Calcit und/oder Aragonit und/oder Dolomit) beinhaltet (Fettes &amp; Desmons, 2007).</skos:definition>
	<skos:exactMatch rdf:resource="http://inspire.ec.europa.eu/codelist/LithologyValue/marble"/>
	<foaf:depiction rdf:resource="https://resource.geosphere.at/img/thes/Marmor.jpg"/>
</rdf:Description>

<rdf:Description rdf:about="https://resource.geosphere.at/thes/lith/241">
	<rdf:type rdf:resource="http://www.w3.org/2004/02/skos/core#Concept"/>
	<dcterms:created rdf:datatype="http://www.w3.org/2001/XMLSchema#dateTime">2012-01-18T10:12:03.000Z</dcterms:created>
	<status xmlns="https://resource.geosphere.at/schema/thes#" rdf:datatype="http://www.w3.org/2001/XMLSchema#integer">1</status>
	<dcterms:hasVersion rdf:datatype="http://www.w3.org/2001/XMLSchema#int">12</dcterms:hasVersion>
	<skos:prefLabel xml:lang="en">Calcitic marble</skos:prefLabel>
	<dcterms:references rdf:resource="https://resource.geosphere.at/thes/citation/216"/>
	<skos:definition xml:lang="de">Marmor dessen Karbonatminerale überwiegend aus Calcit bestehen (verändert nach Fettes &amp; Desmons, 2007).</skos:definition>
	<skos:hiddenLabel xml:lang="de">Calcmarmor</skos:hiddenLabel>
	<skos:prefLabel xml:lang="de">Calcit-Marmor</skos:prefLabel>
	<skos:definition xml:lang="en">A marble in which the carbonate minerals are predominantly calcite (modified from Fettes &amp; Desmons, 2007).</skos:definition>
	<skos:altLabel xml:lang="de">Kalkmarmor</skos:altLabel>
	<skos:broadMatch rdf:resource="http://inspire.ec.europa.eu/codelist/LithologyValue/marble"/>
	<skos:altLabel xml:lang="de">Kalzit-Marmor</skos:altLabel>
	<skos:broadMatch rdf:resource="http://resource.geosciml.org/classifier/cgi/lithology/marble"/>
</rdf:Description>

<rdf:Description rdf:about="https://resource.geosphere.at/thes/lith/111">
	<dcterms:created rdf:datatype="http://www.w3.org/2001/XMLSchema#dateTime">2012-03-12T13:51:26.000Z</dcterms:created>
	<skos:narrower rdf:resource="https://resource.geosphere.at/thes/lith/114"/>
	<skos:prefLabel xml:lang="en">Impure marble</skos:prefLabel>
	<skos:broadMatch rdf:resource="http://inspire.ec.europa.eu/codelist/LithologyValue/marble"/>
	<rdf:type rdf:resource="http://www.w3.org/2004/02/skos/core#Concept"/>
	<dcterms:hasVersion rdf:datatype="http://www.w3.org/2001/XMLSchema#int">7</dcterms:hasVersion>
	<skos:definition xml:lang="de">Marmor, der &lt; 95 Vol.-% Karbonatminerale (Calcit und/oder Aragonit und/oder Dolomit) enthält (Fettes &amp; Desmons, 2007).</skos:definition>
	<skos:broadMatch rdf:resource="http://resource.geosciml.org/classifier/cgi/lithology/marble"/>
	<skos:definition xml:lang="en">A marble that contains &lt; 95% vol. of carbonate minerals (calcite and/or aragonite and/or dolomite) (Fettes &amp; Desmons, 2007).</skos:definition>
	<dcterms:date rdf:datatype="http://www.w3.org/2001/XMLSchema#dateTime">2011-03-16T09:19:05Z</dcterms:date>
	<dcterms:references rdf:resource="https://resource.geosphere.at/thes/citation/216"/>
	<skos:prefLabel xml:lang="de">Unreiner Marmor</skos:prefLabel>
	<skos:altLabel xml:lang="de">Silikatmarmor</skos:altLabel>
</rdf:Description>

<rdf:Description rdf:about="https://resource.geosphere.at/thes/lith/114">
	<skos:prefLabel xml:lang="de">Kalkschiefer</skos:prefLabel>
	<dcterms:hasVersion rdf:datatype="http://www.w3.org/2001/XMLSchema#int">6</dcterms:hasVersion>
	<dcterms:date rdf:datatype="http://www.w3.org/2001/XMLSchema#dateTime">2011-03-16T09:19:05Z</dcterms:date>
	<skos:definition xml:lang="en">A metamorphosed argillaceous limestone containing calcite as a substantial component and with a schistose structure produced by parallelism of platy minerals (Fettes &amp; Desmons, 2007).</skos:definition>
	<skos:broadMatch rdf:resource="http://resource.geosciml.org/classifier/cgi/lithology/marble"/>
	<dcterms:references rdf:resource="https://resource.geosphere.at/thes/citation/216"/>
	<skos:definition xml:lang="de">Metamorpher Kalkmergel, der als Hauptbestandteil Calcit enthält, mit einer schiefrigen Struktur, welche durch die parallele Anordnung von blättrigen Mineralen entsteht (Fettes &amp; Desmons, 2007).</skos:definition>
	<dcterms:created rdf:datatype="http://www.w3.org/2001/XMLSchema#dateTime">2013-04-05T09:31:32.000Z</dcterms:created>
	<skos:broadMatch rdf:resource="http://inspire.ec.europa.eu/codelist/LithologyValue/marble"/>
	<foaf:depiction rdf:resource="https://resource.geosphere.at/img/thes/Kalkschiefer.jpg"/>
	<skos:prefLabel xml:lang="en">Calc-schist</skos:prefLabel>
	<rdf:type rdf:resource="http://www.w3.org/2004/02/skos/core#Concept"/>
	<colourHexCode xmlns="http://dbpedia.org/ontology/">#33B3E6</colourHexCode>
</rdf:Description>

<rdf:Description rdf:about="https://resource.geosphere.at/thes/lith/242">
	<skos:prefLabel xml:lang="de">Dolomit-Marmor</skos:prefLabel>
	<skos:broadMatch rdf:resource="http://inspire.ec.europa.eu/codelist/LithologyValue/marble"/>
	<skos:altLabel xml:lang="de">Dolomitmarmor</skos:altLabel>
	<skos:definition xml:lang="en">A marble in which the carbonate minerals consist predominantly of dolomite (modified from Fettes &amp; Desmons, 2007).</skos:definition>
	<dcterms:hasVersion rdf:datatype="http://www.w3.org/2001/XMLSchema#int">11</dcterms:hasVersion>
	<skos:prefLabel xml:lang="en">Dolomitic marble</skos:prefLabel>
	<dcterms:created rdf:datatype="http://www.w3.org/2001/XMLSchema#dateTime">2012-01-18T10:18:47.000Z</dcterms:created>
	<skos:broadMatch rdf:resource="http://resource.geosciml.org/classifier/cgi/lithology/marble"/>
	<dcterms:references rdf:resource="https://resource.geosphere.at/thes/citation/216"/>
	<rdf:type rdf:resource="http://www.w3.org/2004/02/skos/core#Concept"/>
	<skos:definition xml:lang="de">Marmor dessen Karbonatminerale überwiegend aus Dolomit bestehen (verändert nach Fettes &amp; Desmons., 2007).</skos:definition>
</rdf:Description>

<rdf:Description rdf:about="https://resource.geosphere.at/thes/lith/110">
	<skos:definition xml:lang="de">Marmor, der &gt; 95 Vol.-% Karbonatminerale (Calcit und/oder Aragonit und/oder Dolomit) beinhaltet (Fettes &amp; Desmons, 2007).</skos:definition>
	<skos:prefLabel xml:lang="en">Pure marble</skos:prefLabel>
	<skos:prefLabel xml:lang="de">Reiner Marmor</skos:prefLabel>
	<dcterms:hasVersion rdf:datatype="http://www.w3.org/2001/XMLSchema#int">7</dcterms:hasVersion>
	<rdf:type rdf:resource="http://www.w3.org/2004/02/skos/core#Concept"/>
	<skos:broadMatch rdf:resource="http://resource.geosciml.org/classifier/cgi/lithology/marble"/>
	<skos:definition xml:lang="en">A marble that contains &gt; 95% vol. of carbonate minerals (calcite and/or aragonite and/or dolomite) (Fettes &amp; Desmons, 2007).</skos:definition>
	<dcterms:references rdf:resource="https://resource.geosphere.at/thes/citation/216"/>
	<dcterms:created rdf:datatype="http://www.w3.org/2001/XMLSchema#dateTime">2012-03-12T15:58:31.000Z</dcterms:created>
	<skos:broadMatch rdf:resource="http://inspire.ec.europa.eu/codelist/LithologyValue/marble"/>
	<dcterms:date rdf:datatype="http://www.w3.org/2001/XMLSchema#dateTime">2011-03-16T09:19:05Z</dcterms:date>
</rdf:Description>

<rdf:Description rdf:about="https://resource.geosphere.at/thes/lith/119">
	<skos:exactMatch rdf:resource="http://dbpedia.org/resource/Granulite"/>
	<dcterms:hasVersion rdf:datatype="http://www.w3.org/2001/XMLSchema#int">8</dcterms:hasVersion>
	<dcterms:created rdf:datatype="http://www.w3.org/2001/XMLSchema#dateTime">2012-03-12T13:40:20.000Z</dcterms:created>
	<skos:definition xml:lang="de">Hochgradig metamorphes Gestein, in dem die Fe-Mg-Silikate überwiegend hydroxylfrei sind. Kritisch sind die Anwesenheit von Feldspat bzw. die Abwesenheit von primärem Muskovit. Cordierit kann als Bestandteil vorkommen. Der Begriff beinhaltet mafische (mit &gt; 30 % mafischen Mineralen, überwiegend Pyroxen) Granulite und felsische (mit &lt; 30 % mafischen Mineralen) Granulite (Fettes &amp; Desmons, 2007).</skos:definition>
	<skos:exactMatch rdf:resource="http://inspire.ec.europa.eu/codelist/LithologyValue/granulite"/>
	<dcterms:date rdf:datatype="http://www.w3.org/2001/XMLSchema#dateTime">2011-03-16T09:19:05Z</dcterms:date>
	<skos:exactMatch rdf:resource="http://resource.geosciml.org/classifier/cgi/lithology/granulite"/>
	<skos:definition xml:lang="en">A high-grade metamorphic rock in which Fe-Mg silicates are predominantly hydroxyl-free. The presence of feldspar and the absence of primary muscovite are critical. Cordierite may also be present. The term includes mafic granulites (with &gt; 30% mafic minerals, predominantly pyroxene) and felsic granulites (with &lt; 30% mafic minerals, predominantly pyroxene) (Fettes &amp; Desmons, 2007).</skos:definition>
	<skos:prefLabel xml:lang="en">Granulite</skos:prefLabel>
	<dcterms:references rdf:resource="https://resource.geosphere.at/thes/citation/216"/>
	<rdf:type rdf:resource="http://www.w3.org/2004/02/skos/core#Concept"/>
	<skos:prefLabel xml:lang="de">Granulit</skos:prefLabel>
	<colourHexCode xmlns="http://dbpedia.org/ontology/">#66CC80</colourHexCode>
</rdf:Description>

<rdf:Description rdf:about="https://resource.geosphere.at/thes/lith/118">
	<dcterms:hasVersion rdf:datatype="http://www.w3.org/2001/XMLSchema#int">11</dcterms:hasVersion>
	<skos:exactMatch rdf:resource="http://resource.geosciml.org/classifier/cgi/lithology/amphibolite"/>
	<skos:exactMatch rdf:resource="http://dbpedia.org/resource/Amphibolite"/>
	<rdf:type rdf:resource="http://www.w3.org/2004/02/skos/core#Concept"/>
	<dcterms:references rdf:resource="https://resource.geosphere.at/thes/citation/216"/>
	<colourHexCode xmlns="http://dbpedia.org/ontology/">#40D973</colourHexCode>
	<skos:exactMatch rdf:resource="http://data.bgs.ac.uk/id/EarthMaterialClass/RockName/AMPHB"/>
	<dcterms:date rdf:datatype="http://www.w3.org/2001/XMLSchema#dateTime">2011-03-16T09:19:05Z</dcterms:date>
	<skos:definition xml:lang="en">A gneissose or granofelsic metamorphic rock mainly consisting of green, brown or black amphibole and plagioclase (including albite), which combined form ≥ 75% of the rock and both of which are present as major constituents; the amphibole constitutes ≥ 50% of the total mafic constituents and is present in an amount of ≥ 30%. Other common minerals include quartz , clinopyroxene, garnet, epidote-group minerals, biotite, titanite and scapolite (Fettes &amp; Desmons, 2007 ).</skos:definition>
	<skos:definition xml:lang="de">Metamorphes Gestein mit gneisiger oder felsischer Struktur, welches hauptsächlich aus grünem, braunem und schwarzem Amphibol und Plagioklas (einschließlich Albit) besteht. Beide bilden zusammen ≥ 75 % des Gesteins und beide kommen darin als Hauptbestandteil vor. Der Amphibol bildet ≥ 50 % der mafischen Bestandteile und ist mit einem Anteil von ≥ 30 % am Gesamtgestein präsent. Andere typische Minerale sind Quarz, Klinopyroxen, Granat, Minerale der Epidot-Gruppe, Biotit, Titanit und Skapolith (Fettes &amp; Desmons, 2007)</skos:definition>
	<skos:prefLabel xml:lang="de">Amphibolit</skos:prefLabel>
	<skos:exactMatch rdf:resource="http://inspire.ec.europa.eu/codelist/LithologyValue/amphibolite"/>
	<skos:prefLabel xml:lang="en">Amphibolite</skos:prefLabel>
	<dcterms:created rdf:datatype="http://www.w3.org/2001/XMLSchema#dateTime">2012-03-08T09:35:13.000Z</dcterms:created>
	<foaf:depiction rdf:resource="https://resource.geosphere.at/img/thes/amphibolit.jpg"/>
	<foaf:depiction rdf:resource="https://resource.geosphere.at/img/thes/Grt-Amphibolit.jpg"/>
</rdf:Description>

<rdf:Description rdf:about="https://resource.geosphere.at/thes/lith/129">
	<skos:narrower rdf:resource="https://resource.geosphere.at/thes/lith/130"/>
	<skos:narrower rdf:resource="https://resource.geosphere.at/thes/lith/131"/>
	<foaf:depiction rdf:resource="https://resource.geosphere.at/img/thes/Gneis.jpg"/>
	<skos:narrowMatch rdf:resource="http://resource.geosciml.org/classifier/cgi/lithology/gneiss"/>
	<rdf:type rdf:resource="http://www.w3.org/2004/02/skos/core#Concept"/>
	<skos:exactMatch rdf:resource="http://data.bgs.ac.uk/id/EarthMaterialClass/RockName/GNSS"/>
	<skos:prefLabel xml:lang="de">Gneis</skos:prefLabel>
	<skos:prefLabel xml:lang="en">Gneiss</skos:prefLabel>
	<skos:definition xml:lang="en">A metamorphic rock usually with a gneissose structure (a foliation that is either poorly developed or a spaced foliation so that the rock will split in on a scale of &gt; 1 cm, mineralogical and/or lithological layering is commonly present) where quartz and feldspar are essential components with &gt; 20% feldspar and &lt; 50% mica being the compositional boundary to schist (Fettes &amp; Desmons, 2007; Neuendorf et al., 2005).</skos:definition>
	<dcterms:references rdf:resource="https://resource.geosphere.at/thes/citation/545"/>
	<colourHexCode xmlns="http://dbpedia.org/ontology/">#61E07A</colourHexCode>
	<dcterms:date rdf:datatype="http://www.w3.org/2001/XMLSchema#dateTime">2011-03-16T09:19:05Z</dcterms:date>
	<dcterms:hasVersion rdf:datatype="http://www.w3.org/2001/XMLSchema#int">14</dcterms:hasVersion>
	<skos:exactMatch rdf:resource="http://inspire.ec.europa.eu/codelist/LithologyValue/gneiss"/>
	<dcterms:references rdf:resource="https://resource.geosphere.at/thes/citation/216"/>
	<skos:definition xml:lang="de">Metamorphes Gestein mit üblicherweise gneisiger Struktur (einer Foliation, die entweder schlecht entwickelt ist oder in regelmäßigen Abständen vorkommt, sodass das Gestein eine Spaltbarkeit von &gt; 1 cm zeigt; typisch ist ein mineralogischer und/oder lithologischer Lagenbau), dessen Hauptbestandteile Quarz und Feldspat sind, wobei &gt; 20 % Feldspat und &lt; 50 % Glimmer die Zusammensetzungsgrenze zu Schiefer markieren (Fettes &amp; Desmons, 2007; Neuendorf et al., 2005).</skos:definition>
	<dcterms:created rdf:datatype="http://www.w3.org/2001/XMLSchema#dateTime">2013-04-05T09:28:39.000Z</dcterms:created>
</rdf:Description>

<rdf:Description rdf:about="https://resource.geosphere.at/thes/lith/131">
	<skos:narrower rdf:resource="https://resource.geosphere.at/thes/lith/132"/>
	<skos:exactMatch rdf:resource="http://data.bgs.ac.uk/id/EarthMaterialClass/RockName/PGNSS"/>
	<skos:definition xml:lang="de">Gneis, bei dem Mineralogie und Textur auf einen sedimentären Protolith hinweist. Relativ variable Gesteinszusammensetzung im dm- bis m-Bereich im Vergleich zu Orthogneis (verändert nach Neuendorf et al., 2005).</skos:definition>
	<rdf:type rdf:resource="http://www.w3.org/2004/02/skos/core#Concept"/>
	<skos:definition xml:lang="en">A gneiss with mineralogy and texture indicating derivation from a sedimentary protolith. Relatively variable rock character on a dm-m scale compared to orthogneiss (modified from Neuendorf et al., 2005).</skos:definition>
	<skos:prefLabel xml:lang="en">Paragneiss</skos:prefLabel>
	<dcterms:date rdf:datatype="http://www.w3.org/2001/XMLSchema#dateTime">2011-03-16T09:19:05Z</dcterms:date>
	<colourHexCode xmlns="http://dbpedia.org/ontology/">#85F09E</colourHexCode>
	<skos:exactMatch rdf:resource="http://resource.geosciml.org/classifier/cgi/lithology/paragneiss"/>
	<dcterms:references rdf:resource="https://resource.geosphere.at/thes/citation/545"/>
	<dcterms:hasVersion rdf:datatype="http://www.w3.org/2001/XMLSchema#int">8</dcterms:hasVersion>
	<skos:exactMatch rdf:resource="http://inspire.ec.europa.eu/codelist/LithologyValue/paragneiss"/>
	<foaf:depiction rdf:resource="https://resource.geosphere.at/img/thes/Paragneis.jpg"/>
	<skos:prefLabel xml:lang="de">Paragneis</skos:prefLabel>
	<dcterms:created rdf:datatype="http://www.w3.org/2001/XMLSchema#dateTime">2013-04-05T09:36:24.000Z</dcterms:created>
</rdf:Description>

<rdf:Description rdf:about="https://resource.geosphere.at/thes/lith/132">
	<skos:prefLabel xml:lang="de">Arkosegneis</skos:prefLabel>
	<skos:definition xml:lang="de">Paragneis, dessen Protolith als Arkose (ein Feldspat reicher Sandstein) identifiziert werden kann. Typisch für niedrigmetamorphe Bedingungen (bis zur Grünschieferfazies) mit Quarz und Feldspat als Hauptbestandteile (Vinx, 2007).</skos:definition>
	<dcterms:date rdf:datatype="http://www.w3.org/2001/XMLSchema#dateTime">2011-03-16T09:19:05Z</dcterms:date>
	<skos:broadMatch rdf:resource="http://inspire.ec.europa.eu/codelist/LithologyValue/paragneiss"/>
	<dcterms:hasVersion rdf:datatype="http://www.w3.org/2001/XMLSchema#int">12</dcterms:hasVersion>
	<skos:related rdf:resource="https://resource.geosphere.at/thes/lith/186"/>
	<dcterms:references rdf:resource="https://resource.geosphere.at/thes/citation/878"/>
	<skos:prefLabel xml:lang="en">Arkosic gneiss</skos:prefLabel>
	<skos:definition xml:lang="en">A paragneiss for which the protolith can be identified as an arkose (a feldspar-rich sandstone). Indicative of lower metamorphic conditions (up to greenshist facies), with quartz and feldspar as the major constituents (Vinx, 2007).</skos:definition>
	<skos:broadMatch rdf:resource="http://resource.geosciml.org/classifier/cgi/lithology/paragneiss"/>
	<rdf:type rdf:resource="http://www.w3.org/2004/02/skos/core#Concept"/>
	<dcterms:created rdf:datatype="http://www.w3.org/2001/XMLSchema#dateTime">2012-03-12T09:40:50.000Z</dcterms:created>
</rdf:Description>

<rdf:Description rdf:about="https://resource.geosphere.at/thes/lith/130">
	<skos:narrower rdf:resource="https://resource.geosphere.at/thes/lith/133"/>
	<skos:prefLabel xml:lang="de">Orthogneis</skos:prefLabel>
	<skos:narrower rdf:resource="https://resource.geosphere.at/thes/lith/135"/>
	<skos:narrower rdf:resource="https://resource.geosphere.at/thes/lith/134"/>
	<rdf:type rdf:resource="http://www.w3.org/2004/02/skos/core#Concept"/>
	<skos:exactMatch rdf:resource="http://resource.geosciml.org/classifier/cgi/lithology/orthogneiss"/>
	<skos:exactMatch rdf:resource="http://inspire.ec.europa.eu/codelist/LithologyValue/orthogneiss"/>
	<skos:definition xml:lang="de">Gneis, bei dem Mineralogie und Textur auf einen magmatischen Protolith hinweisen. Üblicherweise mit homogener Gesteinszusammensetzung (verändert nach Neuendorf et al., 2005).</skos:definition>
	<dcterms:references rdf:resource="https://resource.geosphere.at/thes/citation/545"/>
	<skos:exactMatch rdf:resource="http://data.bgs.ac.uk/id/EarthMaterialClass/RockName/OGNSS"/>
	<dcterms:hasVersion rdf:datatype="http://www.w3.org/2001/XMLSchema#int">8</dcterms:hasVersion>
	<dcterms:date rdf:datatype="http://www.w3.org/2001/XMLSchema#dateTime">2011-03-16T09:19:05Z</dcterms:date>
	<skos:prefLabel xml:lang="en">Orthogneiss</skos:prefLabel>
	<dcterms:created rdf:datatype="http://www.w3.org/2001/XMLSchema#dateTime">2012-03-12T15:51:33.000Z</dcterms:created>
	<skos:definition xml:lang="en">A gneiss with mineralogy and texture indicating derivation from an igneous protolith, usually having a homogeneous composition (modified from Neuendorf et al., 2005).</skos:definition>
	<skos:narrower rdf:resource="https://resource.geosphere.at/thes/lith/248"/>
	<colourHexCode xmlns="http://dbpedia.org/ontology/">#73E68C</colourHexCode>
</rdf:Description>

<rdf:Description rdf:about="https://resource.geosphere.at/thes/lith/135">
	<skos:definition xml:lang="en">An orthogneiss for which protolith can be identified as a tonalite (Neuendorf et al., 2005).</skos:definition>
	<skos:prefLabel xml:lang="de">Tonalitgneis</skos:prefLabel>
	<skos:broadMatch rdf:resource="http://inspire.ec.europa.eu/codelist/LithologyValue/orthogneiss"/>
	<rdf:type rdf:resource="http://www.w3.org/2004/02/skos/core#Concept"/>
	<skos:scopeNote xml:lang="de">Beim Benutzen von Protolithnamen zur Benennung von Metamorphiten liegt der Fokus auf der Veranschaulichung der geologischen Entwicklung, jedoch nicht auf dem Grad der Metamorphose.</skos:scopeNote>
	<skos:scopeNote xml:lang="en">The use of protolith names for metamorphic rocks focuses on their geological histories, not on their metamorphic grades.</skos:scopeNote>
	<dcterms:references rdf:resource="https://resource.geosphere.at/thes/citation/545"/>
	<skos:broadMatch rdf:resource="http://resource.geosciml.org/classifier/cgi/lithology/orthogneiss"/>
	<skos:related rdf:resource="https://resource.geosphere.at/thes/lith/28"/>
	<dcterms:hasVersion rdf:datatype="http://www.w3.org/2001/XMLSchema#int">11</dcterms:hasVersion>
	<dcterms:date rdf:datatype="http://www.w3.org/2001/XMLSchema#dateTime">2011-03-16T09:19:05Z</dcterms:date>
	<dcterms:created rdf:datatype="http://www.w3.org/2001/XMLSchema#dateTime">2012-03-12T13:37:33.000Z</dcterms:created>
	<skos:definition xml:lang="de">Orthogneis, dessen Protolith als Tonalit identifiziert werden kann (Neuendorf et al., 2005).</skos:definition>
	<skos:prefLabel xml:lang="en">Tonalite gneiss</skos:prefLabel>
</rdf:Description>

<rdf:Description rdf:about="https://resource.geosphere.at/thes/lith/134">
	<skos:broadMatch rdf:resource="http://inspire.ec.europa.eu/codelist/LithologyValue/orthogneiss"/>
	<skos:prefLabel xml:lang="de">Dioritgneis</skos:prefLabel>
	<dcterms:references rdf:resource="https://resource.geosphere.at/thes/citation/545"/>
	<rdf:type rdf:resource="http://www.w3.org/2004/02/skos/core#Concept"/>
	<skos:definition xml:lang="de">Orthogneis, dessen Protolith als Diorit identifiziert werden kann (Neuendorf et al., 2005).</skos:definition>
	<skos:definition xml:lang="en">An orthogneiss for which the protolith can be identified as a diorite (Neuendorf et al., 2005).</skos:definition>
	<dcterms:hasVersion rdf:datatype="http://www.w3.org/2001/XMLSchema#int">12</dcterms:hasVersion>
	<skos:prefLabel xml:lang="en">Diorite gneiss</skos:prefLabel>
	<skos:scopeNote xml:lang="de">Beim Benutzen von Protolithnamen zur Benennung von Metamorphiten liegt der Fokus auf der Veranschaulichung der geologischen Entwicklung, jedoch nicht auf dem Grad der Metamorphose.</skos:scopeNote>
	<skos:scopeNote xml:lang="en">The use of protolith names for metamorphic rocks focuses on their geological histories, not on their metamorphic grades.</skos:scopeNote>
	<dcterms:created rdf:datatype="http://www.w3.org/2001/XMLSchema#dateTime">2012-03-12T13:37:45.000Z</dcterms:created>
	<dcterms:date rdf:datatype="http://www.w3.org/2001/XMLSchema#dateTime">2011-03-16T09:19:05Z</dcterms:date>
	<skos:broadMatch rdf:resource="http://resource.geosciml.org/classifier/cgi/lithology/orthogneiss"/>
	<skos:related rdf:resource="https://resource.geosphere.at/thes/lith/45"/>
</rdf:Description>

<rdf:Description rdf:about="https://resource.geosphere.at/thes/lith/248">
	<skos:broadMatch rdf:resource="http://resource.geosciml.org/classifier/cgi/lithology/orthogneiss"/>
	<skos:broadMatch rdf:resource="http://inspire.ec.europa.eu/codelist/LithologyValue/orthogneiss"/>
	<skos:prefLabel xml:lang="en">Augen gneiss</skos:prefLabel>
	<skos:prefLabel xml:lang="de">Augengneis</skos:prefLabel>
	<dcterms:hasVersion rdf:datatype="http://www.w3.org/2001/XMLSchema#int">16</dcterms:hasVersion>
	<dcterms:references rdf:resource="https://resource.geosphere.at/thes/citation/216"/>
	<dcterms:created rdf:datatype="http://www.w3.org/2001/XMLSchema#dateTime">2012-01-20T15:21:07.000Z</dcterms:created>
	<rdf:type rdf:resource="http://www.w3.org/2004/02/skos/core#Concept"/>
	<colourHexCode xmlns="http://dbpedia.org/ontology/">#73E68C</colourHexCode>
	<foaf:depiction rdf:resource="https://resource.geosphere.at/img/thes/Augen-Gneis.jpg"/>
	<skos:definition xml:lang="de">Ein Orthogneis, der durch die Anwesenheit von 'Augen' (= linsenartige Kristalle oder Kristallaggregate, welche normalerweise makroskopisch erkennbar sind und durch gerichtete Deformation entstehen) gekennzeichnet ist (verändert nach Fettes et al., 2007).</skos:definition>
	<skos:definition xml:lang="en">A type of orthogneiss characterised by the presence of 'augen' (lensoid grains or grain aggregates), normally on a macroscopic scale, which are usually products of deformation (modified from Fettes et al., 2007).</skos:definition>
	<foaf:page rdf:resource="https://ardigeos.geologie.ac.at/tsv/5254"/>
</rdf:Description>

<rdf:Description rdf:about="https://resource.geosphere.at/thes/lith/133">
	<skos:broadMatch rdf:resource="http://inspire.ec.europa.eu/codelist/LithologyValue/orthogneiss"/>
	<skos:scopeNote xml:lang="en">The use of protolith names for metamorphic rocks focuses on their geological histories, not on their metamorphic grades.</skos:scopeNote>
	<skos:definition xml:lang="de">Orthogneis, dessen Protolith als Granit identifiziert werden kann (Neuendorf et al., 2005).</skos:definition>
	<skos:definition xml:lang="en">An orthogneiss for which the protolith can be identified as a granite (Neuendorf et al., 2005).</skos:definition>
	<dcterms:hasVersion rdf:datatype="http://www.w3.org/2001/XMLSchema#int">11</dcterms:hasVersion>
	<skos:prefLabel xml:lang="en">Granite gneiss</skos:prefLabel>
	<skos:prefLabel xml:lang="de">Granitgneis</skos:prefLabel>
	<dcterms:created rdf:datatype="http://www.w3.org/2001/XMLSchema#dateTime">2012-03-12T13:36:31.000Z</dcterms:created>
	<rdf:type rdf:resource="http://www.w3.org/2004/02/skos/core#Concept"/>
	<skos:broadMatch rdf:resource="http://resource.geosciml.org/classifier/cgi/lithology/orthogneiss"/>
	<dcterms:references rdf:resource="https://resource.geosphere.at/thes/citation/545"/>
	<dcterms:date rdf:datatype="http://www.w3.org/2001/XMLSchema#dateTime">2011-03-16T09:19:05Z</dcterms:date>
	<skos:scopeNote xml:lang="de">Beim Benutzen von Protolithnamen zur Benennung von Metamorphiten liegt der Fokus auf der Veranschaulichung der geologischen Entwicklung, jedoch nicht auf dem Grad der Metamorphose.</skos:scopeNote>
</rdf:Description>

<rdf:Description rdf:about="https://resource.geosphere.at/thes/lith/250">
	<skos:broadMatch rdf:resource="http://resource.geosciml.org/classifier/cgi/lithology/metamorphic_rock"/>
	<skos:prefLabel xml:lang="de">Metavulkanoklastisches Gestein</skos:prefLabel>
	<rdf:type rdf:resource="http://www.w3.org/2004/02/skos/core#Concept"/>
	<dcterms:created rdf:datatype="http://www.w3.org/2001/XMLSchema#dateTime">2019-06-07T09:09:09.739Z</dcterms:created>
	<dcterms:references rdf:resource="https://resource.geosphere.at/thes/citation/545"/>
	<skos:prefLabel xml:lang="en">Metavolcaniclastic rock</skos:prefLabel>
	<skos:definition xml:lang="en">A term for volcanoclastic rocks, that show evidence of having been subjected to metamorphism. (modified after Neuendorf et al., 2005).</skos:definition>
	<dcterms:source rdf:resource="https://www.mindat.org/min-49014.html"/>
	<skos:definition xml:lang="de">Ein Begriff für vulkanoklastische Gesteine, die Anzeichen einer metamorphen Überprägung aufweisen. (modifiziert nach Neuendorf et al., 2005).</skos:definition>
	<skos:broadMatch rdf:resource="http://inspire.ec.europa.eu/codelist/LithologyValue/metamorphicRock"/>
	<skos:scopeNote xml:lang="en">The use of 'meta' together with the protolith names for metamorphic rocks focuses on their geological histories, not on their metamorphic grades.</skos:scopeNote>
	<skos:scopeNote xml:lang="de">Beim Benutzen des Präfixes 'Meta,' in Kombination mit dem Protolithnamen zur Benennung von Metamorphiten, liegt der Fokus auf der Veranschaulichung der geologischen Entwicklung, jedoch nicht auf dem Grad der Metamorphose.</skos:scopeNote>
</rdf:Description>

<rdf:Description rdf:about="https://resource.geosphere.at/thes/lith/142">
	<rdf:type rdf:resource="http://www.w3.org/2004/02/skos/core#Concept"/>
	<skos:broadMatch rdf:resource="http://resource.geosciml.org/classifier/cgi/lithology/metamorphic_rock"/>
	<skos:narrowMatch rdf:resource="http://resource.geosciml.org/classifier/cgi/lithology/spilite"/>
	<skos:prefLabel xml:lang="de">Metagabbro</skos:prefLabel>
	<skos:prefLabel xml:lang="en">Metagabbro</skos:prefLabel>
	<skos:broadMatch rdf:resource="http://inspire.ec.europa.eu/codelist/LithologyValue/metamorphicRock"/>
	<skos:definition xml:lang="de">Gabbro, der metamorph überprägt wurde (Fettes &amp; Desmons, 2007).</skos:definition>
	<skos:scopeNote xml:lang="de">Beim Benutzen des Präfixes 'Meta,' in Kombination mit dem Protolithnamen zur Benennung von Metamorphiten, liegt der Fokus auf der Veranschaulichung der geologischen Entwicklung, jedoch nicht auf dem Grad der Metamorphose.</skos:scopeNote>
	<skos:exactMatch rdf:resource="http://data.bgs.ac.uk/id/EarthMaterialClass/RockName/MGB"/>
	<skos:definition xml:lang="en">A gabbro that has been metamorphosed (Fettes &amp; Desmons, 2007).</skos:definition>
	<skos:related rdf:resource="https://resource.geosphere.at/thes/lith/48"/>
	<dcterms:date rdf:datatype="http://www.w3.org/2001/XMLSchema#dateTime">2011-03-16T09:19:05Z</dcterms:date>
	<dcterms:created rdf:datatype="http://www.w3.org/2001/XMLSchema#dateTime">2012-03-12T14:28:24.000Z</dcterms:created>
	<dcterms:hasVersion rdf:datatype="http://www.w3.org/2001/XMLSchema#int">11</dcterms:hasVersion>
	<dcterms:references rdf:resource="https://resource.geosphere.at/thes/citation/216"/>
	<skos:scopeNote xml:lang="en">The use of protolith names for metamorphic rocks focuses on their geological history, not on their metamorphic grade.</skos:scopeNote>
	<colourHexCode xmlns="http://dbpedia.org/ontology/">#F24073</colourHexCode>
	<skos:broadMatch rdf:resource="http://inspire.ec.europa.eu/codelist/LithologyValue/gabbro"/>
</rdf:Description>

<rdf:Description rdf:about="https://resource.geosphere.at/thes/lith/120">
	<dcterms:hasVersion rdf:datatype="http://www.w3.org/2001/XMLSchema#int">8</dcterms:hasVersion>
	<skos:exactMatch rdf:resource="http://resource.geosciml.org/classifier/cgi/lithology/metasomatic_rock"/>
	<skos:exactMatch rdf:resource="http://inspire.ec.europa.eu/codelist/LithologyValue/metasomaticRock"/>
	<dcterms:date rdf:datatype="http://www.w3.org/2001/XMLSchema#dateTime">2011-03-16T09:19:05Z</dcterms:date>
	<skos:prefLabel xml:lang="en">Metasomatic rock</skos:prefLabel>
	<skos:prefLabel xml:lang="de">Metasomatisches Gestein</skos:prefLabel>
	<skos:altLabel xml:lang="de">Metasomatit</skos:altLabel>
	<skos:definition xml:lang="de">Metamorphes Gestein, dessen chemische Zusammensetzung stark durch Alteration seiner originalen Bestandteile verändert wurde. Metasomatose ist ein durchgreifender metamorpher Prozess im offenen System, wobei die originale Zusammensetzung eines Gesteins durch Reaktion mit einer externen Quelle, d.i. eine fluide Phase, verändert wird (Neuendorf et al., 2005).</skos:definition>
	<skos:altLabel xml:lang="en">Metasomatite</skos:altLabel>
	<dcterms:references rdf:resource="https://resource.geosphere.at/thes/citation/545"/>
	<skos:narrower rdf:resource="https://resource.geosphere.at/thes/lith/121"/>
	<skos:narrower rdf:resource="https://resource.geosphere.at/thes/lith/122"/>
	<skos:definition xml:lang="en">A metamorphic rock which has had its chemical composition substantially changed by alteration of its original constituents. Metasomatism is a pervasive open-system metamorphic process in which the original chemical composition of a rock is changed by reaction with an external fluid medium (Neuendorf et al., 2005).</skos:definition>
	<rdf:type rdf:resource="http://www.w3.org/2004/02/skos/core#Concept"/>
	<skos:related rdf:resource="https://resource.geosphere.at/thes/lith/145"/>
	<dcterms:created rdf:datatype="http://www.w3.org/2001/XMLSchema#dateTime">2012-03-12T14:30:57.000Z</dcterms:created>
	<colourHexCode xmlns="http://dbpedia.org/ontology/">#80E64D</colourHexCode>
</rdf:Description>

<rdf:Description rdf:about="https://resource.geosphere.at/thes/lith/122">
	<skos:prefLabel xml:lang="de">Greisen</skos:prefLabel>
	<skos:prefLabel xml:lang="en">Greisen</skos:prefLabel>
	<skos:exactMatch rdf:resource="http://data.bgs.ac.uk/id/EarthMaterialClass/RockName/GREIS"/>
	<dcterms:hasVersion rdf:datatype="http://www.w3.org/2001/XMLSchema#int">8</dcterms:hasVersion>
	<rdf:type rdf:resource="http://www.w3.org/2004/02/skos/core#Concept"/>
	<skos:definition xml:lang="en">A medium-temperature metasomatic rock characterised by the presence of quartz and white mica, commonly with topaz, fluorite, tourmaline, and locally with amazonite, orthoclase, andalusite and diaspore. Typically, greisens may host Be, W, Mo, Sn and Ta mineralization. They are associated with high-level late-orogenic leucogranites and form as replacements, within the granite body and/or in a wide range of country rocks. Zoning may be present (Fettes &amp; Desmons, 2007).</skos:definition>
	<skos:definition xml:lang="de">Mitteltemperiert metasomatisches Gestein, welches durch die Anwesenheit von Quarz und Hellglimmer gekennzeichnet ist, üblicherweise mit Topas, Fluorit, Turmalin und lokal mit Amazonit, Orthoklas, Andalusit und Diaspor. Typischerweise führen Greisen Be-, W-, Mo-, Sn- und Ta-Mineralisationen. Sie sind assoziiert mit spätorogenen Leukograniten, die in flachem krustalem Niveau intrudierten, und bilden Neubildungen in Granitkörpern und/oder in einer großen Anzahl von Umgebungsgesteinen. Greisen können zoniert sein (Fettes &amp; Desmons, 2007).</skos:definition>
	<dcterms:references rdf:resource="https://resource.geosphere.at/thes/citation/216"/>
	<skos:exactMatch rdf:resource="http://dbpedia.org/resource/Greisen"/>
	<skos:broadMatch rdf:resource="http://resource.geosciml.org/classifier/cgi/lithology/metasomatic_rock"/>
	<skos:broadMatch rdf:resource="http://inspire.ec.europa.eu/codelist/LithologyValue/metasomaticRock"/>
	<dcterms:created rdf:datatype="http://www.w3.org/2001/XMLSchema#dateTime">2012-03-12T13:43:40.000Z</dcterms:created>
	<dcterms:date rdf:datatype="http://www.w3.org/2001/XMLSchema#dateTime">2011-03-16T09:19:05Z</dcterms:date>
</rdf:Description>

<rdf:Description rdf:about="https://resource.geosphere.at/thes/lith/121">
	<skos:exactMatch rdf:resource="http://dbpedia.org/resource/Skarn"/>
	<colourHexCode xmlns="http://dbpedia.org/ontology/">#99E659</colourHexCode>
	<dcterms:hasVersion rdf:datatype="http://www.w3.org/2001/XMLSchema#int">7</dcterms:hasVersion>
	<skos:exactMatch rdf:resource="http://inspire.ec.europa.eu/codelist/LithologyValue/skarn"/>
	<skos:exactMatch rdf:resource="http://resource.geosciml.org/classifier/cgi/lithology/skarn"/>
	<skos:definition xml:lang="en">A metasomatic rock formed at the contact between a silicate rock (or magmatic melt) and a carbonate rock. It consists mainly of Ca-, Mg-, Fe- and Mn-silicates that contain little or no water (Fettes &amp; Desmons, 2007).</skos:definition>
	<skos:definition xml:lang="de">Metasomatisches Gestein, welches am Kontakt zwischen einem silikatischen Gestein (oder magmatischer Schmelze) und einem Karbonatgestein entstanden ist. Es besteht hauptsächlich aus Ca-, Mg-, Fe- und Mn-Silikaten, welche wasserarm oder wasserfrei sind (Fettes &amp; Desmons, 2007).</skos:definition>
	<skos:prefLabel xml:lang="de">Skarn</skos:prefLabel>
	<skos:prefLabel xml:lang="en">Skarn</skos:prefLabel>
	<dcterms:references rdf:resource="https://resource.geosphere.at/thes/citation/216"/>
	<rdf:type rdf:resource="http://www.w3.org/2004/02/skos/core#Concept"/>
	<skos:exactMatch rdf:resource="http://data.bgs.ac.uk/id/EarthMaterialClass/RockName/SKN"/>
	<dcterms:created rdf:datatype="http://www.w3.org/2001/XMLSchema#dateTime">2012-03-12T16:24:04.000Z</dcterms:created>
	<dcterms:date rdf:datatype="http://www.w3.org/2001/XMLSchema#dateTime">2011-03-16T09:19:05Z</dcterms:date>
</rdf:Description>

<rdf:Description rdf:about="https://resource.geosphere.at/thes/lith/144">
	<dcterms:date rdf:datatype="http://www.w3.org/2001/XMLSchema#dateTime">2011-03-16T09:19:05Z</dcterms:date>
	<skos:definition xml:lang="de">Basalt, der metamorph überprägt wurde (Fettes &amp; Desmons, 2007).</skos:definition>
	<skos:definition xml:lang="en">A basalt that has been metamorphosed (Fettes &amp; Desmons, 2007).</skos:definition>
	<dcterms:hasVersion rdf:datatype="http://www.w3.org/2001/XMLSchema#int">10</dcterms:hasVersion>
	<skos:prefLabel xml:lang="de">Metabasalt</skos:prefLabel>
	<skos:prefLabel xml:lang="en">Metabasalt</skos:prefLabel>
	<skos:related rdf:resource="https://resource.geosphere.at/thes/lith/82"/>
	<skos:closeMatch rdf:resource="http://resource.geosciml.org/classifier/cgi/lithology/spilite"/>
	<dcterms:references rdf:resource="https://resource.geosphere.at/thes/citation/216"/>
	<skos:exactMatch rdf:resource="http://data.bgs.ac.uk/id/EarthMaterialClass/RockName/MBA"/>
	<dcterms:created rdf:datatype="http://www.w3.org/2001/XMLSchema#dateTime">2012-03-12T14:26:26.000Z</dcterms:created>
	<rdf:type rdf:resource="http://www.w3.org/2004/02/skos/core#Concept"/>
	<skos:broadMatch rdf:resource="http://inspire.ec.europa.eu/codelist/LithologyValue/metamorphicRock"/>
	<skos:broadMatch rdf:resource="http://resource.geosciml.org/classifier/cgi/lithology/metamorphic_rock"/>
	<skos:scopeNote xml:lang="en">The use of 'meta' together with the protolith names for metamorphic rocks focuses on their geological histories, not on their metamorphic grades.</skos:scopeNote>
	<skos:scopeNote xml:lang="de">Beim Benutzen des Präfixes 'Meta,' in Kombination mit dem Protolithnamen zur Benennung von Metamorphiten, liegt der Fokus auf der Veranschaulichung der geologischen Entwicklung, jedoch nicht auf dem Grad der Metamorphose.</skos:scopeNote>
	<colourHexCode xmlns="http://dbpedia.org/ontology/">#6600FF</colourHexCode>
	<skos:narrowMatch rdf:resource="http://resource.geosciml.org/classifier/cgi/lithology/spilite"/>
	<skos:broadMatch rdf:resource="http://inspire.ec.europa.eu/codelist/LithologyValue/basalt"/>
</rdf:Description>

<rdf:Description rdf:about="https://resource.geosphere.at/thes/lith/143">
	<rdf:type rdf:resource="http://www.w3.org/2004/02/skos/core#Concept"/>
	<skos:definition xml:lang="en">A granite that has been metamorphosed (Fettes &amp; Desmons, 2007).</skos:definition>
	<dcterms:references rdf:resource="https://resource.geosphere.at/thes/citation/216"/>
	<skos:exactMatch rdf:resource="http://data.bgs.ac.uk/id/EarthMaterialClass/RockName/MGN"/>
	<skos:related rdf:resource="https://resource.geosphere.at/thes/lith/26"/>
	<skos:scopeNote xml:lang="en">The use of protolith names for metamorphic rocks focuses on their geological histories, not on their metamorphic grades.</skos:scopeNote>
	<skos:prefLabel xml:lang="de">Metagranit</skos:prefLabel>
	<dcterms:date rdf:datatype="http://www.w3.org/2001/XMLSchema#dateTime">2011-03-16T09:19:05Z</dcterms:date>
	<dcterms:created rdf:datatype="http://www.w3.org/2001/XMLSchema#dateTime">2012-03-12T14:28:41.000Z</dcterms:created>
	<skos:prefLabel xml:lang="en">Metagranite</skos:prefLabel>
	<dcterms:hasVersion rdf:datatype="http://www.w3.org/2001/XMLSchema#int">9</dcterms:hasVersion>
	<skos:definition xml:lang="de">Granit, der metamorph überprägt wurde (Fettes &amp; Desmons, 2007).</skos:definition>
	<skos:broadMatch rdf:resource="http://resource.geosciml.org/classifier/cgi/lithology/metamorphic_rock"/>
	<skos:closeMatch rdf:resource="http://resource.geosciml.org/classifier/cgi/lithology/orthogneiss"/>
	<skos:broadMatch rdf:resource="http://inspire.ec.europa.eu/codelist/LithologyValue/metamorphicRock"/>
	<skos:scopeNote xml:lang="de">Beim Benutzen des Präfixes 'Meta,' in Kombination mit dem Protolithnamen zur Benennung von Metamorphiten, liegt der Fokus auf der Veranschaulichung der geologischen Entwicklung, jedoch nicht auf dem Grad der Metamorphose.</skos:scopeNote>
	<skos:broadMatch rdf:resource="http://inspire.ec.europa.eu/codelist/LithologyValue/granite"/>
</rdf:Description>

<rdf:Description rdf:about="https://resource.geosphere.at/thes/lith/155">
	<dcterms:created rdf:datatype="http://www.w3.org/2001/XMLSchema#dateTime">2012-03-12T13:51:03.000Z</dcterms:created>
	<dcterms:hasVersion rdf:datatype="http://www.w3.org/2001/XMLSchema#int">11</dcterms:hasVersion>
	<skos:definition xml:lang="en">A rock produced by impact metamorphism (metamorphism of local extent, including melting and vaporization, caused by the passage of a shock wave due to the impact of a planetary body on a planetary surface). Impactites include shocked rocks, impact breccias, impact melt, tektites, and impactoclastic airfall (Fettes &amp; Desmons, 2007).</skos:definition>
	<skos:closeMatch rdf:resource="http://resource.geosciml.org/classifier/cgi/lithology/impact_generated_material"/>
	<rdf:type rdf:resource="http://www.w3.org/2004/02/skos/core#Concept"/>
	<dcterms:references rdf:resource="https://resource.geosphere.at/thes/citation/216"/>
	<skos:prefLabel xml:lang="en">Impactite</skos:prefLabel>
	<skos:exactMatch rdf:resource="http://www.wikidata.org/entity/Q976105"/>
	<colourHexCode xmlns="http://dbpedia.org/ontology/">#00B366</colourHexCode>
	<skos:prefLabel xml:lang="de">Impaktit</skos:prefLabel>
	<skos:closeMatch rdf:resource="http://inspire.ec.europa.eu/codelist/LithologyValue/impactGeneratedMaterial"/>
	<skos:definition xml:lang="de">Gestein, welches durch Impaktmetamorphose (Metamorphose von lokaler Ausdehnung durch die Auswirkung von Schockwellen, verursacht durch den Impakt eines planetarischen Körpers auf eine planetarische Oberfläche, Schmelzen und Verdampfen eingeschlossen) entsteht. Das Konzept umfasst geschockte Gesteine, Impaktbrekzien, Impaktschmelzen, Tektite und impaktoplastische Ablagerungen aus der Luft (Fettes &amp; Desmons, 2007).</skos:definition>
	<dcterms:date rdf:datatype="http://www.w3.org/2001/XMLSchema#dateTime">2011-03-16T09:19:05Z</dcterms:date>
</rdf:Description>

<rdf:Description rdf:about="https://resource.geosphere.at/thes/lith/249">
	<skos:exactMatch rdf:resource="http://resource.geosciml.org/classifier/cgi/lithology/anthropogenic_material"/>
	<skos:prefLabel xml:lang="en">Anthropogenic material</skos:prefLabel>
	<skos:prefLabel xml:lang="de">Anthropogenes Material</skos:prefLabel>
	<skos:exactMatch rdf:resource="http://inspire.ec.europa.eu/codelist/LithologyValue/anthropogenicMaterial"/>
	<rdf:type rdf:resource="http://www.w3.org/2004/02/skos/core#Concept"/>
	<dcterms:hasVersion rdf:datatype="http://www.w3.org/2001/XMLSchema#int">9</dcterms:hasVersion>
	<dcterms:created rdf:datatype="http://www.w3.org/2001/XMLSchema#dateTime">2012-01-27T12:29:53.000Z</dcterms:created>
	<colourHexCode xmlns="http://dbpedia.org/ontology/">#C0C0C0</colourHexCode>
</rdf:Description>

<rdf:Description rdf:about="https://resource.geosphere.at/thes/lith/20">
	<skos:broader rdf:resource="https://resource.geosphere.at/thes/lith/5"/>
</rdf:Description>

<rdf:Description rdf:about="https://resource.geosphere.at/thes/lith/130">
	<skos:broader rdf:resource="https://resource.geosphere.at/thes/lith/129"/>
</rdf:Description>

<rdf:Description rdf:about="https://resource.geosphere.at/thes/lith/248">
	<skos:broader rdf:resource="https://resource.geosphere.at/thes/lith/130"/>
</rdf:Description>

<rdf:Description rdf:about="https://resource.geosphere.at/thes/lith/161">
	<skos:broader rdf:resource="https://resource.geosphere.at/thes/lith/159"/>
</rdf:Description>

<rdf:Description rdf:about="https://resource.geosphere.at/thes/lith/87">
	<skos:broader rdf:resource="https://resource.geosphere.at/thes/lith/68"/>
</rdf:Description>

<rdf:Description rdf:about="https://resource.geosphere.at/thes/lith/220">
	<skos:broader rdf:resource="https://resource.geosphere.at/thes/lith/218"/>
</rdf:Description>

<rdf:Description rdf:about="https://resource.geosphere.at/thes/lith/176">
	<skos:broader rdf:resource="https://resource.geosphere.at/thes/lith/173"/>
</rdf:Description>

<rdf:Description rdf:about="https://resource.geosphere.at/thes/lith/31">
	<skos:broader rdf:resource="https://resource.geosphere.at/thes/lith/19"/>
</rdf:Description>

<rdf:Description rdf:about="https://resource.geosphere.at/thes/lith/111">
	<skos:broader rdf:resource="https://resource.geosphere.at/thes/lith/109"/>
</rdf:Description>

<rdf:Description rdf:about="https://resource.geosphere.at/thes/lith/137">
	<skos:broader rdf:resource="https://resource.geosphere.at/thes/lith/136"/>
</rdf:Description>

<rdf:Description rdf:about="https://resource.geosphere.at/thes/lith/245">
	<skos:broader rdf:resource="https://resource.geosphere.at/thes/lith/139"/>
</rdf:Description>

<rdf:Description rdf:about="https://resource.geosphere.at/thes/lith/2">
	<skos:broader rdf:resource="https://resource.geosphere.at/thes/lith/1"/>
</rdf:Description>

<rdf:Description rdf:about="https://resource.geosphere.at/thes/lith/66">
	<skos:broader rdf:resource="https://resource.geosphere.at/thes/lith/6"/>
</rdf:Description>

<rdf:Description rdf:about="https://resource.geosphere.at/thes/lith/134">
	<skos:broader rdf:resource="https://resource.geosphere.at/thes/lith/130"/>
</rdf:Description>

<rdf:Description rdf:about="https://resource.geosphere.at/thes/lith/72">
	<skos:broader rdf:resource="https://resource.geosphere.at/thes/lith/63"/>
</rdf:Description>

<rdf:Description rdf:about="https://resource.geosphere.at/thes/lith/46">
	<skos:broader rdf:resource="https://resource.geosphere.at/thes/lith/20"/>
</rdf:Description>

<rdf:Description rdf:about="https://resource.geosphere.at/thes/lith/77">
	<skos:broader rdf:resource="https://resource.geosphere.at/thes/lith/64"/>
</rdf:Description>

<rdf:Description rdf:about="https://resource.geosphere.at/thes/lith/114">
	<skos:broader rdf:resource="https://resource.geosphere.at/thes/lith/111"/>
</rdf:Description>

<rdf:Description rdf:about="https://resource.geosphere.at/thes/lith/15">
	<skos:broader rdf:resource="https://resource.geosphere.at/thes/lith/3"/>
</rdf:Description>

<rdf:Description rdf:about="https://resource.geosphere.at/thes/lith/120">
	<skos:broader rdf:resource="https://resource.geosphere.at/thes/lith/98"/>
</rdf:Description>

<rdf:Description rdf:about="https://resource.geosphere.at/thes/lith/122">
	<skos:broader rdf:resource="https://resource.geosphere.at/thes/lith/120"/>
</rdf:Description>

<rdf:Description rdf:about="https://resource.geosphere.at/thes/lith/199">
	<skos:broader rdf:resource="https://resource.geosphere.at/thes/lith/196"/>
</rdf:Description>

<rdf:Description rdf:about="https://resource.geosphere.at/thes/lith/50">
	<skos:broader rdf:resource="https://resource.geosphere.at/thes/lith/157"/>
</rdf:Description>

<rdf:Description rdf:about="https://resource.geosphere.at/thes/lith/219">
	<skos:broader rdf:resource="https://resource.geosphere.at/thes/lith/218"/>
</rdf:Description>

<rdf:Description rdf:about="https://resource.geosphere.at/thes/lith/82">
	<skos:broader rdf:resource="https://resource.geosphere.at/thes/lith/66"/>
</rdf:Description>

<rdf:Description rdf:about="https://resource.geosphere.at/thes/lith/60">
	<skos:broader rdf:resource="https://resource.geosphere.at/thes/lith/7"/>
</rdf:Description>

<rdf:Description rdf:about="https://resource.geosphere.at/thes/lith/102">
	<skos:broader rdf:resource="https://resource.geosphere.at/thes/lith/101"/>
</rdf:Description>

<rdf:Description rdf:about="https://resource.geosphere.at/thes/lith/182">
	<skos:broader rdf:resource="https://resource.geosphere.at/thes/lith/161"/>
</rdf:Description>

<rdf:Description rdf:about="https://resource.geosphere.at/thes/lith/215">
	<skos:broader rdf:resource="https://resource.geosphere.at/thes/lith/214"/>
</rdf:Description>

<rdf:Description rdf:about="https://resource.geosphere.at/thes/lith/76">
	<skos:broader rdf:resource="https://resource.geosphere.at/thes/lith/64"/>
</rdf:Description>

<rdf:Description rdf:about="https://resource.geosphere.at/thes/lith/125">
	<skos:broader rdf:resource="https://resource.geosphere.at/thes/lith/136"/>
</rdf:Description>

<rdf:Description rdf:about="https://resource.geosphere.at/thes/lith/14">
	<skos:broader rdf:resource="https://resource.geosphere.at/thes/lith/3"/>
</rdf:Description>

<rdf:Description rdf:about="https://resource.geosphere.at/thes/lith/171">
	<skos:broader rdf:resource="https://resource.geosphere.at/thes/lith/161"/>
</rdf:Description>

<rdf:Description rdf:about="https://resource.geosphere.at/thes/lith/126">
	<skos:broader rdf:resource="https://resource.geosphere.at/thes/lith/98"/>
</rdf:Description>

<rdf:Description rdf:about="https://resource.geosphere.at/thes/lith/133">
	<skos:broader rdf:resource="https://resource.geosphere.at/thes/lith/130"/>
</rdf:Description>

<rdf:Description rdf:about="https://resource.geosphere.at/thes/lith/101">
	<skos:broader rdf:resource="https://resource.geosphere.at/thes/lith/99"/>
</rdf:Description>

<rdf:Description rdf:about="https://resource.geosphere.at/thes/lith/26">
	<skos:broader rdf:resource="https://resource.geosphere.at/thes/lith/18"/>
</rdf:Description>

<rdf:Description rdf:about="https://resource.geosphere.at/thes/lith/162">
	<skos:broader rdf:resource="https://resource.geosphere.at/thes/lith/159"/>
</rdf:Description>

<rdf:Description rdf:about="https://resource.geosphere.at/thes/lith/112">
	<skos:broader rdf:resource="https://resource.geosphere.at/thes/lith/108"/>
</rdf:Description>

<rdf:Description rdf:about="https://resource.geosphere.at/thes/lith/213">
	<skos:broader rdf:resource="https://resource.geosphere.at/thes/lith/166"/>
</rdf:Description>

<rdf:Description rdf:about="https://resource.geosphere.at/thes/lith/37">
	<skos:broader rdf:resource="https://resource.geosphere.at/thes/lith/19"/>
</rdf:Description>

<rdf:Description rdf:about="https://resource.geosphere.at/thes/lith/232">
	<skos:broader rdf:resource="https://resource.geosphere.at/thes/lith/166"/>
</rdf:Description>

<rdf:Description rdf:about="https://resource.geosphere.at/thes/lith/155">
	<skos:broader rdf:resource="https://resource.geosphere.at/thes/lith/97"/>
</rdf:Description>

<rdf:Description rdf:about="https://resource.geosphere.at/thes/lith/121">
	<skos:broader rdf:resource="https://resource.geosphere.at/thes/lith/120"/>
</rdf:Description>

<rdf:Description rdf:about="https://resource.geosphere.at/thes/lith/183">
	<skos:broader rdf:resource="https://resource.geosphere.at/thes/lith/161"/>
</rdf:Description>

<rdf:Description rdf:about="https://resource.geosphere.at/thes/lith/212">
	<skos:broader rdf:resource="https://resource.geosphere.at/thes/lith/209"/>
</rdf:Description>

<rdf:Description rdf:about="https://resource.geosphere.at/thes/lith/107">
	<skos:broader rdf:resource="https://resource.geosphere.at/thes/lith/104"/>
</rdf:Description>

<rdf:Description rdf:about="https://resource.geosphere.at/thes/lith/148">
	<skos:broader rdf:resource="https://resource.geosphere.at/thes/lith/147"/>
</rdf:Description>

<rdf:Description rdf:about="https://resource.geosphere.at/thes/lith/143">
	<skos:broader rdf:resource="https://resource.geosphere.at/thes/lith/98"/>
</rdf:Description>

<rdf:Description rdf:about="https://resource.geosphere.at/thes/lith/177">
	<skos:broader rdf:resource="https://resource.geosphere.at/thes/lith/161"/>
</rdf:Description>

<rdf:Description rdf:about="https://resource.geosphere.at/thes/lith/86">
	<skos:broader rdf:resource="https://resource.geosphere.at/thes/lith/68"/>
</rdf:Description>

<rdf:Description rdf:about="https://resource.geosphere.at/thes/lith/19">
	<skos:broader rdf:resource="https://resource.geosphere.at/thes/lith/5"/>
</rdf:Description>

<rdf:Description rdf:about="https://resource.geosphere.at/thes/lith/194">
	<skos:broader rdf:resource="https://resource.geosphere.at/thes/lith/161"/>
</rdf:Description>

<rdf:Description rdf:about="https://resource.geosphere.at/thes/lith/32">
	<skos:broader rdf:resource="https://resource.geosphere.at/thes/lith/19"/>
</rdf:Description>

<rdf:Description rdf:about="https://resource.geosphere.at/thes/lith/246">
	<skos:broader rdf:resource="https://resource.geosphere.at/thes/lith/139"/>
</rdf:Description>

<rdf:Description rdf:about="https://resource.geosphere.at/thes/lith/57">
	<skos:broader rdf:resource="https://resource.geosphere.at/thes/lith/23"/>
</rdf:Description>

<rdf:Description rdf:about="https://resource.geosphere.at/thes/lith/41">
	<skos:broader rdf:resource="https://resource.geosphere.at/thes/lith/21"/>
</rdf:Description>

<rdf:Description rdf:about="https://resource.geosphere.at/thes/lith/166">
	<skos:broader rdf:resource="https://resource.geosphere.at/thes/lith/160"/>
</rdf:Description>

<rdf:Description rdf:about="https://resource.geosphere.at/thes/lith/218">
	<skos:broader rdf:resource="https://resource.geosphere.at/thes/lith/166"/>
</rdf:Description>

<rdf:Description rdf:about="https://resource.geosphere.at/thes/lith/135">
	<skos:broader rdf:resource="https://resource.geosphere.at/thes/lith/130"/>
</rdf:Description>

<rdf:Description rdf:about="https://resource.geosphere.at/thes/lith/207">
	<skos:broader rdf:resource="https://resource.geosphere.at/thes/lith/205"/>
</rdf:Description>

<rdf:Description rdf:about="https://resource.geosphere.at/thes/lith/151">
	<skos:broader rdf:resource="https://resource.geosphere.at/thes/lith/147"/>
</rdf:Description>

<rdf:Description rdf:about="https://resource.geosphere.at/thes/lith/78">
	<skos:broader rdf:resource="https://resource.geosphere.at/thes/lith/64"/>
</rdf:Description>

<rdf:Description rdf:about="https://resource.geosphere.at/thes/lith/53">
	<skos:broader rdf:resource="https://resource.geosphere.at/thes/lith/22"/>
</rdf:Description>

<rdf:Description rdf:about="https://resource.geosphere.at/thes/lith/192">
	<skos:broader rdf:resource="https://resource.geosphere.at/thes/lith/161"/>
</rdf:Description>

<rdf:Description rdf:about="https://resource.geosphere.at/thes/lith/16">
	<skos:broader rdf:resource="https://resource.geosphere.at/thes/lith/3"/>
</rdf:Description>

<rdf:Description rdf:about="https://resource.geosphere.at/thes/lith/229">
	<skos:broader rdf:resource="https://resource.geosphere.at/thes/lith/166"/>
</rdf:Description>

<rdf:Description rdf:about="https://resource.geosphere.at/thes/lith/198">
	<skos:broader rdf:resource="https://resource.geosphere.at/thes/lith/196"/>
</rdf:Description>

<rdf:Description rdf:about="https://resource.geosphere.at/thes/lith/203">
	<skos:broader rdf:resource="https://resource.geosphere.at/thes/lith/196"/>
</rdf:Description>

<rdf:Description rdf:about="https://resource.geosphere.at/thes/lith/10">
	<skos:broader rdf:resource="https://resource.geosphere.at/thes/lith/4"/>
</rdf:Description>

<rdf:Description rdf:about="https://resource.geosphere.at/thes/lith/42">
	<skos:broader rdf:resource="https://resource.geosphere.at/thes/lith/21"/>
</rdf:Description>

<rdf:Description rdf:about="https://resource.geosphere.at/thes/lith/118">
	<skos:broader rdf:resource="https://resource.geosphere.at/thes/lith/98"/>
</rdf:Description>

<rdf:Description rdf:about="https://resource.geosphere.at/thes/lith/169">
	<skos:broader rdf:resource="https://resource.geosphere.at/thes/lith/160"/>
</rdf:Description>

<rdf:Description rdf:about="https://resource.geosphere.at/thes/lith/231">
	<skos:broader rdf:resource="https://resource.geosphere.at/thes/lith/232"/>
</rdf:Description>

<rdf:Description rdf:about="https://resource.geosphere.at/thes/lith/3">
	<skos:broader rdf:resource="https://resource.geosphere.at/thes/lith/2"/>
</rdf:Description>

<rdf:Description rdf:about="https://resource.geosphere.at/thes/lith/73">
	<skos:broader rdf:resource="https://resource.geosphere.at/thes/lith/64"/>
</rdf:Description>

<rdf:Description rdf:about="https://resource.geosphere.at/thes/lith/47">
	<skos:broader rdf:resource="https://resource.geosphere.at/thes/lith/21"/>
</rdf:Description>

<rdf:Description rdf:about="https://resource.geosphere.at/thes/lith/179">
	<skos:broader rdf:resource="https://resource.geosphere.at/thes/lith/177"/>
</rdf:Description>

<rdf:Description rdf:about="https://resource.geosphere.at/thes/lith/94">
	<skos:broader rdf:resource="https://resource.geosphere.at/thes/lith/5"/>
</rdf:Description>

<rdf:Description rdf:about="https://resource.geosphere.at/thes/lith/115">
	<skos:broader rdf:resource="https://resource.geosphere.at/thes/lith/112"/>
</rdf:Description>

<rdf:Description rdf:about="https://resource.geosphere.at/thes/lith/88">
	<skos:broader rdf:resource="https://resource.geosphere.at/thes/lith/68"/>
</rdf:Description>

<rdf:Description rdf:about="https://resource.geosphere.at/thes/lith/59">
	<skos:broader rdf:resource="https://resource.geosphere.at/thes/lith/5"/>
</rdf:Description>

<rdf:Description rdf:about="https://resource.geosphere.at/thes/lith/103">
	<skos:broader rdf:resource="https://resource.geosphere.at/thes/lith/99"/>
</rdf:Description>

<rdf:Description rdf:about="https://resource.geosphere.at/thes/lith/27">
	<skos:broader rdf:resource="https://resource.geosphere.at/thes/lith/18"/>
</rdf:Description>

<rdf:Description rdf:about="https://resource.geosphere.at/thes/lith/175">
	<skos:broader rdf:resource="https://resource.geosphere.at/thes/lith/173"/>
</rdf:Description>

<rdf:Description rdf:about="https://resource.geosphere.at/thes/lith/197">
	<skos:broader rdf:resource="https://resource.geosphere.at/thes/lith/162"/>
</rdf:Description>

<rdf:Description rdf:about="https://resource.geosphere.at/thes/lith/251">
	<skos:broader rdf:resource="https://resource.geosphere.at/thes/lith/5"/>
</rdf:Description>

<rdf:Description rdf:about="https://resource.geosphere.at/thes/lith/8">
	<skos:broader rdf:resource="https://resource.geosphere.at/thes/lith/4"/>
</rdf:Description>

<rdf:Description rdf:about="https://resource.geosphere.at/thes/lith/252">
	<skos:broader rdf:resource="https://resource.geosphere.at/thes/lith/172"/>
</rdf:Description>

<rdf:Description rdf:about="https://resource.geosphere.at/thes/lith/48">
	<skos:broader rdf:resource="https://resource.geosphere.at/thes/lith/21"/>
</rdf:Description>

<rdf:Description rdf:about="https://resource.geosphere.at/thes/lith/93">
	<skos:broader rdf:resource="https://resource.geosphere.at/thes/lith/5"/>
</rdf:Description>

<rdf:Description rdf:about="https://resource.geosphere.at/thes/lith/65">
	<skos:broader rdf:resource="https://resource.geosphere.at/thes/lith/6"/>
</rdf:Description>

<rdf:Description rdf:about="https://resource.geosphere.at/thes/lith/187">
	<skos:broader rdf:resource="https://resource.geosphere.at/thes/lith/184"/>
</rdf:Description>

<rdf:Description rdf:about="https://resource.geosphere.at/thes/lith/211">
	<skos:broader rdf:resource="https://resource.geosphere.at/thes/lith/209"/>
</rdf:Description>

<rdf:Description rdf:about="https://resource.geosphere.at/thes/lith/180">
	<skos:broader rdf:resource="https://resource.geosphere.at/thes/lith/177"/>
</rdf:Description>

<rdf:Description rdf:about="https://resource.geosphere.at/thes/lith/243">
	<skos:broader rdf:resource="https://resource.geosphere.at/thes/lith/147"/>
</rdf:Description>

<rdf:Description rdf:about="https://resource.geosphere.at/thes/lith/142">
	<skos:broader rdf:resource="https://resource.geosphere.at/thes/lith/98"/>
</rdf:Description>

<rdf:Description rdf:about="https://resource.geosphere.at/thes/lith/258">
	<skos:broader rdf:resource="https://resource.geosphere.at/thes/lith/98"/>
</rdf:Description>

<rdf:Description rdf:about="https://resource.geosphere.at/thes/lith/247">
	<skos:broader rdf:resource="https://resource.geosphere.at/thes/lith/139"/>
</rdf:Description>

<rdf:Description rdf:about="https://resource.geosphere.at/thes/lith/181">
	<skos:broader rdf:resource="https://resource.geosphere.at/thes/lith/161"/>
</rdf:Description>

<rdf:Description rdf:about="https://resource.geosphere.at/thes/lith/33">
	<skos:broader rdf:resource="https://resource.geosphere.at/thes/lith/19"/>
</rdf:Description>

<rdf:Description rdf:about="https://resource.geosphere.at/thes/lith/21">
	<skos:broader rdf:resource="https://resource.geosphere.at/thes/lith/5"/>
</rdf:Description>

<rdf:Description rdf:about="https://resource.geosphere.at/thes/lith/238">
	<skos:broader rdf:resource="https://resource.geosphere.at/thes/lith/169"/>
</rdf:Description>

<rdf:Description rdf:about="https://resource.geosphere.at/thes/lith/4">
	<skos:broader rdf:resource="https://resource.geosphere.at/thes/lith/2"/>
</rdf:Description>

<rdf:Description rdf:about="https://resource.geosphere.at/thes/lith/131">
	<skos:broader rdf:resource="https://resource.geosphere.at/thes/lith/129"/>
</rdf:Description>

<rdf:Description rdf:about="https://resource.geosphere.at/thes/lith/150">
	<skos:broader rdf:resource="https://resource.geosphere.at/thes/lith/147"/>
</rdf:Description>

<rdf:Description rdf:about="https://resource.geosphere.at/thes/lith/206">
	<skos:broader rdf:resource="https://resource.geosphere.at/thes/lith/205"/>
</rdf:Description>

<rdf:Description rdf:about="https://resource.geosphere.at/thes/lith/149">
	<skos:broader rdf:resource="https://resource.geosphere.at/thes/lith/148"/>
</rdf:Description>

<rdf:Description rdf:about="https://resource.geosphere.at/thes/lith/108">
	<skos:broader rdf:resource="https://resource.geosphere.at/thes/lith/98"/>
</rdf:Description>

<rdf:Description rdf:about="https://resource.geosphere.at/thes/lith/228">
	<skos:broader rdf:resource="https://resource.geosphere.at/thes/lith/166"/>
</rdf:Description>

<rdf:Description rdf:about="https://resource.geosphere.at/thes/lith/58">
	<skos:broader rdf:resource="https://resource.geosphere.at/thes/lith/24"/>
</rdf:Description>

<rdf:Description rdf:about="https://resource.geosphere.at/thes/lith/113">
	<skos:broader rdf:resource="https://resource.geosphere.at/thes/lith/108"/>
</rdf:Description>

<rdf:Description rdf:about="https://resource.geosphere.at/thes/lith/202">
	<skos:broader rdf:resource="https://resource.geosphere.at/thes/lith/196"/>
</rdf:Description>

<rdf:Description rdf:about="https://resource.geosphere.at/thes/lith/83">
	<skos:broader rdf:resource="https://resource.geosphere.at/thes/lith/65"/>
</rdf:Description>

<rdf:Description rdf:about="https://resource.geosphere.at/thes/lith/119">
	<skos:broader rdf:resource="https://resource.geosphere.at/thes/lith/98"/>
</rdf:Description>

<rdf:Description rdf:about="https://resource.geosphere.at/thes/lith/136">
	<skos:broader rdf:resource="https://resource.geosphere.at/thes/lith/98"/>
</rdf:Description>

<rdf:Description rdf:about="https://resource.geosphere.at/thes/lith/185">
	<skos:broader rdf:resource="https://resource.geosphere.at/thes/lith/184"/>
</rdf:Description>

<rdf:Description rdf:about="https://resource.geosphere.at/thes/lith/74">
	<skos:broader rdf:resource="https://resource.geosphere.at/thes/lith/64"/>
</rdf:Description>

<rdf:Description rdf:about="https://resource.geosphere.at/thes/lith/90">
	<skos:broader rdf:resource="https://resource.geosphere.at/thes/lith/69"/>
</rdf:Description>

<rdf:Description rdf:about="https://resource.geosphere.at/thes/lith/98">
	<skos:broader rdf:resource="https://resource.geosphere.at/thes/lith/97"/>
</rdf:Description>

<rdf:Description rdf:about="https://resource.geosphere.at/thes/lith/12">
	<skos:broader rdf:resource="https://resource.geosphere.at/thes/lith/3"/>
</rdf:Description>

<rdf:Description rdf:about="https://resource.geosphere.at/thes/lith/189">
	<skos:broader rdf:resource="https://resource.geosphere.at/thes/lith/188"/>
</rdf:Description>

<rdf:Description rdf:about="https://resource.geosphere.at/thes/lith/240">
	<skos:broader rdf:resource="https://resource.geosphere.at/thes/lith/166"/>
</rdf:Description>

<rdf:Description rdf:about="https://resource.geosphere.at/thes/lith/128">
	<skos:broader rdf:resource="https://resource.geosphere.at/thes/lith/98"/>
</rdf:Description>

<rdf:Description rdf:about="https://resource.geosphere.at/thes/lith/196">
	<skos:broader rdf:resource="https://resource.geosphere.at/thes/lith/162"/>
</rdf:Description>

<rdf:Description rdf:about="https://resource.geosphere.at/thes/lith/164">
	<skos:broader rdf:resource="https://resource.geosphere.at/thes/lith/159"/>
</rdf:Description>

<rdf:Description rdf:about="https://resource.geosphere.at/thes/lith/28">
	<skos:broader rdf:resource="https://resource.geosphere.at/thes/lith/18"/>
</rdf:Description>

<rdf:Description rdf:about="https://resource.geosphere.at/thes/lith/9">
	<skos:broader rdf:resource="https://resource.geosphere.at/thes/lith/4"/>
</rdf:Description>

<rdf:Description rdf:about="https://resource.geosphere.at/thes/lith/23">
	<skos:broader rdf:resource="https://resource.geosphere.at/thes/lith/5"/>
</rdf:Description>

<rdf:Description rdf:about="https://resource.geosphere.at/thes/lith/157">
	<skos:broader rdf:resource="https://resource.geosphere.at/thes/lith/5"/>
</rdf:Description>

<rdf:Description rdf:about="https://resource.geosphere.at/thes/lith/17">
	<skos:broader rdf:resource="https://resource.geosphere.at/thes/lith/159"/>
</rdf:Description>

<rdf:Description rdf:about="https://resource.geosphere.at/thes/lith/210">
	<skos:broader rdf:resource="https://resource.geosphere.at/thes/lith/209"/>
</rdf:Description>

<rdf:Description rdf:about="https://resource.geosphere.at/thes/lith/222">
	<skos:broader rdf:resource="https://resource.geosphere.at/thes/lith/166"/>
</rdf:Description>

<rdf:Description rdf:about="https://resource.geosphere.at/thes/lith/54">
	<skos:broader rdf:resource="https://resource.geosphere.at/thes/lith/22"/>
</rdf:Description>

<rdf:Description rdf:about="https://resource.geosphere.at/thes/lith/225">
	<skos:broader rdf:resource="https://resource.geosphere.at/thes/lith/222"/>
</rdf:Description>

<rdf:Description rdf:about="https://resource.geosphere.at/thes/lith/145">
	<skos:broader rdf:resource="https://resource.geosphere.at/thes/lith/98"/>
</rdf:Description>

<rdf:Description rdf:about="https://resource.geosphere.at/thes/lith/140">
	<skos:broader rdf:resource="https://resource.geosphere.at/thes/lith/125"/>
</rdf:Description>

<rdf:Description rdf:about="https://resource.geosphere.at/thes/lith/43">
	<skos:broader rdf:resource="https://resource.geosphere.at/thes/lith/21"/>
</rdf:Description>

<rdf:Description rdf:about="https://resource.geosphere.at/thes/lith/168">
	<skos:broader rdf:resource="https://resource.geosphere.at/thes/lith/160"/>
</rdf:Description>

<rdf:Description rdf:about="https://resource.geosphere.at/thes/lith/80">
	<skos:broader rdf:resource="https://resource.geosphere.at/thes/lith/64"/>
</rdf:Description>

<rdf:Description rdf:about="https://resource.geosphere.at/thes/lith/34">
	<skos:broader rdf:resource="https://resource.geosphere.at/thes/lith/19"/>
</rdf:Description>

<rdf:Description rdf:about="https://resource.geosphere.at/thes/lith/63">
	<skos:broader rdf:resource="https://resource.geosphere.at/thes/lith/6"/>
</rdf:Description>

<rdf:Description rdf:about="https://resource.geosphere.at/thes/lith/184">
	<skos:broader rdf:resource="https://resource.geosphere.at/thes/lith/177"/>
</rdf:Description>

<rdf:Description rdf:about="https://resource.geosphere.at/thes/lith/178">
	<skos:broader rdf:resource="https://resource.geosphere.at/thes/lith/177"/>
</rdf:Description>

<rdf:Description rdf:about="https://resource.geosphere.at/thes/lith/69">
	<skos:broader rdf:resource="https://resource.geosphere.at/thes/lith/6"/>
</rdf:Description>

<rdf:Description rdf:about="https://resource.geosphere.at/thes/lith/239">
	<skos:broader rdf:resource="https://resource.geosphere.at/thes/lith/169"/>
</rdf:Description>

<rdf:Description rdf:about="https://resource.geosphere.at/thes/lith/152">
	<skos:broader rdf:resource="https://resource.geosphere.at/thes/lith/146"/>
</rdf:Description>

<rdf:Description rdf:about="https://resource.geosphere.at/thes/lith/193">
	<skos:broader rdf:resource="https://resource.geosphere.at/thes/lith/192"/>
</rdf:Description>

<rdf:Description rdf:about="https://resource.geosphere.at/thes/lith/89">
	<skos:broader rdf:resource="https://resource.geosphere.at/thes/lith/68"/>
</rdf:Description>

<rdf:Description rdf:about="https://resource.geosphere.at/thes/lith/205">
	<skos:broader rdf:resource="https://resource.geosphere.at/thes/lith/164"/>
</rdf:Description>

<rdf:Description rdf:about="https://resource.geosphere.at/thes/lith/227">
	<skos:broader rdf:resource="https://resource.geosphere.at/thes/lith/166"/>
</rdf:Description>

<rdf:Description rdf:about="https://resource.geosphere.at/thes/lith/123">
	<skos:broader rdf:resource="https://resource.geosphere.at/thes/lith/98"/>
</rdf:Description>

<rdf:Description rdf:about="https://resource.geosphere.at/thes/lith/138">
	<skos:broader rdf:resource="https://resource.geosphere.at/thes/lith/139"/>
</rdf:Description>

<rdf:Description rdf:about="https://resource.geosphere.at/thes/lith/174">
	<skos:broader rdf:resource="https://resource.geosphere.at/thes/lith/173"/>
</rdf:Description>

<rdf:Description rdf:about="https://resource.geosphere.at/thes/lith/38">
	<skos:broader rdf:resource="https://resource.geosphere.at/thes/lith/20"/>
</rdf:Description>

<rdf:Description rdf:about="https://resource.geosphere.at/thes/lith/139">
	<skos:broader rdf:resource="https://resource.geosphere.at/thes/lith/136"/>
</rdf:Description>

<rdf:Description rdf:about="https://resource.geosphere.at/thes/lith/11">
	<skos:broader rdf:resource="https://resource.geosphere.at/thes/lith/3"/>
</rdf:Description>

<rdf:Description rdf:about="https://resource.geosphere.at/thes/lith/84">
	<skos:broader rdf:resource="https://resource.geosphere.at/thes/lith/67"/>
</rdf:Description>

<rdf:Description rdf:about="https://resource.geosphere.at/thes/lith/241">
	<skos:broader rdf:resource="https://resource.geosphere.at/thes/lith/109"/>
</rdf:Description>

<rdf:Description rdf:about="https://resource.geosphere.at/thes/lith/233">
	<skos:broader rdf:resource="https://resource.geosphere.at/thes/lith/232"/>
</rdf:Description>

<rdf:Description rdf:about="https://resource.geosphere.at/thes/lith/64">
	<skos:broader rdf:resource="https://resource.geosphere.at/thes/lith/6"/>
</rdf:Description>

<rdf:Description rdf:about="https://resource.geosphere.at/thes/lith/186">
	<skos:broader rdf:resource="https://resource.geosphere.at/thes/lith/184"/>
</rdf:Description>

<rdf:Description rdf:about="https://resource.geosphere.at/thes/lith/49">
	<skos:broader rdf:resource="https://resource.geosphere.at/thes/lith/21"/>
</rdf:Description>

<rdf:Description rdf:about="https://resource.geosphere.at/thes/lith/201">
	<skos:broader rdf:resource="https://resource.geosphere.at/thes/lith/196"/>
</rdf:Description>

<rdf:Description rdf:about="https://resource.geosphere.at/thes/lith/104">
	<skos:broader rdf:resource="https://resource.geosphere.at/thes/lith/98"/>
</rdf:Description>

<rdf:Description rdf:about="https://resource.geosphere.at/thes/lith/129">
	<skos:broader rdf:resource="https://resource.geosphere.at/thes/lith/98"/>
</rdf:Description>

<rdf:Description rdf:about="https://resource.geosphere.at/thes/lith/146">
	<skos:broader rdf:resource="https://resource.geosphere.at/thes/lith/97"/>
</rdf:Description>

<rdf:Description rdf:about="https://resource.geosphere.at/thes/lith/52">
	<skos:broader rdf:resource="https://resource.geosphere.at/thes/lith/157"/>
</rdf:Description>

<rdf:Description rdf:about="https://resource.geosphere.at/thes/lith/165">
	<skos:broader rdf:resource="https://resource.geosphere.at/thes/lith/159"/>
</rdf:Description>

<rdf:Description rdf:about="https://resource.geosphere.at/thes/lith/254">
	<skos:broader rdf:resource="https://resource.geosphere.at/thes/lith/6"/>
</rdf:Description>

<rdf:Description rdf:about="https://resource.geosphere.at/thes/lith/253">
	<skos:broader rdf:resource="https://resource.geosphere.at/thes/lith/204"/>
</rdf:Description>

<rdf:Description rdf:about="https://resource.geosphere.at/thes/lith/79">
	<skos:broader rdf:resource="https://resource.geosphere.at/thes/lith/64"/>
</rdf:Description>

<rdf:Description rdf:about="https://resource.geosphere.at/thes/lith/44">
	<skos:broader rdf:resource="https://resource.geosphere.at/thes/lith/20"/>
</rdf:Description>

<rdf:Description rdf:about="https://resource.geosphere.at/thes/lith/217">
	<skos:broader rdf:resource="https://resource.geosphere.at/thes/lith/214"/>
</rdf:Description>

<rdf:Description rdf:about="https://resource.geosphere.at/thes/lith/3">
	<skos:broader rdf:resource="https://resource.geosphere.at/thes/lith/159"/>
</rdf:Description>

<rdf:Description rdf:about="https://resource.geosphere.at/thes/lith/22">
	<skos:broader rdf:resource="https://resource.geosphere.at/thes/lith/5"/>
</rdf:Description>

<rdf:Description rdf:about="https://resource.geosphere.at/thes/lith/67">
	<skos:broader rdf:resource="https://resource.geosphere.at/thes/lith/6"/>
</rdf:Description>

<rdf:Description rdf:about="https://resource.geosphere.at/thes/lith/99">
	<skos:broader rdf:resource="https://resource.geosphere.at/thes/lith/98"/>
</rdf:Description>

<rdf:Description rdf:about="https://resource.geosphere.at/thes/lith/154">
	<skos:broader rdf:resource="https://resource.geosphere.at/thes/lith/146"/>
</rdf:Description>

<rdf:Description rdf:about="https://resource.geosphere.at/thes/lith/160">
	<skos:broader rdf:resource="https://resource.geosphere.at/thes/lith/158"/>
</rdf:Description>

<rdf:Description rdf:about="https://resource.geosphere.at/thes/lith/200">
	<skos:broader rdf:resource="https://resource.geosphere.at/thes/lith/196"/>
</rdf:Description>

<rdf:Description rdf:about="https://resource.geosphere.at/thes/lith/96">
	<skos:broader rdf:resource="https://resource.geosphere.at/thes/lith/6"/>
</rdf:Description>

<rdf:Description rdf:about="https://resource.geosphere.at/thes/lith/39">
	<skos:broader rdf:resource="https://resource.geosphere.at/thes/lith/20"/>
</rdf:Description>

<rdf:Description rdf:about="https://resource.geosphere.at/thes/lith/224">
	<skos:broader rdf:resource="https://resource.geosphere.at/thes/lith/222"/>
</rdf:Description>

<rdf:Description rdf:about="https://resource.geosphere.at/thes/lith/191">
	<skos:broader rdf:resource="https://resource.geosphere.at/thes/lith/192"/>
</rdf:Description>

<rdf:Description rdf:about="https://resource.geosphere.at/thes/lith/132">
	<skos:broader rdf:resource="https://resource.geosphere.at/thes/lith/131"/>
</rdf:Description>

<rdf:Description rdf:about="https://resource.geosphere.at/thes/lith/18">
	<skos:broader rdf:resource="https://resource.geosphere.at/thes/lith/5"/>
</rdf:Description>

<rdf:Description rdf:about="https://resource.geosphere.at/thes/lith/144">
	<skos:broader rdf:resource="https://resource.geosphere.at/thes/lith/98"/>
</rdf:Description>

<rdf:Description rdf:about="https://resource.geosphere.at/thes/lith/172">
	<skos:broader rdf:resource="https://resource.geosphere.at/thes/lith/161"/>
</rdf:Description>

<rdf:Description rdf:about="https://resource.geosphere.at/thes/lith/29">
	<skos:broader rdf:resource="https://resource.geosphere.at/thes/lith/19"/>
</rdf:Description>

<rdf:Description rdf:about="https://resource.geosphere.at/thes/lith/55">
	<skos:broader rdf:resource="https://resource.geosphere.at/thes/lith/24"/>
</rdf:Description>

<rdf:Description rdf:about="https://resource.geosphere.at/thes/lith/235">
	<skos:broader rdf:resource="https://resource.geosphere.at/thes/lith/167"/>
</rdf:Description>

<rdf:Description rdf:about="https://resource.geosphere.at/thes/lith/61">
	<skos:broader rdf:resource="https://resource.geosphere.at/thes/lith/7"/>
</rdf:Description>

<rdf:Description rdf:about="https://resource.geosphere.at/thes/lith/35">
	<skos:broader rdf:resource="https://resource.geosphere.at/thes/lith/19"/>
</rdf:Description>

<rdf:Description rdf:about="https://resource.geosphere.at/thes/lith/45">
	<skos:broader rdf:resource="https://resource.geosphere.at/thes/lith/20"/>
</rdf:Description>

<rdf:Description rdf:about="https://resource.geosphere.at/thes/lith/243">
	<skos:broader rdf:resource="https://resource.geosphere.at/thes/lith/162"/>
</rdf:Description>

<rdf:Description rdf:about="https://resource.geosphere.at/thes/lith/105">
	<skos:broader rdf:resource="https://resource.geosphere.at/thes/lith/104"/>
</rdf:Description>

<rdf:Description rdf:about="https://resource.geosphere.at/thes/lith/91">
	<skos:broader rdf:resource="https://resource.geosphere.at/thes/lith/69"/>
</rdf:Description>

<rdf:Description rdf:about="https://resource.geosphere.at/thes/lith/250">
	<skos:broader rdf:resource="https://resource.geosphere.at/thes/lith/98"/>
</rdf:Description>

<rdf:Description rdf:about="https://resource.geosphere.at/thes/lith/109">
	<skos:broader rdf:resource="https://resource.geosphere.at/thes/lith/108"/>
</rdf:Description>

<rdf:Description rdf:about="https://resource.geosphere.at/thes/lith/127">
	<skos:broader rdf:resource="https://resource.geosphere.at/thes/lith/98"/>
</rdf:Description>

<rdf:Description rdf:about="https://resource.geosphere.at/thes/lith/71">
	<skos:broader rdf:resource="https://resource.geosphere.at/thes/lith/62"/>
</rdf:Description>

<rdf:Description rdf:about="https://resource.geosphere.at/thes/lith/226">
	<skos:broader rdf:resource="https://resource.geosphere.at/thes/lith/166"/>
</rdf:Description>

<rdf:Description rdf:about="https://resource.geosphere.at/thes/lith/100">
	<skos:broader rdf:resource="https://resource.geosphere.at/thes/lith/99"/>
</rdf:Description>

<rdf:Description rdf:about="https://resource.geosphere.at/thes/lith/221">
	<skos:broader rdf:resource="https://resource.geosphere.at/thes/lith/218"/>
</rdf:Description>

<rdf:Description rdf:about="https://resource.geosphere.at/thes/lith/30">
	<skos:broader rdf:resource="https://resource.geosphere.at/thes/lith/19"/>
</rdf:Description>

<rdf:Description rdf:about="https://resource.geosphere.at/thes/lith/163">
	<skos:broader rdf:resource="https://resource.geosphere.at/thes/lith/159"/>
</rdf:Description>

<rdf:Description rdf:about="https://resource.geosphere.at/thes/lith/242">
	<skos:broader rdf:resource="https://resource.geosphere.at/thes/lith/109"/>
</rdf:Description>

<rdf:Description rdf:about="https://resource.geosphere.at/thes/lith/244">
	<skos:broader rdf:resource="https://resource.geosphere.at/thes/lith/139"/>
</rdf:Description>

<rdf:Description rdf:about="https://resource.geosphere.at/thes/lith/24">
	<skos:broader rdf:resource="https://resource.geosphere.at/thes/lith/5"/>
</rdf:Description>

<rdf:Description rdf:about="https://resource.geosphere.at/thes/lith/159">
	<skos:broader rdf:resource="https://resource.geosphere.at/thes/lith/158"/>
</rdf:Description>

<rdf:Description rdf:about="https://resource.geosphere.at/thes/lith/106">
	<skos:broader rdf:resource="https://resource.geosphere.at/thes/lith/104"/>
</rdf:Description>

<rdf:Description rdf:about="https://resource.geosphere.at/thes/lith/190">
	<skos:broader rdf:resource="https://resource.geosphere.at/thes/lith/161"/>
</rdf:Description>

<rdf:Description rdf:about="https://resource.geosphere.at/thes/lith/188">
	<skos:broader rdf:resource="https://resource.geosphere.at/thes/lith/177"/>
</rdf:Description>

<rdf:Description rdf:about="https://resource.geosphere.at/thes/lith/70">
	<skos:broader rdf:resource="https://resource.geosphere.at/thes/lith/62"/>
</rdf:Description>

<rdf:Description rdf:about="https://resource.geosphere.at/thes/lith/204">
	<skos:broader rdf:resource="https://resource.geosphere.at/thes/lith/163"/>
</rdf:Description>

<rdf:Description rdf:about="https://resource.geosphere.at/thes/lith/255">
	<skos:broader rdf:resource="https://resource.geosphere.at/thes/lith/98"/>
</rdf:Description>

<rdf:Description rdf:about="https://resource.geosphere.at/thes/lith/116">
	<skos:broader rdf:resource="https://resource.geosphere.at/thes/lith/108"/>
</rdf:Description>

<rdf:Description rdf:about="https://resource.geosphere.at/thes/lith/51">
	<skos:broader rdf:resource="https://resource.geosphere.at/thes/lith/157"/>
</rdf:Description>

<rdf:Description rdf:about="https://resource.geosphere.at/thes/lith/56">
	<skos:broader rdf:resource="https://resource.geosphere.at/thes/lith/23"/>
</rdf:Description>

<rdf:Description rdf:about="https://resource.geosphere.at/thes/lith/167">
	<skos:broader rdf:resource="https://resource.geosphere.at/thes/lith/160"/>
</rdf:Description>

<rdf:Description rdf:about="https://resource.geosphere.at/thes/lith/81">
	<skos:broader rdf:resource="https://resource.geosphere.at/thes/lith/64"/>
</rdf:Description>

<rdf:Description rdf:about="https://resource.geosphere.at/thes/lith/124">
	<skos:broader rdf:resource="https://resource.geosphere.at/thes/lith/123"/>
</rdf:Description>

<rdf:Description rdf:about="https://resource.geosphere.at/thes/lith/216">
	<skos:broader rdf:resource="https://resource.geosphere.at/thes/lith/214"/>
</rdf:Description>

<rdf:Description rdf:about="https://resource.geosphere.at/thes/lith/62">
	<skos:broader rdf:resource="https://resource.geosphere.at/thes/lith/6"/>
</rdf:Description>

<rdf:Description rdf:about="https://resource.geosphere.at/thes/lith/68">
	<skos:broader rdf:resource="https://resource.geosphere.at/thes/lith/6"/>
</rdf:Description>

<rdf:Description rdf:about="https://resource.geosphere.at/thes/lith/75">
	<skos:broader rdf:resource="https://resource.geosphere.at/thes/lith/64"/>
</rdf:Description>

<rdf:Description rdf:about="https://resource.geosphere.at/thes/lith/208">
	<skos:broader rdf:resource="https://resource.geosphere.at/thes/lith/207"/>
</rdf:Description>

<rdf:Description rdf:about="https://resource.geosphere.at/thes/lith/153">
	<skos:broader rdf:resource="https://resource.geosphere.at/thes/lith/146"/>
</rdf:Description>

<rdf:Description rdf:about="https://resource.geosphere.at/thes/lith/13">
	<skos:broader rdf:resource="https://resource.geosphere.at/thes/lith/3"/>
</rdf:Description>

<rdf:Description rdf:about="https://resource.geosphere.at/thes/lith/223">
	<skos:broader rdf:resource="https://resource.geosphere.at/thes/lith/222"/>
</rdf:Description>

<rdf:Description rdf:about="https://resource.geosphere.at/thes/lith/173">
	<skos:broader rdf:resource="https://resource.geosphere.at/thes/lith/161"/>
</rdf:Description>

<rdf:Description rdf:about="https://resource.geosphere.at/thes/lith/117">
	<skos:broader rdf:resource="https://resource.geosphere.at/thes/lith/116"/>
</rdf:Description>

<rdf:Description rdf:about="https://resource.geosphere.at/thes/lith/85">
	<skos:broader rdf:resource="https://resource.geosphere.at/thes/lith/67"/>
</rdf:Description>

<rdf:Description rdf:about="https://resource.geosphere.at/thes/lith/25">
	<skos:broader rdf:resource="https://resource.geosphere.at/thes/lith/18"/>
</rdf:Description>

<rdf:Description rdf:about="https://resource.geosphere.at/thes/lith/110">
	<skos:broader rdf:resource="https://resource.geosphere.at/thes/lith/109"/>
</rdf:Description>

<rdf:Description rdf:about="https://resource.geosphere.at/thes/lith/195">
	<skos:broader rdf:resource="https://resource.geosphere.at/thes/lith/162"/>
</rdf:Description>

<rdf:Description rdf:about="https://resource.geosphere.at/thes/lith/147">
	<skos:broader rdf:resource="https://resource.geosphere.at/thes/lith/146"/>
</rdf:Description>

<rdf:Description rdf:about="https://resource.geosphere.at/thes/lith/141">
	<skos:broader rdf:resource="https://resource.geosphere.at/thes/lith/136"/>
</rdf:Description>

<rdf:Description rdf:about="https://resource.geosphere.at/thes/lith/156">
	<skos:broader rdf:resource="https://resource.geosphere.at/thes/lith/97"/>
</rdf:Description>

<rdf:Description rdf:about="https://resource.geosphere.at/thes/lith/36">
	<skos:broader rdf:resource="https://resource.geosphere.at/thes/lith/19"/>
</rdf:Description>

<rdf:Description rdf:about="https://resource.geosphere.at/thes/lith/236">
	<skos:broader rdf:resource="https://resource.geosphere.at/thes/lith/167"/>
</rdf:Description>

<rdf:Description rdf:about="https://resource.geosphere.at/thes/lith/214">
	<skos:broader rdf:resource="https://resource.geosphere.at/thes/lith/166"/>
</rdf:Description>

<rdf:Description rdf:about="https://resource.geosphere.at/thes/lith/40">
	<skos:broader rdf:resource="https://resource.geosphere.at/thes/lith/20"/>
</rdf:Description>

<rdf:Description rdf:about="https://resource.geosphere.at/thes/lith/0">
	<dcterms:hasVersion rdf:datatype="http://www.w3.org/2001/XMLSchema#int">276</dcterms:hasVersion>
	<dcterms:created rdf:datatype="http://www.w3.org/2001/XMLSchema#dateTime">2012-12-06T09:11:54.000Z</dcterms:created>
	<rdf:type rdf:resource="http://www.w3.org/2004/02/skos/core#ConceptScheme"/>
</rdf:Description>

<rdf:Description rdf:about="https://resource.geosphere.at/thes/lith/158">
	<skos:definition xml:lang="de">An der Erdoberfläche natürlich vorkommendes Material, welches aus festen Partikeln besteht, angehäuft durch einen oder mehrere Ablagerungsprozesse in fluiden Systemen (flüssig oder gasförmig), welche granulare und/oder kristalline Partikel erzeugen, die in Form von Lagen oder Körpern auftreten. Das Konzept beinhaltet Sedimente und Sedimentgesteine (SLTT Appendix C, 2004).</skos:definition>
	<skos:definition xml:lang="en">Naturally-occurring material formed at the Earth’s surface, consisting of solid particles aggregated together by one or more depositional processes operating within fluid systems (either aqueous or gaseous) to yield granular particles and/or crystalline particles that are aggregated into layers or bodies. The term includes both unconsolidated sediments and sedimentary rocks (SLTT Appendix C, 2004).</skos:definition>
	<dcterms:references rdf:resource="https://resource.geosphere.at/thes/citation/547"/>
	<skos:related rdf:resource="https://resource.geosphere.at/thes/lith/97"/>
	<skos:exactMatch rdf:resource="http://inspire.ec.europa.eu/codelist/LithologyValue/sedimentaryMaterial"/>
	<colourHexCode xmlns="http://dbpedia.org/ontology/">#FFF299</colourHexCode>
	<dcterms:hasVersion rdf:datatype="http://www.w3.org/2001/XMLSchema#int">10</dcterms:hasVersion>
	<skos:prefLabel xml:lang="en">Sedimentary material</skos:prefLabel>
	<dcterms:date rdf:datatype="http://www.w3.org/2001/XMLSchema#dateTime">2011-03-22T14:52:39Z</dcterms:date>
	<skos:narrower rdf:resource="https://resource.geosphere.at/thes/lith/160"/>
	<skos:narrower rdf:resource="https://resource.geosphere.at/thes/lith/159"/>
	<rdf:type rdf:resource="http://www.w3.org/2004/02/skos/core#Concept"/>
	<skos:prefLabel xml:lang="de">Sedimentäres Material</skos:prefLabel>
	<skos:exactMatch rdf:resource="http://resource.geosciml.org/classifier/cgi/lithology/sedimentary_material"/>
	<dcterms:created rdf:datatype="http://www.w3.org/2001/XMLSchema#dateTime">2012-03-12T16:21:30.000Z</dcterms:created>
</rdf:Description>

<rdf:Description rdf:about="https://resource.geosphere.at/thes/lith/159">
	<skos:exactMatch rdf:resource="http://data.bgs.ac.uk/id/EarthMaterialClass/RockName/SR"/>
	<skos:exactMatch rdf:resource="http://inspire.ec.europa.eu/codelist/LithologyValue/sedimentaryRock"/>
	<dcterms:references rdf:resource="https://resource.geosphere.at/thes/citation/547"/>
	<skos:prefLabel xml:lang="de">Sedimentgestein</skos:prefLabel>
	<skos:narrower rdf:resource="https://resource.geosphere.at/thes/lith/3"/>
	<rdf:type rdf:resource="http://www.w3.org/2004/02/skos/core#Concept"/>
	<skos:prefLabel xml:lang="en">Sedimentary rock</skos:prefLabel>
	<skos:narrower rdf:resource="https://resource.geosphere.at/thes/lith/17"/>
	<skos:exactMatch rdf:resource="http://www.wikidata.org/entity/Q82480"/>
	<dcterms:references rdf:resource="https://resource.geosphere.at/thes/citation/545"/>
	<colourHexCode xmlns="http://dbpedia.org/ontology/">#E6CC66</colourHexCode>
	<skos:narrower rdf:resource="https://resource.geosphere.at/thes/lith/161"/>
	<skos:narrower rdf:resource="https://resource.geosphere.at/thes/lith/162"/>
	<skos:narrower rdf:resource="https://resource.geosphere.at/thes/lith/163"/>
	<skos:narrower rdf:resource="https://resource.geosphere.at/thes/lith/164"/>
	<skos:narrower rdf:resource="https://resource.geosphere.at/thes/lith/165"/>
	<dcterms:hasVersion rdf:datatype="http://www.w3.org/2001/XMLSchema#int">14</dcterms:hasVersion>
	<skos:definition xml:lang="de">Festgestein, welches durch postdepositionale Konsolidierung (durch Prozesse der Kompaktion, Zementation, Kristallisation oder biogener Verkittung) von Sedimenten entsteht (verändert nach Neuendorf et al., 2005; SLTT Appendix C, 2004).</skos:definition>
	<skos:related rdf:resource="https://resource.geosphere.at/thes/lith/160"/>
	<skos:definition xml:lang="en">A rock formed from post depositional consolidation of sediments (by processes of compaction, cementation, crystallisation, or biogenic binding) (modified from Neuendorf et al., 2005; SLTT Appendix C, 2004).</skos:definition>
	<dcterms:created rdf:datatype="http://www.w3.org/2001/XMLSchema#dateTime">2012-03-12T16:21:46.000Z</dcterms:created>
	<dcterms:date rdf:datatype="http://www.w3.org/2001/XMLSchema#dateTime">2011-03-22T14:52:39Z</dcterms:date>
	<skos:exactMatch rdf:resource="http://resource.geosciml.org/classifier/cgi/lithology/sedimentary_rock"/>
</rdf:Description>

<rdf:Description rdf:about="https://resource.geosphere.at/thes/lith/162">
	<skos:exactMatch rdf:resource="http://inspire.ec.europa.eu/codelist/LithologyValue/carbonateSedimentaryRock"/>
	<skos:related rdf:resource="https://resource.geosphere.at/thes/lith/167"/>
	<dcterms:hasVersion rdf:datatype="http://www.w3.org/2001/XMLSchema#int">12</dcterms:hasVersion>
	<dcterms:date rdf:datatype="http://www.w3.org/2001/XMLSchema#dateTime">2011-03-22T14:52:39Z</dcterms:date>
	<skos:narrower rdf:resource="https://resource.geosphere.at/thes/lith/196"/>
	<skos:narrower rdf:resource="https://resource.geosphere.at/thes/lith/195"/>
	<skos:narrower rdf:resource="https://resource.geosphere.at/thes/lith/197"/>
	<skos:definition xml:lang="de">Ein sedimentäres Gestein mit ≥ 50% primären und/oder rekristallisierten Bestandteilen aus Karbonatmineralen (Calcit/Aragonit/Dolomit). Diese Materialien leiten sich aus Prozessen ab, die innerhalb eines Ablagerungsregimes (innerhalb eines Beckens) wirken und nicht durch Transport in das Ablagerungsregime aus anderen Sedimentquellen kommt (SLTT Appendix C, 2004).</skos:definition>
	<skos:prefLabel xml:lang="de">Karbonatisches Sedimentgestein</skos:prefLabel>
	<colourHexCode xmlns="http://dbpedia.org/ontology/">#4D80FF</colourHexCode>
	<skos:narrower rdf:resource="https://resource.geosphere.at/thes/lith/243"/>
	<skos:prefLabel xml:lang="en">Carbonate sedimentary rock</skos:prefLabel>
	<skos:definition xml:lang="en">A sedimentary rock in which ≥ 50% of the primary and (or) re-crystallized constituents are composed of carbonate minerals (calcite/aragonite/ dolomite). Such materials are intra-basinal in origin - that is, they formed by processes operating within a depositional regime, and were not transported into that regime from other sediment sources (SLTT Appendix C, 2004).</skos:definition>
	<dcterms:references rdf:resource="https://resource.geosphere.at/thes/citation/547"/>
	<dcterms:created rdf:datatype="http://www.w3.org/2001/XMLSchema#dateTime">2012-03-12T10:53:09.000Z</dcterms:created>
	<skos:exactMatch rdf:resource="http://resource.geosciml.org/classifier/cgi/lithology/carbonate_sedimentary_rock"/>
	<rdf:type rdf:resource="http://www.w3.org/2004/02/skos/core#Concept"/>
</rdf:Description>

<rdf:Description rdf:about="https://resource.geosphere.at/thes/lith/195">
	<skos:prefLabel xml:lang="en">Sandy Limestone</skos:prefLabel>
	<skos:closeMatch rdf:resource="http://resource.geosciml.org/classifier/cgi/lithology/carbonate_sedimentary_rock"/>
	<skos:definition xml:lang="de">Karbonatisch-klastisches Sedimentgestein, dessen klastischer Anteil sich auf die Sandfraktion beschränkt. Besteht aus 50–75 % Calcit und 25–50 % Sand (Füchtbauer, 1988).</skos:definition>
	<skos:definition xml:lang="en">A mixed carbonate-clastic rock in which the clastic portion is restricted to sand-sized components. Consists of 50-75% calcite and 25-50% sand (Füchtbauer, 1988).</skos:definition>
	<skos:related rdf:resource="https://resource.geosphere.at/thes/lith/235"/>
	<dcterms:hasVersion rdf:datatype="http://www.w3.org/2001/XMLSchema#int">11</dcterms:hasVersion>
	<dcterms:date rdf:datatype="http://www.w3.org/2001/XMLSchema#dateTime">2011-03-22T14:52:39Z</dcterms:date>
	<rdf:type rdf:resource="http://www.w3.org/2004/02/skos/core#Concept"/>
	<skos:broadMatch rdf:resource="http://inspire.ec.europa.eu/codelist/LithologyValue/limestone"/>
	<dcterms:references rdf:resource="https://resource.geosphere.at/thes/citation/229"/>
	<skos:exactMatch rdf:resource="http://data.bgs.ac.uk/id/EarthMaterialClass/RockName/SALMST"/>
	<dcterms:created rdf:datatype="http://www.w3.org/2001/XMLSchema#dateTime">2012-03-12T16:15:02.000Z</dcterms:created>
	<skos:prefLabel xml:lang="de">Sandkalkstein</skos:prefLabel>
	<skos:related rdf:resource="https://resource.geosphere.at/thes/lith/194"/>
</rdf:Description>

<rdf:Description rdf:about="https://resource.geosphere.at/thes/lith/197">
	<skos:prefLabel xml:lang="de">Dolomit</skos:prefLabel>
	<foaf:depiction rdf:resource="https://resource.geosphere.at/img/thes/Dolomit.jpg"/>
	<skos:prefLabel xml:lang="en">Dolomite</skos:prefLabel>
	<skos:exactMatch rdf:resource="http://resource.geosciml.org/classifier/cgi/lithology/dolostone"/>
	<rdf:type rdf:resource="http://www.w3.org/2004/02/skos/core#Concept"/>
	<dcterms:references rdf:resource="https://resource.geosphere.at/thes/citation/545"/>
	<skos:exactMatch rdf:resource="http://dbpedia.org/resource/Dolostone"/>
	<skos:altLabel xml:lang="en">Dolostone</skos:altLabel>
	<skos:exactMatch rdf:resource="http://inspire.ec.europa.eu/codelist/LithologyValue/dolomite"/>
	<skos:definition xml:lang="en">A carbonate sedimentary rock composed of &gt; 90% dolomite and &lt; 10% calcite. Usually formed by diagenesis and dolomitization of calcite and aragonite (Neuendorf et al., 2005; Vinx 2005).</skos:definition>
	<skos:definition xml:lang="de">Karbonatisches Sedimentgestein, welches zu &gt; 90 % aus Dolomit und &lt; 10 % Calcit besteht. Entsteht überwiegend während der Diagenese durch Dolomitisierung von Calcit and Aragonit (Neuendorf et al., 2005; Vinx, 2005).</skos:definition>
	<colourHexCode xmlns="http://dbpedia.org/ontology/">#73A6F2</colourHexCode>
	<dcterms:created rdf:datatype="http://www.w3.org/2001/XMLSchema#dateTime">2013-04-05T09:25:46.000Z</dcterms:created>
	<dcterms:date rdf:datatype="http://www.w3.org/2001/XMLSchema#dateTime">2011-03-22T14:52:39Z</dcterms:date>
	<dcterms:hasVersion rdf:datatype="http://www.w3.org/2001/XMLSchema#int">10</dcterms:hasVersion>
	<dcterms:references rdf:resource="https://resource.geosphere.at/thes/citation/878"/>
</rdf:Description>

<rdf:Description rdf:about="https://resource.geosphere.at/thes/lith/196">
	<dcterms:date rdf:datatype="http://www.w3.org/2001/XMLSchema#dateTime">2011-03-22T14:52:39Z</dcterms:date>
	<dcterms:references rdf:resource="https://resource.geosphere.at/thes/citation/545"/>
	<skos:related rdf:resource="https://resource.geosphere.at/thes/lith/236"/>
	<skos:exactMatch rdf:resource="http://data.bgs.ac.uk/id/EarthMaterialClass/RockName/LMST"/>
	<skos:prefLabel xml:lang="en">Limestone</skos:prefLabel>
	<rdf:type rdf:resource="http://www.w3.org/2004/02/skos/core#Concept"/>
	<skos:definition xml:lang="en">A carbonate sedimentary rock composed of &gt; 95% calcite (and aragonite) and &lt; 5% dolomite (Neuendorf et al., 2005).</skos:definition>
	<skos:definition xml:lang="de">Karbonatisches Sedimentgestein, welches zu &gt; 95 % aus Calcit (und Aragonit) und &lt; 5 % Dolomit besteht (Neuendorf et al., 2005).</skos:definition>
	<skos:exactMatch rdf:resource="http://resource.geosciml.org/classifier/cgi/lithology/limestone"/>
	<dcterms:hasVersion rdf:datatype="http://www.w3.org/2001/XMLSchema#int">7</dcterms:hasVersion>
	<skos:narrower rdf:resource="https://resource.geosphere.at/thes/lith/198"/>
	<skos:narrower rdf:resource="https://resource.geosphere.at/thes/lith/199"/>
	<skos:exactMatch rdf:resource="http://www.wikidata.org/entity/Q23757"/>
	<dcterms:created rdf:datatype="http://www.w3.org/2001/XMLSchema#dateTime">2014-02-25T12:17:17.000Z</dcterms:created>
	<skos:exactMatch rdf:resource="http://dbpedia.org/resource/Limestone"/>
	<skos:altLabel xml:lang="de">Kalk</skos:altLabel>
	<skos:narrower rdf:resource="https://resource.geosphere.at/thes/lith/201"/>
	<skos:narrower rdf:resource="https://resource.geosphere.at/thes/lith/200"/>
	<skos:narrower rdf:resource="https://resource.geosphere.at/thes/lith/203"/>
	<skos:narrower rdf:resource="https://resource.geosphere.at/thes/lith/202"/>
	<skos:exactMatch rdf:resource="http://inspire.ec.europa.eu/codelist/LithologyValue/limestone"/>
	<colourHexCode xmlns="http://dbpedia.org/ontology/">#66B2F2</colourHexCode>
	<skos:prefLabel xml:lang="de">Kalkstein (Kalk)</skos:prefLabel>
</rdf:Description>

<rdf:Description rdf:about="https://resource.geosphere.at/thes/lith/201">
	<dcterms:references rdf:resource="https://resource.geosphere.at/thes/citation/229"/>
	<skos:prefLabel xml:lang="de">Kalkarenit</skos:prefLabel>
	<skos:altLabel xml:lang="en">Calcarenite</skos:altLabel>
	<skos:definition xml:lang="en">A limestone consisting predominantly (&gt; 50%) of rounded detrital calcite particles (either bigenetic or non-biogenetic) between 0.063 and 2 mm. Interstices are filled with carbonate mud or cement (Füchtbauer, 1988; Neuendorf et al., 2005).</skos:definition>
	<skos:definition xml:lang="de">Kalkstein, der überwiegend (&gt; 50 %) aus detritären Calcitpartikeln (Biogene oder andere Rundkörper) &gt; 0.063 mm und &lt; 2 mm besteht. Die Zwischenräume sind mit feinem Karbonatschlamm oder Zement gefüllt (Füchtbauer, 1988; Neuendorf et al., 2005).</skos:definition>
	<dcterms:references rdf:resource="https://resource.geosphere.at/thes/citation/545"/>
	<skos:broadMatch rdf:resource="http://resource.geosciml.org/classifier/cgi/lithology/limestone"/>
	<rdf:type rdf:resource="http://www.w3.org/2004/02/skos/core#Concept"/>
	<skos:broadMatch rdf:resource="http://inspire.ec.europa.eu/codelist/LithologyValue/limestone"/>
	<dcterms:hasVersion rdf:datatype="http://www.w3.org/2001/XMLSchema#int">11</dcterms:hasVersion>
	<skos:prefLabel xml:lang="en">Calciarenite</skos:prefLabel>
	<dcterms:created rdf:datatype="http://www.w3.org/2001/XMLSchema#dateTime">2012-03-12T10:45:57.000Z</dcterms:created>
	<dcterms:date rdf:datatype="http://www.w3.org/2001/XMLSchema#dateTime">2011-03-22T14:52:39Z</dcterms:date>
</rdf:Description>

<rdf:Description rdf:about="https://resource.geosphere.at/thes/lith/200">
	<skos:prefLabel xml:lang="de">Kalkrudit</skos:prefLabel>
	<dcterms:references rdf:resource="https://resource.geosphere.at/thes/citation/545"/>
	<skos:definition xml:lang="en">A limestone consisting predominantly (&gt; 50%) of rounded detrital calcite particles (either bigenetic or non-biogenetic) &gt; 2mm. Interstices are filled with carbonate mud or cement (Füchtbauer, 1988; Neuendorf et al., 2005).</skos:definition>
	<skos:prefLabel xml:lang="en">Calcirudite</skos:prefLabel>
	<dcterms:hasVersion rdf:datatype="http://www.w3.org/2001/XMLSchema#int">10</dcterms:hasVersion>
	<skos:exactMatch rdf:resource="http://www.wikidata.org/entity/Q2411703"/>
	<dcterms:references rdf:resource="https://resource.geosphere.at/thes/citation/229"/>
	<dcterms:date rdf:datatype="http://www.w3.org/2001/XMLSchema#dateTime">2011-03-22T14:52:39Z</dcterms:date>
	<skos:broadMatch rdf:resource="http://inspire.ec.europa.eu/codelist/LithologyValue/limestone"/>
	<skos:broadMatch rdf:resource="http://resource.geosciml.org/classifier/cgi/lithology/limestone"/>
	<rdf:type rdf:resource="http://www.w3.org/2004/02/skos/core#Concept"/>
	<skos:definition xml:lang="de">Kalkstein, der überwiegend (&gt; 50 %) aus detritären Calcitpartikeln (Biogene oder andere Rundkörper) &gt; 2 mm besteht. Die Zwischenräume sind mit feinem Karbonatschlamm oder Zement gefüllt (Füchtbauer, 1988; Neuendorf et al., 2005).</skos:definition>
	<dcterms:created rdf:datatype="http://www.w3.org/2001/XMLSchema#dateTime">2012-03-12T10:47:48.000Z</dcterms:created>
</rdf:Description>

<rdf:Description rdf:about="https://resource.geosphere.at/thes/lith/203">
	<dcterms:references rdf:resource="https://resource.geosphere.at/thes/citation/229"/>
	<skos:definition xml:lang="en">A limestone consisting predominantly (&gt; 50%) of carbonate mud or detrital particles &lt; 0.004 mm (Füchtbauer, 1988; Neuendorf et al., 2005).</skos:definition>
	<skos:broadMatch rdf:resource="http://inspire.ec.europa.eu/codelist/LithologyValue/limestone"/>
	<skos:broadMatch rdf:resource="http://resource.geosciml.org/classifier/cgi/lithology/limestone"/>
	<dcterms:date rdf:datatype="http://www.w3.org/2001/XMLSchema#dateTime">2011-03-22T14:52:39Z</dcterms:date>
	<skos:prefLabel xml:lang="en">Calcilutite</skos:prefLabel>
	<skos:prefLabel xml:lang="de">Kalklutit</skos:prefLabel>
	<dcterms:references rdf:resource="https://resource.geosphere.at/thes/citation/545"/>
	<dcterms:created rdf:datatype="http://www.w3.org/2001/XMLSchema#dateTime">2012-03-12T10:46:45.000Z</dcterms:created>
	<rdf:type rdf:resource="http://www.w3.org/2004/02/skos/core#Concept"/>
	<skos:exactMatch rdf:resource="http://www.wikidata.org/entity/Q3073804"/>
	<dcterms:hasVersion rdf:datatype="http://www.w3.org/2001/XMLSchema#int">9</dcterms:hasVersion>
	<skos:definition xml:lang="de">Kalkstein, der überwiegend (&gt; 50 %) aus feinem Karbonatschlamm beziehungsweise detritären Partikeln &lt; 0.004 mm besteht (Füchtbauer, 1988; Neuendorf et al., 2005).</skos:definition>
</rdf:Description>

<rdf:Description rdf:about="https://resource.geosphere.at/thes/lith/202">
	<skos:broadMatch rdf:resource="http://inspire.ec.europa.eu/codelist/LithologyValue/limestone"/>
	<rdf:type rdf:resource="http://www.w3.org/2004/02/skos/core#Concept"/>
	<skos:definition xml:lang="en">A limestone consisting predominantly (&gt; 50%) of rounded detrital calcite particles (either bigenetic or non-biogenetic) between 0.004 and 0.063 mm. Interstices are filled with carbonate mud or cement (Füchtbauer, 1988; Neuendorf et al., 2005).</skos:definition>
	<skos:prefLabel xml:lang="en">Calcisiltite</skos:prefLabel>
	<dcterms:date rdf:datatype="http://www.w3.org/2001/XMLSchema#dateTime">2011-03-22T14:52:39Z</dcterms:date>
	<skos:broadMatch rdf:resource="http://resource.geosciml.org/classifier/cgi/lithology/limestone"/>
	<dcterms:references rdf:resource="https://resource.geosphere.at/thes/citation/545"/>
	<dcterms:created rdf:datatype="http://www.w3.org/2001/XMLSchema#dateTime">2012-03-12T10:48:43.000Z</dcterms:created>
	<skos:prefLabel xml:lang="de">Kalksiltit</skos:prefLabel>
	<skos:exactMatch rdf:resource="http://www.wikidata.org/entity/Q3306858"/>
	<skos:definition xml:lang="de">Kalkstein, der überwiegend (&gt; 50 %) aus detritären Calcitpartikeln (Biogene oder andere Rundkörper) &gt; 0.004 mm und &lt; 0.063 mm besteht. Die Zwischenräume sind mit feinem Karbonatschlamm oder Zement gefüllt (Füchtbauer, 1988; Neuendorf et al., 2005).</skos:definition>
	<dcterms:hasVersion rdf:datatype="http://www.w3.org/2001/XMLSchema#int">10</dcterms:hasVersion>
	<dcterms:references rdf:resource="https://resource.geosphere.at/thes/citation/229"/>
</rdf:Description>

<rdf:Description rdf:about="https://resource.geosphere.at/thes/lith/199">
	<skos:exactMatch rdf:resource="http://inspire.ec.europa.eu/codelist/LithologyValue/travertine"/>
	<skos:exactMatch rdf:resource="http://www.wikidata.org/entity/Q187156"/>
	<skos:hiddenLabel xml:lang="en">Calc-sinter</skos:hiddenLabel>
	<dcterms:hasVersion rdf:datatype="http://www.w3.org/2001/XMLSchema#int">19</dcterms:hasVersion>
	<skos:hiddenLabel xml:lang="de">Sinterkalk</skos:hiddenLabel>
	<skos:definition xml:lang="de">Gestein aus biotisch oder abiotisch gefälltem Calciumkarbonat, das in Quellwasser, hydrothermalem Wasser oder Wasser mit Umgebungstemperatur entstanden ist. Das Konzept beinhaltet Kalktuff (Neuendorf et al., 2005).</skos:definition>
	<skos:scopeNote xml:lang="de">Geologische (lithogenetische) Einheiten die aus Travertin aufgebaut sind werden als Sinterkalk bezeichnet.</skos:scopeNote>
	<skos:exactMatch rdf:resource="http://resource.geosciml.org/classifier/cgi/lithology/travertine"/>
	<skos:hiddenLabel xml:lang="de">Kalksinter</skos:hiddenLabel>
	<dcterms:date rdf:datatype="http://www.w3.org/2001/XMLSchema#dateTime">2011-03-22T14:52:39Z</dcterms:date>
	<skos:scopeNote xml:lang="en">Geologic (lithogenetic) units that are composed of Travertine are called calc-sinter.</skos:scopeNote>
	<dcterms:created rdf:datatype="http://www.w3.org/2001/XMLSchema#dateTime">2013-04-05T09:41:07.000Z</dcterms:created>
	<skos:prefLabel xml:lang="de">Travertin</skos:prefLabel>
	<colourHexCode xmlns="http://dbpedia.org/ontology/">#80CCF2</colourHexCode>
	<skos:definition xml:lang="en">A rock made up of calcium carbonate precipitated biotically or abiotically from spring-fed, heated, or ambient-temperature water. The term includes tufa (Neuendorf et al., 2005).</skos:definition>
	<skos:exactMatch rdf:resource="http://dbpedia.org/resource/Travertine"/>
	<skos:prefLabel xml:lang="en">Travertine</skos:prefLabel>
	<rdf:type rdf:resource="http://www.w3.org/2004/02/skos/core#Concept"/>
	<dcterms:references rdf:resource="https://resource.geosphere.at/thes/citation/545"/>
	<foaf:depiction rdf:resource="https://resource.geosphere.at/img/thes/Sinterkalk_Travertin_2.jpg"/>
</rdf:Description>

<rdf:Description rdf:about="https://resource.geosphere.at/thes/lith/198">
	<skos:exactMatch rdf:resource="http://resource.geosciml.org/classifier/cgi/lithology/chalk"/>
	<dcterms:date rdf:datatype="http://www.w3.org/2001/XMLSchema#dateTime">2011-03-22T14:52:39Z</dcterms:date>
	<skos:exactMatch rdf:resource="http://www.wikidata.org/entity/Q183670"/>
	<skos:definition xml:lang="en">A light-coloured (white-gray) marine limestone composed almost entirely of fine crystalline calcite. These porous limestones consist of foraminifera and calcareous algae, and usually contain chert nodules (Neuendorf et al., 2005).</skos:definition>
	<skos:altLabel xml:lang="de">Kreide</skos:altLabel>
	<skos:exactMatch rdf:resource="http://dbpedia.org/resource/Chalk"/>
	<skos:prefLabel xml:lang="de">Schreibkreide</skos:prefLabel>
	<skos:definition xml:lang="de">Heller (weiß-grauer) mariner Kalkstein, welcher fast vollständig aus feinkristallinem Calcit besteht. Diese Kalke sind porös und werden von Foraminiferen oder Kalkalgen aufgebaut, gewöhnlich führen sie Hornsteinknollen (Neuendorf et al., 2005).</skos:definition>
	<colourHexCode xmlns="http://dbpedia.org/ontology/">#73BFF2</colourHexCode>
	<skos:exactMatch rdf:resource="http://data.bgs.ac.uk/id/EarthMaterialClass/RockName/CHLK"/>
	<dcterms:references rdf:resource="https://resource.geosphere.at/thes/citation/545"/>
	<skos:prefLabel xml:lang="en">Chalk</skos:prefLabel>
	<skos:exactMatch rdf:resource="http://inspire.ec.europa.eu/codelist/LithologyValue/chalk"/>
	<dcterms:created rdf:datatype="http://www.w3.org/2001/XMLSchema#dateTime">2012-03-12T11:57:23.000Z</dcterms:created>
	<dcterms:hasVersion rdf:datatype="http://www.w3.org/2001/XMLSchema#int">7</dcterms:hasVersion>
	<rdf:type rdf:resource="http://www.w3.org/2004/02/skos/core#Concept"/>
</rdf:Description>

<rdf:Description rdf:about="https://resource.geosphere.at/thes/lith/243">
	<dcterms:created rdf:datatype="http://www.w3.org/2001/XMLSchema#dateTime">2012-01-18T10:22:23.000Z</dcterms:created>
	<skos:definition xml:lang="en">A rock that consists of cellular or porous limestone or dolostone in which secondary dissolution of readily soluble material (gypsum/anhydrite) has formed cavities. Rauhwackes are mainly formed by sedimentary or tectonic processes (modified from Murawski &amp; Meyer, 1998).</skos:definition>
	<foaf:depiction rdf:resource="https://resource.geosphere.at/img/thes/Rauhwacke.jpg"/>
	<rdf:type rdf:resource="http://www.w3.org/2004/02/skos/core#Concept"/>
	<skos:prefLabel xml:lang="de">Rauwacke</skos:prefLabel>
	<skos:prefLabel xml:lang="en">Rauwacke</skos:prefLabel>
	<skos:broadMatch rdf:resource="http://inspire.ec.europa.eu/codelist/LithologyValue/carbonateSedimentaryRock"/>
	<skos:definition xml:lang="de">Gestein, welches aus zellig-porösem Kalk oder Dolomit besteht. Die Hohlräume sind durch sekundäre Auslaugung von leicht lösbaren Komponenten (Gips/Anhydrit) entstanden. Die primäre Entstehung dieser Gesteine umfasst sowohl sedimentäre als auch tektonische Bildungen. (verändert nach Murawski &amp; Meyer, 1998)</skos:definition>
	<skos:broadMatch rdf:resource="http://resource.geosciml.org/classifier/cgi/lithology/carbonate_sedimentary_rock"/>
	<skos:altLabel xml:lang="de">Rauhwacke</skos:altLabel>
	<skos:altLabel xml:lang="en">Rauhwacke</skos:altLabel>
	<dcterms:hasVersion rdf:datatype="http://www.w3.org/2001/XMLSchema#int">18</dcterms:hasVersion>
	<skos:altLabel xml:lang="de">Zellenkalk</skos:altLabel>
	<dcterms:references rdf:resource="https://resource.geosphere.at/thes/citation/486"/>
	<skos:altLabel xml:lang="de">Rauchwacke</skos:altLabel>
	<skos:altLabel xml:lang="en">Rauchwacke</skos:altLabel>
</rdf:Description>

<rdf:Description rdf:about="https://resource.geosphere.at/thes/lith/161">
	<skos:prefLabel xml:lang="de">Klastisches Sedimentgestein</skos:prefLabel>
	<skos:exactMatch rdf:resource="http://resource.geosciml.org/classifier/cgi/lithology/clastic_sedimentary_rock"/>
	<dcterms:date rdf:datatype="http://www.w3.org/2001/XMLSchema#dateTime">2011-03-22T14:52:39Z</dcterms:date>
	<rdf:type rdf:resource="http://www.w3.org/2004/02/skos/core#Concept"/>
	<dcterms:references rdf:resource="https://resource.geosphere.at/thes/citation/545"/>
	<dcterms:references rdf:resource="https://resource.geosphere.at/thes/citation/547"/>
	<skos:narrower rdf:resource="https://resource.geosphere.at/thes/lith/181"/>
	<skos:narrower rdf:resource="https://resource.geosphere.at/thes/lith/182"/>
	<skos:narrower rdf:resource="https://resource.geosphere.at/thes/lith/183"/>
	<skos:narrower rdf:resource="https://resource.geosphere.at/thes/lith/173"/>
	<skos:narrower rdf:resource="https://resource.geosphere.at/thes/lith/177"/>
	<skos:definition xml:lang="de">Festgestein, welches aus &gt; 50 % klastischen Sedimenten (Fragmente von präexistierenden Gesteinen jeglicher Art, welche vor ihrer Ablagerung durch Wind, Wasser, Eis oder Gravitation transportiert wurden) besteht. Der Begriff beinhaltet karbonatisch-klastische Mischgesteine (verändert nach Neuendorf, 2005; SLTT Appendix C, 2004).</skos:definition>
	<skos:narrower rdf:resource="https://resource.geosphere.at/thes/lith/171"/>
	<skos:narrower rdf:resource="https://resource.geosphere.at/thes/lith/172"/>
	<skos:definition xml:lang="en">A consolidated sedimentary rock consisting of &gt; 50% clastic sediments (fragments of any kind of rock that have been transported by mechanical agents such as wind, water, ice or gravity prior to deposition).The term includes mixed carbonate-clastic sedimentary rocks (modified from Neuendorf et al., 2005; SLTT Appendix C, 2004).</skos:definition>
	<skos:narrower rdf:resource="https://resource.geosphere.at/thes/lith/190"/>
	<skos:narrower rdf:resource="https://resource.geosphere.at/thes/lith/192"/>
	<skos:narrower rdf:resource="https://resource.geosphere.at/thes/lith/194"/>
	<skos:exactMatch rdf:resource="http://inspire.ec.europa.eu/codelist/LithologyValue/clasticSedimentaryRock"/>
	<dcterms:created rdf:datatype="http://www.w3.org/2001/XMLSchema#dateTime">2012-03-12T12:08:25.000Z</dcterms:created>
	<colourHexCode xmlns="http://dbpedia.org/ontology/">#CCB266</colourHexCode>
	<dcterms:hasVersion rdf:datatype="http://www.w3.org/2001/XMLSchema#int">16</dcterms:hasVersion>
	<skos:prefLabel xml:lang="en">Clastic sedimentary rock</skos:prefLabel>
</rdf:Description>

<rdf:Description rdf:about="https://resource.geosphere.at/thes/lith/190">
	<skos:related rdf:resource="https://resource.geosphere.at/thes/lith/230"/>
	<skos:closeMatch rdf:resource="http://resource.geosciml.org/classifier/cgi/lithology/impure_dolostone"/>
	<skos:definition xml:lang="de">Karbonatisch-klastisches Mischgestein, dessen klastischer Anteil sich auf die Tonfraktion beschränkt. Besteht aus 25 bis 75 % Ton und 25-75% Dolomit. Kommt im Vergleich zu kalkigen Mergeln nur untergeordnet vor (Vinx, 2005; Füchtbauer, 1988).</skos:definition>
	<skos:definition xml:lang="en">A mixed carbonate-clastic sedimentary rock in which the clastic portion is restricted to clay-sized components. Dolomitic marl consists of 25-75% clay and 25-75% of dolomite. Dolomitic marlstone is less common than calcareous marlstone (Vinx, 2005; Füchtbauer, 1988).</skos:definition>
	<rdf:type rdf:resource="http://www.w3.org/2004/02/skos/core#Concept"/>
	<dcterms:hasVersion rdf:datatype="http://www.w3.org/2001/XMLSchema#int">13</dcterms:hasVersion>
	<dcterms:date rdf:datatype="http://www.w3.org/2001/XMLSchema#dateTime">2011-03-22T14:52:39Z</dcterms:date>
	<skos:prefLabel xml:lang="en">Dolomitic marlstone</skos:prefLabel>
	<dcterms:references rdf:resource="https://resource.geosphere.at/thes/citation/229"/>
	<dcterms:references rdf:resource="https://resource.geosphere.at/thes/citation/878"/>
	<skos:prefLabel xml:lang="de">Dolomitischer Mergelstein</skos:prefLabel>
	<skos:broadMatch rdf:resource="http://inspire.ec.europa.eu/codelist/LithologyValue/clasticSedimentaryRock"/>
	<dcterms:created rdf:datatype="http://www.w3.org/2001/XMLSchema#dateTime">2012-03-12T14:23:58.000Z</dcterms:created>
	<colourHexCode xmlns="http://dbpedia.org/ontology/">#CCB266</colourHexCode>
</rdf:Description>

<rdf:Description rdf:about="https://resource.geosphere.at/thes/lith/182">
	<skos:relatedMatch rdf:resource="http://dbpedia.org/resource/Fault_breccia"/>
	<skos:related rdf:resource="https://resource.geosphere.at/thes/lith/13"/>
	<skos:related rdf:resource="https://resource.geosphere.at/thes/lith/12"/>
	<skos:altLabel xml:lang="de">Breccie</skos:altLabel>
	<skos:exactMatch rdf:resource="http://dbpedia.org/resource/Breccia"/>
	<skos:exactMatch rdf:resource="http://resource.geosciml.org/classifier/cgi/lithology/breccia"/>
	<colourHexCode xmlns="http://dbpedia.org/ontology/">#F86740</colourHexCode>
	<dcterms:hasVersion rdf:datatype="http://www.w3.org/2001/XMLSchema#int">14</dcterms:hasVersion>
	<dcterms:date rdf:datatype="http://www.w3.org/2001/XMLSchema#dateTime">2011-03-22T14:52:39Z</dcterms:date>
	<skos:prefLabel xml:lang="en">Breccia</skos:prefLabel>
	<dcterms:references rdf:resource="https://resource.geosphere.at/thes/citation/229"/>
	<skos:exactMatch rdf:resource="http://data.bgs.ac.uk/id/EarthMaterialClass/RockName/BREC"/>
	<skos:prefLabel xml:lang="de">Brekzie</skos:prefLabel>
	<rdf:type rdf:resource="http://www.w3.org/2004/02/skos/core#Concept"/>
	<dcterms:created rdf:datatype="http://www.w3.org/2001/XMLSchema#dateTime">2014-09-01T10:33:10.000Z</dcterms:created>
	<skos:definition xml:lang="en">A clastic sedimentary rock that contains &gt; 50% angular mineral and rock fragments with a median grain size &gt; 2mm. A breccia is the solidified equivalent of scree and is usually clast-supported. The matrix can contain sand- or clay-sized particles. The term includes mono- and polymict breccias, i.e. breccias with homogeneous or heterogeneous lithological components (Füchtbauer, 1988; Neuendorf et al., 2005).</skos:definition>
	<skos:exactMatch rdf:resource="http://inspire.ec.europa.eu/codelist/LithologyValue/breccia"/>
	<dcterms:references rdf:resource="https://resource.geosphere.at/thes/citation/545"/>
	<skos:definition xml:lang="de">Klastisches Sedimentgestein, welches zu &gt; 50 % aus nicht gerundeten Mineral- oder Gesteinsbruchstücken von &gt; 2 mm besteht. Stellt das verfestigte Äquivalent von Schutt dar. Die Matrix kann sandig bis tonig sein, zeigt jedoch meist komponentengestütztes Gefüge. Umfasst mono- und polymikte Brekzien, d.s. Brekzien mit lithologisch homogenem oder heterogenem Komponentenbestand (Füchtbauer, 1988; Neuendorf et al., 2005).</skos:definition>
	<skos:related rdf:resource="https://resource.geosphere.at/thes/lith/153"/>
</rdf:Description>

<rdf:Description rdf:about="https://resource.geosphere.at/thes/lith/171">
	<skos:related rdf:resource="https://resource.geosphere.at/thes/lith/172"/>
	<skos:related rdf:resource="https://resource.geosphere.at/thes/lith/213"/>
	<skos:exactMatch rdf:resource="http://data.bgs.ac.uk/id/EarthMaterialClass/RockName/CST"/>
	<skos:definition xml:lang="de">Ungeschichtetes, massiges, klastisches Sedimentgestein mit einer medianen Korngröße &lt; 0.002 mm (Füchtbauer, 1988; DIN 4022).</skos:definition>
	<dcterms:references rdf:resource="https://resource.geosphere.at/thes/citation/78"/>
	<skos:exactMatch rdf:resource="http://inspire.ec.europa.eu/codelist/LithologyValue/claystone"/>
	<dcterms:hasVersion rdf:datatype="http://www.w3.org/2001/XMLSchema#int">10</dcterms:hasVersion>
	<skos:prefLabel xml:lang="en">Claystone</skos:prefLabel>
	<colourHexCode xmlns="http://dbpedia.org/ontology/">#BF996B</colourHexCode>
	<dcterms:references rdf:resource="https://resource.geosphere.at/thes/citation/229"/>
	<skos:exactMatch rdf:resource="http://dbpedia.org/resource/Claystone"/>
	<dcterms:date rdf:datatype="http://www.w3.org/2001/XMLSchema#dateTime">2011-03-22T14:52:39Z</dcterms:date>
	<rdf:type rdf:resource="http://www.w3.org/2004/02/skos/core#Concept"/>
	<skos:definition xml:lang="en">A unbedded, massive, clastic sedimentary rock with a median grain size &lt; 0.002 mm (Füchtbauer; 1988; DIN 4022).</skos:definition>
	<skos:exactMatch rdf:resource="http://resource.geosciml.org/classifier/cgi/lithology/claystone"/>
	<skos:exactMatch rdf:resource="http://www.wikidata.org/entity/Q1932127"/>
	<dcterms:created rdf:datatype="http://www.w3.org/2001/XMLSchema#dateTime">2012-03-12T12:11:27.000Z</dcterms:created>
	<skos:prefLabel xml:lang="de">Tonstein</skos:prefLabel>
</rdf:Description>

<rdf:Description rdf:about="https://resource.geosphere.at/thes/lith/181">
	<rdf:type rdf:resource="http://www.w3.org/2004/02/skos/core#Concept"/>
	<dcterms:hasVersion rdf:datatype="http://www.w3.org/2001/XMLSchema#int">11</dcterms:hasVersion>
	<foaf:depiction rdf:resource="https://resource.geosphere.at/img/thes/Konglomerat.jpg"/>
	<skos:exactMatch rdf:resource="http://www.wikidata.org/entity/Q191704"/>
	<skos:altLabel xml:lang="de">Orthokonglomerat</skos:altLabel>
	<dcterms:references rdf:resource="https://resource.geosphere.at/thes/citation/229"/>
	<dcterms:date rdf:datatype="http://www.w3.org/2001/XMLSchema#dateTime">2011-03-22T14:52:39Z</dcterms:date>
	<skos:definition xml:lang="en">A clastic sedimentary rock that contains &gt; 50% rounded mineral and rock fragments with a median grain size &gt; 2mm (the consolidated equivalent of gravel). The matrix can contain sandy or clay-sized particles but the rock is usually clast-supported. The term includes monomict and polymict conglomerates, i.e. conglomerates with homogeneous or heterogeneous lithological components (Füchtbauer, 1988; Neuendorf et al., 2005).</skos:definition>
	<colourHexCode xmlns="http://dbpedia.org/ontology/">#CCBFA6</colourHexCode>
	<skos:related rdf:resource="https://resource.geosphere.at/thes/lith/222"/>
	<skos:prefLabel xml:lang="de">Konglomerat</skos:prefLabel>
	<dcterms:references rdf:resource="https://resource.geosphere.at/thes/citation/545"/>
	<skos:prefLabel xml:lang="en">Conglomerate</skos:prefLabel>
	<skos:exactMatch rdf:resource="http://data.bgs.ac.uk/id/EarthMaterialClass/RockName/CONG"/>
	<skos:exactMatch rdf:resource="http://inspire.ec.europa.eu/codelist/LithologyValue/conglomerate"/>
	<skos:definition xml:lang="de">Klastisches Sedimentgestein, welches zu &gt; 50 % aus gerundeten Mineral- oder Gesteinsbruchstücken von &gt; 2 mm besteht. Stellt das verfestigte Äquivalent von Kies dar. Die Matrix kann sandig bis tonig sein, zeigt jedoch meist komponentengestütztes Gefüge. Umfasst mono- und polymikte Konglomerate, d.s. Konglomerate mit lithologisch homogenen oder heterogenen Komponenten (Füchtbauer, 1988; Neuendorf et al., 2005).</skos:definition>
	<dcterms:created rdf:datatype="http://www.w3.org/2001/XMLSchema#dateTime">2013-04-05T09:33:32.000Z</dcterms:created>
	<skos:exactMatch rdf:resource="http://resource.geosciml.org/classifier/cgi/lithology/clastic_conglomerate"/>
</rdf:Description>

<rdf:Description rdf:about="https://resource.geosphere.at/thes/lith/192">
	<dcterms:hasVersion rdf:datatype="http://www.w3.org/2001/XMLSchema#int">11</dcterms:hasVersion>
	<dcterms:references rdf:resource="https://resource.geosphere.at/thes/citation/878"/>
	<rdf:type rdf:resource="http://www.w3.org/2004/02/skos/core#Concept"/>
	<dcterms:date rdf:datatype="http://www.w3.org/2001/XMLSchema#dateTime">2011-03-22T14:52:39Z</dcterms:date>
	<dcterms:references rdf:resource="https://resource.geosphere.at/thes/citation/229"/>
	<skos:narrower rdf:resource="https://resource.geosphere.at/thes/lith/191"/>
	<skos:narrower rdf:resource="https://resource.geosphere.at/thes/lith/193"/>
	<skos:prefLabel xml:lang="de">Mergelstein</skos:prefLabel>
	<skos:broadMatch rdf:resource="http://inspire.ec.europa.eu/codelist/LithologyValue/clasticSedimentaryRock"/>
	<skos:closeMatch rdf:resource="http://resource.geosciml.org/classifier/cgi/lithology/impure_carbonate_sedimentary_rock"/>
	<skos:definition xml:lang="de">Karbonatisch-klastisches Mischgestein, dessen klastischer Anteil sich auf die Tonfraktion beschränkt. Besteht aus 25–75 % Ton und 25–75 % Calcit (Vinx, 2005; Füchtbauer, 1988).</skos:definition>
	<skos:prefLabel xml:lang="en">Marlstone</skos:prefLabel>
	<dcterms:created rdf:datatype="http://www.w3.org/2001/XMLSchema#dateTime">2012-03-12T14:21:48.000Z</dcterms:created>
	<skos:related rdf:resource="https://resource.geosphere.at/thes/lith/232"/>
	<skos:definition xml:lang="en">A mixed carbonate-clastic rock in which the clastic portion is restricted to clay-sized components. Marlstone consists of 25-75% clay and 25-75% of calcite (Vinx, 2005; Füchtbauer, 1988).</skos:definition>
	<colourHexCode xmlns="http://dbpedia.org/ontology/">#CCB266</colourHexCode>
</rdf:Description>

<rdf:Description rdf:about="https://resource.geosphere.at/thes/lith/191">
	<skos:prefLabel xml:lang="en">Clay marlstone</skos:prefLabel>
	<skos:closeMatch rdf:resource="http://resource.geosciml.org/classifier/cgi/lithology/impure_carbonate_sedimentary_rock"/>
	<rdf:type rdf:resource="http://www.w3.org/2004/02/skos/core#Concept"/>
	<skos:related rdf:resource="https://resource.geosphere.at/thes/lith/231"/>
	<skos:prefLabel xml:lang="de">Tonmergelstein</skos:prefLabel>
	<skos:definition xml:lang="de">Karbonatisch-klastisches Mischgestein, dessen klastischer Anteil sich auf die Tonfraktion beschränkt. Besteht aus 50–75 % Ton und Calcit (Vinx, 2005; Füchtbauer, 1988).</skos:definition>
	<skos:definition xml:lang="en">A mixed carbonate-clastic rock in which the clastic portion is restricted to clay-sized components. Clay marlstone consists of 50-75% clay and 25-50% calcite (Vinx, 2005; Füchtbauer, 1988).</skos:definition>
	<dcterms:references rdf:resource="https://resource.geosphere.at/thes/citation/878"/>
	<skos:broadMatch rdf:resource="http://inspire.ec.europa.eu/codelist/LithologyValue/clasticSedimentaryRock"/>
	<dcterms:created rdf:datatype="http://www.w3.org/2001/XMLSchema#dateTime">2012-03-12T12:10:03.000Z</dcterms:created>
	<dcterms:hasVersion rdf:datatype="http://www.w3.org/2001/XMLSchema#int">10</dcterms:hasVersion>
	<dcterms:references rdf:resource="https://resource.geosphere.at/thes/citation/229"/>
	<dcterms:date rdf:datatype="http://www.w3.org/2001/XMLSchema#dateTime">2011-03-22T14:52:39Z</dcterms:date>
</rdf:Description>

<rdf:Description rdf:about="https://resource.geosphere.at/thes/lith/193">
	<rdf:type rdf:resource="http://www.w3.org/2004/02/skos/core#Concept"/>
	<dcterms:hasVersion rdf:datatype="http://www.w3.org/2001/XMLSchema#int">11</dcterms:hasVersion>
	<dcterms:references rdf:resource="https://resource.geosphere.at/thes/citation/878"/>
	<skos:broadMatch rdf:resource="http://inspire.ec.europa.eu/codelist/LithologyValue/clasticSedimentaryRock"/>
	<skos:prefLabel xml:lang="de">Kalkmergelstein</skos:prefLabel>
	<skos:closeMatch rdf:resource="http://resource.geosciml.org/classifier/cgi/lithology/impure_carbonate_sedimentary_rock"/>
	<dcterms:references rdf:resource="https://resource.geosphere.at/thes/citation/229"/>
	<dcterms:date rdf:datatype="http://www.w3.org/2001/XMLSchema#dateTime">2011-03-22T14:52:39Z</dcterms:date>
	<skos:definition xml:lang="en">A mixed carbonate-clastic rock in which the clastic portion is restricted to clay-sized components. Consists of 25-50% clay and 50-75% calcite (Vinx, 2005; Füchtbauer, 1988).</skos:definition>
	<skos:related rdf:resource="https://resource.geosphere.at/thes/lith/233"/>
	<dcterms:created rdf:datatype="http://www.w3.org/2001/XMLSchema#dateTime">2012-03-12T10:39:48.000Z</dcterms:created>
	<skos:definition xml:lang="de">Karbonatisch-klastisches Mischgestein, dessen klastischer Anteil sich auf die Tonfraktion beschränkt. Besteht aus 25–50 % Ton und Calcit (Vinx, 2005; Füchtbauer, 1988).</skos:definition>
	<skos:prefLabel xml:lang="en">Calcareous marlstone</skos:prefLabel>
</rdf:Description>

<rdf:Description rdf:about="https://resource.geosphere.at/thes/lith/173">
	<skos:related rdf:resource="https://resource.geosphere.at/thes/lith/214"/>
	<skos:exactMatch rdf:resource="http://www.wikidata.org/entity/Q565731"/>
	<skos:exactMatch rdf:resource="http://inspire.ec.europa.eu/codelist/LithologyValue/siltstone"/>
	<skos:altLabel xml:lang="de">Schluffstein</skos:altLabel>
	<skos:definition xml:lang="de">Klastisches Sedimentgestein mit einer medianen Korngröße &gt; 0.002 mm und ≤ 0.063 mm (Füchtbauer, 1988; DIN 4022).</skos:definition>
	<rdf:type rdf:resource="http://www.w3.org/2004/02/skos/core#Concept"/>
	<skos:narrower rdf:resource="https://resource.geosphere.at/thes/lith/175"/>
	<skos:narrower rdf:resource="https://resource.geosphere.at/thes/lith/174"/>
	<skos:narrower rdf:resource="https://resource.geosphere.at/thes/lith/176"/>
	<skos:definition xml:lang="en">A clastic sedimentary rock with a median grain size between 0.002 and 0.063 mm (Füchtbauer, 1988, DIN 4022).</skos:definition>
	<skos:exactMatch rdf:resource="http://dbpedia.org/resource/Siltstone"/>
	<skos:exactMatch rdf:resource="http://resource.geosciml.org/classifier/cgi/lithology/siltstone"/>
	<skos:prefLabel xml:lang="de">Siltstein</skos:prefLabel>
	<skos:exactMatch rdf:resource="http://data.bgs.ac.uk/id/EarthMaterialClass/RockName/SLST"/>
	<dcterms:references rdf:resource="https://resource.geosphere.at/thes/citation/78"/>
	<dcterms:created rdf:datatype="http://www.w3.org/2001/XMLSchema#dateTime">2012-03-12T16:23:26.000Z</dcterms:created>
	<dcterms:date rdf:datatype="http://www.w3.org/2001/XMLSchema#dateTime">2011-03-22T14:52:39Z</dcterms:date>
	<skos:prefLabel xml:lang="en">Siltstone</skos:prefLabel>
	<colourHexCode xmlns="http://dbpedia.org/ontology/">#CCA680</colourHexCode>
	<dcterms:hasVersion rdf:datatype="http://www.w3.org/2001/XMLSchema#int">12</dcterms:hasVersion>
	<dcterms:references rdf:resource="https://resource.geosphere.at/thes/citation/229"/>
</rdf:Description>

<rdf:Description rdf:about="https://resource.geosphere.at/thes/lith/175">
	<skos:prefLabel xml:lang="de">Mittelsiltstein</skos:prefLabel>
	<skos:altLabel xml:lang="de">Mittelschluffstein</skos:altLabel>
	<skos:definition xml:lang="en">A clastic sedimentary rock with a median grain size between 0.0063 and 0.02 mm (Füchtbauer, 1988; DIN 4022).</skos:definition>
	<skos:exactMatch rdf:resource="http://resource.geosciml.org/classifier/cgi/lithology/siltstone"/>
	<dcterms:references rdf:resource="https://resource.geosphere.at/thes/citation/78"/>
	<dcterms:hasVersion rdf:datatype="http://www.w3.org/2001/XMLSchema#int">13</dcterms:hasVersion>
	<skos:broadMatch rdf:resource="http://inspire.ec.europa.eu/codelist/LithologyValue/siltstone"/>
	<skos:related rdf:resource="https://resource.geosphere.at/thes/lith/216"/>
	<skos:definition xml:lang="de">Klastisches Sedimentgestein mit einer medianen Korngröße &gt; 0.0063 mm und ≤ 0.02 mm (Füchtbauer, 1988; DIN 4022).</skos:definition>
	<dcterms:date rdf:datatype="http://www.w3.org/2001/XMLSchema#dateTime">2011-03-22T14:52:39Z</dcterms:date>
	<dcterms:references rdf:resource="https://resource.geosphere.at/thes/citation/229"/>
	<skos:prefLabel xml:lang="en">Medium siltstone</skos:prefLabel>
	<dcterms:created rdf:datatype="http://www.w3.org/2001/XMLSchema#dateTime">2012-03-12T14:25:35.000Z</dcterms:created>
	<rdf:type rdf:resource="http://www.w3.org/2004/02/skos/core#Concept"/>
</rdf:Description>

<rdf:Description rdf:about="https://resource.geosphere.at/thes/lith/174">
	<dcterms:hasVersion rdf:datatype="http://www.w3.org/2001/XMLSchema#int">13</dcterms:hasVersion>
	<dcterms:references rdf:resource="https://resource.geosphere.at/thes/citation/229"/>
	<dcterms:date rdf:datatype="http://www.w3.org/2001/XMLSchema#dateTime">2011-03-22T14:52:39Z</dcterms:date>
	<skos:broadMatch rdf:resource="http://inspire.ec.europa.eu/codelist/LithologyValue/siltstone"/>
	<skos:broadMatch rdf:resource="http://resource.geosciml.org/classifier/cgi/lithology/siltstone"/>
	<skos:altLabel xml:lang="de">Grobschluffstein</skos:altLabel>
	<skos:prefLabel xml:lang="en">Coarse siltstone</skos:prefLabel>
	<skos:related rdf:resource="https://resource.geosphere.at/thes/lith/215"/>
	<skos:definition xml:lang="de">Klastisches Sedimentgestein mit einer medianen Korngröße &gt; 0.02 mm und ≤ 0.063 mm (Füchtbauer, 1988; DIN 4022).</skos:definition>
	<dcterms:created rdf:datatype="http://www.w3.org/2001/XMLSchema#dateTime">2012-03-12T12:17:19.000Z</dcterms:created>
	<skos:prefLabel xml:lang="de">Grobsiltstein</skos:prefLabel>
	<dcterms:references rdf:resource="https://resource.geosphere.at/thes/citation/78"/>
	<skos:definition xml:lang="en">A clastic sedimentary rock with a median grain size between 0.02 and 0.063 mm (Füchtbauer, 1988; DIN 4022).</skos:definition>
	<rdf:type rdf:resource="http://www.w3.org/2004/02/skos/core#Concept"/>
</rdf:Description>

<rdf:Description rdf:about="https://resource.geosphere.at/thes/lith/176">
	<dcterms:created rdf:datatype="http://www.w3.org/2001/XMLSchema#dateTime">2012-03-12T13:03:33.000Z</dcterms:created>
	<skos:definition xml:lang="en">A clastic sedimentary rock with a median grain size between 0.002 and 0.0063 mm (Füchtbauer, 1988; DIN 4022).</skos:definition>
	<dcterms:references rdf:resource="https://resource.geosphere.at/thes/citation/78"/>
	<skos:prefLabel xml:lang="en">Fine siltstone</skos:prefLabel>
	<dcterms:hasVersion rdf:datatype="http://www.w3.org/2001/XMLSchema#int">13</dcterms:hasVersion>
	<skos:related rdf:resource="https://resource.geosphere.at/thes/lith/217"/>
	<skos:altLabel xml:lang="de">Feinschluffstein</skos:altLabel>
	<skos:broadMatch rdf:resource="http://inspire.ec.europa.eu/codelist/LithologyValue/siltstone"/>
	<rdf:type rdf:resource="http://www.w3.org/2004/02/skos/core#Concept"/>
	<skos:prefLabel xml:lang="de">Feinsiltstein</skos:prefLabel>
	<dcterms:references rdf:resource="https://resource.geosphere.at/thes/citation/229"/>
	<dcterms:date rdf:datatype="http://www.w3.org/2001/XMLSchema#dateTime">2011-03-22T14:52:39Z</dcterms:date>
	<skos:broadMatch rdf:resource="http://resource.geosciml.org/classifier/cgi/lithology/siltstone"/>
	<skos:definition xml:lang="de">Klastisches Sedimentgestein mit einer medianen Korngröße &gt; 0.002 mm und ≤ 0.0063 mm (Füchtbauer, 1988; DIN 4022).</skos:definition>
</rdf:Description>

<rdf:Description rdf:about="https://resource.geosphere.at/thes/lith/183">
	<skos:definition xml:lang="en">A poorly sorted to unsorted clastic sedimentary rock that contains rounded and/or unrounded gravel-sized components that are matrix-supported in silt and clay. Diamictite is the consolidated equivalent of diamicton. The term diamictite is non-genetic but includes genetic terms such as tillite (Neuendorf et al., 2005; Füchtbauer, 1988).</skos:definition>
	<dcterms:references rdf:resource="https://resource.geosphere.at/thes/citation/545"/>
	<skos:prefLabel xml:lang="de">Diamiktit</skos:prefLabel>
	<dcterms:hasVersion rdf:datatype="http://www.w3.org/2001/XMLSchema#int">21</dcterms:hasVersion>
	<skos:exactMatch rdf:resource="http://dbpedia.org/resource/Diamictite"/>
	<skos:exactMatch rdf:resource="http://inspire.ec.europa.eu/codelist/LithologyValue/diamictite"/>
	<skos:related rdf:resource="https://resource.geosphere.at/thes/lith/229"/>
	<skos:exactMatch rdf:resource="http://data.bgs.ac.uk/id/EarthMaterialClass/RockName/DIAMIT"/>
	<dcterms:date rdf:datatype="http://www.w3.org/2001/XMLSchema#dateTime">2011-03-22T14:52:39Z</dcterms:date>
	<rdf:type rdf:resource="http://www.w3.org/2004/02/skos/core#Concept"/>
	<skos:altLabel xml:lang="de">Parakonglomerat</skos:altLabel>
	<foaf:depiction rdf:resource="https://resource.geosphere.at/img/thes/Diamiktit.jpg"/>
	<colourHexCode xmlns="http://dbpedia.org/ontology/">#CCBF8C</colourHexCode>
	<dcterms:references rdf:resource="https://resource.geosphere.at/thes/citation/229"/>
	<skos:definition xml:lang="de">Schlecht sortiertes bis unsortiertes klastisches Sedimentgestein, welches als Komponenten Kies und/oder Schutt enthält und eine siltig-tonige Matrix aufweist. Stellt das verfestigte Äquivalent von Diamikton dar und zeigt ein matrixgestütztes Gefüge. Ist als nicht genetischer Term zu verstehen, der jedoch auch genetisch eindeutige Begriffe wie Tillit umfasst (Neuendorf et al., 2005; Füchtbauer, 1988).</skos:definition>
	<foaf:depiction rdf:resource="http://upload.wikimedia.org/wikipedia/commons/2/20/Geschiebemergel.JPG"/>
	<skos:exactMatch rdf:resource="http://resource.geosciml.org/classifier/cgi/lithology/diamictite"/>
	<skos:prefLabel xml:lang="en">Diamictite</skos:prefLabel>
	<dcterms:created rdf:datatype="http://www.w3.org/2001/XMLSchema#dateTime">2013-06-14T07:09:31.000Z</dcterms:created>
</rdf:Description>

<rdf:Description rdf:about="https://resource.geosphere.at/thes/lith/172">
	<skos:definition xml:lang="en">A bedded clastic sedimentary rock with a median grain size &lt; 0.002 mm (Füchtbauer, 1988; DIN 4022).</skos:definition>
	<colourHexCode xmlns="http://dbpedia.org/ontology/">#D1B08C</colourHexCode>
	<skos:prefLabel xml:lang="en">Shale</skos:prefLabel>
	<skos:exactMatch rdf:resource="http://dbpedia.org/resource/Shale"/>
	<skos:exactMatch rdf:resource="http://www.wikidata.org/entity/Q751300"/>
	<skos:definition xml:lang="de">Geschichtetes klastisches Sedimentgestein mit einer medianen Korngröße &lt; 0.002 mm (Füchtbauer, 1988; DIN 4022).</skos:definition>
	<skos:prefLabel xml:lang="de">Schieferton</skos:prefLabel>
	<skos:exactMatch rdf:resource="http://resource.geosciml.org/classifier/cgi/lithology/shale"/>
	<skos:narrower rdf:resource="https://resource.geosphere.at/thes/lith/252"/>
	<skos:related rdf:resource="https://resource.geosphere.at/thes/lith/213"/>
	<rdf:type rdf:resource="http://www.w3.org/2004/02/skos/core#Concept"/>
	<dcterms:references rdf:resource="https://resource.geosphere.at/thes/citation/78"/>
	<skos:related rdf:resource="https://resource.geosphere.at/thes/lith/137"/>
	<dcterms:created rdf:datatype="http://www.w3.org/2001/XMLSchema#dateTime">2012-03-12T16:22:23.000Z</dcterms:created>
	<dcterms:hasVersion rdf:datatype="http://www.w3.org/2001/XMLSchema#int">12</dcterms:hasVersion>
	<skos:related rdf:resource="https://resource.geosphere.at/thes/lith/171"/>
	<skos:exactMatch rdf:resource="http://inspire.ec.europa.eu/codelist/LithologyValue/shale"/>
	<dcterms:references rdf:resource="https://resource.geosphere.at/thes/citation/229"/>
	<dcterms:date rdf:datatype="http://www.w3.org/2001/XMLSchema#dateTime">2011-03-22T14:52:39Z</dcterms:date>
</rdf:Description>

<rdf:Description rdf:about="https://resource.geosphere.at/thes/lith/252">
	<dcterms:source rdf:resource="https://www.mineralienatlas.de/lexikon/index.php/RockData?lang=de&amp;language=german&amp;rock=Schwarzschiefer"/>
	<status xmlns="https://resource.geosphere.at/schema/thes#" rdf:datatype="http://www.w3.org/2001/XMLSchema#integer">2</status>
	<dcterms:references rdf:resource="https://resource.geosphere.at/thes/citation/229"/>
	<skos:prefLabel xml:lang="de">Schwarzschiefer</skos:prefLabel>
	<skos:prefLabel xml:lang="en">Black shale</skos:prefLabel>
	<skos:scopeNote xml:lang="de">Der Begriff „Schwarzschiefer“ findet meist eine sehr weitläufige Anwendung, als auch kohlenstoffhaltige metamorphe Gesteine wie z. B. graphitführende Schiefer und dunkle Phyllite so bezeichnet werden. Daher wird dieses Konzept mit dem Status „informell“ geführt.</skos:scopeNote>
	<skos:definition xml:lang="de">Schwarzschiefer (engl. black shales) sind dunkle, sehr feingeschichtete Tonsteine mit hohem Gehalt an organischer Substanz (C_org 1-10%). Bei einem Bitumengehalt von mehr als 10% werden derartige Gesteine häufig als „Ölschiefer“ bezeichnet (nach Füchtbauer et. al, 1988: 224, Füchtbauer &amp; Müller, 1977: 257).</skos:definition>
	<dcterms:created rdf:datatype="http://www.w3.org/2001/XMLSchema#dateTime">2015-08-19T11:37:24.000Z</dcterms:created>
	<dcterms:references rdf:resource="https://resource.geosphere.at/thes/citation/545"/>
	<skos:definition xml:lang="en">Black shales are dark, thinly laminated shales exceptionally rich in organic matter (&gt;5% carbon content) and sulfide esp. pyrite and iron sulfide (Neuendorf et al., 2005: 72, Füchtbauer et. al, 1988: 224).</skos:definition>
	<rdf:type rdf:resource="http://www.w3.org/2004/02/skos/core#Concept"/>
	<skos:closeMatch rdf:resource="http://resource.geosciml.org/classifier/cgi/lithology/shale"/>
	<skos:closeMatch rdf:resource="http://inspire.ec.europa.eu/codelist/LithologyValue/shale"/>
	<colourHexCode xmlns="http://dbpedia.org/ontology/">#D1B08C</colourHexCode>
	<skos:broadMatch rdf:resource="http://inspire.ec.europa.eu/codelist/LithologyValue/shale"/>
</rdf:Description>

<rdf:Description rdf:about="https://resource.geosphere.at/thes/lith/194">
	<skos:prefLabel xml:lang="en">Calcareous sandstone</skos:prefLabel>
	<skos:broadMatch rdf:resource="http://inspire.ec.europa.eu/codelist/LithologyValue/clasticSedimentaryRock"/>
	<skos:definition xml:lang="de">Karbonatisch-klastisches Sedimentgestein, dessen klastischer Anteil sich auf die Sandfraktion beschränkt. Besteht aus 25–50 % Calcit und 50–75 % Sand (Füchtbauer, 1988).</skos:definition>
	<dcterms:hasVersion rdf:datatype="http://www.w3.org/2001/XMLSchema#int">8</dcterms:hasVersion>
	<skos:related rdf:resource="https://resource.geosphere.at/thes/lith/195"/>
	<skos:closeMatch rdf:resource="http://resource.geosciml.org/classifier/cgi/lithology/clastic_sandstone"/>
	<skos:exactMatch rdf:resource="http://data.bgs.ac.uk/id/EarthMaterialClass/RockName/CALSST"/>
	<dcterms:date rdf:datatype="http://www.w3.org/2001/XMLSchema#dateTime">2011-03-22T14:52:39Z</dcterms:date>
	<dcterms:references rdf:resource="https://resource.geosphere.at/thes/citation/229"/>
	<skos:prefLabel xml:lang="de">Kalksandstein</skos:prefLabel>
	<rdf:type rdf:resource="http://www.w3.org/2004/02/skos/core#Concept"/>
	<skos:related rdf:resource="https://resource.geosphere.at/thes/lith/234"/>
	<dcterms:created rdf:datatype="http://www.w3.org/2001/XMLSchema#dateTime">2012-03-12T10:41:26.000Z</dcterms:created>
	<skos:definition xml:lang="en">A mixed carbonate-clastic rock in which the clastic portion is restricted to sand-sized components. Consists of 25-50% calcite and 50-75% sand (Füchtbauer, 1988).</skos:definition>
</rdf:Description>

<rdf:Description rdf:about="https://resource.geosphere.at/thes/lith/177">
	<colourHexCode xmlns="http://dbpedia.org/ontology/">#F2D973</colourHexCode>
	<skos:exactMatch rdf:resource="http://data.bgs.ac.uk/id/EarthMaterialClass/RockName/SDST"/>
	<skos:exactMatch rdf:resource="http://dbpedia.org/resource/Sandstone"/>
	<skos:related rdf:resource="https://resource.geosphere.at/thes/lith/218"/>
	<skos:prefLabel xml:lang="en">Sandstone</skos:prefLabel>
	<skos:exactMatch rdf:resource="http://inspire.ec.europa.eu/codelist/LithologyValue/sandstone"/>
	<skos:definition xml:lang="de">Klastisches Sedimentgestein mit einer medianen Korngröße &gt; 0.063 mm und ≤ 2 mm (Füchtbauer, 1988; DIN 4022).</skos:definition>
	<rdf:type rdf:resource="http://www.w3.org/2004/02/skos/core#Concept"/>
	<dcterms:references rdf:resource="https://resource.geosphere.at/thes/citation/78"/>
	<foaf:depiction rdf:resource="https://resource.geosphere.at/img/thes/Sandstein_2.jpg"/>
	<skos:narrower rdf:resource="https://resource.geosphere.at/thes/lith/188"/>
	<skos:narrower rdf:resource="https://resource.geosphere.at/thes/lith/180"/>
	<skos:narrower rdf:resource="https://resource.geosphere.at/thes/lith/184"/>
	<skos:exactMatch rdf:resource="http://www.wikidata.org/entity/Q13085"/>
	<dcterms:hasVersion rdf:datatype="http://www.w3.org/2001/XMLSchema#int">17</dcterms:hasVersion>
	<dcterms:date rdf:datatype="http://www.w3.org/2001/XMLSchema#dateTime">2011-03-22T14:52:39Z</dcterms:date>
	<skos:narrower rdf:resource="https://resource.geosphere.at/thes/lith/179"/>
	<skos:narrower rdf:resource="https://resource.geosphere.at/thes/lith/178"/>
	<dcterms:references rdf:resource="https://resource.geosphere.at/thes/citation/229"/>
	<dcterms:created rdf:datatype="http://www.w3.org/2001/XMLSchema#dateTime">2013-04-05T09:38:52.000Z</dcterms:created>
	<skos:exactMatch rdf:resource="http://resource.geosciml.org/classifier/cgi/lithology/clastic_sandstone"/>
	<skos:definition xml:lang="en">A clastic sedimentary rock with a median grain size between 0.063 and 2 mm (Füchtbauer, 1988; DIN 4022).</skos:definition>
	<skos:prefLabel xml:lang="de">Sandstein</skos:prefLabel>
</rdf:Description>

<rdf:Description rdf:about="https://resource.geosphere.at/thes/lith/179">
	<dcterms:hasVersion rdf:datatype="http://www.w3.org/2001/XMLSchema#int">12</dcterms:hasVersion>
	<dcterms:created rdf:datatype="http://www.w3.org/2001/XMLSchema#dateTime">2012-03-12T14:24:51.000Z</dcterms:created>
	<rdf:type rdf:resource="http://www.w3.org/2004/02/skos/core#Concept"/>
	<dcterms:date rdf:datatype="http://www.w3.org/2001/XMLSchema#dateTime">2011-03-22T14:52:39Z</dcterms:date>
	<dcterms:references rdf:resource="https://resource.geosphere.at/thes/citation/229"/>
	<skos:prefLabel xml:lang="de">Mittelsandstein</skos:prefLabel>
	<skos:prefLabel xml:lang="en">Medium sandstone</skos:prefLabel>
	<skos:definition xml:lang="en">A clastic sedimentary rock with a median grain size between 0.2 and 0.63 mm (Füchtbauer, 1988; DIN 4022).</skos:definition>
	<skos:definition xml:lang="de">Klastisches Sedimentgestein mit einer medianen Korngröße &gt; 0.2 mm und ≤ 0.63 mm (Füchtbauer, 1988; DIN 4022).</skos:definition>
	<skos:broadMatch rdf:resource="http://inspire.ec.europa.eu/codelist/LithologyValue/sandstone"/>
	<skos:broadMatch rdf:resource="http://resource.geosciml.org/classifier/cgi/lithology/arenite"/>
	<dcterms:references rdf:resource="https://resource.geosphere.at/thes/citation/78"/>
	<skos:related rdf:resource="https://resource.geosphere.at/thes/lith/220"/>
</rdf:Description>

<rdf:Description rdf:about="https://resource.geosphere.at/thes/lith/178">
	<skos:prefLabel xml:lang="en">Coarse sandstone</skos:prefLabel>
	<foaf:depiction rdf:resource="https://resource.geosphere.at/img/thes/Grobsandstein.jpg"/>
	<skos:broadMatch rdf:resource="http://resource.geosciml.org/classifier/cgi/lithology/arenite"/>
	<rdf:type rdf:resource="http://www.w3.org/2004/02/skos/core#Concept"/>
	<skos:prefLabel xml:lang="de">Grobsandstein</skos:prefLabel>
	<skos:definition xml:lang="de">Klastisches Sedimentgestein mit einer medianen Korngröße &gt; 0.63 mm und ≤ 2 mm (Füchtbauer, 1988; DIN 4022).</skos:definition>
	<dcterms:references rdf:resource="https://resource.geosphere.at/thes/citation/78"/>
	<skos:broadMatch rdf:resource="http://inspire.ec.europa.eu/codelist/LithologyValue/sandstone"/>
	<dcterms:created rdf:datatype="http://www.w3.org/2001/XMLSchema#dateTime">2013-04-05T09:29:59.000Z</dcterms:created>
	<skos:definition xml:lang="en">A clastic sedimentary rock with a median grain size between 0.63 and 2 mm (Füchtbauer, 1988; DIN 4022).</skos:definition>
	<dcterms:hasVersion rdf:datatype="http://www.w3.org/2001/XMLSchema#int">12</dcterms:hasVersion>
	<skos:related rdf:resource="https://resource.geosphere.at/thes/lith/219"/>
	<dcterms:references rdf:resource="https://resource.geosphere.at/thes/citation/229"/>
	<dcterms:date rdf:datatype="http://www.w3.org/2001/XMLSchema#dateTime">2011-03-22T14:52:39Z</dcterms:date>
</rdf:Description>

<rdf:Description rdf:about="https://resource.geosphere.at/thes/lith/180">
	<dcterms:hasVersion rdf:datatype="http://www.w3.org/2001/XMLSchema#int">12</dcterms:hasVersion>
	<dcterms:created rdf:datatype="http://www.w3.org/2001/XMLSchema#dateTime">2012-03-12T13:02:33.000Z</dcterms:created>
	<skos:definition xml:lang="en">A clastic sedimentary rock with a median grain size between 0.063 and 0.2 mm (Füchtbauer, 1988; DIN 4022).</skos:definition>
	<rdf:type rdf:resource="http://www.w3.org/2004/02/skos/core#Concept"/>
	<dcterms:date rdf:datatype="http://www.w3.org/2001/XMLSchema#dateTime">2011-03-22T14:52:39Z</dcterms:date>
	<dcterms:references rdf:resource="https://resource.geosphere.at/thes/citation/229"/>
	<skos:prefLabel xml:lang="en">Fine sandstone</skos:prefLabel>
	<skos:definition xml:lang="de">Klastisches Sedimentgestein mit einer medianen Korngröße &gt; 0.063 mm und ≤ 0.2 mm (Füchtbauer, 1988; DIN 4022).</skos:definition>
	<skos:broadMatch rdf:resource="http://inspire.ec.europa.eu/codelist/LithologyValue/sandstone"/>
	<skos:broadMatch rdf:resource="http://resource.geosciml.org/classifier/cgi/lithology/arenite"/>
	<skos:prefLabel xml:lang="de">Feinsandstein</skos:prefLabel>
	<dcterms:references rdf:resource="https://resource.geosphere.at/thes/citation/78"/>
	<skos:related rdf:resource="https://resource.geosphere.at/thes/lith/221"/>
</rdf:Description>

<rdf:Description rdf:about="https://resource.geosphere.at/thes/lith/184">
	<colourHexCode xmlns="http://dbpedia.org/ontology/">#F2E080</colourHexCode>
	<skos:exactMatch rdf:resource="http://www.wikidata.org/entity/Q516553"/>
	<dcterms:references rdf:resource="https://resource.geosphere.at/thes/citation/560"/>
	<skos:exactMatch rdf:resource="http://resource.geosciml.org/classifier/cgi/lithology/arenite"/>
	<skos:exactMatch rdf:resource="http://data.bgs.ac.uk/id/EarthMaterialClass/RockName/AREN"/>
	<skos:definition xml:lang="en">A sedimentary rock with sand-sized grains and &lt; 15% matrix material (&lt; 30 µm),. The relative proportions of feldspar, quartz, and lithic fragments are not defined (Pettijohn et al., 1987; Tucker, 2001).</skos:definition>
	<rdf:type rdf:resource="http://www.w3.org/2004/02/skos/core#Concept"/>
	<skos:prefLabel xml:lang="en">Arenite</skos:prefLabel>
	<skos:definition xml:lang="de">Sandstein mit &lt; 15 % Matrix (Komponenten &lt; 30 µm), wobei sich die Sandstein Komponenten aus Feldspat und/oder Quarz und/oder lithischen Fragmenten beliebig zusammensetzen können (Pettijohn et al., 1987; Tucker, 2001).</skos:definition>
	<skos:narrower rdf:resource="https://resource.geosphere.at/thes/lith/186"/>
	<skos:narrower rdf:resource="https://resource.geosphere.at/thes/lith/185"/>
	<skos:narrower rdf:resource="https://resource.geosphere.at/thes/lith/187"/>
	<dcterms:hasVersion rdf:datatype="http://www.w3.org/2001/XMLSchema#int">11</dcterms:hasVersion>
	<skos:exactMatch rdf:resource="http://inspire.ec.europa.eu/codelist/LithologyValue/arenite"/>
	<skos:prefLabel xml:lang="de">Arenit</skos:prefLabel>
	<dcterms:created rdf:datatype="http://www.w3.org/2001/XMLSchema#dateTime">2012-03-12T09:33:32.000Z</dcterms:created>
	<dcterms:references rdf:resource="https://resource.geosphere.at/thes/citation/842"/>
	<dcterms:date rdf:datatype="http://www.w3.org/2001/XMLSchema#dateTime">2011-03-22T14:52:39Z</dcterms:date>
</rdf:Description>

<rdf:Description rdf:about="https://resource.geosphere.at/thes/lith/186">
	<dcterms:references rdf:resource="https://resource.geosphere.at/thes/citation/842"/>
	<dcterms:hasVersion rdf:datatype="http://www.w3.org/2001/XMLSchema#int">11</dcterms:hasVersion>
	<skos:prefLabel xml:lang="de">Arkose</skos:prefLabel>
	<skos:prefLabel xml:lang="en">Arkose</skos:prefLabel>
	<dcterms:date rdf:datatype="http://www.w3.org/2001/XMLSchema#dateTime">2011-03-22T14:52:39Z</dcterms:date>
	<skos:definition xml:lang="de">Arenit mit &gt; 25 % Feldspat und Quarz als Hauptbestandteil. Kann lithische Fragmente führen. Alkalifeldspat ist der dominierende Feldspat. Arkosen leiten sich meist von Graniten und Gneisen ab (Neuendorf et al., 2005; Tucker, 2001).</skos:definition>
	<skos:definition xml:lang="en">An arenite with feldspar (&gt; 25%) and quartz as major constituents. It can also contain lithic fragments. Alkali-feldspar dominates the total feldspar. Most arkoses are derived from granites or gneisses (Neuendorf et al., 2005; Tucker, 2001).</skos:definition>
	<skos:broadMatch rdf:resource="http://inspire.ec.europa.eu/codelist/LithologyValue/arenite"/>
	<skos:closeMatch rdf:resource="http://resource.geosciml.org/classifier/cgi/compositioncategory/arkosic_detrital_mode"/>
	<dcterms:references rdf:resource="https://resource.geosphere.at/thes/citation/545"/>
	<dcterms:created rdf:datatype="http://www.w3.org/2001/XMLSchema#dateTime">2012-03-12T09:34:42.000Z</dcterms:created>
	<skos:related rdf:resource="https://resource.geosphere.at/thes/lith/132"/>
	<skos:exactMatch rdf:resource="http://www.wikidata.org/entity/Q673812"/>
	<rdf:type rdf:resource="http://www.w3.org/2004/02/skos/core#Concept"/>
	<colourHexCode xmlns="http://dbpedia.org/ontology/">#F2E080</colourHexCode>
</rdf:Description>

<rdf:Description rdf:about="https://resource.geosphere.at/thes/lith/185">
	<rdf:type rdf:resource="http://www.w3.org/2004/02/skos/core#Concept"/>
	<skos:broadMatch rdf:resource="http://inspire.ec.europa.eu/codelist/LithologyValue/arenite"/>
	<skos:prefLabel xml:lang="de">Quarz-Arenit</skos:prefLabel>
	<skos:definition xml:lang="de">Ein Arenit mit &gt; 95 % Quarz als Komponenten (Pettijohn et al., 1987; Tucker 2001).</skos:definition>
	<dcterms:references rdf:resource="https://resource.geosphere.at/thes/citation/560"/>
	<dcterms:hasVersion rdf:datatype="http://www.w3.org/2001/XMLSchema#int">9</dcterms:hasVersion>
	<dcterms:created rdf:datatype="http://www.w3.org/2001/XMLSchema#dateTime">2012-03-12T16:03:08.000Z</dcterms:created>
	<skos:definition xml:lang="en">An arenite comprising &gt; 95% quartz grains (Pettijohn et al., 1987; Tucker, 2001).</skos:definition>
	<dcterms:date rdf:datatype="http://www.w3.org/2001/XMLSchema#dateTime">2011-03-22T14:52:39Z</dcterms:date>
	<dcterms:references rdf:resource="https://resource.geosphere.at/thes/citation/842"/>
	<skos:prefLabel xml:lang="en">Quartz arenite</skos:prefLabel>
</rdf:Description>

<rdf:Description rdf:about="https://resource.geosphere.at/thes/lith/187">
	<dcterms:hasVersion rdf:datatype="http://www.w3.org/2001/XMLSchema#int">9</dcterms:hasVersion>
	<skos:definition xml:lang="de">Arenit, der durch &gt; 25 % lithische Fragmente und &lt; 75% Quarz charakterisiert ist. Kann Feldspat führen, wobei die lithischen Fragmente überwiegen. Die Zusammensetzung ist sehr variabel und hängt vom Ausgangsgestein ab (Neuendorf et al., 2005; Tucker, 2001).</skos:definition>
	<skos:broadMatch rdf:resource="http://inspire.ec.europa.eu/codelist/LithologyValue/arenite"/>
	<skos:prefLabel xml:lang="en">Litharenite</skos:prefLabel>
	<skos:prefLabel xml:lang="de">Litharenit</skos:prefLabel>
	<skos:definition xml:lang="en">An arenite that is characterised by &gt; 25% lithic fragments and &lt; 75% quartz. Can contain feldspar but the feldspar components are subordinate to the lithic components. The composition is very variable and dependent on the source material (Neuendorf et al., 2005; Tucker, 2001).</skos:definition>
	<dcterms:date rdf:datatype="http://www.w3.org/2001/XMLSchema#dateTime">2011-03-22T14:52:39Z</dcterms:date>
	<dcterms:references rdf:resource="https://resource.geosphere.at/thes/citation/842"/>
	<dcterms:created rdf:datatype="http://www.w3.org/2001/XMLSchema#dateTime">2012-03-12T14:01:00.000Z</dcterms:created>
	<rdf:type rdf:resource="http://www.w3.org/2004/02/skos/core#Concept"/>
	<dcterms:references rdf:resource="https://resource.geosphere.at/thes/citation/545"/>
</rdf:Description>

<rdf:Description rdf:about="https://resource.geosphere.at/thes/lith/188">
	<dcterms:created rdf:datatype="http://www.w3.org/2001/XMLSchema#dateTime">2012-03-12T16:38:51.000Z</dcterms:created>
	<dcterms:references rdf:resource="https://resource.geosphere.at/thes/citation/560"/>
	<skos:exactMatch rdf:resource="http://inspire.ec.europa.eu/codelist/LithologyValue/wacke"/>
	<dcterms:hasVersion rdf:datatype="http://www.w3.org/2001/XMLSchema#int">9</dcterms:hasVersion>
	<skos:exactMatch rdf:resource="http://resource.geosciml.org/classifier/cgi/lithology/wacke"/>
	<skos:definition xml:lang="en">A sandstone with &gt; 15% matrix material (components &lt; 30 µm). The relative proportions of the different components in the sandstone (feldspar and/or quartz and/or lithic fragments) are variable (Pettijohn et al., 1987; Tucker, 2001).</skos:definition>
	<skos:exactMatch rdf:resource="http://data.bgs.ac.uk/id/EarthMaterialClass/RockName/WACKE"/>
	<rdf:type rdf:resource="http://www.w3.org/2004/02/skos/core#Concept"/>
	<skos:definition xml:lang="de">Sandstein mit &gt; 15 % Matrix (Komponenten &lt; 30 µm), wobei die Komponenten Feldspat und/oder Quarz und/oder lithische Fragmente in beliebigen Mengenverhältnissen auftreten können (Pettijohn et al., 1987; Tucker, 2001).</skos:definition>
	<skos:prefLabel xml:lang="de">Wacke</skos:prefLabel>
	<skos:prefLabel xml:lang="en">Wacke</skos:prefLabel>
	<dcterms:references rdf:resource="https://resource.geosphere.at/thes/citation/842"/>
	<dcterms:date rdf:datatype="http://www.w3.org/2001/XMLSchema#dateTime">2011-03-22T14:52:39Z</dcterms:date>
	<skos:narrower rdf:resource="https://resource.geosphere.at/thes/lith/189"/>
	<colourHexCode xmlns="http://dbpedia.org/ontology/">#F2E691</colourHexCode>
</rdf:Description>

<rdf:Description rdf:about="https://resource.geosphere.at/thes/lith/189">
	<skos:definition xml:lang="en">A dark wacke, often gray or green in colour, that is characterised by a matrix of clay-sized constituents. The matrix typically shows intergrowths of sericite and chlorite and, in addition, quartz and feldspar. The sand-sized components are dominated by quartz, frequent lithic fragments, and variable but subordinate amounts of feldspar (Füchtbauer, 1988; Tucker, 2001).</skos:definition>
	<skos:broadMatch rdf:resource="http://inspire.ec.europa.eu/codelist/LithologyValue/wacke"/>
	<skos:prefLabel xml:lang="de">Grauwacke</skos:prefLabel>
	<skos:definition xml:lang="de">Dunkle, meist graue oder grünliche Wacke, die durch ihre tonige Matrix (&gt; 15 %) charakterisiert ist. Typisch für die Matrix sind Verwachsungen von Serizit und Chlorit und zusätzlich Quarz und Feldspat. Bei den Sandkomponenten überwiegt Quarz gegenüber häufigen lithischen Fragmenten mit wechselndem Feldspatgehalt (Füchtbauer, 1988; Tucker, 2001).</skos:definition>
	<skos:broadMatch rdf:resource="http://resource.geosciml.org/classifier/cgi/lithology/wacke"/>
	<dcterms:hasVersion rdf:datatype="http://www.w3.org/2001/XMLSchema#int">9</dcterms:hasVersion>
	<rdf:type rdf:resource="http://www.w3.org/2004/02/skos/core#Concept"/>
	<dcterms:date rdf:datatype="http://www.w3.org/2001/XMLSchema#dateTime">2011-03-22T14:52:39Z</dcterms:date>
	<dcterms:references rdf:resource="https://resource.geosphere.at/thes/citation/842"/>
	<dcterms:references rdf:resource="https://resource.geosphere.at/thes/citation/229"/>
	<dcterms:created rdf:datatype="http://www.w3.org/2001/XMLSchema#dateTime">2012-03-12T13:42:32.000Z</dcterms:created>
	<skos:prefLabel xml:lang="en">Graywacke</skos:prefLabel>
	<colourHexCode xmlns="http://dbpedia.org/ontology/">#F2E691</colourHexCode>
</rdf:Description>

<rdf:Description rdf:about="https://resource.geosphere.at/thes/lith/164">
	<skos:related rdf:resource="https://resource.geosphere.at/thes/lith/169"/>
	<skos:narrower rdf:resource="https://resource.geosphere.at/thes/lith/205"/>
	<skos:definition xml:lang="de">Sedimentäres Gestein, dessen organischer Anteil hoch genug (≥ 50 % Gewicht im trockenen Zustand) ist, dass es nicht als andersartiges Sedimentgestein identifiziert werden kann. Beinhaltet Kohlenstoff als einen Hauptbestandteil (SLTT Appendix C, 2004; Neuendorf et al., 2005).</skos:definition>
	<dcterms:hasVersion rdf:datatype="http://www.w3.org/2001/XMLSchema#int">13</dcterms:hasVersion>
	<skos:exactMatch rdf:resource="http://resource.geosciml.org/classifier/cgi/lithology/organic_rich_sedimentary_rock"/>
	<skos:prefLabel xml:lang="en">Organic sedimentary rock</skos:prefLabel>
	<skos:exactMatch rdf:resource="http://inspire.ec.europa.eu/codelist/LithologyValue/organicRichSedimentaryRock"/>
	<rdf:type rdf:resource="http://www.w3.org/2004/02/skos/core#Concept"/>
	<skos:prefLabel xml:lang="de">Organisches Sedimentgestein</skos:prefLabel>
	<skos:definition xml:lang="en">A sedimentary rock having a sufficiently high organic content (≥ 50% by weight on a moisture-free basis) to preclude its identification as any other kind of sedimentary rock, and containing carbon as an essential component (SLTT Appendix C, 2004; Neuendorf et al., 2005).</skos:definition>
	<dcterms:date rdf:datatype="http://www.w3.org/2001/XMLSchema#dateTime">2011-03-22T14:52:39Z</dcterms:date>
	<dcterms:created rdf:datatype="http://www.w3.org/2001/XMLSchema#dateTime">2012-03-12T15:51:15.000Z</dcterms:created>
	<dcterms:references rdf:resource="https://resource.geosphere.at/thes/citation/547"/>
	<dcterms:references rdf:resource="https://resource.geosphere.at/thes/citation/545"/>
	<colourHexCode xmlns="http://dbpedia.org/ontology/">#B3B399</colourHexCode>
</rdf:Description>

<rdf:Description rdf:about="https://resource.geosphere.at/thes/lith/205">
	<skos:narrower rdf:resource="https://resource.geosphere.at/thes/lith/207"/>
	<skos:narrower rdf:resource="https://resource.geosphere.at/thes/lith/206"/>
	<skos:exactMatch rdf:resource="http://inspire.ec.europa.eu/codelist/LithologyValue/coal"/>
	<skos:definition xml:lang="en">A readily combustible rock containing &lt; 75% moisture, and &gt; 50% by weight and &gt; 70% vol. of carbonaceous material including inherent water. Coal is formed from various types of plant remains by different degrees of compaction and induration, and categorised as having low, medium or high rank. Sapropelic coals are not distinguished from humic coals under this term (modified from Neuendorf et al., 2005).</skos:definition>
	<dcterms:hasVersion rdf:datatype="http://www.w3.org/2001/XMLSchema#int">11</dcterms:hasVersion>
	<skos:exactMatch rdf:resource="http://resource.geosciml.org/classifier/cgi/lithology/coal"/>
	<skos:prefLabel xml:lang="de">Kohle</skos:prefLabel>
	<skos:exactMatch rdf:resource="http://dbpedia.org/resource/Coal"/>
	<skos:prefLabel xml:lang="en">Coal</skos:prefLabel>
	<skos:exactMatch rdf:resource="http://data.bgs.ac.uk/id/EarthMaterialClass/RockName/COAL"/>
	<colourHexCode xmlns="http://dbpedia.org/ontology/">#B3BFBF</colourHexCode>
	<rdf:type rdf:resource="http://www.w3.org/2004/02/skos/core#Concept"/>
	<dcterms:date rdf:datatype="http://www.w3.org/2001/XMLSchema#dateTime">2011-03-22T14:52:39Z</dcterms:date>
	<dcterms:created rdf:datatype="http://www.w3.org/2001/XMLSchema#dateTime">2012-03-12T12:14:28.000Z</dcterms:created>
	<skos:exactMatch rdf:resource="http://www.wikidata.org/entity/Q24489"/>
	<skos:definition xml:lang="de">Leicht brennbares Gestein, das &lt; 75 % Wassergehalt und &gt; 50 Gew.-% bzw. &gt; 70 Vol.-% kohleartiges Material enthält, inklusive anhaftendes Wasser. Gebildet durch Kompaktion und Induration von verschiedenen Pflanzenresten. Diese Kategorie beinhaltet niedrig- bis hochwertige Kohlen. Sapropelische Kohlen werden in dieser Kategorie nicht von humischen Kohlen unterschieden (verändert nach Neuendorf et al., 2005).</skos:definition>
	<dcterms:references rdf:resource="https://resource.geosphere.at/thes/citation/545"/>
</rdf:Description>

<rdf:Description rdf:about="https://resource.geosphere.at/thes/lith/207">
	<dcterms:created rdf:datatype="http://www.w3.org/2001/XMLSchema#dateTime">2012-03-12T13:46:34.000Z</dcterms:created>
	<rdf:type rdf:resource="http://www.w3.org/2004/02/skos/core#Concept"/>
	<skos:prefLabel xml:lang="de">Steinkohle</skos:prefLabel>
	<skos:definition xml:lang="de">Schwarze, glänzende, harte Kohle mit einem Brennwert &gt; 23.86 MJ/kg. Sie unterscheidet sich von Braunkohle durch höhere Festigkeit, höheren Inkohlungsgrad und Brennwert. Sammelbegriff für alle höherwertigen Kohlen (Neuendorf et al., 2005; Murawski &amp; Meyer, 1998).</skos:definition>
	<skos:definition xml:lang="en">Any black-lustre, hard, coal with a caloric content of &gt; 23.86 MJ/kg on a moist mineral-free basis. Can be distinguished from lignite as black coal has higher degrees of consolidation and coalification, and a higher caloric value. This term includes all medium to high rank coals (Neuendorf et al., 2005; Murawski &amp; Meyer, 1998).</skos:definition>
	<skos:broadMatch rdf:resource="http://inspire.ec.europa.eu/codelist/LithologyValue/coal"/>
	<dcterms:references rdf:resource="https://resource.geosphere.at/thes/citation/545"/>
	<skos:broadMatch rdf:resource="http://resource.geosciml.org/classifier/cgi/lithology/coal"/>
	<dcterms:hasVersion rdf:datatype="http://www.w3.org/2001/XMLSchema#int">10</dcterms:hasVersion>
	<dcterms:references rdf:resource="https://resource.geosphere.at/thes/citation/486"/>
	<skos:prefLabel xml:lang="en">Hard coal</skos:prefLabel>
	<skos:altLabel xml:lang="de">Hartkohle</skos:altLabel>
	<dcterms:date rdf:datatype="http://www.w3.org/2001/XMLSchema#dateTime">2011-03-22T14:52:39Z</dcterms:date>
	<skos:narrower rdf:resource="https://resource.geosphere.at/thes/lith/208"/>
</rdf:Description>

<rdf:Description rdf:about="https://resource.geosphere.at/thes/lith/208">
	<skos:exactMatch rdf:resource="http://data.bgs.ac.uk/id/EarthMaterialClass/RockName/ANTHRA"/>
	<dcterms:date rdf:datatype="http://www.w3.org/2001/XMLSchema#dateTime">2011-03-22T14:52:39Z</dcterms:date>
	<rdf:type rdf:resource="http://www.w3.org/2004/02/skos/core#Concept"/>
	<skos:exactMatch rdf:resource="http://inspire.ec.europa.eu/codelist/LithologyValue/anthraciteCoal"/>
	<skos:definition xml:lang="de">Sehr harte, höchstwertige Kohle mit schwarzem bis semimetallischem Glanz, muscheligem Bruch und einem Gehalt an festem Kohlenstoff von &gt; 91 % (Neuendorf et al., 2005).</skos:definition>
	<skos:exactMatch rdf:resource="http://www.wikidata.org/entity/Q182458"/>
	<colourHexCode xmlns="http://dbpedia.org/ontology/">#BFBFBF</colourHexCode>
	<skos:definition xml:lang="en">The highest rank coal, very hard, glossy, black, with a semi-metallic lustre and semi-conchoidal fracture. It has a fixed carbon content of &gt;91% on a dry, mineral-matter-free basis (Neuendorf et al., 2005).</skos:definition>
	<skos:exactMatch rdf:resource="http://resource.geosciml.org/classifier/cgi/lithology/anthracite_coal"/>
	<skos:prefLabel xml:lang="en">Anthracite</skos:prefLabel>
	<dcterms:references rdf:resource="https://resource.geosphere.at/thes/citation/545"/>
	<dcterms:created rdf:datatype="http://www.w3.org/2001/XMLSchema#dateTime">2012-03-12T09:25:47.000Z</dcterms:created>
	<skos:prefLabel xml:lang="de">Anthrazit</skos:prefLabel>
	<dcterms:hasVersion rdf:datatype="http://www.w3.org/2001/XMLSchema#int">11</dcterms:hasVersion>
</rdf:Description>

<rdf:Description rdf:about="https://resource.geosphere.at/thes/lith/206">
	<dcterms:references rdf:resource="https://resource.geosphere.at/thes/citation/545"/>
	<dcterms:references rdf:resource="https://resource.geosphere.at/thes/citation/547"/>
	<skos:exactMatch rdf:resource="http://data.bgs.ac.uk/id/EarthMaterialClass/RockName/LIGN"/>
	<skos:definition xml:lang="de">Braunes, verfestigtes, organisches, sedimentäres Material, welches einen Brennwert &lt; 19.31 MJ/kg, &lt; 75 % Feuchtigkeit und &lt; 69 % festen Kohlenstoff besitzt (Neuendorf et al., 2005; SLTT Appendix C, 2004).</skos:definition>
	<rdf:type rdf:resource="http://www.w3.org/2004/02/skos/core#Concept"/>
	<skos:exactMatch rdf:resource="http://inspire.ec.europa.eu/codelist/LithologyValue/lignite"/>
	<skos:prefLabel xml:lang="de">Braunkohle</skos:prefLabel>
	<dcterms:date rdf:datatype="http://www.w3.org/2001/XMLSchema#dateTime">2011-03-22T14:52:39Z</dcterms:date>
	<dcterms:hasVersion rdf:datatype="http://www.w3.org/2001/XMLSchema#int">13</dcterms:hasVersion>
	<skos:altLabel xml:lang="en">Brown coal</skos:altLabel>
	<skos:prefLabel xml:lang="en">Lignite</skos:prefLabel>
	<colourHexCode xmlns="http://dbpedia.org/ontology/">#BFB3A6</colourHexCode>
	<dcterms:created rdf:datatype="http://www.w3.org/2001/XMLSchema#dateTime">2012-03-12T13:59:26.000Z</dcterms:created>
	<skos:definition xml:lang="en">A brown, consolidated, organic sedimentary material having a calorific value of &lt; 19.31 MJ/kg on a moist mineral-free basis, with &lt; 75% moisture and &lt; 69% fixed carbon (Neuendorf et al., 2005; SLTT Appendix C, 2004).</skos:definition>
	<skos:exactMatch rdf:resource="http://resource.geosciml.org/classifier/cgi/lithology/lignite"/>
	<skos:altLabel xml:lang="de">Lignit</skos:altLabel>
</rdf:Description>

<rdf:Description rdf:about="https://resource.geosphere.at/thes/lith/3">
	<skos:prefLabel xml:lang="de">Pyroklastisches Gestein</skos:prefLabel>
	<skos:definition xml:lang="en">An igneous rock that contains more than 75% vol. of pyroclasts, i.e. clasts formed by a result of volcanic process. Excludes tuffites (Le Maitre et al. 2005).</skos:definition>
	<skos:exactMatch rdf:resource="http://resource.geosciml.org/classifier/cgi/lithology/pyroclastic_rock"/>
	<colourHexCode xmlns="http://dbpedia.org/ontology/">#A64DBF</colourHexCode>
	<skos:definition xml:lang="de">Magmatisches Gestein dessen Volumen zu mehr als 75% aus Pyroklasten besteht, d.h. Klasten welche von vulkanischen Prozessen geformt werden. Beinhaltet keine Tuffite. (Le Maitre et al. 2005)</skos:definition>
	<dcterms:references rdf:resource="https://resource.geosphere.at/thes/citation/477"/>
	<skos:prefLabel xml:lang="en">Pyroclastic rock</skos:prefLabel>
	<skos:narrower rdf:resource="https://resource.geosphere.at/thes/lith/16"/>
	<dcterms:created rdf:datatype="http://www.w3.org/2001/XMLSchema#dateTime">2012-03-12T16:42:43.000Z</dcterms:created>
	<skos:narrower rdf:resource="https://resource.geosphere.at/thes/lith/13"/>
	<skos:narrower rdf:resource="https://resource.geosphere.at/thes/lith/14"/>
	<skos:narrower rdf:resource="https://resource.geosphere.at/thes/lith/15"/>
	<skos:narrower rdf:resource="https://resource.geosphere.at/thes/lith/11"/>
	<skos:narrower rdf:resource="https://resource.geosphere.at/thes/lith/12"/>
	<rdf:type rdf:resource="http://www.w3.org/2004/02/skos/core#Concept"/>
	<dcterms:hasVersion rdf:datatype="http://www.w3.org/2001/XMLSchema#int">12</dcterms:hasVersion>
	<skos:exactMatch rdf:resource="http://inspire.ec.europa.eu/codelist/LithologyValue/pyroclasticRock"/>
	<dcterms:date rdf:datatype="http://www.w3.org/2001/XMLSchema#dateTime">2011-03-15T15:22:10Z</dcterms:date>
	<skos:exactMatch rdf:resource="http://www.wikidata.org/entity/Q512121"/>
</rdf:Description>

<rdf:Description rdf:about="https://resource.geosphere.at/thes/lith/15">
	<dcterms:hasVersion rdf:datatype="http://www.w3.org/2001/XMLSchema#int">8</dcterms:hasVersion>
	<skos:broadMatch rdf:resource="http://resource.geosciml.org/classifier/cgi/lithology/ash_tuff_lapillistone_and_lapilli_tuff"/>
	<colourHexCode xmlns="http://dbpedia.org/ontology/">#B259CC</colourHexCode>
	<skos:prefLabel xml:lang="en">Lapilli tuff</skos:prefLabel>
	<skos:broadMatch rdf:resource="http://inspire.ec.europa.eu/codelist/LithologyValue/ashTuffLapillistoneAndLapilliTuff"/>
	<dcterms:references rdf:resource="https://resource.geosphere.at/thes/citation/477"/>
	<dcterms:date rdf:datatype="http://www.w3.org/2001/XMLSchema#dateTime">2011-03-15T15:22:10Z</dcterms:date>
	<skos:prefLabel xml:lang="de">Lapillituff</skos:prefLabel>
	<dcterms:created rdf:datatype="http://www.w3.org/2001/XMLSchema#dateTime">2012-03-12T13:55:41.000Z</dcterms:created>
	<rdf:type rdf:resource="http://www.w3.org/2004/02/skos/core#Concept"/>
	<skos:definition xml:lang="de">Pyroklastisches Gestein mit &lt; 25 % Bomben/Blöcken und mehr als 75 % Lapilli und Asche (Le Maitre et al., 2005).</skos:definition>
	<skos:definition xml:lang="en">Pyroclastic rock consisting of less than 25% bombs/blocks and more than 75% lapilli and ash (Le Maitre et al., 2005).</skos:definition>
</rdf:Description>

<rdf:Description rdf:about="https://resource.geosphere.at/thes/lith/16">
	<dcterms:hasVersion rdf:datatype="http://www.w3.org/2001/XMLSchema#int">7</dcterms:hasVersion>
	<skos:altLabel xml:lang="en">Ash tuff</skos:altLabel>
	<skos:prefLabel xml:lang="de">Tuff</skos:prefLabel>
	<skos:prefLabel xml:lang="en">Tuff</skos:prefLabel>
	<skos:definition xml:lang="en">Pyroclastic rock with more than 75% ash (diameter &lt; 2 mm) (Le Maitre et al., 2005).</skos:definition>
	<skos:exactMatch rdf:resource="http://data.bgs.ac.uk/id/EarthMaterialClass/RockName/TUF"/>
	<skos:closeMatch rdf:resource="http://inspire.ec.europa.eu/codelist/LithologyValue/tuffite"/>
	<skos:definition xml:lang="de">Pyroklastisches Gestein mit mehr als 75 % Asche mit Partikeldurchmessern &lt; 2 mm (Le Maitre et al., 2005).</skos:definition>
	<dcterms:date rdf:datatype="http://www.w3.org/2001/XMLSchema#dateTime">2011-03-15T15:22:10Z</dcterms:date>
	<dcterms:references rdf:resource="https://resource.geosphere.at/thes/citation/477"/>
	<rdf:type rdf:resource="http://www.w3.org/2004/02/skos/core#Concept"/>
	<skos:altLabel xml:lang="de">Aschentuff</skos:altLabel>
	<skos:related rdf:resource="https://resource.geosphere.at/thes/lith/10"/>
	<skos:related rdf:resource="https://resource.geosphere.at/thes/lith/17"/>
	<skos:broadMatch rdf:resource="http://resource.geosciml.org/classifier/cgi/lithology/ash_tuff_lapillistone_and_lapilli_tuff"/>
	<skos:exactMatch rdf:resource="http://www.wikidata.org/entity/Q484924"/>
	<dcterms:created rdf:datatype="http://www.w3.org/2001/XMLSchema#dateTime">2012-03-12T16:33:11.000Z</dcterms:created>
	<colourHexCode xmlns="http://dbpedia.org/ontology/">#8033B2</colourHexCode>
</rdf:Description>

<rdf:Description rdf:about="https://resource.geosphere.at/thes/lith/13">
	<dcterms:created rdf:datatype="http://www.w3.org/2001/XMLSchema#dateTime">2012-03-12T16:33:56.000Z</dcterms:created>
	<dcterms:date rdf:datatype="http://www.w3.org/2001/XMLSchema#dateTime">2011-03-15T15:22:10Z</dcterms:date>
	<rdf:type rdf:resource="http://www.w3.org/2004/02/skos/core#Concept"/>
	<skos:broadMatch rdf:resource="http://resource.geosciml.org/classifier/cgi/lithology/tuff_breccia_agglomerate_or_pyroclastic_breccia"/>
	<dcterms:hasVersion rdf:datatype="http://www.w3.org/2001/XMLSchema#int">7</dcterms:hasVersion>
	<colourHexCode xmlns="http://dbpedia.org/ontology/">#BF66D9</colourHexCode>
	<skos:prefLabel xml:lang="de">Tuff Brekzie</skos:prefLabel>
	<skos:broadMatch rdf:resource="http://inspire.ec.europa.eu/codelist/LithologyValue/tuffBrecciaAgglomerateOrPyroclasticBreccia"/>
	<skos:definition xml:lang="en">Pyroclastic rock with bombs/blocks (diameter &gt; 64 mm) in the range of 25-75% (Le Maitre et al., 2005).</skos:definition>
	<skos:related rdf:resource="https://resource.geosphere.at/thes/lith/182"/>
	<skos:definition xml:lang="de">Pyroklastisches Gestein mit Anteilen von Bomben/Blöcken (Durchmesser &gt; 64 mm) im Bereich von 25–75 % (Le Maitre et al., 2005).</skos:definition>
	<skos:prefLabel xml:lang="en">Tuff breccia</skos:prefLabel>
	<dcterms:references rdf:resource="https://resource.geosphere.at/thes/citation/477"/>
</rdf:Description>

<rdf:Description rdf:about="https://resource.geosphere.at/thes/lith/14">
	<skos:definition xml:lang="de">Pyroklastisches Gestein, welches zu mehr als 75 % aus Lapilli (Durchmesser &gt; 2 mm und &lt; 64 mm) besteht (Le Maitre et al., 2005).</skos:definition>
	<dcterms:references rdf:resource="https://resource.geosphere.at/thes/citation/477"/>
	<dcterms:date rdf:datatype="http://www.w3.org/2001/XMLSchema#dateTime">2011-03-15T15:22:10Z</dcterms:date>
	<skos:broadMatch rdf:resource="http://inspire.ec.europa.eu/codelist/LithologyValue/ashTuffLapillistoneAndLapilliTuff"/>
	<skos:exactMatch rdf:resource="http://data.bgs.ac.uk/id/EarthMaterialClass/RockName/LPST"/>
	<skos:definition xml:lang="en">Pyroclastic rock with more than 75% lapilli (diameter between 2 and 64 mm) (Le Maitre et al., 2005).</skos:definition>
	<skos:prefLabel xml:lang="de">Lapillistein</skos:prefLabel>
	<dcterms:hasVersion rdf:datatype="http://www.w3.org/2001/XMLSchema#int">7</dcterms:hasVersion>
	<rdf:type rdf:resource="http://www.w3.org/2004/02/skos/core#Concept"/>
	<skos:broadMatch rdf:resource="http://resource.geosciml.org/classifier/cgi/lithology/ash_tuff_lapillistone_and_lapilli_tuff"/>
	<skos:prefLabel xml:lang="en">Lapillistone</skos:prefLabel>
	<dcterms:created rdf:datatype="http://www.w3.org/2001/XMLSchema#dateTime">2012-03-12T13:56:39.000Z</dcterms:created>
	<skos:related rdf:resource="https://resource.geosphere.at/thes/lith/9"/>
	<colourHexCode xmlns="http://dbpedia.org/ontology/">#B259CC</colourHexCode>
</rdf:Description>

<rdf:Description rdf:about="https://resource.geosphere.at/thes/lith/11">
	<rdf:type rdf:resource="http://www.w3.org/2004/02/skos/core#Concept"/>
	<skos:definition xml:lang="de">Pyroklastisches Gestein mit mehr als 75 % Bomben (Durchmesser &gt; 64 mm) und zumindest teilweise geschmolzen während der Bildung oder des Transports (Le Maitre et al., 2005).</skos:definition>
	<skos:definition xml:lang="en">Agglomerate is a pyroclastic rock comprising &gt; 75% volcanic bombs (diameter &gt; 64 mm), which has been at least partially molten during formation or transport (Le Maitre et al., 2005).</skos:definition>
	<skos:related rdf:resource="https://resource.geosphere.at/thes/lith/8"/>
	<dcterms:references rdf:resource="https://resource.geosphere.at/thes/citation/477"/>
	<dcterms:date rdf:datatype="http://www.w3.org/2001/XMLSchema#dateTime">2011-03-15T15:22:10Z</dcterms:date>
	<skos:broadMatch rdf:resource="http://resource.geosciml.org/classifier/cgi/lithology/tuff_breccia_agglomerate_or_pyroclastic_breccia"/>
	<skos:exactMatch rdf:resource="http://dbpedia.org/resource/Agglomerate"/>
	<dcterms:hasVersion rdf:datatype="http://www.w3.org/2001/XMLSchema#int">10</dcterms:hasVersion>
	<skos:exactMatch rdf:resource="http://data.bgs.ac.uk/id/EarthMaterialClass/RockName/AGG"/>
	<colourHexCode xmlns="http://dbpedia.org/ontology/">#BF66D9</colourHexCode>
	<skos:prefLabel xml:lang="de">Agglomerat</skos:prefLabel>
	<skos:closeMatch rdf:resource="http://inspire.ec.europa.eu/codelist/LithologyValue/tuffBrecciaAgglomerateOrPyroclasticBreccia"/>
	<skos:prefLabel xml:lang="en">Agglomerate</skos:prefLabel>
	<dcterms:created rdf:datatype="http://www.w3.org/2001/XMLSchema#dateTime">2012-03-08T09:30:55.000Z</dcterms:created>
</rdf:Description>

<rdf:Description rdf:about="https://resource.geosphere.at/thes/lith/12">
	<skos:definition xml:lang="de">Pyroklastisches Gestein mit mehr als 75 % Blöcken mit Durchmessern &gt; 64 mm (Le Maitre et al., 2005).</skos:definition>
	<skos:definition xml:lang="en">Pyroclastic rock with more than 75% angular blocks (diameter &gt; 64 mm) (Le Maitre et al., 2005).</skos:definition>
	<rdf:type rdf:resource="http://www.w3.org/2004/02/skos/core#Concept"/>
	<skos:broadMatch rdf:resource="http://resource.geosciml.org/classifier/cgi/lithology/tuff_breccia_agglomerate_or_pyroclastic_breccia"/>
	<skos:related rdf:resource="https://resource.geosphere.at/thes/lith/182"/>
	<colourHexCode xmlns="http://dbpedia.org/ontology/">#BF66D9</colourHexCode>
	<skos:prefLabel xml:lang="en">Pyroclastic breccia</skos:prefLabel>
	<skos:broadMatch rdf:resource="http://inspire.ec.europa.eu/codelist/LithologyValue/tuffBrecciaAgglomerateOrPyroclasticBreccia"/>
	<dcterms:date rdf:datatype="http://www.w3.org/2001/XMLSchema#dateTime">2011-03-15T15:22:10Z</dcterms:date>
	<dcterms:hasVersion rdf:datatype="http://www.w3.org/2001/XMLSchema#int">7</dcterms:hasVersion>
	<dcterms:references rdf:resource="https://resource.geosphere.at/thes/citation/477"/>
	<skos:prefLabel xml:lang="de">Pyroklastische Brekzie</skos:prefLabel>
	<dcterms:created rdf:datatype="http://www.w3.org/2001/XMLSchema#dateTime">2012-03-12T15:59:12.000Z</dcterms:created>
</rdf:Description>

<rdf:Description rdf:about="https://resource.geosphere.at/thes/lith/163">
	<dcterms:created rdf:datatype="http://www.w3.org/2001/XMLSchema#dateTime">2012-03-12T10:27:57.000Z</dcterms:created>
	<skos:prefLabel xml:lang="en">Biochemical-biogenic sedimentary rock</skos:prefLabel>
	<skos:definition xml:lang="en">A sedimentary rock that is formed (directly or indirectly) by the chemical processes and activities of living organisms. Carbonate sedimentary rocks are not included (Neuendorf et al., 2005).</skos:definition>
	<dcterms:hasVersion rdf:datatype="http://www.w3.org/2001/XMLSchema#int">13</dcterms:hasVersion>
	<skos:closeMatch rdf:resource="http://inspire.ec.europa.eu/codelist/LithologyValue/biogenicSilicaSedimentaryRock"/>
	<skos:prefLabel xml:lang="de">Biochemisch-biogenes Sedimentgestein</skos:prefLabel>
	<skos:narrower rdf:resource="https://resource.geosphere.at/thes/lith/204"/>
	<skos:definition xml:lang="de">Sedimentäres Gestein, das durch direkte oder indirekte chemische Prozesse oder Aktivitäten von lebenden Organismen gebildet wird. Karbonatische Sedimentgesteine sind im Konzept nicht inkludiert (Neuendorf et al., 2005).</skos:definition>
	<dcterms:date rdf:datatype="http://www.w3.org/2001/XMLSchema#dateTime">2011-03-22T14:52:39Z</dcterms:date>
	<skos:closeMatch rdf:resource="http://resource.geosciml.org/classifier/cgi/lithology/biogenic_silica_sedimentary_rock"/>
	<rdf:type rdf:resource="http://www.w3.org/2004/02/skos/core#Concept"/>
	<dcterms:references rdf:resource="https://resource.geosphere.at/thes/citation/545"/>
</rdf:Description>

<rdf:Description rdf:about="https://resource.geosphere.at/thes/lith/204">
	<skos:definition xml:lang="de">Mikrokristallines Sedimentgestein, welches überwiegend aus kleinen Quarzkristallen (&lt; 30 µm) besteht. Kann kleine Mengen Verunreinigungen (Eisenoxide, Calcit etc.) und Opal enthalten. Zeigt typischerweise muscheligen Bruch. Kommt in Form von Knollen in Kalksteinen oder Dolomiten oder als lagiges Kieselgestein vor. Der Begriff beinhaltet auch Diatomit und Radiolarit (Neuendorf et al., 2005).</skos:definition>
	<dcterms:references rdf:resource="https://resource.geosphere.at/thes/citation/545"/>
	<skos:altLabel xml:lang="de">Kieslgestein</skos:altLabel>
	<skos:altLabel xml:lang="en">Flint</skos:altLabel>
	<skos:prefLabel xml:lang="de">Hornstein</skos:prefLabel>
	<skos:exactMatch rdf:resource="http://data.bgs.ac.uk/id/EarthMaterialClass/RockName/CHRT"/>
	<dcterms:hasVersion rdf:datatype="http://www.w3.org/2001/XMLSchema#int">10</dcterms:hasVersion>
	<skos:prefLabel xml:lang="en">Chert</skos:prefLabel>
	<skos:definition xml:lang="en">A microcrystalline sedimentary rock consisting predominantly of fine quartz crystals (&lt; 30 µm); it can contain small quantities of impurities (iron oxides, calcite) and opal. Chert usually shows a conchoidal fracture. It occurs as nodules in limestones, dolomites, and chalk, or as bedded chert. The term chert includes diatomite and radiolarite (Neuendorf et al., 2005).</skos:definition>
	<dcterms:date rdf:datatype="http://www.w3.org/2001/XMLSchema#dateTime">2011-03-22T14:52:39Z</dcterms:date>
	<skos:exactMatch rdf:resource="http://resource.geosciml.org/classifier/cgi/lithology/non_clastic_siliceous_sedimentary_rock"/>
	<dcterms:created rdf:datatype="http://www.w3.org/2001/XMLSchema#dateTime">2012-03-12T12:00:27.000Z</dcterms:created>
	<skos:exactMatch rdf:resource="http://inspire.ec.europa.eu/codelist/LithologyValue/nonClasticSiliceousSedimentaryMaterial"/>
	<skos:exactMatch rdf:resource="http://dbpedia.org/resource/Chert"/>
	<skos:related rdf:resource="https://resource.geosphere.at/thes/lith/237"/>
	<skos:narrower rdf:resource="https://resource.geosphere.at/thes/lith/253"/>
	<skos:exactMatch rdf:resource="http://www.wikidata.org/entity/Q1070438"/>
	<rdf:type rdf:resource="http://www.w3.org/2004/02/skos/core#Concept"/>
	<colourHexCode xmlns="http://dbpedia.org/ontology/">#6363EB</colourHexCode>
</rdf:Description>

<rdf:Description rdf:about="https://resource.geosphere.at/thes/lith/253">
	<dcterms:references rdf:resource="https://resource.geosphere.at/thes/citation/1143"/>
	<status xmlns="https://resource.geosphere.at/schema/thes#" rdf:datatype="http://www.w3.org/2001/XMLSchema#integer">1</status>
	<skos:prefLabel xml:lang="de">Radiolarit</skos:prefLabel>
	<skos:exactMatch rdf:resource="http://dbpedia.org/resource/Radiolarite"/>
	<skos:definition xml:lang="en">Radiolarite is a marine chert (sedimentary silica) whose (recognizable) microfossil components mainly consist of the silicious skeletons of radiolaria (single-celled marine microorganisms). (Brandl et al. 2014: 2)</skos:definition>
	<skos:altLabel xml:lang="de">Kieselschiefer</skos:altLabel>
	<skos:definition xml:lang="de">Radiolarit ist ein mariner Hornstein (sedimentäres Kieselgestein), dessen (erkennbare) mikrofossile Komponenten zu einem überwiegenden Teil aus den Kieselskeletten von Radiolarien (einzelligen marinen Mikroorganismen) bestehen. (Brandl et al. 2014: 2)</skos:definition>
	<skos:prefLabel xml:lang="en">Radiolarite</skos:prefLabel>
	<dcterms:created rdf:datatype="http://www.w3.org/2001/XMLSchema#dateTime">2017-01-18T13:37:27.000Z</dcterms:created>
	<rdf:type rdf:resource="http://www.w3.org/2004/02/skos/core#Concept"/>
	<skos:broadMatch rdf:resource="http://inspire.ec.europa.eu/codelist/LithologyValue/biogenicSilicaSedimentaryRock"/>
	<skos:broadMatch rdf:resource="http://resource.geosciml.org/classifier/cgi/lithology/biogenic_silica_sedimentary_rock"/>
	<skos:exactMatch rdf:resource="http://www.wikidata.org/entity/Q379386"/>
	<colourHexCode xmlns="http://dbpedia.org/ontology/">#6363EB</colourHexCode>
</rdf:Description>

<rdf:Description rdf:about="https://resource.geosphere.at/thes/lith/17">
	<skos:related rdf:resource="https://resource.geosphere.at/thes/lith/16"/>
	<skos:prefLabel xml:lang="en">Tuffite</skos:prefLabel>
	<skos:exactMatch rdf:resource="http://www.wikidata.org/entity/Q452064"/>
	<skos:definition xml:lang="en">A rock consisting of a mixture of pyroclastic and normal clastic (epiclastic) material, but with pyroclastic material making up 25-75% of the total by volume. Tuffite can be further classified according to the average grain size of the clasts (Le Maitre et al., 2005).</skos:definition>
	<skos:exactMatch rdf:resource="http://resource.geosciml.org/classifier/cgi/lithology/tuffite"/>
	<colourHexCode xmlns="http://dbpedia.org/ontology/">#8033B2</colourHexCode>
	<dcterms:date rdf:datatype="http://www.w3.org/2001/XMLSchema#dateTime">2011-03-15T15:22:10Z</dcterms:date>
	<skos:exactMatch rdf:resource="http://dbpedia.org/resource/Tuffite"/>
	<dcterms:references rdf:resource="https://resource.geosphere.at/thes/citation/477"/>
	<skos:prefLabel xml:lang="de">Tuffit</skos:prefLabel>
	<skos:exactMatch rdf:resource="http://data.bgs.ac.uk/id/EarthMaterialClass/RockName/TUFT"/>
	<dcterms:created rdf:datatype="http://www.w3.org/2001/XMLSchema#dateTime">2012-03-12T16:34:45.000Z</dcterms:created>
	<skos:definition xml:lang="de">Gestein, welches aus einer Mischung von pyroklastischem und normal klastischem (epiklastischem) Material besteht. Die Menge an pyroklastischem Material liegt im Bereich von 25–75 %. Tuffite können anhand der durchschnittlichen Korngröße der Klasten weiter untergliedert werden (Le Maitre et al., 2005).</skos:definition>
	<skos:exactMatch rdf:resource="http://inspire.ec.europa.eu/codelist/LithologyValue/tuffite"/>
	<rdf:type rdf:resource="http://www.w3.org/2004/02/skos/core#Concept"/>
	<dcterms:hasVersion rdf:datatype="http://www.w3.org/2001/XMLSchema#int">9</dcterms:hasVersion>
</rdf:Description>

<rdf:Description rdf:about="https://resource.geosphere.at/thes/lith/165">
	<skos:definition xml:lang="de">Sedimentäres Gestein, das hauptsächlich aus Material besteht, welches durch Fällung aus einer Lösung oder einer kolloidalen Suspension (Evaporation) oder durch Ablagerung von unlöslichen Abscheidungsprodukten (Mischung von unlöslichen Salzen) entstanden ist.(SLTT Appendix C, 2004)</skos:definition>
	<skos:prefLabel xml:lang="en">Chemical sedimentary rock</skos:prefLabel>
	<dcterms:references rdf:resource="https://resource.geosphere.at/thes/citation/547"/>
	<skos:definition xml:lang="en">A sedimentary rock composed primarily of material formed directly by precipitation from solution or colloidal suspension (evaporation), or by deposition of insoluble precipitates (mixing of insoluble salts). (SLTT Appendix C, 2004)</skos:definition>
	<rdf:type rdf:resource="http://www.w3.org/2004/02/skos/core#Concept"/>
	<skos:closeMatch rdf:resource="http://inspire.ec.europa.eu/codelist/LithologyValue/chemicalSedimentaryMaterial"/>
	<dcterms:hasVersion rdf:datatype="http://www.w3.org/2001/XMLSchema#int">12</dcterms:hasVersion>
	<dcterms:date rdf:datatype="http://www.w3.org/2001/XMLSchema#dateTime">2011-03-22T14:52:39Z</dcterms:date>
	<dcterms:created rdf:datatype="http://www.w3.org/2001/XMLSchema#dateTime">2012-03-12T11:59:39.000Z</dcterms:created>
	<skos:prefLabel xml:lang="de">Chemisches Sedimentgestein</skos:prefLabel>
	<skos:closeMatch rdf:resource="http://resource.geosciml.org/classifier/cgi/lithology/chemical_sedimentary_material"/>
</rdf:Description>

<rdf:Description rdf:about="https://resource.geosphere.at/thes/lith/160">
	<skos:definition xml:lang="de">Aus festen Bruchstücken bestehendes Material, welches durch Verwitterung von Gesteinen entsteht und durch Luft, Wasser, Eis, Wind transportiert und/oder abgelagert wird. Oder Material, welches durch natürliche Ursachen wie chemische Fällung aus Lösung bzw. Abscheidung durch Organismen entsteht. Bildet sich in Form von lockeren, unkonsolidierten Lagen und Körpern an der Erdoberfläche (Neuendorf et al., 2005).</skos:definition>
	<dcterms:references rdf:resource="https://resource.geosphere.at/thes/citation/545"/>
	<skos:exactMatch rdf:resource="http://data.bgs.ac.uk/id/EarthMaterialClass/RockName/SED"/>
	<skos:related rdf:resource="https://resource.geosphere.at/thes/lith/159"/>
	<skos:exactMatch rdf:resource="http://dbpedia.org/resource/Sediment"/>
	<rdf:type rdf:resource="http://www.w3.org/2004/02/skos/core#Concept"/>
	<skos:prefLabel xml:lang="de">Sediment</skos:prefLabel>
	<skos:prefLabel xml:lang="en">Sediment</skos:prefLabel>
	<colourHexCode xmlns="http://dbpedia.org/ontology/">#FFFF80</colourHexCode>
	<skos:narrower rdf:resource="https://resource.geosphere.at/thes/lith/166"/>
	<skos:narrower rdf:resource="https://resource.geosphere.at/thes/lith/167"/>
	<skos:narrower rdf:resource="https://resource.geosphere.at/thes/lith/168"/>
	<skos:narrower rdf:resource="https://resource.geosphere.at/thes/lith/169"/>
	<dcterms:hasVersion rdf:datatype="http://www.w3.org/2001/XMLSchema#int">9</dcterms:hasVersion>
	<skos:definition xml:lang="en">Solid fragmental material that originates from the weathering of rocks and is transported or deposited by air/water/ice, or accumulates by other natural agents such as chemical precipitation from solution or secretion by organisms. Forms in layers on the Earth's surface, in a loose or unconsolidated form (Neuendorf et al., 2005).</skos:definition>
	<skos:exactMatch rdf:resource="http://inspire.ec.europa.eu/codelist/LithologyValue/sediment"/>
	<foaf:depiction rdf:resource="https://resource.geosphere.at/img/thes/Sediment.jpg"/>
	<dcterms:created rdf:datatype="http://www.w3.org/2001/XMLSchema#dateTime">2013-04-05T09:39:36.000Z</dcterms:created>
	<dcterms:date rdf:datatype="http://www.w3.org/2001/XMLSchema#dateTime">2011-03-22T14:52:39Z</dcterms:date>
	<skos:exactMatch rdf:resource="http://resource.geosciml.org/classifier/cgi/lithology/sediment"/>
</rdf:Description>

<rdf:Description rdf:about="https://resource.geosphere.at/thes/lith/168">
	<skos:closeMatch rdf:resource="http://resource.geosciml.org/classifier/cgi/lithology/biogenic_sediment"/>
	<skos:closeMatch rdf:resource="http://inspire.ec.europa.eu/codelist/LithologyValue/biogenicSediment"/>
	<dcterms:hasVersion rdf:datatype="http://www.w3.org/2001/XMLSchema#int">15</dcterms:hasVersion>
	<skos:definition xml:lang="de">Sediment, das durch direkte oder indirekte chemische Prozesse oder Aktivitäten von lebenden Organismen gebildet wird. Karbonatische Sedimente sind im Konzept nicht inkludiert (Neuendorf et al., 2005).</skos:definition>
	<skos:definition xml:lang="en">A sediment that is formed (directly or indirectly) by the chemical processes and activities of living organisms. Carbonate sediments are not included (Neuendorf et al., 2005).</skos:definition>
	<colourHexCode xmlns="http://dbpedia.org/ontology/">#D9CC80</colourHexCode>
	<dcterms:date rdf:datatype="http://www.w3.org/2001/XMLSchema#dateTime">2011-03-22T14:52:39Z</dcterms:date>
	<skos:prefLabel xml:lang="de">Chemisches und biochemisches Sediment</skos:prefLabel>
	<dcterms:created rdf:datatype="http://www.w3.org/2001/XMLSchema#dateTime">2012-03-12T10:26:44.000Z</dcterms:created>
	<dcterms:references rdf:resource="https://resource.geosphere.at/thes/citation/545"/>
	<rdf:type rdf:resource="http://www.w3.org/2004/02/skos/core#Concept"/>
</rdf:Description>

<rdf:Description rdf:about="https://resource.geosphere.at/thes/lith/237">
	<dcterms:date rdf:datatype="http://www.w3.org/2001/XMLSchema#dateTime">2011-03-22T14:52:39Z</dcterms:date>
	<dcterms:references rdf:resource="https://resource.geosphere.at/thes/citation/545"/>
	<skos:definition xml:lang="en">A marine sediment consisting of &gt; 30% skeletal remains of pelagic siliceous organisms (such as radiolarians or diatoms) and clay minerals (Neuendorf et al. 2005).</skos:definition>
	<skos:definition xml:lang="de">Ein marines Sediment aus &gt; 30% Skelettresten von silikatischen pelagischen Organismen (wie Radiolarien und Diatomeen) und Tonmineralen (Neuendorf et al. 2005).</skos:definition>
	<rdf:type rdf:resource="http://www.w3.org/2004/02/skos/core#Concept"/>
	<skos:exactMatch rdf:resource="http://inspire.ec.europa.eu/codelist/LithologyValue/siliceousOoze"/>
	<dcterms:hasVersion rdf:datatype="http://www.w3.org/2001/XMLSchema#int">8</dcterms:hasVersion>
	<skos:exactMatch rdf:resource="http://resource.geosciml.org/classifier/cgi/lithology/siliceous_ooze"/>
	<colourHexCode xmlns="http://dbpedia.org/ontology/">#EDE0B2</colourHexCode>
	<skos:related rdf:resource="https://resource.geosphere.at/thes/lith/204"/>
	<dcterms:created rdf:datatype="http://www.w3.org/2001/XMLSchema#dateTime">2012-03-12T16:22:57.000Z</dcterms:created>
</rdf:Description>

<rdf:Description rdf:about="https://resource.geosphere.at/thes/lith/167">
	<dcterms:hasVersion rdf:datatype="http://www.w3.org/2001/XMLSchema#int">13</dcterms:hasVersion>
	<skos:related rdf:resource="https://resource.geosphere.at/thes/lith/162"/>
	<rdf:type rdf:resource="http://www.w3.org/2004/02/skos/core#Concept"/>
	<skos:exactMatch rdf:resource="http://resource.geosciml.org/classifier/cgi/lithology/carbonate_sediment"/>
	<dcterms:date rdf:datatype="http://www.w3.org/2001/XMLSchema#dateTime">2011-03-22T14:52:39Z</dcterms:date>
	<skos:prefLabel xml:lang="de">Karbonatisches Sediment</skos:prefLabel>
	<skos:prefLabel xml:lang="en">Carbonate sediment</skos:prefLabel>
	<skos:definition xml:lang="de">Ein Sediment mit ≥ 50% primären und/oder rekristallisierten Bestandteilen aus Karbonatmineralen (Calcit/Aragonit/Dolomit). Diese Materialien leiten sich aus Prozessen ab die innerhalb eines Ablagerungsregimes (innerhalb eines Beckens) wirken und nicht durch Transport in das Ablagerungsregime aus anderen Sedimentquellen kommt (SLTT Appendix C, 2004).</skos:definition>
	<skos:exactMatch rdf:resource="http://inspire.ec.europa.eu/codelist/LithologyValue/carbonateSediment"/>
	<colourHexCode xmlns="http://dbpedia.org/ontology/">#0DB3C9</colourHexCode>
	<skos:definition xml:lang="en">A sediment in which ≥ 50% of the primary and (or) re-crystallized constituents are composed of carbonate minerals (calcite/aragonite/dolomite). Such materials are intra-basinal in origin - that is, they formed by processes operating within a depositional regime, and were not transported into that regime from other sediment sources (SLTT Appendix C, 2004).</skos:definition>
	<dcterms:references rdf:resource="https://resource.geosphere.at/thes/citation/547"/>
	<dcterms:created rdf:datatype="http://www.w3.org/2001/XMLSchema#dateTime">2012-03-12T10:52:20.000Z</dcterms:created>
	<skos:narrower rdf:resource="https://resource.geosphere.at/thes/lith/235"/>
	<skos:narrower rdf:resource="https://resource.geosphere.at/thes/lith/236"/>
</rdf:Description>

<rdf:Description rdf:about="https://resource.geosphere.at/thes/lith/236">
	<skos:definition xml:lang="de">Marines Sediment aus &gt; 30 % Skelettresten von karbonatischen, pelagischen Organismen (wie Foraminiferen, Pteropoda oder Coccolithophorida) und Tonmineralen (Neuendorf et al., 2005).</skos:definition>
	<skos:definition xml:lang="en">A marine sediment consisting of &gt; 30% skeletal remains of pelagic calcareous organisms (such as foraminifera, pteropods or cocolithophorids) and clay minerals (Neuendorf et al., 2005).</skos:definition>
	<dcterms:references rdf:resource="https://resource.geosphere.at/thes/citation/545"/>
	<skos:prefLabel xml:lang="en">Calcareous ooze</skos:prefLabel>
	<dcterms:hasVersion rdf:datatype="http://www.w3.org/2001/XMLSchema#int">7</dcterms:hasVersion>
	<skos:exactMatch rdf:resource="http://resource.geosciml.org/classifier/cgi/lithology/carbonate_ooze"/>
	<skos:exactMatch rdf:resource="http://inspire.ec.europa.eu/codelist/LithologyValue/ooze"/>
	<dcterms:date rdf:datatype="http://www.w3.org/2001/XMLSchema#dateTime">2011-03-22T14:52:39Z</dcterms:date>
	<dcterms:created rdf:datatype="http://www.w3.org/2001/XMLSchema#dateTime">2012-01-25T15:17:18.000Z</dcterms:created>
	<rdf:type rdf:resource="http://www.w3.org/2004/02/skos/core#Concept"/>
	<skos:prefLabel xml:lang="de">Kalkschlamm</skos:prefLabel>
	<skos:related rdf:resource="https://resource.geosphere.at/thes/lith/196"/>
	<colourHexCode xmlns="http://dbpedia.org/ontology/">#E6D9A6</colourHexCode>
</rdf:Description>

<rdf:Description rdf:about="https://resource.geosphere.at/thes/lith/235">
	<skos:prefLabel xml:lang="de">Sandkalk</skos:prefLabel>
	<skos:closeMatch rdf:resource="http://resource.geosciml.org/classifier/cgi/lithology/carbonate_sedimentary_material"/>
	<skos:prefLabel xml:lang="en">Sandy Lime</skos:prefLabel>
	<skos:related rdf:resource="https://resource.geosphere.at/thes/lith/195"/>
	<dcterms:date rdf:datatype="http://www.w3.org/2001/XMLSchema#dateTime">2011-03-22T14:52:39Z</dcterms:date>
	<dcterms:hasVersion rdf:datatype="http://www.w3.org/2001/XMLSchema#int">11</dcterms:hasVersion>
	<skos:closeMatch rdf:resource="http://inspire.ec.europa.eu/codelist/LithologyValue/carbonateSedimentaryMaterial"/>
	<dcterms:references rdf:resource="https://resource.geosphere.at/thes/citation/229"/>
	<rdf:type rdf:resource="http://www.w3.org/2004/02/skos/core#Concept"/>
	<skos:related rdf:resource="https://resource.geosphere.at/thes/lith/234"/>
	<skos:definition xml:lang="de">Karbonatisch-klastisches Sediment, dessen klastischer Anteil sich auf die Sandfraktion beschränkt. Besteht aus 50–75 % Calcit und 25–50 % Sand (Füchtbauer, 1988).</skos:definition>
	<dcterms:created rdf:datatype="http://www.w3.org/2001/XMLSchema#dateTime">2012-03-12T16:14:43.000Z</dcterms:created>
	<skos:definition xml:lang="en">A mixed carbonate-clastic sediment in which the clastic portion is restricted to sand-sized components. Consists of 50-75% calcite and 25-50% sand (Füchtbauer, 1988).</skos:definition>
</rdf:Description>

<rdf:Description rdf:about="https://resource.geosphere.at/thes/lith/169">
	<skos:closeMatch rdf:resource="http://inspire.ec.europa.eu/codelist/LithologyValue/organicRichSedimentaryMaterial"/>
	<dcterms:hasVersion rdf:datatype="http://www.w3.org/2001/XMLSchema#int">16</dcterms:hasVersion>
	<dcterms:date rdf:datatype="http://www.w3.org/2001/XMLSchema#dateTime">2011-03-22T14:52:39Z</dcterms:date>
	<skos:narrower rdf:resource="https://resource.geosphere.at/thes/lith/239"/>
	<skos:narrower rdf:resource="https://resource.geosphere.at/thes/lith/238"/>
	<skos:closeMatch rdf:resource="http://resource.geosciml.org/classifier/cgi/lithology/organic_rich_sedimentary_material"/>
	<dcterms:created rdf:datatype="http://www.w3.org/2001/XMLSchema#dateTime">2012-03-12T15:51:04.000Z</dcterms:created>
	<rdf:type rdf:resource="http://www.w3.org/2004/02/skos/core#Concept"/>
	<skos:related rdf:resource="https://resource.geosphere.at/thes/lith/164"/>
	<colourHexCode xmlns="http://dbpedia.org/ontology/">#42413C</colourHexCode>
</rdf:Description>

<rdf:Description rdf:about="https://resource.geosphere.at/thes/lith/238">
	<skos:exactMatch rdf:resource="http://inspire.ec.europa.eu/codelist/LithologyValue/peat"/>
	<skos:definition xml:lang="de">Unverfestigte Ablagerung aus Pflanzenresten mit hohem Wasseranteil (≥ 75 %). Der Kohlenstoffanteil beträgt rund 60 % und der Sauerstoffanteil liegt bei 30 % im trockenen Zustand. Wird durch Inkohlung zu Braunkohle (Neuendorf et al., 2005; Tucker, 2001).</skos:definition>
	<rdf:type rdf:resource="http://www.w3.org/2004/02/skos/core#Concept"/>
	<skos:exactMatch rdf:resource="http://resource.geosciml.org/classifier/cgi/lithology/peat"/>
	<colourHexCode xmlns="http://dbpedia.org/ontology/">#E6D994</colourHexCode>
	<skos:definition xml:lang="en">An unconsolidated deposit of plant remains with a high water content (≥ 75%), a fixed carbon content of about 60%, and an oxygen content of about 30% (on a moist mineral free basis). Forms lignite during coalification (Neuendorf et al., 2005; Tucker, 2001).</skos:definition>
	<skos:prefLabel xml:lang="en">Peat</skos:prefLabel>
	<dcterms:references rdf:resource="https://resource.geosphere.at/thes/citation/545"/>
	<skos:exactMatch rdf:resource="http://dbpedia.org/resource/Peat"/>
	<skos:exactMatch rdf:resource="http://www.wikidata.org/entity/Q184624"/>
	<skos:exactMatch rdf:resource="http://data.bgs.ac.uk/id/EarthMaterialClass/RockName/PEAT"/>
	<skos:prefLabel xml:lang="de">Torf</skos:prefLabel>
	<dcterms:created rdf:datatype="http://www.w3.org/2001/XMLSchema#dateTime">2012-03-12T15:53:20.000Z</dcterms:created>
	<dcterms:date rdf:datatype="http://www.w3.org/2001/XMLSchema#dateTime">2011-03-22T14:52:39Z</dcterms:date>
	<dcterms:hasVersion rdf:datatype="http://www.w3.org/2001/XMLSchema#int">11</dcterms:hasVersion>
	<dcterms:references rdf:resource="https://resource.geosphere.at/thes/citation/842"/>
</rdf:Description>

<rdf:Description rdf:about="https://resource.geosphere.at/thes/lith/239">
	<skos:exactMatch rdf:resource="http://dbpedia.org/resource/Sapropel"/>
	<skos:exactMatch rdf:resource="http://resource.geosciml.org/classifier/cgi/lithology/sapropel"/>
	<skos:definition xml:lang="de">Unverfestigter, gallertiger Schlamm, der sich aus Pflanzenresten zusammensetzt (meistens Algen) und unter anaeroben Bedingungen verfault. Gebildet am Meeresgrund bzw. am Grund von Seen (Neuendorf et al., 2005).</skos:definition>
	<dcterms:date rdf:datatype="http://www.w3.org/2001/XMLSchema#dateTime">2011-03-22T14:52:39Z</dcterms:date>
	<skos:exactMatch rdf:resource="http://inspire.ec.europa.eu/codelist/LithologyValue/sapropel"/>
	<colourHexCode xmlns="http://dbpedia.org/ontology/">#EBDE9E</colourHexCode>
	<skos:definition xml:lang="en">An unconsolidated jelly-like ooze composed of plant remains (most often algae), putrefying under anaerobic conditions on the shallow lake and sea floor (Neuendorf et al., 2005).</skos:definition>
	<skos:altLabel xml:lang="de">Faulschlamm</skos:altLabel>
	<dcterms:created rdf:datatype="http://www.w3.org/2001/XMLSchema#dateTime">2012-03-12T16:16:26.000Z</dcterms:created>
	<dcterms:references rdf:resource="https://resource.geosphere.at/thes/citation/545"/>
	<skos:prefLabel xml:lang="de">Sapropel</skos:prefLabel>
	<skos:prefLabel xml:lang="en">Sapropel</skos:prefLabel>
	<rdf:type rdf:resource="http://www.w3.org/2004/02/skos/core#Concept"/>
	<dcterms:hasVersion rdf:datatype="http://www.w3.org/2001/XMLSchema#int">9</dcterms:hasVersion>
</rdf:Description>

<rdf:Description rdf:about="https://resource.geosphere.at/thes/lith/170">
	<colourHexCode xmlns="http://dbpedia.org/ontology/">#99CCE6</colourHexCode>
	<skos:prefLabel xml:lang="en">Chemical sediment</skos:prefLabel>
	<dcterms:date rdf:datatype="http://www.w3.org/2001/XMLSchema#dateTime">2011-03-22T14:52:39Z</dcterms:date>
	<dcterms:hasVersion rdf:datatype="http://www.w3.org/2001/XMLSchema#int">11</dcterms:hasVersion>
	<skos:closeMatch rdf:resource="http://inspire.ec.europa.eu/codelist/LithologyValue/chemicalSedimentaryMaterial"/>
	<skos:definition xml:lang="en">A sediment composed primarily of material formed directly by precipitation from solution or colloidal suspension (evaporation), or by deposition of insoluble precipitates (mixing of insoluble salts). (Neuendorf et al., 2005)</skos:definition>
	<skos:prefLabel xml:lang="de">Chemisches Sediment</skos:prefLabel>
	<dcterms:created rdf:datatype="http://www.w3.org/2001/XMLSchema#dateTime">2012-03-12T11:58:51.000Z</dcterms:created>
	<rdf:type rdf:resource="http://www.w3.org/2004/02/skos/core#Concept"/>
	<dcterms:references rdf:resource="https://resource.geosphere.at/thes/citation/545"/>
	<skos:closeMatch rdf:resource="http://resource.geosciml.org/classifier/cgi/lithology/chemical_sedimentary_material"/>
	<skos:definition xml:lang="de">Sediment, das hauptsächlich aus Material besteht, welches durch Fällung aus einer Lösung oder einer kolloidalen Suspension (Evaporation) oder durch Ablagerung von unlöslichen Abscheidungsprodukten (Mischung von unlöslichen Salzen) entstanden ist. (Neuendorf et al., 2005)</skos:definition>
</rdf:Description>

<rdf:Description rdf:about="https://resource.geosphere.at/thes/lith/209">
	<skos:exactMatch rdf:resource="http://resource.geosciml.org/classifier/cgi/lithology/evaporite"/>
	<rdf:type rdf:resource="http://www.w3.org/2004/02/skos/core#Concept"/>
	<colourHexCode xmlns="http://dbpedia.org/ontology/">#99CCE6</colourHexCode>
	<dcterms:hasVersion rdf:datatype="http://www.w3.org/2001/XMLSchema#int">14</dcterms:hasVersion>
	<skos:exactMatch rdf:resource="http://inspire.ec.europa.eu/codelist/LithologyValue/evaporite"/>
	<skos:definition xml:lang="en">A chemical sedimentary rock containing &gt; 50% non-carbonate salts, which can include chlorite, sulphate, or borate minerals. Usually formed from a saline solution by precipitation due to vaporization of the solvent (Neuendorf et al., 2005; SLTT Appendix C, 2004).</skos:definition>
	<skos:narrower rdf:resource="https://resource.geosphere.at/thes/lith/212"/>
	<skos:narrower rdf:resource="https://resource.geosphere.at/thes/lith/211"/>
	<skos:narrower rdf:resource="https://resource.geosphere.at/thes/lith/210"/>
	<skos:prefLabel xml:lang="de">Evaporit</skos:prefLabel>
	<dcterms:date rdf:datatype="http://www.w3.org/2001/XMLSchema#dateTime">2011-03-22T14:52:39Z</dcterms:date>
	<dcterms:references rdf:resource="https://resource.geosphere.at/thes/citation/545"/>
	<dcterms:references rdf:resource="https://resource.geosphere.at/thes/citation/547"/>
	<skos:definition xml:lang="de">Chemisches Sedimentgestein, welches &gt; 50 % nicht-karbonatische Minerale wie Chlorid-, Nitrat-, Sulfat- oder Boratminerale enthält. Typischerweise durch Fällung aus einer salzigen Lösung infolge Verdunstung des Lösungsmittels gebildet (Neuendorf et al., 2005; SLTT Appendix C, 2004).</skos:definition>
	<skos:prefLabel xml:lang="en">Evaporite</skos:prefLabel>
	<dcterms:created rdf:datatype="http://www.w3.org/2001/XMLSchema#dateTime">2012-03-12T12:53:27.000Z</dcterms:created>
	<skos:exactMatch rdf:resource="http://dbpedia.org/resource/Evaporite"/>
	<skos:exactMatch rdf:resource="http://www.wikidata.org/entity/Q491689"/>
</rdf:Description>

<rdf:Description rdf:about="https://resource.geosphere.at/thes/lith/212">
	<skos:definition xml:lang="en">An evaporite composed of &gt; 50% anhydrite (CaSO4). Often associated with gypsum and halite , forming thick interbedded layers with limestone and shale (Neuendorf et al., 2005).</skos:definition>
	<skos:broadMatch rdf:resource="http://inspire.ec.europa.eu/codelist/LithologyValue/gypsumOrAnhydrite"/>
	<skos:prefLabel xml:lang="de">Anhydrit</skos:prefLabel>
	<skos:related rdf:resource="https://resource.geosphere.at/thes/lith/211"/>
	<skos:definition xml:lang="de">Evaporit, der sich zu &gt; 50% aus Anhydrit (CaSO4) zusammensetzt. Bildet oft im Verbund mit Gips und Halit dicke Einschaltungen in Kalkstein und Schieferton (Neuendorf et al., 2005).</skos:definition>
	<dcterms:references rdf:resource="https://resource.geosphere.at/thes/citation/545"/>
	<dcterms:hasVersion rdf:datatype="http://www.w3.org/2001/XMLSchema#int">7</dcterms:hasVersion>
	<foaf:depiction rdf:resource="https://resource.geosphere.at/img/thes/Anhydrit.jpg"/>
	<dcterms:date rdf:datatype="http://www.w3.org/2001/XMLSchema#dateTime">2011-03-22T14:52:39Z</dcterms:date>
	<rdf:type rdf:resource="http://www.w3.org/2004/02/skos/core#Concept"/>
	<skos:exactMatch rdf:resource="http://dbpedia.org/resource/Anhydrite"/>
	<skos:prefLabel xml:lang="en">Anhydrite</skos:prefLabel>
	<dcterms:created rdf:datatype="http://www.w3.org/2001/XMLSchema#dateTime">2013-04-05T09:22:56.000Z</dcterms:created>
	<skos:broadMatch rdf:resource="http://resource.geosciml.org/classifier/cgi/lithology/rock_gypsum_or_anhydrite"/>
	<colourHexCode xmlns="http://dbpedia.org/ontology/">#B2E6F2</colourHexCode>
</rdf:Description>

<rdf:Description rdf:about="https://resource.geosphere.at/thes/lith/211">
	<skos:prefLabel xml:lang="en">Gypsum</skos:prefLabel>
	<skos:exactMatch rdf:resource="http://data.bgs.ac.uk/id/EarthMaterialClass/RockName/GYPS"/>
	<dcterms:hasVersion rdf:datatype="http://www.w3.org/2001/XMLSchema#int">8</dcterms:hasVersion>
	<dcterms:date rdf:datatype="http://www.w3.org/2001/XMLSchema#dateTime">2011-03-22T14:52:39Z</dcterms:date>
	<skos:definition xml:lang="en">An evaporite composed of &gt; 50% gypsum (CaSO4 • 2H2O), often associated with anhydrite and halite, forming thick interbedded layers with limestone and shale (Neuendorf et al., 2005).</skos:definition>
	<skos:related rdf:resource="https://resource.geosphere.at/thes/lith/212"/>
	<foaf:depiction rdf:resource="https://resource.geosphere.at/img/thes/Gips.jpg"/>
	<skos:definition xml:lang="de">Evaporit, der sich zu &gt; 50 % aus Gips (CaSO4 • 2H2O) zusammensetzt. Bildet oft im Verbund mit Anhydrit und Halit dicke Einschaltungen in Kalkstein und Schieferton (Neuendorf et al., 2005).</skos:definition>
	<skos:exactMatch rdf:resource="http://dbpedia.org/resource/Gypsum"/>
	<rdf:type rdf:resource="http://www.w3.org/2004/02/skos/core#Concept"/>
	<skos:broadMatch rdf:resource="http://inspire.ec.europa.eu/codelist/LithologyValue/gypsumOrAnhydrite"/>
	<dcterms:references rdf:resource="https://resource.geosphere.at/thes/citation/545"/>
	<dcterms:created rdf:datatype="http://www.w3.org/2001/XMLSchema#dateTime">2013-04-05T09:27:13.000Z</dcterms:created>
	<skos:broadMatch rdf:resource="http://resource.geosciml.org/classifier/cgi/lithology/rock_gypsum_or_anhydrite"/>
	<colourHexCode xmlns="http://dbpedia.org/ontology/">#B2E6F2</colourHexCode>
	<skos:prefLabel xml:lang="de">Gips</skos:prefLabel>
</rdf:Description>

<rdf:Description rdf:about="https://resource.geosphere.at/thes/lith/210">
	<dcterms:hasVersion rdf:datatype="http://www.w3.org/2001/XMLSchema#int">6</dcterms:hasVersion>
	<skos:exactMatch rdf:resource="http://inspire.ec.europa.eu/codelist/LithologyValue/rockSalt"/>
	<skos:definition xml:lang="de">Evaporit, der sich zu &gt; 50 % aus (grobkristallinem) Halit (NaCl) zusammensetzt. Typischerweise durch Eisenoxide gefärbt und mit feinkörnigen Sedimenten (Ton) vermischt.</skos:definition>
	<dcterms:date rdf:datatype="http://www.w3.org/2001/XMLSchema#dateTime">2011-03-22T14:52:39Z</dcterms:date>
	<skos:definition xml:lang="en">An evaporite composed of &gt; 50% crystalline halite (NaCl), typically stained by iron-oxides and mixed with fine-grained sediments (clay) (Neuendorf et al., 2005).</skos:definition>
	<dcterms:references rdf:resource="https://resource.geosphere.at/thes/citation/545"/>
	<skos:exactMatch rdf:resource="http://www.wikidata.org/entity/Q2341557"/>
	<dcterms:created rdf:datatype="http://www.w3.org/2001/XMLSchema#dateTime">2013-04-05T09:41:54.000Z</dcterms:created>
	<colourHexCode xmlns="http://dbpedia.org/ontology/">#AADAF2</colourHexCode>
	<foaf:depiction rdf:resource="https://resource.geosphere.at/img/thes/Steinsalz.jpg"/>
	<skos:prefLabel xml:lang="de">Steinsalz</skos:prefLabel>
	<rdf:type rdf:resource="http://www.w3.org/2004/02/skos/core#Concept"/>
	<skos:prefLabel xml:lang="en">Rock salt</skos:prefLabel>
	<skos:exactMatch rdf:resource="http://resource.geosciml.org/classifier/cgi/lithology/rock_salt"/>
</rdf:Description>

<rdf:Description rdf:about="https://resource.geosphere.at/thes/lith/4">
	<skos:definition xml:lang="de">Überwiegend unverfestigte, pyroklastische Ablagerung, welche zu mehr als 75 Vol.-% aus Pyroklasten besteht (Le Maitre et al., 2005).</skos:definition>
	<skos:exactMatch rdf:resource="http://dbpedia.org/resource/Tephra"/>
	<colourHexCode xmlns="http://dbpedia.org/ontology/">#B24DCC</colourHexCode>
	<skos:prefLabel xml:lang="de">Tephra</skos:prefLabel>
	<skos:prefLabel xml:lang="en">Tephra</skos:prefLabel>
	<skos:definition xml:lang="en">Predominantly unconsolidated pyroclastic deposits that contain more than 75% pyroclasts (by volume) (Le Maitre et al., 2005).</skos:definition>
	<skos:narrower rdf:resource="https://resource.geosphere.at/thes/lith/9"/>
	<skos:narrower rdf:resource="https://resource.geosphere.at/thes/lith/8"/>
	<skos:exactMatch rdf:resource="http://resource.geosciml.org/classifier/cgi/lithology/tephra"/>
	<dcterms:hasVersion rdf:datatype="http://www.w3.org/2001/XMLSchema#int">13</dcterms:hasVersion>
	<dcterms:date rdf:datatype="http://www.w3.org/2001/XMLSchema#dateTime">2011-03-15T15:22:10Z</dcterms:date>
	<dcterms:created rdf:datatype="http://www.w3.org/2001/XMLSchema#dateTime">2012-03-12T16:29:32.000Z</dcterms:created>
	<dcterms:references rdf:resource="https://resource.geosphere.at/thes/citation/477"/>
	<rdf:type rdf:resource="http://www.w3.org/2004/02/skos/core#Concept"/>
	<skos:exactMatch rdf:resource="http://inspire.ec.europa.eu/codelist/LithologyValue/tephra"/>
	<skos:narrower rdf:resource="https://resource.geosphere.at/thes/lith/10"/>
</rdf:Description>

<rdf:Description rdf:about="https://resource.geosphere.at/thes/lith/10">
	<skos:closeMatch rdf:resource="http://inspire.ec.europa.eu/codelist/LithologyValue/tephra"/>
	<dcterms:hasVersion rdf:datatype="http://www.w3.org/2001/XMLSchema#int">9</dcterms:hasVersion>
	<skos:broadMatch rdf:resource="http://resource.geosciml.org/classifier/cgi/lithology/ash_and_lapilli"/>
	<skos:prefLabel xml:lang="de">Asche</skos:prefLabel>
	<dcterms:date rdf:datatype="http://www.w3.org/2001/XMLSchema#dateTime">2011-03-15T15:22:10Z</dcterms:date>
	<skos:exactMatch rdf:resource="http://dbpedia.org/resource/Volcanic_ash"/>
	<dcterms:references rdf:resource="https://resource.geosphere.at/thes/citation/477"/>
	<skos:prefLabel xml:lang="en">Ash</skos:prefLabel>
	<skos:exactMatch rdf:resource="http://data.bgs.ac.uk/id/EarthMaterialClass/RockName/ASH"/>
	<skos:definition xml:lang="en">Unconsolidated pyroclastic deposit in which &gt;75% of the material has a grain size &lt; 2 mm (Le Maitre et al., 2005).</skos:definition>
	<dcterms:created rdf:datatype="http://www.w3.org/2001/XMLSchema#dateTime">2012-03-12T10:15:26.000Z</dcterms:created>
	<rdf:type rdf:resource="http://www.w3.org/2004/02/skos/core#Concept"/>
	<skos:definition xml:lang="de">Unverfestigte pyroklastische Ablagerung, welche zu mehr als 75 % aus Material mit Durchmesser &lt; 2 mm besteht (Le Maitre et al., 2005).</skos:definition>
	<skos:related rdf:resource="https://resource.geosphere.at/thes/lith/16"/>
	<colourHexCode xmlns="http://dbpedia.org/ontology/">#B24DCC</colourHexCode>
</rdf:Description>

<rdf:Description rdf:about="https://resource.geosphere.at/thes/lith/8">
	<dcterms:references rdf:resource="https://resource.geosphere.at/thes/citation/477"/>
	<colourHexCode xmlns="http://dbpedia.org/ontology/">#CC59D9</colourHexCode>
	<skos:prefLabel xml:lang="en">Block tephra</skos:prefLabel>
	<skos:exactMatch rdf:resource="http://data.bgs.ac.uk/id/EarthMaterialClass/RockName/BLTPH"/>
	<skos:related rdf:resource="https://resource.geosphere.at/thes/lith/11"/>
	<skos:definition xml:lang="de">Unverfestigte pyroklastische Ablagerung, welche zu mehr als 75 % aus vulkanischen Blöcken (Durchmesser &gt; 64 mm) besteht (Le Maitre et al., 2005).</skos:definition>
	<skos:prefLabel xml:lang="de">Block-Tephra</skos:prefLabel>
	<skos:broadMatch rdf:resource="http://inspire.ec.europa.eu/codelist/LithologyValue/ashBrecciaBombOrBlockTephra"/>
	<dcterms:hasVersion rdf:datatype="http://www.w3.org/2001/XMLSchema#int">7</dcterms:hasVersion>
	<rdf:type rdf:resource="http://www.w3.org/2004/02/skos/core#Concept"/>
	<skos:broadMatch rdf:resource="http://resource.geosciml.org/classifier/cgi/lithology/ash_breccia_bomb_or_block_tephra"/>
	<dcterms:date rdf:datatype="http://www.w3.org/2001/XMLSchema#dateTime">2011-03-15T15:22:10Z</dcterms:date>
	<skos:definition xml:lang="en">An unconsolidated pyroclastic deposit, more than 75% of which is composed of volcanic blocks (diameter &gt; 64 mm) (Le Maitre et al., 2005).</skos:definition>
	<dcterms:created rdf:datatype="http://www.w3.org/2001/XMLSchema#dateTime">2012-03-12T10:29:10.000Z</dcterms:created>
</rdf:Description>

<rdf:Description rdf:about="https://resource.geosphere.at/thes/lith/9">
	<skos:prefLabel xml:lang="de">Lapilli-Tephra</skos:prefLabel>
	<skos:broadMatch rdf:resource="http://resource.geosciml.org/classifier/cgi/lithology/ash_and_lapilli"/>
	<dcterms:date rdf:datatype="http://www.w3.org/2001/XMLSchema#dateTime">2011-03-15T15:22:10Z</dcterms:date>
	<skos:definition xml:lang="en">Unconsolidated pyroclastic deposit with more than 75% lapilli (diameter between 2 and 64 mm) (Le Maitre et al., 2005).</skos:definition>
	<skos:related rdf:resource="https://resource.geosphere.at/thes/lith/14"/>
	<skos:definition xml:lang="de">Unverfestigte pyroklastische Ablagerung, welche zu mehr als 75 % aus Lapilli (Durchmesser &gt; 2 mm und &lt; 64 mm) besteht (Le Maitre et al., 2005).</skos:definition>
	<dcterms:hasVersion rdf:datatype="http://www.w3.org/2001/XMLSchema#int">9</dcterms:hasVersion>
	<dcterms:references rdf:resource="https://resource.geosphere.at/thes/citation/477"/>
	<colourHexCode xmlns="http://dbpedia.org/ontology/">#BF4DCC</colourHexCode>
	<rdf:type rdf:resource="http://www.w3.org/2004/02/skos/core#Concept"/>
	<dcterms:created rdf:datatype="http://www.w3.org/2001/XMLSchema#dateTime">2012-03-12T13:55:05.000Z</dcterms:created>
	<skos:broadMatch rdf:resource="http://inspire.ec.europa.eu/codelist/LithologyValue/ashAndLapilli"/>
	<skos:prefLabel xml:lang="en">Lapilli tephra</skos:prefLabel>
</rdf:Description>

<rdf:Description rdf:about="https://resource.geosphere.at/thes/lith/166">
	<skos:narrower rdf:resource="https://resource.geosphere.at/thes/lith/232"/>
	<dcterms:created rdf:datatype="http://www.w3.org/2001/XMLSchema#dateTime">2012-03-12T12:03:50.000Z</dcterms:created>
	<skos:narrower rdf:resource="https://resource.geosphere.at/thes/lith/228"/>
	<skos:narrower rdf:resource="https://resource.geosphere.at/thes/lith/229"/>
	<skos:narrower rdf:resource="https://resource.geosphere.at/thes/lith/222"/>
	<skos:prefLabel xml:lang="de">Klastisches Sediment</skos:prefLabel>
	<skos:narrower rdf:resource="https://resource.geosphere.at/thes/lith/226"/>
	<skos:narrower rdf:resource="https://resource.geosphere.at/thes/lith/227"/>
	<rdf:type rdf:resource="http://www.w3.org/2004/02/skos/core#Concept"/>
	<skos:exactMatch rdf:resource="http://inspire.ec.europa.eu/codelist/LithologyValue/clasticSedimentaryMaterial"/>
	<skos:definition xml:lang="de">Sediment, welches durch die Akkumulierung von zerbrochenen Fragmenten gebildet wird, welche sich aus präexistierenden Gesteinen und Mineralen ableiten und als separate Partikel vor ihrer Ablagerung von mechanischen Kräften (wie Wind, Wasser, Eis oder Gravitation) transportiert wurden. Der Begriff beinhaltet karbonatisch-klastische Mischgesteine (verändert nach Neuendorf et al., 2005).</skos:definition>
	<skos:exactMatch rdf:resource="http://resource.geosciml.org/classifier/cgi/lithology/clastic_sediment"/>
	<dcterms:references rdf:resource="https://resource.geosphere.at/thes/citation/545"/>
	<skos:prefLabel xml:lang="en">Clastic sediment</skos:prefLabel>
	<dcterms:hasVersion rdf:datatype="http://www.w3.org/2001/XMLSchema#int">11</dcterms:hasVersion>
	<skos:narrower rdf:resource="https://resource.geosphere.at/thes/lith/218"/>
	<skos:narrower rdf:resource="https://resource.geosphere.at/thes/lith/213"/>
	<skos:narrower rdf:resource="https://resource.geosphere.at/thes/lith/214"/>
	<dcterms:date rdf:datatype="http://www.w3.org/2001/XMLSchema#dateTime">2011-03-22T14:52:39Z</dcterms:date>
	<skos:definition xml:lang="en">A sediment formed by the accumulation of broken fragments derived from pre-existing rocks or minerals and transported as separate particles by mechanical agents (such as wind, water, ice, gravity) prior to deposition. The term includes mixed carbonate-clastic sediments (modified from Neuendorf et al., 2005).</skos:definition>
	<skos:narrower rdf:resource="https://resource.geosphere.at/thes/lith/240"/>
	<colourHexCode xmlns="http://dbpedia.org/ontology/">#D9FDD3</colourHexCode>
</rdf:Description>

<rdf:Description rdf:about="https://resource.geosphere.at/thes/lith/234">
	<dcterms:created rdf:datatype="http://www.w3.org/2001/XMLSchema#dateTime">2012-03-12T10:40:46.000Z</dcterms:created>
	<dcterms:hasVersion rdf:datatype="http://www.w3.org/2001/XMLSchema#int">8</dcterms:hasVersion>
	<skos:definition xml:lang="de">Karbonatisch-klastisches Sediment, dessen klastischer Anteil sich auf die Sandfraktion beschränkt. Besteht aus 25–50 % Calcit und 50–75 % Sand (Füchtbauer, 1988).</skos:definition>
	<skos:related rdf:resource="https://resource.geosphere.at/thes/lith/194"/>
	<skos:broadMatch rdf:resource="http://inspire.ec.europa.eu/codelist/LithologyValue/sand"/>
	<dcterms:references rdf:resource="https://resource.geosphere.at/thes/citation/229"/>
	<dcterms:date rdf:datatype="http://www.w3.org/2001/XMLSchema#dateTime">2011-03-22T14:52:39Z</dcterms:date>
	<skos:prefLabel xml:lang="en">Calcareous sand</skos:prefLabel>
	<skos:related rdf:resource="https://resource.geosphere.at/thes/lith/235"/>
	<skos:definition xml:lang="en">A mixed carbonate-clastic rock in which the clastic portion is restricted to sand-sized components. Consists of 25-50% calcite and 50-75% sand (Füchtbauer, 1988).</skos:definition>
	<skos:closeMatch rdf:resource="http://resource.geosciml.org/classifier/cgi/lithology/sand"/>
	<rdf:type rdf:resource="http://www.w3.org/2004/02/skos/core#Concept"/>
	<skos:prefLabel xml:lang="de">Kalksand</skos:prefLabel>
</rdf:Description>

<rdf:Description rdf:about="https://resource.geosphere.at/thes/lith/222">
	<skos:exactMatch rdf:resource="http://resource.geosciml.org/classifier/cgi/lithology/gravel"/>
	<skos:prefLabel xml:lang="en">Gravel</skos:prefLabel>
	<dcterms:references rdf:resource="https://resource.geosphere.at/thes/citation/78"/>
	<skos:related rdf:resource="https://resource.geosphere.at/thes/lith/181"/>
	<dcterms:hasVersion rdf:datatype="http://www.w3.org/2001/XMLSchema#int">13</dcterms:hasVersion>
	<skos:exactMatch rdf:resource="http://inspire.ec.europa.eu/codelist/LithologyValue/gravel"/>
	<dcterms:references rdf:resource="https://resource.geosphere.at/thes/citation/229"/>
	<skos:exactMatch rdf:resource="http://www.wikidata.org/entity/Q133833"/>
	<skos:exactMatch rdf:resource="http://data.bgs.ac.uk/id/EarthMaterialClass/RockName/GRAV"/>
	<dcterms:date rdf:datatype="http://www.w3.org/2001/XMLSchema#dateTime">2011-03-22T14:52:39Z</dcterms:date>
	<dcterms:created rdf:datatype="http://www.w3.org/2001/XMLSchema#dateTime">2013-04-05T09:32:52.000Z</dcterms:created>
	<foaf:depiction rdf:resource="https://resource.geosphere.at/img/thes/Kies.jpg"/>
	<skos:narrower rdf:resource="https://resource.geosphere.at/thes/lith/223"/>
	<skos:narrower rdf:resource="https://resource.geosphere.at/thes/lith/224"/>
	<skos:narrower rdf:resource="https://resource.geosphere.at/thes/lith/225"/>
	<colourHexCode xmlns="http://dbpedia.org/ontology/">#FFFFCC</colourHexCode>
	<skos:definition xml:lang="de">Ein klastisches Sediment welches zu &gt; 50% aus Geröllen (gerundeten Mineral- oder Gesteinsbruchstücken) von &gt; 2 mm besteht (nach Füchtbauer 1988, DIN 4022).</skos:definition>
	<rdf:type rdf:resource="http://www.w3.org/2004/02/skos/core#Concept"/>
	<skos:exactMatch rdf:resource="http://dbpedia.org/resource/Gravel"/>
	<skos:definition xml:lang="en">A clastic sedimentary rock that contains &gt; 50% rounded mineral and rock fragments with a median grain size &gt; 2 mm (Füchtbauer 1988, DIN 4022).</skos:definition>
	<skos:prefLabel xml:lang="de">Kies</skos:prefLabel>
</rdf:Description>

<rdf:Description rdf:about="https://resource.geosphere.at/thes/lith/223">
	<skos:broadMatch rdf:resource="http://resource.geosciml.org/classifier/cgi/lithology/gravel"/>
	<dcterms:references rdf:resource="https://resource.geosphere.at/thes/citation/78"/>
	<dcterms:date rdf:datatype="http://www.w3.org/2001/XMLSchema#dateTime">2011-03-22T14:52:39Z</dcterms:date>
	<dcterms:hasVersion rdf:datatype="http://www.w3.org/2001/XMLSchema#int">12</dcterms:hasVersion>
	<skos:definition xml:lang="en">A clastic sedimentary rock that contains &gt; 50% rounded mineral and rock fragments with a median grain size between 20 and 63 mm (Füchtbauer, 1988; DIN 4022).</skos:definition>
	<skos:broadMatch rdf:resource="http://inspire.ec.europa.eu/codelist/LithologyValue/gravel"/>
	<dcterms:references rdf:resource="https://resource.geosphere.at/thes/citation/229"/>
	<skos:definition xml:lang="de">Klastisches Sediment, welches zu &gt; 50 % aus Geröllen (gerundeten Mineral- oder Gesteinsbruchstücken) mit einer medianen Korngröße von &gt; 20 mm und ≤ 63 mm besteht (Füchtbauer, 1988; DIN 4022).</skos:definition>
	<rdf:type rdf:resource="http://www.w3.org/2004/02/skos/core#Concept"/>
	<dcterms:created rdf:datatype="http://www.w3.org/2001/XMLSchema#dateTime">2012-03-12T12:15:13.000Z</dcterms:created>
	<skos:prefLabel xml:lang="de">Grobkies</skos:prefLabel>
	<skos:prefLabel xml:lang="en">Coarse gravel</skos:prefLabel>
</rdf:Description>

<rdf:Description rdf:about="https://resource.geosphere.at/thes/lith/225">
	<dcterms:references rdf:resource="https://resource.geosphere.at/thes/citation/229"/>
	<skos:broadMatch rdf:resource="http://inspire.ec.europa.eu/codelist/LithologyValue/gravel"/>
	<skos:definition xml:lang="en">A clastic sedimentary rock that contains &gt; 50% rounded mineral and rock fragments with a median grain size between 2 and 6.3 mm (Füchtbauer, 1988; DIN 4022).</skos:definition>
	<skos:prefLabel xml:lang="en">Fine gravel</skos:prefLabel>
	<skos:definition xml:lang="de">Klastisches Sediment, welches zu &gt; 50 % aus Geröllen (gerundeten Mineral- oder Gesteinsbruchstücken) mit einer medianen Korngröße von &gt; 2 mm und ≤ 6.3 mm besteht (Füchtbauer, 1988; DIN 4022).</skos:definition>
	<rdf:type rdf:resource="http://www.w3.org/2004/02/skos/core#Concept"/>
	<dcterms:references rdf:resource="https://resource.geosphere.at/thes/citation/78"/>
	<skos:broadMatch rdf:resource="http://resource.geosciml.org/classifier/cgi/lithology/gravel"/>
	<dcterms:created rdf:datatype="http://www.w3.org/2001/XMLSchema#dateTime">2012-03-12T13:01:45.000Z</dcterms:created>
	<dcterms:hasVersion rdf:datatype="http://www.w3.org/2001/XMLSchema#int">11</dcterms:hasVersion>
	<skos:prefLabel xml:lang="de">Feinkies</skos:prefLabel>
	<dcterms:date rdf:datatype="http://www.w3.org/2001/XMLSchema#dateTime">2011-03-22T14:52:39Z</dcterms:date>
</rdf:Description>

<rdf:Description rdf:about="https://resource.geosphere.at/thes/lith/224">
	<skos:prefLabel xml:lang="en">Medium gravel</skos:prefLabel>
	<skos:definition xml:lang="de">Klastisches Sediment, welches zu &gt; 50 % aus Geröllen (gerundete Mineral- oder Gesteinsbruchstücke) mit einer medianen Korngröße von &gt; 6.3 mm und ≤ 20 mm besteht (Füchtbauer, 1988; DIN 4022).</skos:definition>
	<dcterms:references rdf:resource="https://resource.geosphere.at/thes/citation/78"/>
	<dcterms:hasVersion rdf:datatype="http://www.w3.org/2001/XMLSchema#int">11</dcterms:hasVersion>
	<dcterms:references rdf:resource="https://resource.geosphere.at/thes/citation/229"/>
	<skos:definition xml:lang="en">A clastic sedimentary rock that contains &gt; 50% rounded mineral and rock fragments with a median grain size between 6.3 mm and 20 mm (Füchtbauer, 1988; DIN 4022).</skos:definition>
	<dcterms:created rdf:datatype="http://www.w3.org/2001/XMLSchema#dateTime">2012-03-12T14:24:23.000Z</dcterms:created>
	<dcterms:date rdf:datatype="http://www.w3.org/2001/XMLSchema#dateTime">2011-03-22T14:52:39Z</dcterms:date>
	<skos:prefLabel xml:lang="de">Mittelkies</skos:prefLabel>
	<skos:broadMatch rdf:resource="http://inspire.ec.europa.eu/codelist/LithologyValue/gravel"/>
	<rdf:type rdf:resource="http://www.w3.org/2004/02/skos/core#Concept"/>
	<skos:broadMatch rdf:resource="http://resource.geosciml.org/classifier/cgi/lithology/gravel"/>
</rdf:Description>

<rdf:Description rdf:about="https://resource.geosphere.at/thes/lith/214">
	<skos:exactMatch rdf:resource="http://inspire.ec.europa.eu/codelist/LithologyValue/silt"/>
	<skos:exactMatch rdf:resource="http://resource.geosciml.org/classifier/cgi/lithology/silt"/>
	<rdf:type rdf:resource="http://www.w3.org/2004/02/skos/core#Concept"/>
	<colourHexCode xmlns="http://dbpedia.org/ontology/">#F2E6BF</colourHexCode>
	<skos:altLabel xml:lang="de">Schluff</skos:altLabel>
	<skos:definition xml:lang="de">Klastisches Sediment mit einer medianen Korngröße &gt; 0.002 mm und ≤ 0.063 mm (Füchtbauer, 1988; DIN 4022).</skos:definition>
	<skos:prefLabel xml:lang="de">Silt</skos:prefLabel>
	<skos:prefLabel xml:lang="en">Silt</skos:prefLabel>
	<skos:exactMatch rdf:resource="http://dbpedia.org/resource/Silt"/>
	<skos:related rdf:resource="https://resource.geosphere.at/thes/lith/173"/>
	<skos:exactMatch rdf:resource="http://data.bgs.ac.uk/id/EarthMaterialClass/RockName/SILT"/>
	<skos:narrower rdf:resource="https://resource.geosphere.at/thes/lith/217"/>
	<skos:narrower rdf:resource="https://resource.geosphere.at/thes/lith/215"/>
	<skos:narrower rdf:resource="https://resource.geosphere.at/thes/lith/216"/>
	<dcterms:references rdf:resource="https://resource.geosphere.at/thes/citation/78"/>
	<dcterms:created rdf:datatype="http://www.w3.org/2001/XMLSchema#dateTime">2012-03-12T16:23:13.000Z</dcterms:created>
	<skos:definition xml:lang="en">A clastic sediment with a median grain size between 0.002 and 0.063 mm (Füchtbauer, 1988; DIN 4022).</skos:definition>
	<dcterms:date rdf:datatype="http://www.w3.org/2001/XMLSchema#dateTime">2011-03-22T14:52:39Z</dcterms:date>
	<skos:exactMatch rdf:resource="http://www.wikidata.org/entity/Q270699"/>
	<dcterms:hasVersion rdf:datatype="http://www.w3.org/2001/XMLSchema#int">10</dcterms:hasVersion>
	<dcterms:references rdf:resource="https://resource.geosphere.at/thes/citation/229"/>
</rdf:Description>

<rdf:Description rdf:about="https://resource.geosphere.at/thes/lith/216">
	<rdf:type rdf:resource="http://www.w3.org/2004/02/skos/core#Concept"/>
	<dcterms:references rdf:resource="https://resource.geosphere.at/thes/citation/78"/>
	<dcterms:hasVersion rdf:datatype="http://www.w3.org/2001/XMLSchema#int">12</dcterms:hasVersion>
	<skos:definition xml:lang="de">Klastisches Sediment mit einer medianen Korngröße &gt; 0.0063 mm und ≤ 0.02 mm (Füchtbauer, 1988; DIN 4022).</skos:definition>
	<skos:related rdf:resource="https://resource.geosphere.at/thes/lith/175"/>
	<skos:broadMatch rdf:resource="http://resource.geosciml.org/classifier/cgi/lithology/silt"/>
	<dcterms:date rdf:datatype="http://www.w3.org/2001/XMLSchema#dateTime">2011-03-22T14:52:39Z</dcterms:date>
	<skos:prefLabel xml:lang="de">Mittelsilt</skos:prefLabel>
	<dcterms:references rdf:resource="https://resource.geosphere.at/thes/citation/229"/>
	<skos:definition xml:lang="en">A clastic sediment with a median grain size between 0.0063 mm and 0.02 mm (Füchtbauer, 1988; DIN 4022).</skos:definition>
	<skos:altLabel xml:lang="de">Mittelschluff</skos:altLabel>
	<skos:broadMatch rdf:resource="http://inspire.ec.europa.eu/codelist/LithologyValue/silt"/>
	<skos:prefLabel xml:lang="en">Medium silt</skos:prefLabel>
	<dcterms:created rdf:datatype="http://www.w3.org/2001/XMLSchema#dateTime">2012-03-12T14:25:10.000Z</dcterms:created>
</rdf:Description>

<rdf:Description rdf:about="https://resource.geosphere.at/thes/lith/215">
	<skos:related rdf:resource="https://resource.geosphere.at/thes/lith/174"/>
	<dcterms:references rdf:resource="https://resource.geosphere.at/thes/citation/229"/>
	<skos:altLabel xml:lang="de">Grobschluff</skos:altLabel>
	<skos:prefLabel xml:lang="de">Grobsilt</skos:prefLabel>
	<dcterms:hasVersion rdf:datatype="http://www.w3.org/2001/XMLSchema#int">12</dcterms:hasVersion>
	<dcterms:date rdf:datatype="http://www.w3.org/2001/XMLSchema#dateTime">2011-03-22T14:52:39Z</dcterms:date>
	<skos:definition xml:lang="de">Klastisches Sediment mit einer medianen Korngröße &gt; 0.02 mm und ≤ 0.063 mm (Füchtbauer, 1988; DIN 4022).</skos:definition>
	<skos:exactMatch rdf:resource="http://resource.geosciml.org/classifier/cgi/lithology/silt"/>
	<skos:definition xml:lang="en">A clastic sediment with a median grain size between 0.02 and 0.063 mm (Füchtbauer, 1988; DIN 4022).</skos:definition>
	<skos:prefLabel xml:lang="en">Coarse silt</skos:prefLabel>
	<skos:broadMatch rdf:resource="http://inspire.ec.europa.eu/codelist/LithologyValue/silt"/>
	<dcterms:references rdf:resource="https://resource.geosphere.at/thes/citation/78"/>
	<dcterms:created rdf:datatype="http://www.w3.org/2001/XMLSchema#dateTime">2012-03-12T12:16:51.000Z</dcterms:created>
	<rdf:type rdf:resource="http://www.w3.org/2004/02/skos/core#Concept"/>
</rdf:Description>

<rdf:Description rdf:about="https://resource.geosphere.at/thes/lith/217">
	<skos:altLabel xml:lang="de">Feinschluff</skos:altLabel>
	<skos:prefLabel xml:lang="de">Feinsilt</skos:prefLabel>
	<dcterms:references rdf:resource="https://resource.geosphere.at/thes/citation/78"/>
	<skos:definition xml:lang="en">A clastic sediment with a median grain size between 0.002 and 0.0063 mm (Füchtbauer, 1988; DIN 4022).</skos:definition>
	<dcterms:hasVersion rdf:datatype="http://www.w3.org/2001/XMLSchema#int">12</dcterms:hasVersion>
	<skos:broadMatch rdf:resource="http://inspire.ec.europa.eu/codelist/LithologyValue/silt"/>
	<skos:broadMatch rdf:resource="http://resource.geosciml.org/classifier/cgi/lithology/silt"/>
	<skos:prefLabel xml:lang="en">Fine silt</skos:prefLabel>
	<dcterms:references rdf:resource="https://resource.geosphere.at/thes/citation/229"/>
	<skos:definition xml:lang="de">Klastisches Sediment mit einer medianen Korngröße &gt; 0.002 mm und ≤ 0.0063 mm (Füchtbauer, 1988; DIN 4022).</skos:definition>
	<dcterms:date rdf:datatype="http://www.w3.org/2001/XMLSchema#dateTime">2011-03-22T14:52:39Z</dcterms:date>
	<rdf:type rdf:resource="http://www.w3.org/2004/02/skos/core#Concept"/>
	<dcterms:created rdf:datatype="http://www.w3.org/2001/XMLSchema#dateTime">2012-03-12T13:03:04.000Z</dcterms:created>
	<skos:related rdf:resource="https://resource.geosphere.at/thes/lith/176"/>
</rdf:Description>

<rdf:Description rdf:about="https://resource.geosphere.at/thes/lith/213">
	<dcterms:references rdf:resource="https://resource.geosphere.at/thes/citation/229"/>
	<skos:exactMatch rdf:resource="http://inspire.ec.europa.eu/codelist/LithologyValue/clay"/>
	<skos:prefLabel xml:lang="en">Clay</skos:prefLabel>
	<skos:exactMatch rdf:resource="http://resource.geosciml.org/classifier/cgi/lithology/clay"/>
	<skos:definition xml:lang="de">Klastisches Sediment mit einer medianen Korngröße &lt; 0.002 mm (Füchtbauer, 1988; DIN 4022).</skos:definition>
	<skos:exactMatch rdf:resource="http://www.wikidata.org/entity/Q42302"/>
	<skos:definition xml:lang="en">A clastic sediment with a median grain size &lt; 0.002 mm (Füchtbauer, 1988; DIN 4022).</skos:definition>
	<rdf:type rdf:resource="http://www.w3.org/2004/02/skos/core#Concept"/>
	<dcterms:references rdf:resource="https://resource.geosphere.at/thes/citation/78"/>
	<skos:exactMatch rdf:resource="http://dbpedia.org/resource/Clay"/>
	<skos:exactMatch rdf:resource="http://data.bgs.ac.uk/id/EarthMaterialClass/RockName/CLAY"/>
	<dcterms:hasVersion rdf:datatype="http://www.w3.org/2001/XMLSchema#int">8</dcterms:hasVersion>
	<skos:prefLabel xml:lang="de">Ton</skos:prefLabel>
	<colourHexCode xmlns="http://dbpedia.org/ontology/">#FAF2BF</colourHexCode>
	<skos:related rdf:resource="https://resource.geosphere.at/thes/lith/172"/>
	<skos:related rdf:resource="https://resource.geosphere.at/thes/lith/171"/>
	<dcterms:date rdf:datatype="http://www.w3.org/2001/XMLSchema#dateTime">2011-03-22T14:52:39Z</dcterms:date>
	<dcterms:created rdf:datatype="http://www.w3.org/2001/XMLSchema#dateTime">2012-01-25T15:39:02.000Z</dcterms:created>
</rdf:Description>

<rdf:Description rdf:about="https://resource.geosphere.at/thes/lith/227">
	<skos:definition xml:lang="en">A clastic sediment with a median grain size between 63 and 200 mm (Füchtbauer, 1988; DIN 4022).</skos:definition>
	<dcterms:references rdf:resource="https://resource.geosphere.at/thes/citation/229"/>
	<dcterms:hasVersion rdf:datatype="http://www.w3.org/2001/XMLSchema#int">12</dcterms:hasVersion>
	<dcterms:date rdf:datatype="http://www.w3.org/2001/XMLSchema#dateTime">2011-03-22T14:52:39Z</dcterms:date>
	<skos:prefLabel xml:lang="de">Steine</skos:prefLabel>
	<skos:definition xml:lang="de">Klastisches Sediment mit einer medianen Korngröße &gt; 63 mm und ≤ 200 mm (Füchtbauer, 1988; DIN 4022).</skos:definition>
	<skos:closeMatch rdf:resource="http://resource.geosciml.org/classifier/cgi/lithology/cobble_gravel_size_sediment"/>
	<skos:prefLabel xml:lang="en">Cobbles</skos:prefLabel>
	<skos:exactMatch rdf:resource="http://data.bgs.ac.uk/id/EarthMaterialClass/RockName/L"/>
	<dcterms:created rdf:datatype="http://www.w3.org/2001/XMLSchema#dateTime">2013-10-21T08:22:31.000Z</dcterms:created>
	<skos:closeMatch rdf:resource="http://inspire.ec.europa.eu/codelist/LithologyValue/cobbleGravelSizeSediment"/>
	<dcterms:references rdf:resource="https://resource.geosphere.at/thes/citation/78"/>
	<rdf:type rdf:resource="http://www.w3.org/2004/02/skos/core#Concept"/>
</rdf:Description>

<rdf:Description rdf:about="https://resource.geosphere.at/thes/lith/226">
	<skos:closeMatch rdf:resource="http://inspire.ec.europa.eu/codelist/LithologyValue/gravel"/>
	<dcterms:created rdf:datatype="http://www.w3.org/2001/XMLSchema#dateTime">2012-03-12T16:20:46.000Z</dcterms:created>
	<rdf:type rdf:resource="http://www.w3.org/2004/02/skos/core#Concept"/>
	<dcterms:references rdf:resource="https://resource.geosphere.at/thes/citation/545"/>
	<skos:altLabel xml:lang="en">Tallus</skos:altLabel>
	<skos:closeMatch rdf:resource="http://resource.geosciml.org/classifier/cgi/lithology/gravel"/>
	<skos:definition xml:lang="de">Klastisches Sediment, welches zu &gt; 50 % aus nicht gerundeten Mineral- oder Gesteinsbruchstücken mit einer medianen Korngröße von &gt; 2 mm besteht (Füchtbauer, 1988; Neuendorf et al., 2005).</skos:definition>
	<colourHexCode xmlns="http://dbpedia.org/ontology/">#FFFFCC</colourHexCode>
	<skos:definition xml:lang="en">A clastic sedimentary rock that contains &gt; 50% unrounded mineral and rock fragments with a median grain size &gt; 2mm (Füchtbauer, 1988; Neuendorf et al., 2005).</skos:definition>
	<skos:prefLabel xml:lang="en">Scree</skos:prefLabel>
	<dcterms:hasVersion rdf:datatype="http://www.w3.org/2001/XMLSchema#int">9</dcterms:hasVersion>
	<skos:prefLabel xml:lang="de">Schutt</skos:prefLabel>
	<dcterms:date rdf:datatype="http://www.w3.org/2001/XMLSchema#dateTime">2011-03-22T14:52:39Z</dcterms:date>
	<dcterms:references rdf:resource="https://resource.geosphere.at/thes/citation/229"/>
</rdf:Description>

<rdf:Description rdf:about="https://resource.geosphere.at/thes/lith/229">
	<skos:exactMatch rdf:resource="http://resource.geosciml.org/classifier/cgi/lithology/diamicton"/>
	<skos:definition xml:lang="en">A poorly sorted to unsortet clastic sediment that contains rounded and/or unrounded gravel-sized components that are matrix-supported in silt and clay. Diamicton is the unconsolidated equivalent of diamictite. The term diamicton is non-genetic but includes genetic terms such as till (Neuendorf et al., 2005; Füchtbauer, 1988).</skos:definition>
	<skos:altLabel xml:lang="de">Diamikton</skos:altLabel>
	<skos:exactMatch rdf:resource="http://inspire.ec.europa.eu/codelist/LithologyValue/diamicton"/>
	<dcterms:hasVersion rdf:datatype="http://www.w3.org/2001/XMLSchema#int">11</dcterms:hasVersion>
	<skos:prefLabel xml:lang="de">Diamikt</skos:prefLabel>
	<skos:exactMatch rdf:resource="http://dbpedia.org/resource/Diamicton"/>
	<colourHexCode xmlns="http://dbpedia.org/ontology/">#F2F2BF</colourHexCode>
	<dcterms:references rdf:resource="https://resource.geosphere.at/thes/citation/229"/>
	<skos:definition xml:lang="de">Schlecht sortiertes bis unsortiertes klastisches Sediment, welches als Komponenten Kies und/oder Schutt enthält und eine siltig-tonige Matrix aufweist. Stellt das unverfestigte Äquivalent von Diamiktit dar und zeigt ein matrixgestütztes Gefüge. Ist als nicht genetischer Term zu verstehen, der jedoch auch genetisch eindeutige Begriffe wie Till umfasst (nach Neuendorf et al., 2005; Füchtbauer, 1988).</skos:definition>
	<dcterms:date rdf:datatype="http://www.w3.org/2001/XMLSchema#dateTime">2011-03-22T14:52:39Z</dcterms:date>
	<rdf:type rdf:resource="http://www.w3.org/2004/02/skos/core#Concept"/>
	<skos:prefLabel xml:lang="en">Diamicton</skos:prefLabel>
	<skos:exactMatch rdf:resource="http://data.bgs.ac.uk/id/EarthMaterialClass/RockName/DMTN"/>
	<dcterms:created rdf:datatype="http://www.w3.org/2001/XMLSchema#dateTime">2012-03-12T12:39:04.000Z</dcterms:created>
	<skos:related rdf:resource="https://resource.geosphere.at/thes/lith/183"/>
	<dcterms:references rdf:resource="https://resource.geosphere.at/thes/citation/545"/>
</rdf:Description>

<rdf:Description rdf:about="https://resource.geosphere.at/thes/lith/218">
	<skos:narrower rdf:resource="https://resource.geosphere.at/thes/lith/219"/>
	<skos:narrower rdf:resource="https://resource.geosphere.at/thes/lith/220"/>
	<skos:narrower rdf:resource="https://resource.geosphere.at/thes/lith/221"/>
	<colourHexCode xmlns="http://dbpedia.org/ontology/">#FFFFB2</colourHexCode>
	<rdf:type rdf:resource="http://www.w3.org/2004/02/skos/core#Concept"/>
	<dcterms:references rdf:resource="https://resource.geosphere.at/thes/citation/78"/>
	<skos:definition xml:lang="en">A clastic sediment with a median grain size between 0.063 and 2 mm (Füchtbauer, 1988; DIN 4022).</skos:definition>
	<skos:exactMatch rdf:resource="http://resource.geosciml.org/classifier/cgi/lithology/sand"/>
	<skos:exactMatch rdf:resource="http://dbpedia.org/resource/Sand"/>
	<dcterms:date rdf:datatype="http://www.w3.org/2001/XMLSchema#dateTime">2011-03-22T14:52:39Z</dcterms:date>
	<dcterms:hasVersion rdf:datatype="http://www.w3.org/2001/XMLSchema#int">11</dcterms:hasVersion>
	<skos:related rdf:resource="https://resource.geosphere.at/thes/lith/177"/>
	<skos:prefLabel xml:lang="de">Sand</skos:prefLabel>
	<skos:prefLabel xml:lang="en">Sand</skos:prefLabel>
	<skos:exactMatch rdf:resource="http://www.wikidata.org/entity/Q34679"/>
	<dcterms:references rdf:resource="https://resource.geosphere.at/thes/citation/229"/>
	<dcterms:created rdf:datatype="http://www.w3.org/2001/XMLSchema#dateTime">2012-03-12T16:14:14.000Z</dcterms:created>
	<skos:exactMatch rdf:resource="http://data.bgs.ac.uk/id/EarthMaterialClass/RockName/SANDU"/>
	<skos:exactMatch rdf:resource="http://inspire.ec.europa.eu/codelist/LithologyValue/sand"/>
	<skos:definition xml:lang="de">Klastisches Sediment mit einer medianen Korngröße &gt; 0.063 mm und ≤ 2 mm (Füchtbauer, 1988; DIN 4022).</skos:definition>
</rdf:Description>

<rdf:Description rdf:about="https://resource.geosphere.at/thes/lith/219">
	<rdf:type rdf:resource="http://www.w3.org/2004/02/skos/core#Concept"/>
	<skos:definition xml:lang="de">Klastisches Sediment mit einer medianen Korngröße &gt; 0.63 mm und ≤ 2 mm (Füchtbauer, 1988; DIN 4022).</skos:definition>
	<skos:related rdf:resource="https://resource.geosphere.at/thes/lith/178"/>
	<skos:broadMatch rdf:resource="http://resource.geosciml.org/classifier/cgi/lithology/sand"/>
	<skos:prefLabel xml:lang="de">Grobsand</skos:prefLabel>
	<skos:prefLabel xml:lang="en">Coarse sand</skos:prefLabel>
	<dcterms:references rdf:resource="https://resource.geosphere.at/thes/citation/78"/>
	<skos:broadMatch rdf:resource="http://inspire.ec.europa.eu/codelist/LithologyValue/sand"/>
	<skos:definition xml:lang="en">A clastic sediment with a median grain size between 0.63 and 2 mm (Füchtbauer, 1988; DIN 4022).</skos:definition>
	<dcterms:hasVersion rdf:datatype="http://www.w3.org/2001/XMLSchema#int">12</dcterms:hasVersion>
	<dcterms:references rdf:resource="https://resource.geosphere.at/thes/citation/229"/>
	<dcterms:created rdf:datatype="http://www.w3.org/2001/XMLSchema#dateTime">2012-03-12T12:15:54.000Z</dcterms:created>
	<dcterms:date rdf:datatype="http://www.w3.org/2001/XMLSchema#dateTime">2011-03-22T14:52:39Z</dcterms:date>
</rdf:Description>

<rdf:Description rdf:about="https://resource.geosphere.at/thes/lith/221">
	<foaf:depiction rdf:resource="https://resource.geosphere.at/img/thes/Feinsand.jpg"/>
	<skos:prefLabel xml:lang="de">Feinsand</skos:prefLabel>
	<dcterms:date rdf:datatype="http://www.w3.org/2001/XMLSchema#dateTime">2011-03-22T14:52:39Z</dcterms:date>
	<rdf:type rdf:resource="http://www.w3.org/2004/02/skos/core#Concept"/>
	<dcterms:references rdf:resource="https://resource.geosphere.at/thes/citation/229"/>
	<skos:related rdf:resource="https://resource.geosphere.at/thes/lith/180"/>
	<skos:broadMatch rdf:resource="http://inspire.ec.europa.eu/codelist/LithologyValue/sand"/>
	<skos:broadMatch rdf:resource="http://resource.geosciml.org/classifier/cgi/lithology/sand"/>
	<dcterms:created rdf:datatype="http://www.w3.org/2001/XMLSchema#dateTime">2013-04-05T09:26:33.000Z</dcterms:created>
	<skos:prefLabel xml:lang="en">Fine sand</skos:prefLabel>
	<skos:definition xml:lang="de">Klastisches Sediment mit einer medianen Korngröße &gt; 0.063 mm und ≤ 0.2 mm (Füchtbauer, 1988; DIN 4022).</skos:definition>
	<dcterms:references rdf:resource="https://resource.geosphere.at/thes/citation/78"/>
	<skos:definition xml:lang="en">A clastic sediment with a median grain size between 0.063 and 0.2 mm (Füchtbauer, 1988; DIN 4022).</skos:definition>
	<dcterms:hasVersion rdf:datatype="http://www.w3.org/2001/XMLSchema#int">12</dcterms:hasVersion>
</rdf:Description>

<rdf:Description rdf:about="https://resource.geosphere.at/thes/lith/220">
	<dcterms:created rdf:datatype="http://www.w3.org/2001/XMLSchema#dateTime">2013-04-05T09:35:52.000Z</dcterms:created>
	<rdf:type rdf:resource="http://www.w3.org/2004/02/skos/core#Concept"/>
	<foaf:depiction rdf:resource="https://resource.geosphere.at/img/thes/Mittelsand.jpg"/>
	<skos:related rdf:resource="https://resource.geosphere.at/thes/lith/179"/>
	<skos:broadMatch rdf:resource="http://resource.geosciml.org/classifier/cgi/lithology/sand"/>
	<skos:prefLabel xml:lang="de">Mittelsand</skos:prefLabel>
	<skos:definition xml:lang="en">A clastic sediment with a median grain size &gt; 0.2 mm and ≤ 0.63 mm (Füchtbauer. 1988; DIN 4022).</skos:definition>
	<skos:definition xml:lang="de">Klastisches Sediment mit einer medianen Korngröße &gt; 0.2 mm und ≤ 0.63 mm (Füchtbauer, 1988; DIN 4022).</skos:definition>
	<dcterms:references rdf:resource="https://resource.geosphere.at/thes/citation/78"/>
	<skos:broadMatch rdf:resource="http://inspire.ec.europa.eu/codelist/LithologyValue/sand"/>
	<dcterms:hasVersion rdf:datatype="http://www.w3.org/2001/XMLSchema#int">12</dcterms:hasVersion>
	<dcterms:references rdf:resource="https://resource.geosphere.at/thes/citation/229"/>
	<skos:prefLabel xml:lang="en">Medium sand</skos:prefLabel>
	<dcterms:date rdf:datatype="http://www.w3.org/2001/XMLSchema#dateTime">2011-03-22T14:52:39Z</dcterms:date>
</rdf:Description>

<rdf:Description rdf:about="https://resource.geosphere.at/thes/lith/228">
	<rdf:type rdf:resource="http://www.w3.org/2004/02/skos/core#Concept"/>
	<dcterms:references rdf:resource="https://resource.geosphere.at/thes/citation/78"/>
	<skos:closeMatch rdf:resource="http://inspire.ec.europa.eu/codelist/LithologyValue/boulderGravelSizeSediment"/>
	<skos:prefLabel xml:lang="en">Blocks</skos:prefLabel>
	<dcterms:hasVersion rdf:datatype="http://www.w3.org/2001/XMLSchema#int">14</dcterms:hasVersion>
	<skos:closeMatch rdf:resource="http://resource.geosciml.org/classifier/cgi/lithology/boulder_gravel_size_sediment"/>
	<skos:definition xml:lang="de">Klastisches Sediment mit einer medianen Korngröße von &gt; 200 mm (Füchtbauer, 1988; DIN 4022).</skos:definition>
	<skos:altLabel xml:lang="en">Block size sediment</skos:altLabel>
	<dcterms:date rdf:datatype="http://www.w3.org/2001/XMLSchema#dateTime">2011-03-22T14:52:39Z</dcterms:date>
	<dcterms:references rdf:resource="https://resource.geosphere.at/thes/citation/229"/>
	<skos:altLabel xml:lang="de">Blockwerk</skos:altLabel>
	<dcterms:created rdf:datatype="http://www.w3.org/2001/XMLSchema#dateTime">2013-10-21T08:26:58.000Z</dcterms:created>
	<skos:definition xml:lang="en">A clastic sediment with a median grain size &gt; 200 mm (Füchtbauer, 1988; DIN 4022).</skos:definition>
	<skos:prefLabel xml:lang="de">Blöcke</skos:prefLabel>
</rdf:Description>

<rdf:Description rdf:about="https://resource.geosphere.at/thes/lith/230">
	<skos:definition xml:lang="de">Karbonatisch-klastisches Sediment, dessen klastischer Anteil sich auf die Tonfraktion beschränkt. Besteht aus 25 bis 75 % Ton und 25-75% Dolomit. Kommt im Vergleich zu kalkigen Mergeln nur untergeordnet vor (Vinx, 2005; Füchtbauer, 1988).</skos:definition>
	<dcterms:hasVersion rdf:datatype="http://www.w3.org/2001/XMLSchema#int">13</dcterms:hasVersion>
	<skos:definition xml:lang="en">A mixed carbonate-clastic sediment in which the clastic portion is restricted to clay-sized components. Dolomitic marl consists of 25-75% clay and 25-75% of dolomite. Dolomitic marl is less common than calcareous marl (Vinx, 2005; Füchtbauer, 1988).</skos:definition>
	<dcterms:references rdf:resource="https://resource.geosphere.at/thes/citation/878"/>
	<skos:closeMatch rdf:resource="http://resource.geosciml.org/classifier/cgi/lithology/impure_dolomitic_sediment"/>
	<skos:prefLabel xml:lang="en">Dolomitic marl</skos:prefLabel>
	<dcterms:references rdf:resource="https://resource.geosphere.at/thes/citation/229"/>
	<skos:closeMatch rdf:resource="http://inspire.ec.europa.eu/codelist/LithologyValue/impureDolomiticSediment"/>
	<dcterms:date rdf:datatype="http://www.w3.org/2001/XMLSchema#dateTime">2011-03-22T14:52:39Z</dcterms:date>
	<rdf:type rdf:resource="http://www.w3.org/2004/02/skos/core#Concept"/>
	<skos:prefLabel xml:lang="de">Dolomitischer Mergel</skos:prefLabel>
	<skos:related rdf:resource="https://resource.geosphere.at/thes/lith/190"/>
	<dcterms:created rdf:datatype="http://www.w3.org/2001/XMLSchema#dateTime">2012-03-12T14:23:10.000Z</dcterms:created>
</rdf:Description>

<rdf:Description rdf:about="https://resource.geosphere.at/thes/lith/240">
	<skos:closeMatch rdf:resource="http://resource.geosciml.org/classifier/cgi/lithology/mud_size_sediment"/>
	<dcterms:date rdf:datatype="http://www.w3.org/2001/XMLSchema#dateTime">2011-03-22T14:52:39Z</dcterms:date>
	<skos:definition xml:lang="en">A clastic sediment comprising a mixture of sand, silt, and clay, often exhibiting a yellow/brown colour and usually free of carbonate material (occasionally with minor carbonate). Loam often forms as an alteration product of pre-existing unconsolidated or consolidated rocks. The term includes loess , altered (in situ) loam, and transported loam (modified from Neuendorf et al., 2005).</skos:definition>
	<skos:prefLabel xml:lang="de">Lehm</skos:prefLabel>
	<dcterms:references rdf:resource="https://resource.geosphere.at/thes/citation/545"/>
	<skos:prefLabel xml:lang="en">Loam</skos:prefLabel>
	<skos:exactMatch rdf:resource="http://dbpedia.org/resource/Loam"/>
	<dcterms:created rdf:datatype="http://www.w3.org/2001/XMLSchema#dateTime">2012-03-12T14:04:28.000Z</dcterms:created>
	<skos:closeMatch rdf:resource="http://inspire.ec.europa.eu/codelist/LithologyValue/mudSizeSediment"/>
	<skos:definition xml:lang="de">Klastisches Sediment, das eine Mischung aus Sand, Silt &amp; Ton darstellt und meist gelblich/braun und in der Regel kalkfrei (selten kalkarm) ist. Meist ein Verwitterungsprodukt aus Locker/Festgesteinen. Das Konzept umfasst Lösslehm, Verwitterungslehm, Umlagerungslehm (verändert nach Neuendorf et al., 2005).</skos:definition>
	<dcterms:hasVersion rdf:datatype="http://www.w3.org/2001/XMLSchema#int">9</dcterms:hasVersion>
	<rdf:type rdf:resource="http://www.w3.org/2004/02/skos/core#Concept"/>
	<colourHexCode xmlns="http://dbpedia.org/ontology/">#FFFF00</colourHexCode>
</rdf:Description>

<rdf:Description rdf:about="https://resource.geosphere.at/thes/lith/232">
	<rdf:type rdf:resource="http://www.w3.org/2004/02/skos/core#Concept"/>
	<skos:closeMatch rdf:resource="http://inspire.ec.europa.eu/codelist/LithologyValue/impureCalcareousCarbonateSediment"/>
	<skos:definition xml:lang="de">Karbonatisch-klastisches Sediment, dessen klastischer Anteil sich auf die Tonfraktion beschränkt. Besteht aus 25–75 % Ton und 25-75% Calcit (Vinx, 2005; Füchtbauer, 1988).</skos:definition>
	<skos:definition xml:lang="en">A mixed carbonate-clastic sediment in which the clastic portion is restricted to clay-sized components. Marl consists of 25-75% clay and 25-75% of calcite (Vinx, 2005; Füchtbauer, 1988).</skos:definition>
	<skos:closeMatch rdf:resource="http://resource.geosciml.org/classifier/cgi/lithology/impure_calcareous_carbonate_sediment"/>
	<foaf:depiction rdf:resource="https://resource.geosphere.at/img/thes/Mergel.jpg"/>
	<skos:prefLabel xml:lang="de">Mergel</skos:prefLabel>
	<skos:exactMatch rdf:resource="http://www.wikidata.org/entity/Q184053"/>
	<dcterms:references rdf:resource="https://resource.geosphere.at/thes/citation/878"/>
	<skos:related rdf:resource="https://resource.geosphere.at/thes/lith/192"/>
	<dcterms:hasVersion rdf:datatype="http://www.w3.org/2001/XMLSchema#int">15</dcterms:hasVersion>
	<skos:prefLabel xml:lang="en">Marl</skos:prefLabel>
	<dcterms:references rdf:resource="https://resource.geosphere.at/thes/citation/229"/>
	<dcterms:created rdf:datatype="http://www.w3.org/2001/XMLSchema#dateTime">2013-04-05T09:35:18.000Z</dcterms:created>
	<skos:narrower rdf:resource="https://resource.geosphere.at/thes/lith/231"/>
	<skos:narrower rdf:resource="https://resource.geosphere.at/thes/lith/233"/>
	<dcterms:date rdf:datatype="http://www.w3.org/2001/XMLSchema#dateTime">2011-03-22T14:52:39Z</dcterms:date>
	<skos:exactMatch rdf:resource="http://dbpedia.org/resource/Marl"/>
	<colourHexCode xmlns="http://dbpedia.org/ontology/">#DEEFFE</colourHexCode>
</rdf:Description>

<rdf:Description rdf:about="https://resource.geosphere.at/thes/lith/233">
	<skos:definition xml:lang="de">Karbonatisch-klastisches Sediment, dessen klastischer Anteil sich auf die Tonfraktion beschränkt. Besteht aus 25–50 % Ton und 50–75 % Calcit (Vinx, 2005; Füchtbauer, 1988).</skos:definition>
	<skos:closeMatch rdf:resource="http://inspire.ec.europa.eu/codelist/LithologyValue/impureCalcareousCarbonateSediment"/>
	<skos:closeMatch rdf:resource="http://resource.geosciml.org/classifier/cgi/lithology/impure_calcareous_carbonate_sediment"/>
	<dcterms:date rdf:datatype="http://www.w3.org/2001/XMLSchema#dateTime">2011-03-22T14:52:39Z</dcterms:date>
	<rdf:type rdf:resource="http://www.w3.org/2004/02/skos/core#Concept"/>
	<dcterms:references rdf:resource="https://resource.geosphere.at/thes/citation/229"/>
	<skos:related rdf:resource="https://resource.geosphere.at/thes/lith/193"/>
	<skos:prefLabel xml:lang="de">Kalkmergel</skos:prefLabel>
	<dcterms:created rdf:datatype="http://www.w3.org/2001/XMLSchema#dateTime">2012-03-12T10:39:09.000Z</dcterms:created>
	<dcterms:hasVersion rdf:datatype="http://www.w3.org/2001/XMLSchema#int">9</dcterms:hasVersion>
	<dcterms:references rdf:resource="https://resource.geosphere.at/thes/citation/878"/>
	<skos:definition xml:lang="en">A mixed carbonate-clastic sediment in which the clastic portion is restricted to clay-sized components. Consists of 25-50% clay and 50-75% calcite (Vinx, 2005; Füchtbauer, 1988).</skos:definition>
	<skos:prefLabel xml:lang="en">Calcareous marl</skos:prefLabel>
</rdf:Description>

<rdf:Description rdf:about="https://resource.geosphere.at/thes/lith/231">
	<skos:related rdf:resource="https://resource.geosphere.at/thes/lith/191"/>
	<dcterms:created rdf:datatype="http://www.w3.org/2001/XMLSchema#dateTime">2012-03-12T12:09:30.000Z</dcterms:created>
	<skos:definition xml:lang="de">Karbonatisch-klastisches Sediment, dessen klastischer Anteil sich auf die Tonfraktion beschränkt. Besteht aus 50–75 % Ton und 25–50 % Calcit (Vinx, 2005; Füchtbauer, 1988).</skos:definition>
	<skos:prefLabel xml:lang="de">Tonmergel</skos:prefLabel>
	<skos:closeMatch rdf:resource="http://inspire.ec.europa.eu/codelist/LithologyValue/impureCalcareousCarbonateSediment"/>
	<rdf:type rdf:resource="http://www.w3.org/2004/02/skos/core#Concept"/>
	<skos:prefLabel xml:lang="en">Clay marl</skos:prefLabel>
	<skos:definition xml:lang="en">A mixed carbonate-clastic sediment in which the clastic portion is restricted to clay-sized components. Clay marl consists of 50-75% clay and 25-50% calcite (Vinx, 2005; Füchtbauer, 1988).</skos:definition>
	<dcterms:hasVersion rdf:datatype="http://www.w3.org/2001/XMLSchema#int">9</dcterms:hasVersion>
	<skos:closeMatch rdf:resource="http://resource.geosciml.org/classifier/cgi/lithology/impure_calcareous_carbonate_sediment"/>
	<dcterms:date rdf:datatype="http://www.w3.org/2001/XMLSchema#dateTime">2011-03-22T14:52:39Z</dcterms:date>
	<dcterms:references rdf:resource="https://resource.geosphere.at/thes/citation/229"/>
	<dcterms:references rdf:resource="https://resource.geosphere.at/thes/citation/878"/>
</rdf:Description>

<rdf:Description rdf:about="https://resource.geosphere.at/thes/lith/2">
	<dcterms:date rdf:datatype="http://www.w3.org/2001/XMLSchema#dateTime">2011-03-15T15:22:10Z</dcterms:date>
	<skos:definition xml:lang="de">Pyroklastika werden durch Fragmentierung in Folge von explosiven vulkanischen Eruptionen oder Prozessen gebildet. Sie sind verfestigte oder unverfestigte Ablagerungen aus Pyroklasten, die einen Volumenanteil von &gt; 75 % ausmachen müssen (Le Maitre et al., 2005).</skos:definition>
	<skos:exactMatch rdf:resource="http://resource.geosciml.org/classifier/cgi/lithology/pyroclastic_material"/>
	<skos:prefLabel xml:lang="de">Pyroklastika</skos:prefLabel>
	<skos:scopeNote xml:lang="de">Die Gliederung der Pyroklastika ist rein deskriptiv und erfolgt auf Basis der durchschnittlichen Pyroklastengröße.</skos:scopeNote>
	<skos:exactMatch rdf:resource="http://inspire.ec.europa.eu/codelist/LithologyValue/pyroclasticRock"/>
	<rdf:type rdf:resource="http://www.w3.org/2004/02/skos/core#Concept"/>
</rdf:Description>

<rdf:Description rdf:about="https://resource.geosphere.at/thes/lith/256">
	<dcterms:created rdf:datatype="http://www.w3.org/2001/XMLSchema#dateTime">2025-09-18T14:13:37.662Z</dcterms:created>
	<skos:topConceptOf rdf:resource="https://resource.geosphere.at/thes/lith/0"/>
	<rdf:type rdf:resource="http://www.w3.org/2004/02/skos/core#Concept"/>
	<skos:prefLabel xml:lang="de">Gestein</skos:prefLabel>
</rdf:Description>

<rdf:Description rdf:about="https://resource.geosphere.at/thes/lith/0">
	<skos:hasTopConcept rdf:resource="https://resource.geosphere.at/thes/lith/256"/>
</rdf:Description>

<rdf:Description rdf:about="https://resource.geosphere.at/thes/lith/256">
	<skos:prefLabel xml:lang="en">Rock</skos:prefLabel>
	<dcterms:modified rdf:datatype="http://www.w3.org/2001/XMLSchema#dateTime">2025-09-30T14:50:29.785Z</dcterms:modified>
	<skos:definition xml:lang="de">Ein Gestein tritt zumeist als heterogenes Mineralaggregat aus einem oder verschiedenen Mineralen auf. Im Vergleich dazu ist die Lithologie die Beschreibung von Gesteinen auf Basis ihrer charakteristischen Merkmale, vorrangig ihrer Zusammensetzung und Textur. Somit ist ein Gesteinsbegriff das Kernelement jeder lithologischen Beschreibung. (aus Linner et al, 2024, S. 11)</skos:definition>
	<skos:definition xml:lang="en">A rock usually occurs as a heterogeneous mineral aggregate of one or more minerals. In comparison, lithology is the description of rocks based on their characteristic features, primarily their composition and texture. Thus, a rock term is the core element of any lithological description. (after Linner et al, 2024, p. 11)</skos:definition>
	<dcterms:references rdf:resource="https://resource.geosphere.at/thes/citation/593"/>
</rdf:Description>

<rdf:Description rdf:about="https://resource.geosphere.at/thes/lith/249">
	<dcterms:references rdf:resource="https://resource.geosphere.at/thes/citation/1320"/>
	<skos:definition xml:lang="de">Material, das bekanntermaßen künstlichen (CGI; abgerufen am 19.09.2025)</skos:definition>
	<skos:definition xml:lang="en">Material known to have artificial (human-related) origin. (CGI; link acce</skos:definition>
</rdf:Description>

<rdf:Description rdf:about="https://resource.geosphere.at/thes/lith/1">
	<skos:scopeNote xml:lang="de">Standard</skos:scopeNote>
</rdf:Description>

<rdf:Description rdf:about="https://resource.geosphere.at/thes/lith/256">
	<skos:scopeNote xml:lang="de">Standard</skos:scopeNote>
	<skos:scopeNote xml:lang="en">standard</skos:scopeNote>
</rdf:Description>

<rdf:Description rdf:about="https://resource.geosphere.at/thes/lith/1">
	<skos:scopeNote xml:lang="en">standard</skos:scopeNote>
	<skos:narrower rdf:resource="https://resource.geosphere.at/thes/lith/257"/>
</rdf:Description>

<rdf:Description rdf:about="https://resource.geosphere.at/thes/lith/257">
	<dcterms:created rdf:datatype="http://www.w3.org/2001/XMLSchema#dateTime">2025-09-19T09:04:11.359Z</dcterms:created>
	<rdf:type rdf:resource="http://www.w3.org/2004/02/skos/core#Concept"/>
	<skos:broader rdf:resource="https://resource.geosphere.at/thes/lith/1"/>
	<skos:prefLabel xml:lang="de">Magmatisches Gestein</skos:prefLabel>
	<skos:prefLabel xml:lang="en">Igneous rock</skos:prefLabel>
	<skos:definition xml:lang="de">Gestein, welches aus (teilweise) geschmolzenem Material (Magma) und als Resultat eines magmatischen Prozesses wie Intrusion und Abkühlung von Magma oder einer vulkanischen Eruption entstanden ist (Neuendorf et al., 2005).</skos:definition>
	<skos:definition xml:lang="de">Rock solidified from molten or partially molten material (magma) as the result of an igneous process such as intrusion and cooling of magma, or volcanic eruption (Neuendorf et al., 2005).</skos:definition>
	<skos:scopeNote xml:lang="de">Standard</skos:scopeNote>
	<skos:scopeNote xml:lang="en">standard</skos:scopeNote>
	<dcterms:references rdf:resource="https://resource.geosphere.at/thes/citation/545"/>
</rdf:Description>

<rdf:Description rdf:about="https://resource.geosphere.at/thes/lith/5">
	<skos:broader rdf:resource="https://resource.geosphere.at/thes/lith/257"/>
</rdf:Description>

<rdf:Description rdf:about="https://resource.geosphere.at/thes/lith/257">
	<skos:narrower rdf:resource="https://resource.geosphere.at/thes/lith/5"/>
	<skos:narrower rdf:resource="https://resource.geosphere.at/thes/lith/7"/>
</rdf:Description>

<rdf:Description rdf:about="https://resource.geosphere.at/thes/lith/7">
	<skos:broader rdf:resource="https://resource.geosphere.at/thes/lith/257"/>
</rdf:Description>

<rdf:Description rdf:about="https://resource.geosphere.at/thes/lith/257">
	<skos:narrower rdf:resource="https://resource.geosphere.at/thes/lith/6"/>
</rdf:Description>

<rdf:Description rdf:about="https://resource.geosphere.at/thes/lith/6">
	<skos:broader rdf:resource="https://resource.geosphere.at/thes/lith/257"/>
</rdf:Description>

<rdf:Description rdf:about="https://resource.geosphere.at/thes/lith/257">
	<dcterms:modified rdf:datatype="http://www.w3.org/2001/XMLSchema#dateTime">2025-09-19T09:08:46.060Z</dcterms:modified>
</rdf:Description>

<rdf:Description rdf:about="https://resource.geosphere.at/thes/lith/5">
	<skos:definition xml:lang="de">Magmatisches Gestein, welches durch langsame Abkühlung eines Magmas entstanden ist und eine grobkörnige Textur (Korngröße über 3 mm) aufweist. Einzelne Kristalle sind mit freiem Auge sichtbar. Die Klassifikation beruht hauptsächslich auf dem QAPF-Doppeldreieck (Le Maitre et al., 2005).</skos:definition>
	<skos:definition xml:lang="en">Igneous rock that formed by slow cooling and has a relatively coarse-grained texture (grain-size larger than 3 mm) in which the individual crystals can be seen with the unaided eye. The classification is mostly based on the QAPF double triangle (Le Maitre et al., 2005).</skos:definition>
	<skos:scopeNote xml:lang="de">Standard</skos:scopeNote>
	<skos:scopeNote xml:lang="en">standard</skos:scopeNote>
	<skos:prefLabel xml:lang="de">Plutonisches Gestein</skos:prefLabel>
	<skos:altLabel xml:lang="de">Plutonit</skos:altLabel>
</rdf:Description>

<rdf:Description rdf:about="https://resource.geosphere.at/thes/lith/50">
	<dcterms:modified rdf:datatype="http://www.w3.org/2001/XMLSchema#dateTime">2025-09-19T11:14:42.286Z</dcterms:modified>
</rdf:Description>

<rdf:Description rdf:about="https://resource.geosphere.at/thes/lith/157">
	<skos:scopeNote xml:lang="de">Standard</skos:scopeNote>
	<skos:scopeNote xml:lang="en">standard</skos:scopeNote>
	<dcterms:modified rdf:datatype="http://www.w3.org/2001/XMLSchema#dateTime">2025-09-19T11:12:22.515Z</dcterms:modified>
</rdf:Description>

<rdf:Description rdf:about="https://resource.geosphere.at/thes/lith/51">
	<skos:scopeNote xml:lang="de">Standard</skos:scopeNote>
	<skos:scopeNote xml:lang="en">standard</skos:scopeNote>
	<dcterms:modified rdf:datatype="http://www.w3.org/2001/XMLSchema#dateTime">2025-09-19T11:13:28.876Z</dcterms:modified>
</rdf:Description>

<rdf:Description rdf:about="https://resource.geosphere.at/thes/lith/52">
	<skos:scopeNote xml:lang="de">Standard</skos:scopeNote>
	<skos:scopeNote xml:lang="en">standard</skos:scopeNote>
	<dcterms:modified rdf:datatype="http://www.w3.org/2001/XMLSchema#dateTime">2025-09-19T11:14:05.447Z</dcterms:modified>
</rdf:Description>

<rdf:Description rdf:about="https://resource.geosphere.at/thes/lith/50">
	<skos:scopeNote xml:lang="de">Standard</skos:scopeNote>
	<skos:scopeNote xml:lang="en">standard</skos:scopeNote>
</rdf:Description>

<rdf:Description rdf:about="https://resource.geosphere.at/thes/lith/93">
	<skos:scopeNote xml:lang="de">Standard</skos:scopeNote>
	<skos:scopeNote xml:lang="en">standard</skos:scopeNote>
	<dcterms:modified rdf:datatype="http://www.w3.org/2001/XMLSchema#dateTime">2025-09-19T11:18:27.811Z</dcterms:modified>
</rdf:Description>

<rdf:Description rdf:about="https://resource.geosphere.at/thes/lith/20">
	<skos:scopeNote xml:lang="de">Standard</skos:scopeNote>
	<skos:scopeNote xml:lang="en">standard</skos:scopeNote>
	<dcterms:modified rdf:datatype="http://www.w3.org/2001/XMLSchema#dateTime">2025-09-19T11:24:25.373Z</dcterms:modified>
</rdf:Description>

<rdf:Description rdf:about="https://resource.geosphere.at/thes/lith/45">
	<skos:scopeNote xml:lang="de">Standard</skos:scopeNote>
	<skos:scopeNote xml:lang="en">standard</skos:scopeNote>
	<dcterms:modified rdf:datatype="http://www.w3.org/2001/XMLSchema#dateTime">2025-09-19T11:27:28.128Z</dcterms:modified>
</rdf:Description>

<rdf:Description rdf:about="https://resource.geosphere.at/thes/lith/46">
	<skos:scopeNote xml:lang="de">Standard</skos:scopeNote>
	<skos:scopeNote xml:lang="en">standard</skos:scopeNote>
	<dcterms:modified rdf:datatype="http://www.w3.org/2001/XMLSchema#dateTime">2025-09-19T11:28:39.240Z</dcterms:modified>
</rdf:Description>

<rdf:Description rdf:about="https://resource.geosphere.at/thes/lith/40">
	<skos:scopeNote xml:lang="de">Standard</skos:scopeNote>
	<skos:scopeNote xml:lang="en">standard</skos:scopeNote>
	<dcterms:modified rdf:datatype="http://www.w3.org/2001/XMLSchema#dateTime">2025-09-19T11:29:59.802Z</dcterms:modified>
</rdf:Description>

<rdf:Description rdf:about="https://resource.geosphere.at/thes/lith/39">
	<skos:scopeNote xml:lang="de">Standard</skos:scopeNote>
	<skos:scopeNote xml:lang="en">standard</skos:scopeNote>
	<dcterms:modified rdf:datatype="http://www.w3.org/2001/XMLSchema#dateTime">2025-09-19T11:30:25.327Z</dcterms:modified>
</rdf:Description>

<rdf:Description rdf:about="https://resource.geosphere.at/thes/lith/44">
	<skos:scopeNote xml:lang="de">Standard</skos:scopeNote>
	<skos:scopeNote xml:lang="en">standard</skos:scopeNote>
	<dcterms:modified rdf:datatype="http://www.w3.org/2001/XMLSchema#dateTime">2025-09-19T11:30:44.673Z</dcterms:modified>
</rdf:Description>

<rdf:Description rdf:about="https://resource.geosphere.at/thes/lith/38">
	<skos:scopeNote xml:lang="de">Standard</skos:scopeNote>
	<skos:scopeNote xml:lang="en">standard</skos:scopeNote>
	<dcterms:modified rdf:datatype="http://www.w3.org/2001/XMLSchema#dateTime">2025-09-19T11:31:08.730Z</dcterms:modified>
</rdf:Description>

<rdf:Description rdf:about="https://resource.geosphere.at/thes/lith/23">
	<skos:scopeNote xml:lang="de">Standard</skos:scopeNote>
	<skos:scopeNote xml:lang="en">standard</skos:scopeNote>
	<dcterms:modified rdf:datatype="http://www.w3.org/2001/XMLSchema#dateTime">2025-09-19T11:33:36.501Z</dcterms:modified>
</rdf:Description>

<rdf:Description rdf:about="https://resource.geosphere.at/thes/lith/57">
	<skos:scopeNote xml:lang="de">Standard</skos:scopeNote>
	<skos:scopeNote xml:lang="en">standard</skos:scopeNote>
	<dcterms:modified rdf:datatype="http://www.w3.org/2001/XMLSchema#dateTime">2025-09-19T11:34:02.511Z</dcterms:modified>
</rdf:Description>

<rdf:Description rdf:about="https://resource.geosphere.at/thes/lith/56">
	<skos:scopeNote xml:lang="de">Standard</skos:scopeNote>
	<skos:scopeNote xml:lang="en">standard</skos:scopeNote>
	<dcterms:modified rdf:datatype="http://www.w3.org/2001/XMLSchema#dateTime">2025-09-19T11:34:23.008Z</dcterms:modified>
</rdf:Description>

<rdf:Description rdf:about="https://resource.geosphere.at/thes/lith/24">
	<skos:prefLabel xml:lang="de">Foid-gabbroisches Gestein</skos:prefLabel>
	<skos:altLabel xml:lang="de">Foid-gabbroides Gestein</skos:altLabel>
	<skos:scopeNote xml:lang="de">Standard</skos:scopeNote>
	<skos:scopeNote xml:lang="en">standard</skos:scopeNote>
	<dcterms:modified rdf:datatype="http://www.w3.org/2001/XMLSchema#dateTime">2025-09-19T11:36:09.653Z</dcterms:modified>
</rdf:Description>

<rdf:Description rdf:about="https://resource.geosphere.at/thes/lith/58">
	<skos:scopeNote xml:lang="de">Standard</skos:scopeNote>
	<skos:scopeNote xml:lang="en">standard</skos:scopeNote>
	<dcterms:modified rdf:datatype="http://www.w3.org/2001/XMLSchema#dateTime">2025-09-19T11:36:40.302Z</dcterms:modified>
</rdf:Description>

<rdf:Description rdf:about="https://resource.geosphere.at/thes/lith/55">
	<skos:scopeNote xml:lang="de">Standard</skos:scopeNote>
	<skos:scopeNote xml:lang="en">standard</skos:scopeNote>
	<dcterms:modified rdf:datatype="http://www.w3.org/2001/XMLSchema#dateTime">2025-09-19T11:37:00.650Z</dcterms:modified>
</rdf:Description>

<rdf:Description rdf:about="https://resource.geosphere.at/thes/lith/19">
	<skos:scopeNote xml:lang="de">Standard</skos:scopeNote>
	<skos:scopeNote xml:lang="en">standard</skos:scopeNote>
	<dcterms:modified rdf:datatype="http://www.w3.org/2001/XMLSchema#dateTime">2025-09-19T11:38:57.338Z</dcterms:modified>
</rdf:Description>

<rdf:Description rdf:about="https://resource.geosphere.at/thes/lith/30">
	<skos:scopeNote xml:lang="de">Standard</skos:scopeNote>
	<skos:scopeNote xml:lang="en">standard</skos:scopeNote>
	<dcterms:modified rdf:datatype="http://www.w3.org/2001/XMLSchema#dateTime">2025-09-19T11:39:17.163Z</dcterms:modified>
</rdf:Description>

<rdf:Description rdf:about="https://resource.geosphere.at/thes/lith/31">
	<skos:scopeNote xml:lang="de">Standard</skos:scopeNote>
	<skos:scopeNote xml:lang="en">standard</skos:scopeNote>
	<dcterms:modified rdf:datatype="http://www.w3.org/2001/XMLSchema#dateTime">2025-09-19T11:39:34.630Z</dcterms:modified>
</rdf:Description>

<rdf:Description rdf:about="https://resource.geosphere.at/thes/lith/37">
	<skos:scopeNote xml:lang="de">Standard</skos:scopeNote>
	<skos:scopeNote xml:lang="en">standard</skos:scopeNote>
	<dcterms:modified rdf:datatype="http://www.w3.org/2001/XMLSchema#dateTime">2025-09-19T11:39:57.319Z</dcterms:modified>
</rdf:Description>

<rdf:Description rdf:about="https://resource.geosphere.at/thes/lith/34">
	<skos:scopeNote xml:lang="de">Standard</skos:scopeNote>
	<skos:scopeNote xml:lang="en">standard</skos:scopeNote>
	<dcterms:modified rdf:datatype="http://www.w3.org/2001/XMLSchema#dateTime">2025-09-19T11:40:16.365Z</dcterms:modified>
</rdf:Description>

<rdf:Description rdf:about="https://resource.geosphere.at/thes/lith/36">
	<skos:scopeNote xml:lang="de">Standard</skos:scopeNote>
	<skos:scopeNote xml:lang="en">standard</skos:scopeNote>
	<dcterms:modified rdf:datatype="http://www.w3.org/2001/XMLSchema#dateTime">2025-09-19T11:41:41.418Z</dcterms:modified>
</rdf:Description>

<rdf:Description rdf:about="https://resource.geosphere.at/thes/lith/29">
	<skos:scopeNote xml:lang="de">Standard</skos:scopeNote>
	<skos:scopeNote xml:lang="en">standard</skos:scopeNote>
	<dcterms:modified rdf:datatype="http://www.w3.org/2001/XMLSchema#dateTime">2025-09-19T11:42:08.258Z</dcterms:modified>
</rdf:Description>

<rdf:Description rdf:about="https://resource.geosphere.at/thes/lith/35">
	<skos:scopeNote xml:lang="de">Standard</skos:scopeNote>
	<skos:scopeNote xml:lang="en">standard</skos:scopeNote>
	<dcterms:modified rdf:datatype="http://www.w3.org/2001/XMLSchema#dateTime">2025-09-19T11:42:27.826Z</dcterms:modified>
</rdf:Description>

<rdf:Description rdf:about="https://resource.geosphere.at/thes/lith/32">
	<skos:scopeNote xml:lang="de">Standard</skos:scopeNote>
	<skos:scopeNote xml:lang="en">standard</skos:scopeNote>
	<dcterms:modified rdf:datatype="http://www.w3.org/2001/XMLSchema#dateTime">2025-09-19T11:42:51.372Z</dcterms:modified>
</rdf:Description>

<rdf:Description rdf:about="https://resource.geosphere.at/thes/lith/33">
	<skos:scopeNote xml:lang="de">Standard</skos:scopeNote>
	<skos:scopeNote xml:lang="en">standard</skos:scopeNote>
	<dcterms:modified rdf:datatype="http://www.w3.org/2001/XMLSchema#dateTime">2025-09-19T11:43:27.930Z</dcterms:modified>
</rdf:Description>

<rdf:Description rdf:about="https://resource.geosphere.at/thes/lith/22">
	<skos:scopeNote xml:lang="de">Standard</skos:scopeNote>
	<skos:scopeNote xml:lang="en">standard</skos:scopeNote>
	<dcterms:modified rdf:datatype="http://www.w3.org/2001/XMLSchema#dateTime">2025-09-19T11:44:40.132Z</dcterms:modified>
</rdf:Description>

<rdf:Description rdf:about="https://resource.geosphere.at/thes/lith/54">
	<skos:scopeNote xml:lang="de">Standard</skos:scopeNote>
	<skos:scopeNote xml:lang="en">standard</skos:scopeNote>
	<dcterms:modified rdf:datatype="http://www.w3.org/2001/XMLSchema#dateTime">2025-09-19T11:44:55.708Z</dcterms:modified>
</rdf:Description>

<rdf:Description rdf:about="https://resource.geosphere.at/thes/lith/53">
	<skos:scopeNote xml:lang="de">Standard</skos:scopeNote>
	<skos:scopeNote xml:lang="en">standard</skos:scopeNote>
	<dcterms:modified rdf:datatype="http://www.w3.org/2001/XMLSchema#dateTime">2025-09-19T11:45:18.536Z</dcterms:modified>
</rdf:Description>

<rdf:Description rdf:about="https://resource.geosphere.at/thes/lith/94">
	<skos:scopeNote xml:lang="de">Standard</skos:scopeNote>
	<skos:scopeNote xml:lang="en">standard</skos:scopeNote>
	<dcterms:modified rdf:datatype="http://www.w3.org/2001/XMLSchema#dateTime">2025-09-19T15:28:53.681Z</dcterms:modified>
</rdf:Description>

<rdf:Description rdf:about="https://resource.geosphere.at/thes/lith/21">
	<skos:prefLabel xml:lang="de">Gabbroisches Gestein</skos:prefLabel>
	<skos:altLabel xml:lang="de">Gabbroides Gestein</skos:altLabel>
	<skos:scopeNote xml:lang="de">Standard</skos:scopeNote>
	<skos:scopeNote xml:lang="en">standard</skos:scopeNote>
	<dcterms:modified rdf:datatype="http://www.w3.org/2001/XMLSchema#dateTime">2025-09-19T15:31:01.596Z</dcterms:modified>
</rdf:Description>

<rdf:Description rdf:about="https://resource.geosphere.at/thes/lith/49">
	<skos:scopeNote xml:lang="de">Standard</skos:scopeNote>
	<skos:scopeNote xml:lang="en">standard</skos:scopeNote>
	<dcterms:modified rdf:datatype="http://www.w3.org/2001/XMLSchema#dateTime">2025-09-19T15:31:39.199Z</dcterms:modified>
</rdf:Description>

<rdf:Description rdf:about="https://resource.geosphere.at/thes/lith/43">
	<skos:scopeNote xml:lang="de">Standard</skos:scopeNote>
	<skos:scopeNote xml:lang="en">standard</skos:scopeNote>
	<dcterms:modified rdf:datatype="http://www.w3.org/2001/XMLSchema#dateTime">2025-09-19T15:31:59.227Z</dcterms:modified>
</rdf:Description>

<rdf:Description rdf:about="https://resource.geosphere.at/thes/lith/48">
	<skos:scopeNote xml:lang="de">Standard</skos:scopeNote>
	<skos:scopeNote xml:lang="en">standard</skos:scopeNote>
</rdf:Description>

<rdf:Description rdf:about="https://resource.geosphere.at/thes/lith/42">
	<skos:scopeNote xml:lang="de">Standard</skos:scopeNote>
	<skos:scopeNote xml:lang="en">standard</skos:scopeNote>
	<dcterms:modified rdf:datatype="http://www.w3.org/2001/XMLSchema#dateTime">2025-09-19T15:32:39.189Z</dcterms:modified>
</rdf:Description>

<rdf:Description rdf:about="https://resource.geosphere.at/thes/lith/47">
	<skos:scopeNote xml:lang="de">Standard</skos:scopeNote>
	<skos:scopeNote xml:lang="en">standard</skos:scopeNote>
	<dcterms:modified rdf:datatype="http://www.w3.org/2001/XMLSchema#dateTime">2025-09-19T15:32:57.223Z</dcterms:modified>
</rdf:Description>

<rdf:Description rdf:about="https://resource.geosphere.at/thes/lith/41">
	<skos:scopeNote xml:lang="de">Standard</skos:scopeNote>
	<skos:scopeNote xml:lang="en">standard</skos:scopeNote>
	<dcterms:modified rdf:datatype="http://www.w3.org/2001/XMLSchema#dateTime">2025-09-19T15:33:16.259Z</dcterms:modified>
</rdf:Description>

<rdf:Description rdf:about="https://resource.geosphere.at/thes/lith/6">
	<skos:narrower rdf:resource="https://resource.geosphere.at/thes/lith/95"/>
</rdf:Description>

<rdf:Description rdf:about="https://resource.geosphere.at/thes/lith/95">
	<skos:broader rdf:resource="https://resource.geosphere.at/thes/lith/6"/>
</rdf:Description>

<rdf:Description rdf:about="https://resource.geosphere.at/thes/lith/5">
	<dcterms:modified rdf:datatype="http://www.w3.org/2001/XMLSchema#dateTime">2025-09-19T15:34:48.312Z</dcterms:modified>
</rdf:Description>

<rdf:Description rdf:about="https://resource.geosphere.at/thes/lith/251">
	<dcterms:modified rdf:datatype="http://www.w3.org/2001/XMLSchema#dateTime">2025-09-19T15:36:09.688Z</dcterms:modified>
</rdf:Description>

<rdf:Description rdf:about="https://resource.geosphere.at/thes/lith/18">
	<skos:scopeNote xml:lang="de">Standard</skos:scopeNote>
	<skos:scopeNote xml:lang="en">standard</skos:scopeNote>
	<dcterms:modified rdf:datatype="http://www.w3.org/2001/XMLSchema#dateTime">2025-09-19T15:37:00.595Z</dcterms:modified>
</rdf:Description>

<rdf:Description rdf:about="https://resource.geosphere.at/thes/lith/259">
	<skos:prefLabel xml:lang="de">Gabbronorit</skos:prefLabel>
</rdf:Description>

<rdf:Description rdf:about="https://resource.geosphere.at/thes/lith/48">
	<skos:narrower rdf:resource="https://resource.geosphere.at/thes/lith/259"/>
</rdf:Description>

<rdf:Description rdf:about="https://resource.geosphere.at/thes/lith/259">
	<skos:broader rdf:resource="https://resource.geosphere.at/thes/lith/48"/>
	<dcterms:created rdf:datatype="http://www.w3.org/2001/XMLSchema#dateTime">2025-09-22T12:06:20.838Z</dcterms:created>
	<rdf:type rdf:resource="http://www.w3.org/2004/02/skos/core#Concept"/>
</rdf:Description>

<rdf:Description rdf:about="https://resource.geosphere.at/thes/lith/260">
	<dcterms:created rdf:datatype="http://www.w3.org/2001/XMLSchema#dateTime">2025-09-22T12:06:41.448Z</dcterms:created>
	<skos:broader rdf:resource="https://resource.geosphere.at/thes/lith/48"/>
	<skos:prefLabel xml:lang="de">Hornblende-Gabbro</skos:prefLabel>
	<rdf:type rdf:resource="http://www.w3.org/2004/02/skos/core#Concept"/>
</rdf:Description>

<rdf:Description rdf:about="https://resource.geosphere.at/thes/lith/48">
	<skos:narrower rdf:resource="https://resource.geosphere.at/thes/lith/260"/>
</rdf:Description>

<rdf:Description rdf:about="https://resource.geosphere.at/thes/lith/261">
	<skos:prefLabel xml:lang="de">Norit</skos:prefLabel>
	<rdf:type rdf:resource="http://www.w3.org/2004/02/skos/core#Concept"/>
</rdf:Description>

<rdf:Description rdf:about="https://resource.geosphere.at/thes/lith/48">
	<skos:narrower rdf:resource="https://resource.geosphere.at/thes/lith/261"/>
</rdf:Description>

<rdf:Description rdf:about="https://resource.geosphere.at/thes/lith/261">
	<dcterms:created rdf:datatype="http://www.w3.org/2001/XMLSchema#dateTime">2025-09-22T12:06:51.950Z</dcterms:created>
	<skos:broader rdf:resource="https://resource.geosphere.at/thes/lith/48"/>
</rdf:Description>

<rdf:Description rdf:about="https://resource.geosphere.at/thes/lith/262">
	<dcterms:created rdf:datatype="http://www.w3.org/2001/XMLSchema#dateTime">2025-09-22T12:07:08.112Z</dcterms:created>
	<skos:broader rdf:resource="https://resource.geosphere.at/thes/lith/48"/>
	<rdf:type rdf:resource="http://www.w3.org/2004/02/skos/core#Concept"/>
</rdf:Description>

<rdf:Description rdf:about="https://resource.geosphere.at/thes/lith/48">
	<skos:narrower rdf:resource="https://resource.geosphere.at/thes/lith/262"/>
</rdf:Description>

<rdf:Description rdf:about="https://resource.geosphere.at/thes/lith/263">
	<skos:prefLabel xml:lang="de">Troktolith</skos:prefLabel>
	<rdf:type rdf:resource="http://www.w3.org/2004/02/skos/core#Concept"/>
</rdf:Description>

<rdf:Description rdf:about="https://resource.geosphere.at/thes/lith/48">
	<skos:narrower rdf:resource="https://resource.geosphere.at/thes/lith/263"/>
</rdf:Description>

<rdf:Description rdf:about="https://resource.geosphere.at/thes/lith/263">
	<dcterms:created rdf:datatype="http://www.w3.org/2001/XMLSchema#dateTime">2025-09-22T12:07:31.655Z</dcterms:created>
	<skos:broader rdf:resource="https://resource.geosphere.at/thes/lith/48"/>
</rdf:Description>

<rdf:Description rdf:about="https://resource.geosphere.at/thes/lith/259">
	<skos:prefLabel xml:lang="en">Gabbronorite</skos:prefLabel>
	<skos:scopeNote xml:lang="de">Standard</skos:scopeNote>
	<skos:scopeNote xml:lang="en">standard</skos:scopeNote>
	<skos:definition xml:lang="de">Gabbro, welcher hauptsächlich aus Plagioklas sowie fast gleichen Anteilen von Klinopyroxen und Orthopyroxen besteht (Gillespie &amp; Styles, 1999).</skos:definition>
	<skos:definition xml:lang="en">Gabbro containing mostly plagioclase with almost equal amount of clinopyroxene and orthopyroxene (Gillespie &amp; Styles, 1999).</skos:definition>
	<dcterms:references rdf:resource="https://resource.geosphere.at/thes/citation/665"/>
	<dcterms:modified rdf:datatype="http://www.w3.org/2001/XMLSchema#dateTime">2025-09-22T12:23:13.532Z</dcterms:modified>
</rdf:Description>

<rdf:Description rdf:about="https://resource.geosphere.at/thes/lith/260">
	<dcterms:references rdf:resource="https://resource.geosphere.at/thes/citation/665"/>
</rdf:Description>

<rdf:Description rdf:about="https://resource.geosphere.at/thes/lith/261">
	<dcterms:references rdf:resource="https://resource.geosphere.at/thes/citation/665"/>
</rdf:Description>

<rdf:Description rdf:about="https://resource.geosphere.at/thes/lith/262">
	<dcterms:references rdf:resource="https://resource.geosphere.at/thes/citation/665"/>
</rdf:Description>

<rdf:Description rdf:about="https://resource.geosphere.at/thes/lith/263">
	<dcterms:references rdf:resource="https://resource.geosphere.at/thes/citation/665"/>
</rdf:Description>

<rdf:Description rdf:about="https://resource.geosphere.at/thes/lith/48">
	<dcterms:modified rdf:datatype="http://www.w3.org/2001/XMLSchema#dateTime">2025-09-22T12:23:57.410Z</dcterms:modified>
</rdf:Description>

<rdf:Description rdf:about="https://resource.geosphere.at/thes/lith/263">
	<dcterms:modified rdf:datatype="http://www.w3.org/2001/XMLSchema#dateTime">2025-09-22T12:37:34.002Z</dcterms:modified>
</rdf:Description>

<rdf:Description rdf:about="https://resource.geosphere.at/thes/lith/260">
	<skos:definition xml:lang="de">Gabbro, welcher hauptsächlich aus Plagioklas und Hornblende besteht, mit weniger als 5 Vol.-% Pyroxen. (Gillespie &amp; Styles, 1999)</skos:definition>
	<skos:definition xml:lang="en">Gabbro containing mostly plagioclase and hornblende, with less than 5 % pyroxene by volume. (Gillespie &amp; Styles, 1999)</skos:definition>
</rdf:Description>

<rdf:Description rdf:about="https://resource.geosphere.at/thes/lith/261">
	<skos:scopeNote xml:lang="de">Standard</skos:scopeNote>
	<skos:prefLabel xml:lang="en">Norite</skos:prefLabel>
	<skos:definition xml:lang="de">Gabbro, welcher hauptsächlich aus Plagioklas und Orthopyroxen besteht. (Gillespie &amp; Styles, 1999)</skos:definition>
	<skos:definition xml:lang="en">Gabbro containing mostly plagioclase and orthopyroxene. (Gillespie &amp; Styles, 1999)</skos:definition>
	<dcterms:modified rdf:datatype="http://www.w3.org/2001/XMLSchema#dateTime">2025-09-22T12:33:31.033Z</dcterms:modified>
</rdf:Description>

<rdf:Description rdf:about="https://resource.geosphere.at/thes/lith/262">
	<skos:prefLabel xml:lang="de">Pyroxen-Hornblende-Gabbro</skos:prefLabel>
	<skos:prefLabel xml:lang="en">Pyroxene hornblende gabbro</skos:prefLabel>
	<skos:definition xml:lang="de">Gabbro, welcher hauptsächlich aus Plagioklas sowie fast gleichen Anteilen von Pyroxen und Hornblende besteht. (Gillespie &amp; Styles, 1999)</skos:definition>
	<skos:definition xml:lang="en">Gabbro containing mostly plagioclase with almost equal amount of pyroxene and hornblende. (Gillespie &amp; Styles, 1999)</skos:definition>
	<skos:scopeNote xml:lang="de">Standard</skos:scopeNote>
	<dcterms:modified rdf:datatype="http://www.w3.org/2001/XMLSchema#dateTime">2025-09-22T12:35:46.744Z</dcterms:modified>
</rdf:Description>

<rdf:Description rdf:about="https://resource.geosphere.at/thes/lith/260">
	<skos:scopeNote xml:lang="de">Standard</skos:scopeNote>
	<dcterms:modified rdf:datatype="http://www.w3.org/2001/XMLSchema#dateTime">2025-09-22T12:35:58.305Z</dcterms:modified>
</rdf:Description>

<rdf:Description rdf:about="https://resource.geosphere.at/thes/lith/263">
	<skos:prefLabel xml:lang="en">Troctolite</skos:prefLabel>
	<skos:definition xml:lang="de">Gabbro, welcher hauptsächlich aus Plagioklas und Olivin besteht. (Gillespie &amp; Styles, 1999)</skos:definition>
	<skos:definition xml:lang="en">Gabbro containing mostly plagioclase and olivine. (Gillespie &amp; Styles, 1999)</skos:definition>
	<skos:scopeNote xml:lang="de">Standard</skos:scopeNote>
</rdf:Description>

<rdf:Description rdf:about="https://resource.geosphere.at/thes/lith/5">
	<skos:narrower rdf:resource="https://resource.geosphere.at/thes/lith/264"/>
</rdf:Description>

<rdf:Description rdf:about="https://resource.geosphere.at/thes/lith/264">
	<dcterms:created rdf:datatype="http://www.w3.org/2001/XMLSchema#dateTime">2025-09-22T12:43:05.466Z</dcterms:created>
	<skos:prefLabel xml:lang="de">Orbiculit</skos:prefLabel>
	<skos:broader rdf:resource="https://resource.geosphere.at/thes/lith/5"/>
	<rdf:type rdf:resource="http://www.w3.org/2004/02/skos/core#Concept"/>
	<skos:prefLabel xml:lang="en">Orbiculite</skos:prefLabel>
	<skos:definition xml:lang="de">Plutonisches Gestein mit einer ungewöhnlichen magmatischen Struktur. Kugelige oder kugelähnliche Gebilde, sogenannte Orbicule, befinden sich in einer körnigen oder porphyrischen Grundmasse. Die Orbicule gliedern sich in einen Kern- und konzentrisch strukturierten Randbereich (Schalen). Diese extrem seltenen Strukturen finden sich in verschiedenster chemischer und mineralogischer Zusammensetzung, dabei bevorzugt in granitischen und dioritischen Gesteinen (Meyer, 1989). (aus Linner et al., 2024)</skos:definition>
	<skos:definition xml:lang="en">Plutonic rock with an uncommon magmatic structure. The typical feature are spheroidal structures, called orbicules, within a granular or porphyric matrix. The orbicules contain a core in the middle surrounded by a concentric structured rim (shells). This extremely rare structures occur preferentially in granitic and dioritic rocks, but cover a wide range of chemical and mineralogical composition (Meyer, 1989). (from Linner et al., 2024)</skos:definition>
	<skos:scopeNote xml:lang="de">Standard</skos:scopeNote>
	<dcterms:modified rdf:datatype="http://www.w3.org/2001/XMLSchema#dateTime">2025-09-22T12:44:57.334Z</dcterms:modified>
</rdf:Description>

<rdf:Description rdf:about="https://resource.geosphere.at/thes/lith/265">
	<dcterms:created rdf:datatype="http://www.w3.org/2001/XMLSchema#dateTime">2025-09-22T12:46:09.086Z</dcterms:created>
	<skos:broader rdf:resource="https://resource.geosphere.at/thes/lith/5"/>
	<rdf:type rdf:resource="http://www.w3.org/2004/02/skos/core#Concept"/>
</rdf:Description>

<rdf:Description rdf:about="https://resource.geosphere.at/thes/lith/5">
	<skos:narrower rdf:resource="https://resource.geosphere.at/thes/lith/265"/>
</rdf:Description>

<rdf:Description rdf:about="https://resource.geosphere.at/thes/lith/265">
	<skos:prefLabel xml:lang="de">Charnockitisches Gestein</skos:prefLabel>
</rdf:Description>

<rdf:Description rdf:about="https://resource.geosphere.at/thes/lith/266">
	<dcterms:created rdf:datatype="http://www.w3.org/2001/XMLSchema#dateTime">2025-09-22T12:46:38.791Z</dcterms:created>
	<skos:prefLabel xml:lang="de">Alkalifeldspat-Charnockit</skos:prefLabel>
</rdf:Description>

<rdf:Description rdf:about="https://resource.geosphere.at/thes/lith/265">
	<skos:narrower rdf:resource="https://resource.geosphere.at/thes/lith/266"/>
</rdf:Description>

<rdf:Description rdf:about="https://resource.geosphere.at/thes/lith/266">
	<skos:broader rdf:resource="https://resource.geosphere.at/thes/lith/265"/>
	<rdf:type rdf:resource="http://www.w3.org/2004/02/skos/core#Concept"/>
</rdf:Description>

<rdf:Description rdf:about="https://resource.geosphere.at/thes/lith/265">
	<skos:narrower rdf:resource="https://resource.geosphere.at/thes/lith/267"/>
</rdf:Description>

<rdf:Description rdf:about="https://resource.geosphere.at/thes/lith/267">
	<skos:broader rdf:resource="https://resource.geosphere.at/thes/lith/265"/>
	<dcterms:created rdf:datatype="http://www.w3.org/2001/XMLSchema#dateTime">2025-09-22T12:46:48.267Z</dcterms:created>
	<skos:prefLabel xml:lang="de">Charnockit</skos:prefLabel>
	<rdf:type rdf:resource="http://www.w3.org/2004/02/skos/core#Concept"/>
</rdf:Description>

<rdf:Description rdf:about="https://resource.geosphere.at/thes/lith/268">
	<rdf:type rdf:resource="http://www.w3.org/2004/02/skos/core#Concept"/>
	<skos:prefLabel xml:lang="de">Enderbit</skos:prefLabel>
	<dcterms:created rdf:datatype="http://www.w3.org/2001/XMLSchema#dateTime">2025-09-22T12:46:57.046Z</dcterms:created>
	<skos:broader rdf:resource="https://resource.geosphere.at/thes/lith/265"/>
</rdf:Description>

<rdf:Description rdf:about="https://resource.geosphere.at/thes/lith/265">
	<skos:narrower rdf:resource="https://resource.geosphere.at/thes/lith/268"/>
</rdf:Description>

<rdf:Description rdf:about="https://resource.geosphere.at/thes/lith/269">
	<skos:broader rdf:resource="https://resource.geosphere.at/thes/lith/265"/>
</rdf:Description>

<rdf:Description rdf:about="https://resource.geosphere.at/thes/lith/265">
	<skos:narrower rdf:resource="https://resource.geosphere.at/thes/lith/269"/>
</rdf:Description>

<rdf:Description rdf:about="https://resource.geosphere.at/thes/lith/269">
	<dcterms:created rdf:datatype="http://www.w3.org/2001/XMLSchema#dateTime">2025-09-22T12:47:04.507Z</dcterms:created>
	<rdf:type rdf:resource="http://www.w3.org/2004/02/skos/core#Concept"/>
	<skos:prefLabel xml:lang="de">Jotunit</skos:prefLabel>
</rdf:Description>

<rdf:Description rdf:about="https://resource.geosphere.at/thes/lith/270">
	<rdf:type rdf:resource="http://www.w3.org/2004/02/skos/core#Concept"/>
	<dcterms:created rdf:datatype="http://www.w3.org/2001/XMLSchema#dateTime">2025-09-22T12:47:10.457Z</dcterms:created>
	<skos:broader rdf:resource="https://resource.geosphere.at/thes/lith/265"/>
	<skos:prefLabel xml:lang="de">Mangerit</skos:prefLabel>
</rdf:Description>

<rdf:Description rdf:about="https://resource.geosphere.at/thes/lith/265">
	<skos:narrower rdf:resource="https://resource.geosphere.at/thes/lith/270"/>
	<skos:narrower rdf:resource="https://resource.geosphere.at/thes/lith/271"/>
</rdf:Description>

<rdf:Description rdf:about="https://resource.geosphere.at/thes/lith/271">
	<skos:broader rdf:resource="https://resource.geosphere.at/thes/lith/265"/>
	<skos:prefLabel xml:lang="de">Opdalit</skos:prefLabel>
	<rdf:type rdf:resource="http://www.w3.org/2004/02/skos/core#Concept"/>
	<dcterms:created rdf:datatype="http://www.w3.org/2001/XMLSchema#dateTime">2025-09-22T12:47:16.783Z</dcterms:created>
</rdf:Description>

<rdf:Description rdf:about="https://resource.geosphere.at/thes/lith/265">
	<skos:scopeNote xml:lang="de">Standard</skos:scopeNote>
	<skos:prefLabel xml:lang="en">Charnockitic rock</skos:prefLabel>
	<skos:definition xml:lang="de">Plutonisches Gestein, welches durch das Vorhandensein von Orthopyroxen und häufiges Auftreten von Perthit, Mesoperthit oder Antiperthit gekennzeichnet ist (Streckeisen, 1976). Die Klassifikation beruht auf der oberen Hälfte des QAPF-Doppeldreiecks (Le Maitre et al., 2005).</skos:definition>
	<skos:definition xml:lang="en">Plutonic rock characterized by the presence of orthopyroxene and, in many of the rocks, perthite, mesoperthite or antiperthite (Streckeisen, 1976). The classification is based on the upper half of the QAPF double triangle (Le Maitre et al., 2005).</skos:definition>
</rdf:Description>

<rdf:Description rdf:about="https://resource.geosphere.at/thes/lith/267">
	<dcterms:modified rdf:datatype="http://www.w3.org/2001/XMLSchema#dateTime">2025-09-22T12:52:23.007Z</dcterms:modified>
</rdf:Description>

<rdf:Description rdf:about="https://resource.geosphere.at/thes/lith/265">
	<dcterms:references rdf:resource="https://resource.geosphere.at/thes/citation/477"/>
	<dcterms:modified rdf:datatype="http://www.w3.org/2001/XMLSchema#dateTime">2025-09-22T12:49:36.268Z</dcterms:modified>
</rdf:Description>

<rdf:Description rdf:about="https://resource.geosphere.at/thes/lith/266">
	<dcterms:references rdf:resource="https://resource.geosphere.at/thes/citation/477"/>
</rdf:Description>

<rdf:Description rdf:about="https://resource.geosphere.at/thes/lith/267">
	<dcterms:references rdf:resource="https://resource.geosphere.at/thes/citation/477"/>
</rdf:Description>

<rdf:Description rdf:about="https://resource.geosphere.at/thes/lith/268">
	<dcterms:references rdf:resource="https://resource.geosphere.at/thes/citation/477"/>
</rdf:Description>

<rdf:Description rdf:about="https://resource.geosphere.at/thes/lith/269">
	<dcterms:references rdf:resource="https://resource.geosphere.at/thes/citation/477"/>
</rdf:Description>

<rdf:Description rdf:about="https://resource.geosphere.at/thes/lith/270">
	<dcterms:references rdf:resource="https://resource.geosphere.at/thes/citation/477"/>
</rdf:Description>

<rdf:Description rdf:about="https://resource.geosphere.at/thes/lith/271">
	<dcterms:references rdf:resource="https://resource.geosphere.at/thes/citation/477"/>
</rdf:Description>

<rdf:Description rdf:about="https://resource.geosphere.at/thes/lith/266">
	<skos:prefLabel xml:lang="en">Alkali-feldspar charnockite</skos:prefLabel>
	<skos:definition xml:lang="de">Charnockitisches Gestein, welches vergleichbar einem Alkalifeldspat-Granit einen Plagioklasfaktor kleiner als 10 aufweist und typischerweise Orthopyroxen enthält (Le Maitre et al., 2005).</skos:definition>
	<skos:definition xml:lang="en">Charnockitic rock comparable to alkali feldspar granite, in which the plagioclase ratio is lower than 10, and characteristically containing orthopyroxene (Le Maitre et al., 2005).</skos:definition>
	<skos:scopeNote xml:lang="de">Standard</skos:scopeNote>
	<dcterms:modified rdf:datatype="http://www.w3.org/2001/XMLSchema#dateTime">2025-09-22T12:51:22.510Z</dcterms:modified>
</rdf:Description>

<rdf:Description rdf:about="https://resource.geosphere.at/thes/lith/267">
	<skos:prefLabel xml:lang="en">Charnockite</skos:prefLabel>
	<skos:definition xml:lang="de">Charnockitisches Gestein, welches einem Granit vergleichbar aus Quarz und Feldspat in bestimmten Anteilen besteht und typischerweise Orthopyroxen enthält (Le Maitre et al., 2005).</skos:definition>
	<skos:definition xml:lang="en">Charnockitic rock with quartz and feldspar proportions comparable to granite and characteristically contains orthopyroxene (Le Maitre et al., 2005).</skos:definition>
	<skos:notation>Standard</skos:notation>
</rdf:Description>

<rdf:Description rdf:about="https://resource.geosphere.at/thes/lith/268">
	<skos:prefLabel xml:lang="en">Enderbite</skos:prefLabel>
	<skos:scopeNote xml:lang="de">Standard</skos:scopeNote>
	<skos:definition xml:lang="de">Charnockitisches Gestein, welches einem Tonalit vergleichbar aus Quarz und intermediärem Plagioklas besteht und typischerweise Orthopyroxen enthält (Le Maitre et al., 2005).</skos:definition>
	<skos:definition xml:lang="en">Charnockitic rock comparable to tonalite essentially consisting of quartz and intermediate plagioclase, and characteristically containing orthopyroxene (Le Maitre et al., 2005).</skos:definition>
	<dcterms:modified rdf:datatype="http://www.w3.org/2001/XMLSchema#dateTime">2025-09-22T12:59:29.945Z</dcterms:modified>
</rdf:Description>

<rdf:Description rdf:about="https://resource.geosphere.at/thes/lith/269">
	<skos:prefLabel xml:lang="en">Jotunite</skos:prefLabel>
	<skos:scopeNote xml:lang="de">Standard</skos:scopeNote>
	<skos:definition xml:lang="de">Charnockitisches Gestein, welches einem Monzodiorit vergleichbar aus mehr Plagioklas als Alkalifeldspat und einem Quarzanteil kleiner als 5 Vol.-% besteht und typischerweise Orthopyroxen enthält (Le Maitre et al., 2005).</skos:definition>
	<skos:definition xml:lang="en">Charnockitic rock comparable to monzodiorite with more plagioclase than alkali feldspar and the quartz fraction lower than 5 % by volume and characteristically contains orthopyroxene (Le Maitre et al., 2005).</skos:definition>
	<dcterms:modified rdf:datatype="http://www.w3.org/2001/XMLSchema#dateTime">2025-09-22T13:00:44.569Z</dcterms:modified>
</rdf:Description>

<rdf:Description rdf:about="https://resource.geosphere.at/thes/lith/270">
	<skos:prefLabel xml:lang="en">Mangerite</skos:prefLabel>
	<skos:scopeNote xml:lang="de">Standard</skos:scopeNote>
	<skos:definition xml:lang="de">Charnockitisches Gestein, welches einem Monzonit vergleichbar zu gleichen Anteilen aus Plagioklas und Alkalifeldspat besteht und typischerweise Orthopyroxen enthält (Le Maitre et al., 2005).</skos:definition>
	<dcterms:modified rdf:datatype="http://www.w3.org/2001/XMLSchema#dateTime">2025-09-22T13:01:50.236Z</dcterms:modified>
	<skos:definition xml:lang="en">Charnockitic rock comparable to monzonite consisting of approximately equal amounts of plagioclase and alkali feldspar, and which characteristically contains orthopyroxene (Le Maitre et al., 2005).</skos:definition>
</rdf:Description>

<rdf:Description rdf:about="https://resource.geosphere.at/thes/lith/271">
	<skos:prefLabel xml:lang="en">Opdalite</skos:prefLabel>
	<skos:definition xml:lang="de">Charnockitisches Gestein, welches vergleichbar einem Granodiorit aus Quarz, Natrium-Plagioklas (Albit) sowie geringeren Anteilen Alkalifeldspat besteht und typischerweise Orthopyroxen enthält (Le Maitre et al., 2005).</skos:definition>
	<skos:definition xml:lang="en">Charnockitic rock comparable to granodiorite consisting essentially of quartz, sodic plagioclase (albite), as well as smaller quantities of alkali feldspar, and which characteristically contains orthopyroxene (Le Maitre et al., 2005).</skos:definition>
	<dcterms:modified rdf:datatype="http://www.w3.org/2001/XMLSchema#dateTime">2025-09-22T13:02:36.453Z</dcterms:modified>
	<skos:scopeNote xml:lang="de">Standard</skos:scopeNote>
</rdf:Description>

<rdf:Description rdf:about="https://resource.geosphere.at/thes/lith/25">
	<dcterms:modified rdf:datatype="http://www.w3.org/2001/XMLSchema#dateTime">2025-09-22T13:03:42.167Z</dcterms:modified>
	<skos:scopeNote xml:lang="de">Standard</skos:scopeNote>
</rdf:Description>

<rdf:Description rdf:about="https://resource.geosphere.at/thes/lith/26">
	<dcterms:modified rdf:datatype="http://www.w3.org/2001/XMLSchema#dateTime">2025-09-22T13:05:30.402Z</dcterms:modified>
	<skos:scopeNote xml:lang="de">Standard</skos:scopeNote>
</rdf:Description>

<rdf:Description rdf:about="https://resource.geosphere.at/thes/lith/27">
	<skos:scopeNote xml:lang="de">Standard</skos:scopeNote>
	<dcterms:modified rdf:datatype="http://www.w3.org/2001/XMLSchema#dateTime">2025-09-22T13:05:38.021Z</dcterms:modified>
</rdf:Description>

<rdf:Description rdf:about="https://resource.geosphere.at/thes/lith/28">
	<skos:scopeNote xml:lang="de">Standard</skos:scopeNote>
	<dcterms:modified rdf:datatype="http://www.w3.org/2001/XMLSchema#dateTime">2025-09-22T13:05:44.371Z</dcterms:modified>
</rdf:Description>

<rdf:Description rdf:about="https://resource.geosphere.at/thes/lith/59">
	<dcterms:modified rdf:datatype="http://www.w3.org/2001/XMLSchema#dateTime">2025-09-22T13:06:34.619Z</dcterms:modified>
	<skos:scopeNote xml:lang="de">Standard</skos:scopeNote>
</rdf:Description>

<rdf:Description rdf:about="https://resource.geosphere.at/thes/lith/7">
	<skos:scopeNote xml:lang="de">Standard</skos:scopeNote>
	<skos:definition xml:lang="de">Magmatisches Gestein mit einem Farbindex M &gt; 90 %. Der Farbindex entspricht dem Anteil mafischer Minerale wie Olivin, Orthopyroxen, Klinopyroxen, Hornblende und untergeordnet Biotit. Umfasst Ultramafit (ultramafischer Plutonit) und Ultramafitit (ultramafischer Vulkanit). Die Verwendung dieser Begriffe wird jedoch von der IUGS nicht empfohlen (Le Maitre et al., 2005).</skos:definition>
	<dcterms:modified rdf:datatype="http://www.w3.org/2001/XMLSchema#dateTime">2025-09-22T14:27:59.428Z</dcterms:modified>
</rdf:Description>

<rdf:Description rdf:about="https://resource.geosphere.at/thes/lith/272">
	<rdf:type rdf:resource="http://www.w3.org/2004/02/skos/core#Concept"/>
</rdf:Description>

<rdf:Description rdf:about="https://resource.geosphere.at/thes/lith/7">
	<skos:narrower rdf:resource="https://resource.geosphere.at/thes/lith/272"/>
</rdf:Description>

<rdf:Description rdf:about="https://resource.geosphere.at/thes/lith/272">
	<skos:prefLabel xml:lang="de">Chromitfels</skos:prefLabel>
	<skos:broader rdf:resource="https://resource.geosphere.at/thes/lith/7"/>
	<dcterms:created rdf:datatype="http://www.w3.org/2001/XMLSchema#dateTime">2025-09-22T14:28:40.100Z</dcterms:created>
</rdf:Description>

<rdf:Description rdf:about="https://resource.geosphere.at/thes/lith/273">
	<skos:broader rdf:resource="https://resource.geosphere.at/thes/lith/7"/>
</rdf:Description>

<rdf:Description rdf:about="https://resource.geosphere.at/thes/lith/7">
	<skos:narrower rdf:resource="https://resource.geosphere.at/thes/lith/273"/>
</rdf:Description>

<rdf:Description rdf:about="https://resource.geosphere.at/thes/lith/273">
	<rdf:type rdf:resource="http://www.w3.org/2004/02/skos/core#Concept"/>
	<dcterms:created rdf:datatype="http://www.w3.org/2001/XMLSchema#dateTime">2025-09-22T14:28:47.163Z</dcterms:created>
	<skos:prefLabel xml:lang="de">Hornblendit</skos:prefLabel>
	<skos:prefLabel xml:lang="en">Hornblendite</skos:prefLabel>
	<skos:scopeNote xml:lang="de">Standard</skos:scopeNote>
	<skos:definition xml:lang="de">Ultramafisches Gestein, welches hauptsächlich aus Olivin, Pyroxen und Hornblende, mit mehr Hornblende als Pyroxen im relativen Volumenanteil und weniger als 40 Vol.-% Olivin, besteht. (Le Maitre et al., 2005)</skos:definition>
	<skos:definition xml:lang="en">Ultramafic rock formed essentially of olivine, pyroxene and hornblende and containing more hornblende than pyroxene in relative volumetric proportion and less than 40 % olivine by volume. (Le Maitre et al., 2005)</skos:definition>
</rdf:Description>

<rdf:Description rdf:about="https://resource.geosphere.at/thes/lith/272">
	<skos:prefLabel xml:lang="en">Chromitite</skos:prefLabel>
	<skos:scopeNote xml:lang="de">Standard</skos:scopeNote>
	<skos:definition xml:lang="de">Ultramafisches Gestein, welches hauptsächlich aus Chromit (zu mehr als 90 Vol.-%) besteht (Gillespie &amp; Styles, 1999; Le Maitre et al., 2005).</skos:definition>
	<skos:definition xml:lang="en">Ultramafic rock consisting essentially of chromite (more than 90 % by volume; Gillespie &amp; Styles, 1999; Le Maitre et al., 2005).</skos:definition>
</rdf:Description>

<rdf:Description rdf:about="https://resource.geosphere.at/thes/lith/60">
	<skos:scopeNote xml:lang="de">Standard</skos:scopeNote>
</rdf:Description>

<rdf:Description rdf:about="https://resource.geosphere.at/thes/lith/61">
	<skos:scopeNote xml:lang="de">Standard</skos:scopeNote>
</rdf:Description>

<rdf:Description rdf:about="https://resource.geosphere.at/thes/lith/274">
	<rdf:type rdf:resource="http://www.w3.org/2004/02/skos/core#Concept"/>
</rdf:Description>

<rdf:Description rdf:about="https://resource.geosphere.at/thes/lith/60">
	<skos:narrower rdf:resource="https://resource.geosphere.at/thes/lith/274"/>
</rdf:Description>

<rdf:Description rdf:about="https://resource.geosphere.at/thes/lith/274">
	<dcterms:created rdf:datatype="http://www.w3.org/2001/XMLSchema#dateTime">2025-09-22T14:37:59.528Z</dcterms:created>
	<skos:broader rdf:resource="https://resource.geosphere.at/thes/lith/60"/>
	<skos:prefLabel xml:lang="de">Dunit</skos:prefLabel>
</rdf:Description>

<rdf:Description rdf:about="https://resource.geosphere.at/thes/lith/275">
	<skos:prefLabel xml:lang="de">Harzburgit</skos:prefLabel>
	<skos:broader rdf:resource="https://resource.geosphere.at/thes/lith/60"/>
	<dcterms:created rdf:datatype="http://www.w3.org/2001/XMLSchema#dateTime">2025-09-22T14:38:09.567Z</dcterms:created>
	<rdf:type rdf:resource="http://www.w3.org/2004/02/skos/core#Concept"/>
</rdf:Description>

<rdf:Description rdf:about="https://resource.geosphere.at/thes/lith/60">
	<skos:narrower rdf:resource="https://resource.geosphere.at/thes/lith/275"/>
</rdf:Description>

<rdf:Description rdf:about="https://resource.geosphere.at/thes/lith/276">
	<rdf:type rdf:resource="http://www.w3.org/2004/02/skos/core#Concept"/>
</rdf:Description>

<rdf:Description rdf:about="https://resource.geosphere.at/thes/lith/60">
	<skos:narrower rdf:resource="https://resource.geosphere.at/thes/lith/276"/>
</rdf:Description>

<rdf:Description rdf:about="https://resource.geosphere.at/thes/lith/276">
	<skos:broader rdf:resource="https://resource.geosphere.at/thes/lith/60"/>
	<dcterms:created rdf:datatype="http://www.w3.org/2001/XMLSchema#dateTime">2025-09-22T14:38:18.764Z</dcterms:created>
	<skos:prefLabel xml:lang="de">Lherzolith</skos:prefLabel>
</rdf:Description>

<rdf:Description rdf:about="https://resource.geosphere.at/thes/lith/277">
	<dcterms:created rdf:datatype="http://www.w3.org/2001/XMLSchema#dateTime">2025-09-22T14:38:29.650Z</dcterms:created>
	<skos:broader rdf:resource="https://resource.geosphere.at/thes/lith/60"/>
	<rdf:type rdf:resource="http://www.w3.org/2004/02/skos/core#Concept"/>
	<skos:prefLabel xml:lang="de">Wehrlit</skos:prefLabel>
</rdf:Description>

<rdf:Description rdf:about="https://resource.geosphere.at/thes/lith/60">
	<skos:narrower rdf:resource="https://resource.geosphere.at/thes/lith/277"/>
</rdf:Description>

<rdf:Description rdf:about="https://resource.geosphere.at/thes/lith/274">
	<skos:prefLabel xml:lang="en">Dunite</skos:prefLabel>
	<skos:scopeNote xml:lang="de">Standard</skos:scopeNote>
	<skos:definition xml:lang="de">Peridotit, welcher zu mehr als 90 Vol.-% Olivin (normiert auf Olivin, Pyroxen und Hornblende) besteht (Le Maitre et al., 2005).</skos:definition>
	<skos:definition xml:lang="en">Peridotite containing more than 90 % olivine by volume (normalized over olivine, pyroxene, hornblende; Le Maitre et al., 2005).</skos:definition>
</rdf:Description>

<rdf:Description rdf:about="https://resource.geosphere.at/thes/lith/275">
	<skos:prefLabel xml:lang="en">Harzburgite</skos:prefLabel>
	<skos:scopeNote xml:lang="de">Standard</skos:scopeNote>
	<skos:definition xml:lang="de">Peridotit, welcher hauptsächlich aus Olivin, Orthopyroxen und Klinopyroxen mit weniger als 5 Vol.-% Klinopyroxen und weniger als 90 Vol.-% Olivin besteht (Le Maitre et al., 2005).</skos:definition>
	<skos:definition xml:lang="en">Peridotite formed essentially of olivine, orthopyroxene and clinopyroxene, containing less than 5 % clinopyroxene and less than 90 % olivine by volume (Le Maitre et al., 2005).</skos:definition>
</rdf:Description>

<rdf:Description rdf:about="https://resource.geosphere.at/thes/lith/278">
	<skos:prefLabel xml:lang="de">Websterit</skos:prefLabel>
	<skos:broader rdf:resource="https://resource.geosphere.at/thes/lith/61"/>
	<dcterms:created rdf:datatype="http://www.w3.org/2001/XMLSchema#dateTime">2025-09-29T12:19:11.653Z</dcterms:created>
</rdf:Description>

<rdf:Description rdf:about="https://resource.geosphere.at/thes/lith/61">
	<skos:narrower rdf:resource="https://resource.geosphere.at/thes/lith/278"/>
</rdf:Description>

<rdf:Description rdf:about="https://resource.geosphere.at/thes/lith/278">
	<rdf:type rdf:resource="http://www.w3.org/2004/02/skos/core#Concept"/>
</rdf:Description>

<rdf:Description rdf:about="https://resource.geosphere.at/thes/lith/61">
	<skos:narrower rdf:resource="https://resource.geosphere.at/thes/lith/279"/>
</rdf:Description>

<rdf:Description rdf:about="https://resource.geosphere.at/thes/lith/279">
	<skos:prefLabel xml:lang="de">Orthopyroxenit</skos:prefLabel>
	<rdf:type rdf:resource="http://www.w3.org/2004/02/skos/core#Concept"/>
	<dcterms:created rdf:datatype="http://www.w3.org/2001/XMLSchema#dateTime">2025-09-29T12:19:28.777Z</dcterms:created>
	<skos:broader rdf:resource="https://resource.geosphere.at/thes/lith/61"/>
</rdf:Description>

<rdf:Description rdf:about="https://resource.geosphere.at/thes/lith/280">
	<dcterms:created rdf:datatype="http://www.w3.org/2001/XMLSchema#dateTime">2025-09-29T12:19:37.972Z</dcterms:created>
	<rdf:type rdf:resource="http://www.w3.org/2004/02/skos/core#Concept"/>
	<skos:prefLabel xml:lang="de">Klinopyroxenit</skos:prefLabel>
	<skos:broader rdf:resource="https://resource.geosphere.at/thes/lith/61"/>
</rdf:Description>

<rdf:Description rdf:about="https://resource.geosphere.at/thes/lith/61">
	<skos:narrower rdf:resource="https://resource.geosphere.at/thes/lith/280"/>
</rdf:Description>

<rdf:Description rdf:about="https://resource.geosphere.at/thes/lith/281">
	<skos:prefLabel xml:lang="de">Granat-Lherzolith</skos:prefLabel>
</rdf:Description>

<rdf:Description rdf:about="https://resource.geosphere.at/thes/lith/276">
	<skos:narrower rdf:resource="https://resource.geosphere.at/thes/lith/281"/>
</rdf:Description>

<rdf:Description rdf:about="https://resource.geosphere.at/thes/lith/281">
	<rdf:type rdf:resource="http://www.w3.org/2004/02/skos/core#Concept"/>
	<skos:broader rdf:resource="https://resource.geosphere.at/thes/lith/276"/>
	<dcterms:created rdf:datatype="http://www.w3.org/2001/XMLSchema#dateTime">2025-09-29T12:20:09.003Z</dcterms:created>
</rdf:Description>

<rdf:Description rdf:about="https://resource.geosphere.at/thes/lith/282">
	<skos:broader rdf:resource="https://resource.geosphere.at/thes/lith/280"/>
	<dcterms:created rdf:datatype="http://www.w3.org/2001/XMLSchema#dateTime">2025-09-29T12:20:37.630Z</dcterms:created>
	<rdf:type rdf:resource="http://www.w3.org/2004/02/skos/core#Concept"/>
	<skos:prefLabel xml:lang="de">Granat-Klinopyroxenit</skos:prefLabel>
</rdf:Description>

<rdf:Description rdf:about="https://resource.geosphere.at/thes/lith/280">
	<skos:narrower rdf:resource="https://resource.geosphere.at/thes/lith/282"/>
</rdf:Description>

<rdf:Description rdf:about="https://resource.geosphere.at/thes/lith/60">
	<skos:definition xml:lang="en">Ultramafic rock formed essentially of olivine, pyroxene and hornblende, containing more than 40 % olivine by volume (Le Maitre et al., 2005).</skos:definition>
	<skos:definition xml:lang="de">Ultramafisches Gestein, welches hauptsächlich aus Olivin, Pyroxen und Hornblende mit mehr als 40 Vol.-% Olivin besteht (Le Maitre et al., 2005).</skos:definition>
</rdf:Description>

<rdf:Description rdf:about="https://resource.geosphere.at/thes/lith/276">
	<skos:prefLabel xml:lang="en">Lherzolite</skos:prefLabel>
	<skos:scopeNote xml:lang="de">Standard</skos:scopeNote>
	<skos:definition xml:lang="de">Peridotit, welcher hauptsächlich aus Olivin, Orthopyroxen und Klinopyroxen mit mehr als 5 Vol.-% Orthopyroxen, mehr als 5 Vol.-% Klinopyroxen und weniger als 90 Vol.-% Olivin besteht (Le Maitre et al., 2005).</skos:definition>
	<skos:definition xml:lang="en">Peridotite formed essentially of olivine, orthopyroxene and clinopyroxene, containing more than 5 % clinopyroxene, more than 5 % orthopyroxene and less than 90 % olivine by volume (Le Maitre et al., 2005).</skos:definition>
</rdf:Description>

<rdf:Description rdf:about="https://resource.geosphere.at/thes/lith/281">
	<skos:prefLabel xml:lang="en">Garnet lherzolite</skos:prefLabel>
	<skos:scopeNote xml:lang="de">Standard</skos:scopeNote>
	<skos:definition xml:lang="de">Ein Lherzolith, welcher mehr als 5 Vol.-% Granat enthält (Le Maitre et al., 2005).</skos:definition>
	<skos:definition xml:lang="en">Lherzolite containing more than 5 % garnet by volume (Le Maitre et al., 2005).</skos:definition>
</rdf:Description>

<rdf:Description rdf:about="https://resource.geosphere.at/thes/lith/277">
	<skos:prefLabel xml:lang="en">Wehrlite</skos:prefLabel>
	<skos:scopeNote xml:lang="de">Standard</skos:scopeNote>
	<skos:definition xml:lang="de">Peridotit, welcher hauptsächlich aus Olivin, Orthopyroxen und Klinopyroxen mit weniger als 5 Vol.-% Orthopyroxen und weniger als 90 Vol.-% Olivin am Gesamtanteil der genannten drei Minerale besteht (Le Maitre et al., 2005).</skos:definition>
	<skos:definition xml:lang="en">Peridotite formed essentially of olivine, orthopyroxene and clinopyroxene, containing less than 5 % orthopyroxene and less than 90 % olivine by volume among the quoted mineral phases (Le Maitre et al., 2005).</skos:definition>
	<dcterms:modified rdf:datatype="http://www.w3.org/2001/XMLSchema#dateTime">2025-09-29T12:37:22.626Z</dcterms:modified>
</rdf:Description>

<rdf:Description rdf:about="https://resource.geosphere.at/thes/lith/280">
	<skos:prefLabel xml:lang="en">Clinopyroxenite</skos:prefLabel>
	<skos:scopeNote xml:lang="de">Standard</skos:scopeNote>
	<skos:definition xml:lang="de">Pyroxenit, welcher zu mehr als 90 Vol.-% Klinopyroxen (normiert auf Olivin, Klinopyroxen und Orthopyroxen) besteht (Le Maitre et al., 2005).</skos:definition>
	<skos:definition xml:lang="en">Pyroxenite containing more than 90 % clinopyroxene by volume (normalized over olivine, clinopyroxene and orthopyroxene; Le Maitre et al.; 2005).</skos:definition>
	<dcterms:modified rdf:datatype="http://www.w3.org/2001/XMLSchema#dateTime">2025-09-29T12:37:29.620Z</dcterms:modified>
</rdf:Description>

<rdf:Description rdf:about="https://resource.geosphere.at/thes/lith/282">
	<skos:prefLabel xml:lang="en">Garnet clinopyroxenite</skos:prefLabel>
	<skos:scopeNote xml:lang="de">Standard</skos:scopeNote>
	<skos:definition xml:lang="de">Klinopyroxenit, welcher mehr als 5 Vol.-% Granat enthält (Le Maitre et al., 2005).</skos:definition>
	<skos:definition xml:lang="en">Clinopyroxenite containing more than 5 % garnet by volume (Le Maitre et al., 2005).</skos:definition>
</rdf:Description>

<rdf:Description rdf:about="https://resource.geosphere.at/thes/lith/279">
	<skos:prefLabel xml:lang="en">Orthopyroxenite</skos:prefLabel>
	<skos:scopeNote xml:lang="de">Standard</skos:scopeNote>
	<skos:definition xml:lang="de">Pyroxenit, welcher zu mehr als 90 Vol.-% Orthopyroxen (normiert auf Olivin, Klinopyroxen und Orthopyroxen) besteht (Le Maitre et al., 2005).</skos:definition>
	<skos:definition xml:lang="en">Pyroxenite containing more than 90 % orthopyroxene by volume (normalized over olivine, clinopyroxene and orthopyroxene; Le Maitre et al.; 2005).</skos:definition>
	<dcterms:modified rdf:datatype="http://www.w3.org/2001/XMLSchema#dateTime">2025-09-29T12:37:35.491Z</dcterms:modified>
</rdf:Description>

<rdf:Description rdf:about="https://resource.geosphere.at/thes/lith/278">
	<skos:prefLabel xml:lang="en">Websterite</skos:prefLabel>
	<skos:scopeNote xml:lang="de">Standard</skos:scopeNote>
	<skos:definition xml:lang="de">Pyroxenit, welcher hauptsächlich aus Olivin, Klinopyroxen und Orthopyroxen mehr als 10 Vol.-% Orthopyroxen, mehr als 10 Vol.-% Klinopyroxen und weniger als 5 Vol.-% Olivin in relativem Anteil besteht (Le Maitre et al., 2005).</skos:definition>
	<skos:definition xml:lang="en">Pyroxenite formed essentially of olivine, clinopyroxene and orthopyroxene, containing more than 10 % orthopyroxene, more than 10 % clinopyroxene and less than 5 % olivine in relative volumetric proportion (Le Maitre, 2005).</skos:definition>
	<dcterms:modified rdf:datatype="http://www.w3.org/2001/XMLSchema#dateTime">2025-09-29T12:37:38.146Z</dcterms:modified>
</rdf:Description>

<rdf:Description rdf:about="https://resource.geosphere.at/thes/lith/272">
	<dcterms:references rdf:resource="https://resource.geosphere.at/thes/citation/665"/>
	<dcterms:references rdf:resource="https://resource.geosphere.at/thes/citation/477"/>
	<dcterms:modified rdf:datatype="http://www.w3.org/2001/XMLSchema#dateTime">2025-09-29T12:37:04.010Z</dcterms:modified>
</rdf:Description>

<rdf:Description rdf:about="https://resource.geosphere.at/thes/lith/273">
	<dcterms:references rdf:resource="https://resource.geosphere.at/thes/citation/477"/>
	<dcterms:modified rdf:datatype="http://www.w3.org/2001/XMLSchema#dateTime">2025-09-29T12:37:06.730Z</dcterms:modified>
</rdf:Description>

<rdf:Description rdf:about="https://resource.geosphere.at/thes/lith/60">
	<dcterms:modified rdf:datatype="http://www.w3.org/2001/XMLSchema#dateTime">2025-09-29T12:37:09.124Z</dcterms:modified>
</rdf:Description>

<rdf:Description rdf:about="https://resource.geosphere.at/thes/lith/274">
	<dcterms:references rdf:resource="https://resource.geosphere.at/thes/citation/477"/>
	<dcterms:modified rdf:datatype="http://www.w3.org/2001/XMLSchema#dateTime">2025-09-29T12:37:11.466Z</dcterms:modified>
</rdf:Description>

<rdf:Description rdf:about="https://resource.geosphere.at/thes/lith/275">
	<dcterms:references rdf:resource="https://resource.geosphere.at/thes/citation/477"/>
	<dcterms:modified rdf:datatype="http://www.w3.org/2001/XMLSchema#dateTime">2025-09-29T12:37:14.205Z</dcterms:modified>
</rdf:Description>

<rdf:Description rdf:about="https://resource.geosphere.at/thes/lith/276">
	<dcterms:references rdf:resource="https://resource.geosphere.at/thes/citation/477"/>
	<dcterms:modified rdf:datatype="http://www.w3.org/2001/XMLSchema#dateTime">2025-09-29T12:37:16.705Z</dcterms:modified>
</rdf:Description>

<rdf:Description rdf:about="https://resource.geosphere.at/thes/lith/281">
	<dcterms:references rdf:resource="https://resource.geosphere.at/thes/citation/477"/>
	<dcterms:modified rdf:datatype="http://www.w3.org/2001/XMLSchema#dateTime">2025-09-29T12:37:19.808Z</dcterms:modified>
</rdf:Description>

<rdf:Description rdf:about="https://resource.geosphere.at/thes/lith/277">
	<dcterms:references rdf:resource="https://resource.geosphere.at/thes/citation/477"/>
</rdf:Description>

<rdf:Description rdf:about="https://resource.geosphere.at/thes/lith/61">
	<dcterms:modified rdf:datatype="http://www.w3.org/2001/XMLSchema#dateTime">2025-09-29T12:37:25.713Z</dcterms:modified>
</rdf:Description>

<rdf:Description rdf:about="https://resource.geosphere.at/thes/lith/280">
	<dcterms:references rdf:resource="https://resource.geosphere.at/thes/citation/477"/>
</rdf:Description>

<rdf:Description rdf:about="https://resource.geosphere.at/thes/lith/282">
	<dcterms:references rdf:resource="https://resource.geosphere.at/thes/citation/477"/>
	<dcterms:modified rdf:datatype="http://www.w3.org/2001/XMLSchema#dateTime">2025-09-29T12:37:32.441Z</dcterms:modified>
</rdf:Description>

<rdf:Description rdf:about="https://resource.geosphere.at/thes/lith/279">
	<dcterms:references rdf:resource="https://resource.geosphere.at/thes/citation/477"/>
</rdf:Description>

<rdf:Description rdf:about="https://resource.geosphere.at/thes/lith/278">
	<dcterms:references rdf:resource="https://resource.geosphere.at/thes/citation/477"/>
</rdf:Description>

<rdf:Description rdf:about="https://resource.geosphere.at/thes/lith/6">
	<skos:prefLabel xml:lang="en">Volcanic and hypabyssal rock</skos:prefLabel>
	<skos:altLabel xml:lang="en">Volcanic rock</skos:altLabel>
	<skos:prefLabel xml:lang="de">Vulkanisches und hypabyssisches Gestein</skos:prefLabel>
	<skos:altLabel xml:lang="de">Vulkanit</skos:altLabel>
</rdf:Description>

<rdf:Description rdf:about="https://resource.geosphere.at/thes/lith/65">
	<skos:scopeNote xml:lang="de">Standard</skos:scopeNote>
	<skos:definition xml:lang="de">Vulkanisches Gestein, welches in der QAPF-Klassifikation durch Q kleiner als 20 Vol.-%, F kleiner als 10 Vol.-%, einem Plagioklasfaktor größer als 65 und einem SiO2-Gehalt über 52 Gew.-% charakterisiert wird oder im TAS-Diagramm im Feld O1, O2, S2 oder S3 liegt (verändert nach Gillespie &amp; Styles, 1999; Le Bas et al., 1986; Le Maitre et al., 2005).</skos:definition>
	<skos:definition xml:lang="en">Volcanic rock characterized in the QAPF classification by Q lower than 20 % by volume, F lower than 10 % by volume, a plagioclase ratio larger than 65 and a SiO2 content above 52 % by weight or plots in field O1, O2, S2 or S3 of the TAS-diagram (modified after Gillespie &amp; Styles, 1999; Le Bas et al., 1986; Le Maitre et al., 2005).</skos:definition>
	<dcterms:references rdf:resource="https://resource.geosphere.at/thes/citation/665"/>
	<dcterms:references rdf:resource="https://resource.geosphere.at/thes/citation/901"/>
</rdf:Description>

<rdf:Description rdf:about="https://resource.geosphere.at/thes/lith/83">
	<skos:scopeNote xml:lang="de">Standard</skos:scopeNote>
	<skos:altLabel xml:lang="de">Andesit (TAS)</skos:altLabel>
	<skos:altLabel xml:lang="en">Andesite (TAS)</skos:altLabel>
	<skos:scopeNote xml:lang="de">Zur Klassifikation von feinkörnigen oder glasigen Vulkaniten, deren Bestimmung des modalen Mineralbestandes nicht möglich ist, wird das TAS-Diagramm (Total Alkali vs. Silica) verwendet (Le Bas et al., 1986).</skos:scopeNote>
	<skos:definition xml:lang="de">Intermediäres vulkanisches Gestein, gewöhnlich porphyrisch, welches sich aus Plagioklas (häufig mit Zonierung von Labradorit zu Oligoklas), Pyroxen, Hornblende und/oder Biotit zusammensetzt. Modal definiert in QAPF-Feldern 9-10. Im TAS-Diagramm liegt das Gestein im Feld O2. (Le Bas et al., 1986; Le Maitre et al., 2005)</skos:definition>
	<skos:definition xml:lang="en">An intermediate volcanic rock composed essentially of plagioclase (frequently zoned from labradorite to oligoclase), pyroxene, hornblende and/or biotite. Defined modally in QAPF-fields 9-10. Rock with a bulk rock composition plotting in field O2 of the TAS-diagram. (Le Bas et al., 1986; Le Maitre et al., 2005)</skos:definition>
	<skos:scopeNote xml:lang="en">The TAS-diagram (Total Alkali vs. Silica) is used to classify fine-grained or glassy volcanic rocks with no determinable mineral mode (Le Bas et al., 1986).</skos:scopeNote>
</rdf:Description>

<rdf:Description rdf:about="https://resource.geosphere.at/thes/lith/65">
	<skos:narrower rdf:resource="https://resource.geosphere.at/thes/lith/283"/>
</rdf:Description>

<rdf:Description rdf:about="https://resource.geosphere.at/thes/lith/283">
	<skos:broader rdf:resource="https://resource.geosphere.at/thes/lith/65"/>
	<rdf:type rdf:resource="http://www.w3.org/2004/02/skos/core#Concept"/>
	<skos:prefLabel xml:lang="de">Basaltischer Andesit</skos:prefLabel>
	<dcterms:created rdf:datatype="http://www.w3.org/2001/XMLSchema#dateTime">2025-09-29T14:39:47.702Z</dcterms:created>
</rdf:Description>

<rdf:Description rdf:about="https://resource.geosphere.at/thes/lith/284">
	<skos:broader rdf:resource="https://resource.geosphere.at/thes/lith/65"/>
	<skos:prefLabel xml:lang="de">Basaltischer Trachyandesit</skos:prefLabel>
	<dcterms:created rdf:datatype="http://www.w3.org/2001/XMLSchema#dateTime">2025-09-29T14:40:07.255Z</dcterms:created>
	<rdf:type rdf:resource="http://www.w3.org/2004/02/skos/core#Concept"/>
</rdf:Description>

<rdf:Description rdf:about="https://resource.geosphere.at/thes/lith/65">
	<skos:narrower rdf:resource="https://resource.geosphere.at/thes/lith/284"/>
</rdf:Description>

<rdf:Description rdf:about="https://resource.geosphere.at/thes/lith/285">
	<dcterms:created rdf:datatype="http://www.w3.org/2001/XMLSchema#dateTime">2025-09-29T14:40:19.334Z</dcterms:created>
</rdf:Description>

<rdf:Description rdf:about="https://resource.geosphere.at/thes/lith/65">
	<skos:narrower rdf:resource="https://resource.geosphere.at/thes/lith/285"/>
</rdf:Description>

<rdf:Description rdf:about="https://resource.geosphere.at/thes/lith/285">
	<skos:prefLabel xml:lang="de">Trachyandesit</skos:prefLabel>
	<skos:broader rdf:resource="https://resource.geosphere.at/thes/lith/65"/>
	<rdf:type rdf:resource="http://www.w3.org/2004/02/skos/core#Concept"/>
</rdf:Description>

<rdf:Description rdf:about="https://resource.geosphere.at/thes/lith/283">
	<skos:prefLabel xml:lang="en">Basaltic andesite</skos:prefLabel>
	<skos:altLabel xml:lang="de">Basaltischer Andesit (TAS)</skos:altLabel>
	<skos:altLabel xml:lang="en">Basaltic andesite (TAS)</skos:altLabel>
	<skos:scopeNote xml:lang="de">Standard</skos:scopeNote>
	<skos:scopeNote xml:lang="en">The TAS-diagram (Total Alkali vs. Silica) is used to classify fine-grained or glassy volcanic rocks with no determinable mineral mode (Le Bas et al., 1986).</skos:scopeNote>
	<skos:scopeNote xml:lang="de">Zur Klassifikation von feinkörnigen oder glasigen Vulkaniten, deren Bestimmung des modalen Mineralbestandes nicht möglich ist, wird das TAS-Diagramm (Total Alkali vs. Silica) verwendet (Le Bas et al., 1986).</skos:scopeNote>
	<skos:definition xml:lang="de">Andesitisches Gestein mit einer chemischen Zusammensetzung, die im TAS-Diagramm (Gew.-% SiO2 : Gew.-% Na2O+K2O) im Feld O1 liegt und durch die Punkte (52 : 0), (52 : 5), (57 : 5,9) und (57 : 0) definiert wird (Le Bas et al., 1986; Le Maitre et al., 2005).</skos:definition>
	<skos:definition xml:lang="en">Andesitic rock with a bulk rock composition plotting in field O1 of the TAS-diagram (SiO2 % by weight, Na2O+K2O % by weight), which is defined by points (52, 0), (52, 5), (57, 5.9) and (57, 0) (Le Bas et al., 1986; Le Maitre et al., 2005).</skos:definition>
</rdf:Description>

<rdf:Description rdf:about="https://resource.geosphere.at/thes/lith/284">
	<skos:prefLabel xml:lang="en">Basaltic trachyandesite</skos:prefLabel>
	<skos:altLabel xml:lang="de">Basaltischer Trachyandesit (TAS)</skos:altLabel>
	<skos:altLabel xml:lang="en">Basaltic trachyandesite (TAS)</skos:altLabel>
	<skos:scopeNote xml:lang="de">Standard</skos:scopeNote>
	<skos:scopeNote xml:lang="de">Zur Klassifikation von feinkörnigen oder glasigen Vulkaniten, deren Bestimmung des modalen Mineralbestandes nicht möglich ist, wird das TAS-Diagramm (Total Alkali vs. Silica) verwendet (Le Bas et al., 1986).</skos:scopeNote>
	<skos:scopeNote xml:lang="en">The TAS-diagram (Total Alkali vs. Silica) is used to classify fine-grained or glassy volcanic rocks with no determinable mineral mode (Le Bas et al., 1986).</skos:scopeNote>
	<skos:definition xml:lang="en">Andesitic rock with a bulk rock composition plotting in field S2 of the TAS-diagram (SiO2 % by weight, Na2O+K2O % by weight), which is defined by points (52, 5), (49.4, 7.3), (53, 9.3) und (57, 5.9). (Le Bas et al., 1986; Le Maitre et al., 2005)</skos:definition>
	<skos:definition xml:lang="de">Andesitisches Gestein mit einer chemischen Zusammensetzung, die im TAS-Diagramm (Gew.-% SiO2 : Gew.-% Na2O+K2O) im Feld S2 liegt und durch die Punkte (52 : 5), (49,4 : 7,3), (53 : 9,3) und (57 : 5,9) definiert wird. (Le Bas et al., 1986; Le Maitre et al., 2005)</skos:definition>
</rdf:Description>

<rdf:Description rdf:about="https://resource.geosphere.at/thes/lith/285">
	<skos:prefLabel xml:lang="en">Trachyandesite</skos:prefLabel>
	<skos:altLabel xml:lang="de">Trachyandesit (TAS)</skos:altLabel>
	<skos:altLabel xml:lang="en">Trachyandesite (TAS)</skos:altLabel>
	<skos:definition xml:lang="de">Andesitisches Gestein mit einer chemischen Zusammensetzung, die im TAS-Diagramm (Gew.-% SiO2 : Gew.-% Na2O+K2O) im Feld S3 liegt und durch die Punkte (57 : 5,9) (53 : 9,3), (57,6 : 11,7) und (63 : 7) definiert wird. (Le Bas et al., 1986; Le Maitre et al., 2005)</skos:definition>
	<skos:definition xml:lang="en">Andesitic rock with a bulk rock composition plotting in field S3 of the TAS-diagram (SiO2 % by weight, Na2O+K2O % by weight), which is defined by points (57, 5.9) (53, 9.3), (57.6, 11.7) and (63, 7). (Le Bas et al., 1986; Le Maitre et al., 2005)</skos:definition>
</rdf:Description>

<rdf:Description rdf:about="https://resource.geosphere.at/thes/lith/65">
	<dcterms:modified rdf:datatype="http://www.w3.org/2001/XMLSchema#dateTime">2025-09-30T10:14:39.854Z</dcterms:modified>
</rdf:Description>

<rdf:Description rdf:about="https://resource.geosphere.at/thes/lith/83">
	<dcterms:references rdf:resource="https://resource.geosphere.at/thes/citation/901"/>
	<dcterms:modified rdf:datatype="http://www.w3.org/2001/XMLSchema#dateTime">2025-09-30T10:15:11.831Z</dcterms:modified>
</rdf:Description>

<rdf:Description rdf:about="https://resource.geosphere.at/thes/lith/283">
	<dcterms:references rdf:resource="https://resource.geosphere.at/thes/citation/901"/>
	<dcterms:references rdf:resource="https://resource.geosphere.at/thes/citation/477"/>
	<dcterms:modified rdf:datatype="http://www.w3.org/2001/XMLSchema#dateTime">2025-09-30T10:15:31.236Z</dcterms:modified>
</rdf:Description>

<rdf:Description rdf:about="https://resource.geosphere.at/thes/lith/284">
	<dcterms:references rdf:resource="https://resource.geosphere.at/thes/citation/901"/>
	<dcterms:references rdf:resource="https://resource.geosphere.at/thes/citation/477"/>
	<dcterms:modified rdf:datatype="http://www.w3.org/2001/XMLSchema#dateTime">2025-09-30T10:16:10.938Z</dcterms:modified>
</rdf:Description>

<rdf:Description rdf:about="https://resource.geosphere.at/thes/lith/285">
	<dcterms:references rdf:resource="https://resource.geosphere.at/thes/citation/901"/>
	<dcterms:references rdf:resource="https://resource.geosphere.at/thes/citation/477"/>
</rdf:Description>

<rdf:Description rdf:about="https://resource.geosphere.at/thes/lith/66">
	<dcterms:references rdf:resource="https://resource.geosphere.at/thes/citation/665"/>
	<dcterms:references rdf:resource="https://resource.geosphere.at/thes/citation/901"/>
</rdf:Description>

<rdf:Description rdf:about="https://resource.geosphere.at/thes/lith/82">
	<dcterms:references rdf:resource="https://resource.geosphere.at/thes/citation/901"/>
</rdf:Description>

<rdf:Description rdf:about="https://resource.geosphere.at/thes/lith/66">
	<skos:definition xml:lang="de">Vulkanisches Gestein, welches in der QAPF-Klassifikation durch Q kleiner als 20 Vol.-%, F kleiner als 10 Vol.-%, einem Plagioklasfaktor größer als 65 und einem SiO2-Gehalt unter 52 Gew.-% charakterisiert wird oder im TAS-Diagramm im Feld B oder S1 liegt. (verändert nach Gillespie &amp; Styles, 1999; Le Bas et al., 1986; Le Maitre et al., 2005)</skos:definition>
	<skos:definition xml:lang="en">Volcanic rock characterized in the QAPF classification by Q lower than 20 % by volume, F lower than 10 % by volume, a plagioclase ratio larger than 65 and a SiO2 content below 52 % by weight or plots in field B or S1 of the TAS-diagram. (modified after Gillespie &amp; Styles, 1999; Le Bas et al., 1986; Le Maitre et al., 2005)</skos:definition>
</rdf:Description>

<rdf:Description rdf:about="https://resource.geosphere.at/thes/lith/82">
	<skos:altLabel xml:lang="de">Basalt (TAS)</skos:altLabel>
	<skos:altLabel xml:lang="en">Basalt (TAS)</skos:altLabel>
	<skos:scopeNote xml:lang="de">Standard</skos:scopeNote>
</rdf:Description>

<rdf:Description rdf:about="https://resource.geosphere.at/thes/lith/66">
	<skos:scopeNote xml:lang="de">Standard</skos:scopeNote>
</rdf:Description>

<rdf:Description rdf:about="https://resource.geosphere.at/thes/lith/285">
	<skos:scopeNote xml:lang="de">Standard</skos:scopeNote>
	<skos:scopeNote xml:lang="de">Zur Klassifikation von feinkörnigen oder glasigen Vulkaniten, deren Bestimmung des modalen Mineralbestandes nicht möglich ist, wird das TAS-Diagramm (Total Alkali vs. Silica) verwendet (Le Bas et al., 1986).</skos:scopeNote>
	<skos:scopeNote xml:lang="en">The TAS-diagram (Total Alkali vs. Silica) is used to classify fine-grained or glassy volcanic rocks with no determinable mineral mode (Le Bas et al., 1986).</skos:scopeNote>
	<dcterms:modified rdf:datatype="http://www.w3.org/2001/XMLSchema#dateTime">2025-09-30T10:20:14.013Z</dcterms:modified>
</rdf:Description>

<rdf:Description rdf:about="https://resource.geosphere.at/thes/lith/66">
	<skos:scopeNote xml:lang="de">Zur Klassifikation von feinkörnigen oder glasigen Vulkaniten, deren Bestimmung des modalen Mineralbestandes nicht möglich ist, wird das TAS-Diagramm (Total Alkali vs. Silica) verwendet (Le Bas et al., 1986).</skos:scopeNote>
	<skos:scopeNote xml:lang="en">The TAS-diagram (Total Alkali vs. Silica) is used to classify fine-grained or glassy volcanic rocks with no determinable mineral mode (Le Bas et al., 1986).</skos:scopeNote>
	<dcterms:modified rdf:datatype="http://www.w3.org/2001/XMLSchema#dateTime">2025-09-30T10:20:58.619Z</dcterms:modified>
</rdf:Description>

<rdf:Description rdf:about="https://resource.geosphere.at/thes/lith/82">
	<skos:scopeNote xml:lang="de">Zur Klassifikation von feinkörnigen oder glasigen Vulkaniten, deren Bestimmung des modalen Mineralbestandes nicht möglich ist, wird das TAS-Diagramm (Total Alkali vs. Silica) verwendet (Le Bas et al., 1986).</skos:scopeNote>
	<skos:scopeNote xml:lang="en">The TAS-diagram (Total Alkali vs. Silica) is used to classify fine-grained or glassy volcanic rocks with no determinable mineral mode (Le Bas et al., 1986).</skos:scopeNote>
	<skos:definition xml:lang="de">Vulkanisches Gestein, welches sich aus Kalzium-Plagioklas und Pyroxen zusammensetzt. Olivin, untergeordnet Foide und Quarz können vorkommen. Modal definiert in QAPF-Feldern 9-10. nsgesamt liegt der SiO2-Gehalt bei unter 52 Gew.-%.  Auf Basis der chemischen Zusammensetzung im TAS-Diagramm Feld B. (Le Bas et al., 1986; Le Maitre et al., 2005)</skos:definition>
	<skos:definition xml:lang="en">A volcanic rock composed essentially of calcic plagioclase and pyroxene. Olivine, minor foids and quartz may also be present. Defined modally in QAPF-fields 9-10. In total, the SiO2 content is below 52 % by weight.  (Le Maitre et al., 2005). Bulk rock composition plotting in field B of the TAS-diagram. (Le Bas et al., 1986; Le Maitre et al., 2005)</skos:definition>
	<dcterms:modified rdf:datatype="http://www.w3.org/2001/XMLSchema#dateTime">2025-09-30T10:24:48.386Z</dcterms:modified>
</rdf:Description>

<rdf:Description rdf:about="https://resource.geosphere.at/thes/lith/286">
	<dcterms:created rdf:datatype="http://www.w3.org/2001/XMLSchema#dateTime">2025-09-30T10:25:49.158Z</dcterms:created>
	<rdf:type rdf:resource="http://www.w3.org/2004/02/skos/core#Concept"/>
</rdf:Description>

<rdf:Description rdf:about="https://resource.geosphere.at/thes/lith/66">
	<skos:narrower rdf:resource="https://resource.geosphere.at/thes/lith/286"/>
</rdf:Description>

<rdf:Description rdf:about="https://resource.geosphere.at/thes/lith/286">
	<skos:prefLabel xml:lang="de">Trachybasalt</skos:prefLabel>
	<skos:broader rdf:resource="https://resource.geosphere.at/thes/lith/66"/>
	<skos:prefLabel xml:lang="en">Trachybasalt</skos:prefLabel>
	<skos:altLabel xml:lang="de">Trachybasalt (TAS)</skos:altLabel>
	<skos:altLabel xml:lang="en">Trachybasalt (TAS)</skos:altLabel>
	<skos:scopeNote xml:lang="de">Standard</skos:scopeNote>
	<skos:scopeNote xml:lang="de">Zur Klassifikation von feinkörnigen oder glasigen Vulkaniten, deren Bestimmung des modalen Mineralbestandes nicht möglich ist, wird das TAS-Diagramm (Total Alkali vs. Silica) verwendet (Le Bas et al., 1986).</skos:scopeNote>
	<skos:scopeNote xml:lang="en">The TAS-diagram (Total Alkali vs. Silica) is used to classify fine-grained or glassy volcanic rocks with no determinable mineral mode (Le Bas et al., 1986).</skos:scopeNote>
	<skos:definition xml:lang="de">Basaltisches Gestein mit einer chemischen Zusammensetzung, die im TAS-Diagramm (Gew.-% SiO2 : Gew.-% Na2O+K2O) im Feld S1 liegt und durch die Punkte (45 : 5), (49,4 : 7,3) und (52 : 5) definiert wird. (Le Bas et al., 1986; Le Maitre et al., 2005)</skos:definition>
	<skos:definition xml:lang="en">Basaltic rock with a bulk rock composition plotting in field S1 of the TAS-diagram (SiO2 % by weight, Na2O+K2O % by weight), which is defined by points (45, 5), (49.4, 7.3) and (52, 5). (Le Bas et al., 1986; Le Maitre et al., 2005)</skos:definition>
	<dcterms:modified rdf:datatype="http://www.w3.org/2001/XMLSchema#dateTime">2025-09-30T10:28:04.724Z</dcterms:modified>
</rdf:Description>

<rdf:Description rdf:about="https://resource.geosphere.at/thes/lith/63">
	<skos:scopeNote xml:lang="de">Standard</skos:scopeNote>
	<skos:definition xml:lang="de">Vulkanisches Gestein, welches in der QAPF-Klassifikation durch Q zwischen 20 und 60 Vol.-% und einem Plagioklasfaktor größer als 65 charakterisiert wird oder im TAS-Diagramm im Feld O3 oder T liegt (verändert nach Gillespie &amp; Styles, 1999; Le Bas et al., 1986; Le Maitre et al., 2005).</skos:definition>
	<skos:definition xml:lang="en">Volcanic rock that is characterized in the QAPF classification by Q between 20 and 60 % by volume and a plagioclase ratio larger than 65 or plots in field O3 or T of the TAS-diagram (modified after Gillespie &amp; Styles, 1999; Le Bas et al., 1986; Le Maitre et al., 2005).</skos:definition>
	<dcterms:modified rdf:datatype="http://www.w3.org/2001/XMLSchema#dateTime">2025-09-30T10:41:08.590Z</dcterms:modified>
</rdf:Description>

<rdf:Description rdf:about="https://resource.geosphere.at/thes/lith/72">
	<skos:scopeNote xml:lang="de">Standard</skos:scopeNote>
	<skos:altLabel xml:lang="de">Dazit (TAS)</skos:altLabel>
	<skos:altLabel xml:lang="en">Dacite (TAS)</skos:altLabel>
	<skos:definition xml:lang="de">Vulkanisches Gestein, welches aus Quarz, Natrium-Plagioklas und geringeren Anteilen Biotit und/oder Hornblende und/oder Pyroxen besteht. Vulkanisches Äquivalent von Granodiorit und Tonalit. Modal definiert in QAPF-Feldern 4-5. Basierend auf der chemischen Zusammensetzung, liegt das Gestein im Feld O3 im TAS-Diagramm. (Le Bas et al., 1986; Le Maitre et al., 2005)</skos:definition>
	<skos:definition xml:lang="en">A volcanic rock consisting essentially of quartz and sodic plagioclase, with minor biotite and/or hornblende and/or pyroxene. Defined modally in QAPF-field 4-5. Bulk rock composition plotting in field O3 of the TAS-diagram (Le Maitre et al., 2005). (Le Bas et al., 1986; Le Maitre et al., 2005)</skos:definition>
</rdf:Description>

<rdf:Description rdf:about="https://resource.geosphere.at/thes/lith/287">
	<skos:prefLabel xml:lang="de">Trachydazit</skos:prefLabel>
	<dcterms:created rdf:datatype="http://www.w3.org/2001/XMLSchema#dateTime">2025-09-30T11:35:43.307Z</dcterms:created>
</rdf:Description>

<rdf:Description rdf:about="https://resource.geosphere.at/thes/lith/63">
	<skos:narrower rdf:resource="https://resource.geosphere.at/thes/lith/287"/>
</rdf:Description>

<rdf:Description rdf:about="https://resource.geosphere.at/thes/lith/287">
	<rdf:type rdf:resource="http://www.w3.org/2004/02/skos/core#Concept"/>
	<skos:broader rdf:resource="https://resource.geosphere.at/thes/lith/63"/>
	<skos:prefLabel xml:lang="en">Trachydacite</skos:prefLabel>
	<skos:altLabel xml:lang="de">Trachydazit (TAS)</skos:altLabel>
	<skos:altLabel xml:lang="en">Trachydacite (TAS)</skos:altLabel>
	<skos:scopeNote xml:lang="de">Standard</skos:scopeNote>
</rdf:Description>

<rdf:Description rdf:about="https://resource.geosphere.at/thes/lith/72">
	<skos:scopeNote xml:lang="de">Zur Klassifikation von feinkörnigen oder glasigen Vulkaniten, deren Bestimmung des modalen Mineralbestandes nicht möglich ist, wird das TAS-Diagramm (Total Alkali vs. Silica) verwendet (Le Bas et al., 1986).</skos:scopeNote>
	<skos:scopeNote xml:lang="en">The TAS-diagram (Total Alkali vs. Silica) is used to classify fine-grained or glassy volcanic rocks with no determinable mineral mode (Le Bas et al., 1986).</skos:scopeNote>
</rdf:Description>

<rdf:Description rdf:about="https://resource.geosphere.at/thes/lith/287">
	<skos:scopeNote xml:lang="de">Zur Klassifikation von feinkörnigen oder glasigen Vulkaniten, deren Bestimmung des modalen Mineralbestandes nicht möglich ist, wird das TAS-Diagramm (Total Alkali vs. Silica) verwendet (Le Bas et al., 1986).</skos:scopeNote>
	<skos:scopeNote xml:lang="en">The TAS-diagram (Total Alkali vs. Silica) is used to classify fine-grained or glassy volcanic rocks with no determinable mineral mode (Le Bas et al., 1986).</skos:scopeNote>
	<skos:definition xml:lang="de">Dazitisches Gestein mit einer chemischen Zusammensetzung, die im TAS-Diagramm (Gew.-% SiO2 : Gew.-% Na2O+K2O) im Feld T liegt und durch die Punkte (63 : 7), (57,6 : 11,7), (69 : 17,9) und (69 : 8) definiert wird. Liegt im gleichen Feld wie Trachyt (TAS) und unterscheidet sich von diesem im normativen Quarzbestand von größer 20 Vol.-%. (Le Bas et al., 1986; Le Maitre et al., 2005)</skos:definition>
	<skos:definition xml:lang="en">Dacitic rock with a bulk rock composition plotting in field T of the TAS-diagram (SiO2 % by weight, Na2O+K2O % by weight), which is defined by points (63, 7), (57.6, 11.7), (69, 17.9) and (69, 8). Plots in the same field as trachyte (TAS) and differs from it in the normative quartz value above 20 % by volume. (Le Bas et al., 1986; Le Maitre et al., 2005)</skos:definition>
</rdf:Description>

<rdf:Description rdf:about="https://resource.geosphere.at/thes/lith/96">
	<skos:scopeNote xml:lang="de">Standard</skos:scopeNote>
	<skos:definition xml:lang="de">Hypabyssisches Gestein, welches in der Korngröße zwischen Basalt und Gabbro liegt und die chemische Zusammensetzung eines basaltischen oder andesitischen Gesteins hat. Der Begriff beinhaltet Mikrogabbro und teilweise Diabas. (Le Maitre et al., 2005)</skos:definition>
	<skos:definition xml:lang="en">Hypabyssal rock that is intermediate in grain size between basalt and gabbro and has the chemical composition of a basaltic or andesitic rock. The term includes microgabbro and partly diabase. (Le Maitre et al., 2005)</skos:definition>
</rdf:Description>

<rdf:Description rdf:about="https://resource.geosphere.at/thes/lith/69">
	<skos:narrower rdf:resource="https://resource.geosphere.at/thes/lith/92"/>
</rdf:Description>

<rdf:Description rdf:about="https://resource.geosphere.at/thes/lith/92">
	<skos:broader rdf:resource="https://resource.geosphere.at/thes/lith/69"/>
</rdf:Description>

<rdf:Description rdf:about="https://resource.geosphere.at/thes/lith/6">
	<dcterms:modified rdf:datatype="http://www.w3.org/2001/XMLSchema#dateTime">2025-09-30T11:44:21.452Z</dcterms:modified>
</rdf:Description>

<rdf:Description rdf:about="https://resource.geosphere.at/thes/lith/92">
	<skos:definition xml:lang="de">Foiditisches Gestein mit einer chemischen Zusammensetzung, die im TAS-Diagramm (Gew.-% SiO2 : Gew.-% Na2O+K2O) im Feld F liegt und durch die Punkte (41 : 0), (41 : 7), (52,5 : 14) und (47,4 : 16,3) definiert wird. Enthält kein normatives Ca2SiO4. (Le Bas et al., 1986; Le Maitre et al., 2005)</skos:definition>
	<skos:definition xml:lang="en">Foiditic rock with a bulk rock composition plotting in field F of the TAS-diagram (SiO2 % by weight, Na2O+K2O % by weight), which is defined by points (41, 0), (41, 7), (52.5, 14) and (47.4, 16.3). Does not contain normative Ca2SiO4. (Le Bas et al., 1986; Le Maitre et al., 2005)</skos:definition>
</rdf:Description>

<rdf:Description rdf:about="https://resource.geosphere.at/thes/lith/69">
	<skos:definition xml:lang="de">Vulkanisches Gestein, welches in der QAPF-Klassifikation durch einen F größer als 60 Vol.-% charakterisiert wird. (Gillespie &amp; Styles, 1999; Le Maitre et al., 2005)</skos:definition>
	<skos:definition xml:lang="en">Volcanic rock characterised in the QAPF classification by F larger than 60 % by volume. (Gillespie &amp; Styles, 1999; Le Maitre et al., 2005)</skos:definition>
	<skos:scopeNote xml:lang="de">Standard</skos:scopeNote>
	<skos:scopeNote xml:lang="de">Zur Klassifikation von feinkörnigen oder glasigen Vulkaniten, deren Bestimmung des modalen Mineralbestandes nicht möglich ist, wird das TAS-Diagramm (Total Alkali vs. Silica) verwendet. (Le Bas et al., 1986)</skos:scopeNote>
	<skos:scopeNote xml:lang="en">The TAS-diagram (Total Alkali vs. Silica) is used to classify fine-grained or glassy volcanic rocks with no determinable mineral mode. (Le Bas et al., 1986)</skos:scopeNote>
</rdf:Description>

<rdf:Description rdf:about="https://resource.geosphere.at/thes/lith/288">
	<rdf:type rdf:resource="http://www.w3.org/2004/02/skos/core#Concept"/>
	<skos:broader rdf:resource="https://resource.geosphere.at/thes/lith/69"/>
	<skos:prefLabel xml:lang="de">Basanitischer Foidit</skos:prefLabel>
</rdf:Description>

<rdf:Description rdf:about="https://resource.geosphere.at/thes/lith/69">
	<skos:narrower rdf:resource="https://resource.geosphere.at/thes/lith/288"/>
</rdf:Description>

<rdf:Description rdf:about="https://resource.geosphere.at/thes/lith/288">
	<dcterms:created rdf:datatype="http://www.w3.org/2001/XMLSchema#dateTime">2025-09-30T11:51:57.097Z</dcterms:created>
	<skos:prefLabel xml:lang="en">Basanitic foidite</skos:prefLabel>
	<skos:scopeNote xml:lang="de">Standard</skos:scopeNote>
	<skos:definition xml:lang="de">Foiditisches Gestein, welches in der QAPF-Klassifikation durch einen F kleiner als 90 Vol.-% und einem Plagioklasfaktor größer als 50 charakterisiert wird. Der normative Olivinbestand ist größer als 10 Vol.-%. (Le Maitre et al., 2005)</skos:definition>
	<skos:definition xml:lang="en">Foiditic rock characterised in the QAPF classification by F lower than 90 % by volume and a plagioclase ratio larger than 50. The normative olivine value is above 10 % by volume. (Le Maitre et al., 2005)</skos:definition>
</rdf:Description>

<rdf:Description rdf:about="https://resource.geosphere.at/thes/lith/92">
	<skos:scopeNote xml:lang="de">Standard</skos:scopeNote>
	<skos:scopeNote xml:lang="de">Zur Klassifikation von feinkörnigen oder glasigen Vulkaniten, deren Bestimmung des modalen Mineralbestandes nicht möglich ist, wird das TAS-Diagramm (Total Alkali vs. Silica) verwendet (Le Bas et al., 1986).</skos:scopeNote>
	<skos:scopeNote xml:lang="en">The TAS-diagram (Total Alkali vs. Silica) is used to classify fine-grained or glassy volcanic rocks with no determinable mineral mode (Le Bas et al., 1986).</skos:scopeNote>
	<skos:altLabel xml:lang="de">Foidit (TAS)</skos:altLabel>
	<skos:altLabel xml:lang="en">Foidite (TAS)</skos:altLabel>
</rdf:Description>

<rdf:Description rdf:about="https://resource.geosphere.at/thes/lith/90">
	<skos:scopeNote xml:lang="de">Standard</skos:scopeNote>
	<skos:definition xml:lang="de">Alkalisches vulkanisches, foiditisches Gestein, welches in der QAPF-Klassifikation durch einen F kleiner als 90 Vol.-% und einem Plagioklasfaktor kleiner als 50 charakterisiert wird. (Le Maitre et al., 2005)</skos:definition>
	<skos:definition xml:lang="en">An alkaline volcanic, foiditic rock characterised in the QAPF classification by F lower than 90 % by volume and a plagioclase ratio lower than 50 (Le Maitre et al., 2005).</skos:definition>
</rdf:Description>

<rdf:Description rdf:about="https://resource.geosphere.at/thes/lith/91">
	<skos:definition xml:lang="en">Foiditic rock characterised in the QAPF classification by F lower than 90 % by volume and a plagioclase ratio larger than 50. The normative olivine value is below 10 % by volume. (Le Maitre et al., 2005)</skos:definition>
	<skos:scopeNote xml:lang="de">Standard</skos:scopeNote>
</rdf:Description>

<rdf:Description rdf:about="https://resource.geosphere.at/thes/lith/6">
	<skos:narrower rdf:resource="https://resource.geosphere.at/thes/lith/289"/>
</rdf:Description>

<rdf:Description rdf:about="https://resource.geosphere.at/thes/lith/289">
	<rdf:type rdf:resource="http://www.w3.org/2004/02/skos/core#Concept"/>
	<skos:broader rdf:resource="https://resource.geosphere.at/thes/lith/6"/>
	<skos:prefLabel xml:lang="de">Lamproit</skos:prefLabel>
	<dcterms:created rdf:datatype="http://www.w3.org/2001/XMLSchema#dateTime">2025-09-30T12:00:20.507Z</dcterms:created>
	<skos:prefLabel xml:lang="en">Lamproite</skos:prefLabel>
	<skos:scopeNote xml:lang="de">Standard</skos:scopeNote>
	<skos:definition xml:lang="de">Vulkanisches oder hypabyssisches Gestein, welches reich an Kalium (ultrapotassisch, K2O/Na2O größer als 3) und Magnesium ist, sowie einen peralkalischen Charakter mit (K2O+Na2O)/Al2O3 typischerweise größer als 1 aufweist. (Le Maitre et al., 2005)</skos:definition>
	<skos:definition xml:lang="en">Volcanic or hypabyssal rock that is magnesium rich with ultrapotassic (K2O/Na2O larger than 3) and peralkaline (K2O+Na2O)/Al2O3 typically larger than 1) characteristics .(Le Maitre et al., 2005)</skos:definition>
</rdf:Description>

<rdf:Description rdf:about="https://resource.geosphere.at/thes/lith/95">
	<skos:scopeNote xml:lang="de">Standard</skos:scopeNote>
	<skos:definition xml:lang="de">Magmatisches Gestein, dessen mafische Minerale (Biotit, Amphibol, Pyroxen) porphyrisch als Einsprenglinge auftreten, während die Feldspäte auf die Grundmasse beschränkt sind. Typisches Vorkommen als Gänge und kleine Intrusionen. Die Lamprophyre sind entsprechend der vorherrschenden mafischen Minerale klassifiziert. (Le Maitre et al., 2005).</skos:definition>
	<skos:definition xml:lang="en">A magmatic rock that is highly porphyric in mafic minerals (biotite, amphibole, pyroxene), with any feldspar being confined to the groundmass. Lamprophyres commonly occur as dykes or small intrusions, and classification is according to their predominant mafic minerals. (Le Maitre et al., 2005).</skos:definition>
	<skos:narrower rdf:resource="https://resource.geosphere.at/thes/lith/290"/>
</rdf:Description>

<rdf:Description rdf:about="https://resource.geosphere.at/thes/lith/290">
	<skos:broader rdf:resource="https://resource.geosphere.at/thes/lith/95"/>
	<skos:prefLabel xml:lang="de">Camptonit</skos:prefLabel>
	<rdf:type rdf:resource="http://www.w3.org/2004/02/skos/core#Concept"/>
	<dcterms:created rdf:datatype="http://www.w3.org/2001/XMLSchema#dateTime">2025-09-30T12:04:48.557Z</dcterms:created>
</rdf:Description>

<rdf:Description rdf:about="https://resource.geosphere.at/thes/lith/291">
	<dcterms:created rdf:datatype="http://www.w3.org/2001/XMLSchema#dateTime">2025-09-30T12:04:54.088Z</dcterms:created>
	<skos:broader rdf:resource="https://resource.geosphere.at/thes/lith/95"/>
</rdf:Description>

<rdf:Description rdf:about="https://resource.geosphere.at/thes/lith/95">
	<skos:narrower rdf:resource="https://resource.geosphere.at/thes/lith/291"/>
</rdf:Description>

<rdf:Description rdf:about="https://resource.geosphere.at/thes/lith/291">
	<rdf:type rdf:resource="http://www.w3.org/2004/02/skos/core#Concept"/>
	<skos:prefLabel xml:lang="de">Kersantit</skos:prefLabel>
</rdf:Description>

<rdf:Description rdf:about="https://resource.geosphere.at/thes/lith/95">
	<skos:narrower rdf:resource="https://resource.geosphere.at/thes/lith/292"/>
</rdf:Description>

<rdf:Description rdf:about="https://resource.geosphere.at/thes/lith/292">
	<skos:broader rdf:resource="https://resource.geosphere.at/thes/lith/95"/>
	<dcterms:created rdf:datatype="http://www.w3.org/2001/XMLSchema#dateTime">2025-09-30T12:05:02.466Z</dcterms:created>
	<rdf:type rdf:resource="http://www.w3.org/2004/02/skos/core#Concept"/>
	<skos:prefLabel xml:lang="de">Minette</skos:prefLabel>
</rdf:Description>

<rdf:Description rdf:about="https://resource.geosphere.at/thes/lith/293">
	<skos:prefLabel xml:lang="de">Monchiquit</skos:prefLabel>
	<dcterms:created rdf:datatype="http://www.w3.org/2001/XMLSchema#dateTime">2025-09-30T12:05:12.781Z</dcterms:created>
	<skos:broader rdf:resource="https://resource.geosphere.at/thes/lith/95"/>
</rdf:Description>

<rdf:Description rdf:about="https://resource.geosphere.at/thes/lith/95">
	<skos:narrower rdf:resource="https://resource.geosphere.at/thes/lith/293"/>
</rdf:Description>

<rdf:Description rdf:about="https://resource.geosphere.at/thes/lith/293">
	<rdf:type rdf:resource="http://www.w3.org/2004/02/skos/core#Concept"/>
</rdf:Description>

<rdf:Description rdf:about="https://resource.geosphere.at/thes/lith/95">
	<skos:narrower rdf:resource="https://resource.geosphere.at/thes/lith/294"/>
</rdf:Description>

<rdf:Description rdf:about="https://resource.geosphere.at/thes/lith/294">
	<skos:broader rdf:resource="https://resource.geosphere.at/thes/lith/95"/>
	<rdf:type rdf:resource="http://www.w3.org/2004/02/skos/core#Concept"/>
	<dcterms:created rdf:datatype="http://www.w3.org/2001/XMLSchema#dateTime">2025-09-30T12:05:18.800Z</dcterms:created>
</rdf:Description>

<rdf:Description rdf:about="https://resource.geosphere.at/thes/lith/295">
	<dcterms:created rdf:datatype="http://www.w3.org/2001/XMLSchema#dateTime">2025-09-30T12:05:27.570Z</dcterms:created>
	<skos:prefLabel xml:lang="de">Spessartit</skos:prefLabel>
</rdf:Description>

<rdf:Description rdf:about="https://resource.geosphere.at/thes/lith/95">
	<skos:narrower rdf:resource="https://resource.geosphere.at/thes/lith/295"/>
</rdf:Description>

<rdf:Description rdf:about="https://resource.geosphere.at/thes/lith/295">
	<skos:broader rdf:resource="https://resource.geosphere.at/thes/lith/95"/>
	<rdf:type rdf:resource="http://www.w3.org/2004/02/skos/core#Concept"/>
</rdf:Description>

<rdf:Description rdf:about="https://resource.geosphere.at/thes/lith/296">
	<dcterms:created rdf:datatype="http://www.w3.org/2001/XMLSchema#dateTime">2025-09-30T12:05:35.561Z</dcterms:created>
</rdf:Description>

<rdf:Description rdf:about="https://resource.geosphere.at/thes/lith/95">
	<skos:narrower rdf:resource="https://resource.geosphere.at/thes/lith/296"/>
</rdf:Description>

<rdf:Description rdf:about="https://resource.geosphere.at/thes/lith/296">
	<skos:broader rdf:resource="https://resource.geosphere.at/thes/lith/95"/>
	<rdf:type rdf:resource="http://www.w3.org/2004/02/skos/core#Concept"/>
	<skos:prefLabel xml:lang="de">Vogesit</skos:prefLabel>
</rdf:Description>

<rdf:Description rdf:about="https://resource.geosphere.at/thes/lith/290">
	<skos:scopeNote xml:lang="de">Standard</skos:scopeNote>
	<skos:prefLabel xml:lang="en">Camptonite</skos:prefLabel>
</rdf:Description>

<rdf:Description rdf:about="https://resource.geosphere.at/thes/lith/291">
	<skos:prefLabel xml:lang="en">Kersantite</skos:prefLabel>
	<skos:scopeNote xml:lang="de">Standard</skos:scopeNote>
</rdf:Description>

<rdf:Description rdf:about="https://resource.geosphere.at/thes/lith/292">
	<skos:prefLabel xml:lang="en">Minette</skos:prefLabel>
</rdf:Description>

<rdf:Description rdf:about="https://resource.geosphere.at/thes/lith/290">
	<skos:definition xml:lang="de">Lamprophyr mit verschiedener Kombination von Einsprenglingen aus Olivin, Klinopyroxen, Amphibol und Biotit. In der Grundmasse, die auch Feldspatvertreter (Foide) enthält, dominiert Plagioklas über Alkalifeldspat (Le Maitre et al., 2005).</skos:definition>
</rdf:Description>

<rdf:Description rdf:about="https://resource.geosphere.at/thes/lith/291">
	<skos:definition xml:lang="de">Lamprophyr mit mehr Biotit als Hornblende sowie fallweise Klinopyroxen oder Olivin als Einsprenglinge und in der Grundmasse. Feldspäte sind auf die Grundmasse beschränkt, und es überwiegt Plagioklas (Le Maitre et al., 2005).</skos:definition>
</rdf:Description>

<rdf:Description rdf:about="https://resource.geosphere.at/thes/lith/292">
	<skos:definition xml:lang="de">Lamprophyr mit mehr Biotit als Hornblende sowie fallweise Klinopyroxen oder Olivin als Einsprenglinge und in der Grundmasse. Feldspäte sind auf die Grundmasse beschränkt, und es überwiegt Kalifeldspat (Le Maitre et al., 2005).</skos:definition>
	<skos:definition xml:lang="en">Lamprophyre with phenocrysts of biotite exceeding hornblende and occasionally clinopyroxene or olivine as phenocrysts and in the groundmass. Feldspars are restricted to the groundmass and alkali feldspar prevails (Le Maitre et al., 2005).</skos:definition>
</rdf:Description>

<rdf:Description rdf:about="https://resource.geosphere.at/thes/lith/291">
	<skos:definition xml:lang="en">Lamprophyre with phenocrysts of biotite exceeding hornblende and occasionally clinopyroxene or olivine as phenocrysts and in the groundmass. Feldspars are restricted to the groundmass and plagioclase prevails (Le Maitre et al., 2005).</skos:definition>
</rdf:Description>

<rdf:Description rdf:about="https://resource.geosphere.at/thes/lith/290">
	<skos:definition xml:lang="en">Lamprophyre with any combination of phenocrysts of olivine, clinopyroxene, amphibole and biotite. Plagioclase dominates over alkali feldspar in the groundmass which also contains feldspathoids (Le Maitre et al., 2005).</skos:definition>
</rdf:Description>

<rdf:Description rdf:about="https://resource.geosphere.at/thes/lith/293">
	<skos:scopeNote xml:lang="de">Standard</skos:scopeNote>
	<skos:definition xml:lang="de">Lamprophyr mit verschiedenen Kombinationen von Einsprenglingen aus Olivin, Klinopyroxen, Amphibol und Biotit. Die feldspatfreie Grundmasse enthält Glas und Feldspatvertreter (Foide), im Besonderen Analcim (Le Maitre et al., 2005).</skos:definition>
	<skos:definition xml:lang="en">Lamprophyre with any combination of phenocrysts of olivine, clinopyroxene, amphibole and biotite. The feldspar-free groundmass contains glass and feldspathoids, especially analcime (Le Maitre et al., 2005).</skos:definition>
	<skos:prefLabel xml:lang="en">Monchiquite</skos:prefLabel>
	<dcterms:modified rdf:datatype="http://www.w3.org/2001/XMLSchema#dateTime">2025-09-30T12:43:10.029Z</dcterms:modified>
</rdf:Description>

<rdf:Description rdf:about="https://resource.geosphere.at/thes/lith/294">
	<skos:prefLabel xml:lang="de">Sannait</skos:prefLabel>
	<skos:prefLabel xml:lang="en">Sannaite</skos:prefLabel>
	<skos:scopeNote xml:lang="de">Standard</skos:scopeNote>
	<skos:definition xml:lang="de">Lamprophyr mit verschiedenen Kombinationen von Einsprenglingen aus Olivin, Klinopyroxen, Amphibol und Biotit. In der Grundmasse, die auch Nephelin enthält, dominiert Alkalifeldspat über Plagioklas (Le Maitre et al., 2005).</skos:definition>
	<skos:definition xml:lang="en">Lamprophyre with any combination of phenocrysts of olivine, clinopyroxene, amphibole and biotite. Alkalifeldspar is dominating over plagioclase in the groundmass which also contains nepheline (Le Maitre et al., 2005).</skos:definition>
</rdf:Description>

<rdf:Description rdf:about="https://resource.geosphere.at/thes/lith/295">
	<skos:prefLabel xml:lang="en">Spessartite</skos:prefLabel>
	<skos:scopeNote xml:lang="de">Standard</skos:scopeNote>
	<skos:definition xml:lang="de">Lamprophyr mit Hornblende und Klinopyroxen sowie mitunter Olivin als Einsprenglinge und in der Grundmasse. Feldspäte sind auf die Grundmasse beschränkt, und es überwiegt Plagioklas (Le Maitre et al., 2005).</skos:definition>
	<skos:definition xml:lang="en">Lamprophyre with phenocrysts of hornblende and clinopyroxene as well as occasionally olivine as phenocryst and in the groundmass. Feldspars are restricted to the groundmass and plagioclase prevails (Le Maitre et al., 2005).</skos:definition>
</rdf:Description>

<rdf:Description rdf:about="https://resource.geosphere.at/thes/lith/296">
	<skos:prefLabel xml:lang="en">Vogesite</skos:prefLabel>
	<skos:scopeNote xml:lang="de">Standard</skos:scopeNote>
	<skos:definition xml:lang="de">Lamprophyr mit Hornblende und Klinopyroxen sowie mitunter Olivin als Einsprenglinge und in der Grundmasse. Feldspäte sind auf die Grundmasse beschränkt, und es überwiegt Kalifeldspat (Le Maitre et al., 2005).</skos:definition>
	<skos:definition xml:lang="en">Lamprophyre with phenocrysts of hornblende and clinopyroxene as well as occasionally olivine as phenocryst and in the groundmass. Feldspars are restricted to the groundmass and alkali feldspar prevails (Le Maitre et al., 2005).</skos:definition>
</rdf:Description>

<rdf:Description rdf:about="https://resource.geosphere.at/thes/lith/297">
	<rdf:type rdf:resource="http://www.w3.org/2004/02/skos/core#Concept"/>
</rdf:Description>

<rdf:Description rdf:about="https://resource.geosphere.at/thes/lith/6">
	<skos:narrower rdf:resource="https://resource.geosphere.at/thes/lith/297"/>
</rdf:Description>

<rdf:Description rdf:about="https://resource.geosphere.at/thes/lith/297">
	<skos:broader rdf:resource="https://resource.geosphere.at/thes/lith/6"/>
	<skos:prefLabel xml:lang="de">Obsidian</skos:prefLabel>
	<dcterms:created rdf:datatype="http://www.w3.org/2001/XMLSchema#dateTime">2025-09-30T12:12:29.524Z</dcterms:created>
	<skos:prefLabel xml:lang="en">Obsidian</skos:prefLabel>
	<skos:scopeNote xml:lang="de">Standard</skos:scopeNote>
	<skos:definition xml:lang="de">Vulkanisches Gestein, meistens Gesteinsglas rhyolithischer Zusammensetzung, mit mehr als 80 Vol.-% Glasanteil, mehr als 70 Gew.-% SiO2 und maximal 3-4 Gew.-% H2O (verändert nach Gillespie &amp; Styles, 1999; Licker, 2003).</skos:definition>
	<skos:definition xml:lang="en">Volcanic rock, usually glass of rhyolitic composition, with more than 80 % volumetric glass content, more than 70 % silica by weight and at most 3-4 % water by weight (modified after Gillespie &amp; Styles, 1999; Licker, 2003).</skos:definition>
</rdf:Description>

<rdf:Description rdf:about="https://resource.geosphere.at/thes/lith/67">
	<skos:scopeNote xml:lang="de">Standard</skos:scopeNote>
</rdf:Description>

<rdf:Description rdf:about="https://resource.geosphere.at/thes/lith/84">
	<skos:scopeNote xml:lang="de">Standard</skos:scopeNote>
</rdf:Description>

<rdf:Description rdf:about="https://resource.geosphere.at/thes/lith/85">
	<skos:scopeNote xml:lang="de">Standard</skos:scopeNote>
</rdf:Description>

<rdf:Description rdf:about="https://resource.geosphere.at/thes/lith/62">
	<skos:scopeNote xml:lang="de">Standard</skos:scopeNote>
</rdf:Description>

<rdf:Description rdf:about="https://resource.geosphere.at/thes/lith/70">
	<skos:scopeNote xml:lang="de">Standard</skos:scopeNote>
</rdf:Description>

<rdf:Description rdf:about="https://resource.geosphere.at/thes/lith/71">
	<skos:scopeNote xml:lang="de">Standard</skos:scopeNote>
</rdf:Description>

<rdf:Description rdf:about="https://resource.geosphere.at/thes/lith/68">
	<skos:scopeNote xml:lang="de">Standard</skos:scopeNote>
</rdf:Description>

<rdf:Description rdf:about="https://resource.geosphere.at/thes/lith/88">
	<skos:scopeNote xml:lang="de">Standard</skos:scopeNote>
	<skos:altLabel xml:lang="de">Basanit (TAS)</skos:altLabel>
	<skos:altLabel xml:lang="en">Basanite (TAS)</skos:altLabel>
	<skos:definition xml:lang="de">Vulkanisches Gestein, welches aus Plagioklas, Klinopyroxen, wesentlichen Anteilen Feldspatvertreter und Olivin besteht. Modal definiert in QAPF-Feld 14. Liegt im gleichen Feld wie Tephrit (TAS U1) und unterscheidet sich von diesem im normativen Olivinbestand von größer 10 Vol.-% (Le Bas et al., 1986; Le Maitre et al., 2005).</skos:definition>
	<skos:definition xml:lang="en">A volcanic rock containing sodic plagioclase, clinopyroxene, essential foids and olivine. Defined modally in QAPF-field 14. Plots in the same field as tephrite (TAS U1) and differs from it in the normative olivine value above 10 % by volume (Le Bas et al., 1986; Le Maitre et al., 2005).</skos:definition>
	<skos:scopeNote xml:lang="de">Zur Klassifikation von feinkörnigen oder glasigen Vulkaniten, deren Bestimmung des modalen Mineralbestandes nicht möglich ist, wird das TAS-Diagramm (Total Alkali vs. Silica) verwendet (Le Bas et al., 1986).</skos:scopeNote>
	<skos:scopeNote xml:lang="en">The TAS-diagram (Total Alkali vs. Silica) is used to classify fine-grained or glassy volcanic rocks with no determinable mineral mode (Le Bas et al., 1986).</skos:scopeNote>
</rdf:Description>

<rdf:Description rdf:about="https://resource.geosphere.at/thes/lith/86">
	<dcterms:modified rdf:datatype="http://www.w3.org/2001/XMLSchema#dateTime">2025-09-30T13:26:20.668Z</dcterms:modified>
	<skos:definition xml:lang="de">Tephritisches Gestein, welches in der QAPF-Klassifikation durch einem Plagioklasfaktor kleiner als 90 charakterisiert wird. Der normative Olivinbestand ist größer als 10 Vol.-% (Le Maitre et al., 2005).</skos:definition>
	<skos:definition xml:lang="en">Tephritic rock characterized in the QAPF classification by a plagioclase ratio lower than 90. The normative olivine value is above 10 % by volume (Le Maitre et al., 2005).</skos:definition>
</rdf:Description>

<rdf:Description rdf:about="https://resource.geosphere.at/thes/lith/87">
	<skos:scopeNote xml:lang="de">Standard</skos:scopeNote>
	<skos:definition xml:lang="de">Tephritisches Gestein, welches in der QAPF-Klassifikation durch einem Plagioklasfaktor kleiner als 90 charakterisiert wird. Der normative Olivinbestand ist kleiner als 10 Vol.-% (Le Maitre et al., 2005).</skos:definition>
	<skos:definition xml:lang="en">Tephritic rock characterized in the QAPF classification by a plagioclase ratio lower than 90. The normative olivine value is below 10 % by volume (Le Maitre et al., 2005).</skos:definition>
	<dcterms:modified rdf:datatype="http://www.w3.org/2001/XMLSchema#dateTime">2025-09-30T12:23:38.064Z</dcterms:modified>
</rdf:Description>

<rdf:Description rdf:about="https://resource.geosphere.at/thes/lith/89">
	<skos:altLabel xml:lang="de">Tephrit (TAS)</skos:altLabel>
	<skos:altLabel xml:lang="en">Tephrite (TAS)</skos:altLabel>
	<skos:definition xml:lang="de">Alkalisches vulkanisches Gestein, welches aus Kalzium-Plagioklas, Klinopyroxen und Feldspatvertretern besteht. Modal definiert in QAPF-Feld 14. Basierend auf der chemischen Zusammensetzung im Feld U1, somit  im gleichen Feld wie Basanit (TAS) und unterscheidet sich von diesem im normativen Olivinbestand von kleiner 10 Vol.-% (Le Bas et al., 1986; Le Maitre et al., 2005).</skos:definition>
	<skos:definition xml:lang="en">An alkaline volcanic rock consisting of calcic plagioclase, clinopyroxene, and feldspathoids. Defined modally in QAPF-field 14. Plots in the same TAS field as basanite (U1) and differs from it in the normative olivine value below 10 % by volume (Le Bas et al., 1986; Le Maitre et al., 2005).</skos:definition>
	<skos:scopeNote xml:lang="de">Standard</skos:scopeNote>
	<skos:scopeNote xml:lang="de">Zur Klassifikation von feinkörnigen oder glasigen Vulkaniten, deren Bestimmung des modalen Mineralbestandes nicht möglich ist, wird das TAS-Diagramm (Total Alkali vs. Silica) verwendet (Le Bas et al., 1986).</skos:scopeNote>
	<skos:scopeNote xml:lang="en">The TAS-diagram (Total Alkali vs. Silica) is used to classify fine-grained or glassy volcanic rocks with no determinable mineral mode (Le Bas et al., 1986).</skos:scopeNote>
</rdf:Description>

<rdf:Description rdf:about="https://resource.geosphere.at/thes/lith/64">
	<skos:scopeNote xml:lang="de">Standard</skos:scopeNote>
</rdf:Description>

<rdf:Description rdf:about="https://resource.geosphere.at/thes/lith/74">
	<skos:scopeNote xml:lang="de">Standard</skos:scopeNote>
</rdf:Description>

<rdf:Description rdf:about="https://resource.geosphere.at/thes/lith/75">
	<skos:scopeNote xml:lang="de">Standard</skos:scopeNote>
</rdf:Description>

<rdf:Description rdf:about="https://resource.geosphere.at/thes/lith/81">
	<skos:scopeNote xml:lang="de">Standard</skos:scopeNote>
</rdf:Description>

<rdf:Description rdf:about="https://resource.geosphere.at/thes/lith/78">
	<skos:scopeNote xml:lang="de">Standard</skos:scopeNote>
</rdf:Description>

<rdf:Description rdf:about="https://resource.geosphere.at/thes/lith/80">
	<skos:scopeNote xml:lang="de">Standard</skos:scopeNote>
</rdf:Description>

<rdf:Description rdf:about="https://resource.geosphere.at/thes/lith/73">
	<skos:scopeNote xml:lang="de">Standard</skos:scopeNote>
</rdf:Description>

<rdf:Description rdf:about="https://resource.geosphere.at/thes/lith/79">
	<skos:scopeNote xml:lang="de">Standard</skos:scopeNote>
</rdf:Description>

<rdf:Description rdf:about="https://resource.geosphere.at/thes/lith/76">
	<skos:scopeNote xml:lang="de">Standard</skos:scopeNote>
</rdf:Description>

<rdf:Description rdf:about="https://resource.geosphere.at/thes/lith/77">
	<skos:scopeNote xml:lang="de">Standard</skos:scopeNote>
	<skos:altLabel xml:lang="de">Trachyt (TAS)</skos:altLabel>
	<skos:altLabel xml:lang="en">Trachyte (TAS)</skos:altLabel>
	<skos:scopeNote xml:lang="de">Zur Klassifikation von feinkörnigen oder glasigen Vulkaniten, deren Bestimmung des modalen Mineralbestandes nicht möglich ist, wird das TAS-Diagramm (Total Alkali vs. Silica) verwendet (Le Bas et al., 1986).</skos:scopeNote>
	<skos:scopeNote xml:lang="de">The TAS-diagram (Total Alkali vs. Silica) is used to classify fine-grained or glassy volcanic rocks with no determinable mineral mode (Le Bas et al., 1986).</skos:scopeNote>
	<skos:definition xml:lang="de">Vulkanisches Gestein, welches hauptsächlich aus Alkalifeldspat besteht. Modal definiert in QAPF-Feld 7. Liegt im gleichen TAS Feld wie Trachydazit (T) und unterscheidet sich von diesem im normativen Quarzbestand von kleiner 20 Vol.-% (Le Bas et al., 1986; Le Maitre et al., 2005).</skos:definition>
	<skos:definition xml:lang="en">A volcanic rock consisting essentially of alkali feldspar. Defined modally in QAPF-field 7. Plots in the same TAS field as trachydacite (T) and differs from it in the normative quartz value below 20 % by volume (Le Bas et al., 1986; Le Maitre et al., 2005).</skos:definition>
</rdf:Description>

<rdf:Description rdf:about="https://resource.geosphere.at/thes/lith/72">
	<dcterms:modified rdf:datatype="http://www.w3.org/2001/XMLSchema#dateTime">2025-09-30T12:39:50.235Z</dcterms:modified>
	<dcterms:references rdf:resource="https://resource.geosphere.at/thes/citation/901"/>
</rdf:Description>

<rdf:Description rdf:about="https://resource.geosphere.at/thes/lith/287">
	<dcterms:references rdf:resource="https://resource.geosphere.at/thes/citation/901"/>
	<dcterms:references rdf:resource="https://resource.geosphere.at/thes/citation/477"/>
	<dcterms:modified rdf:datatype="http://www.w3.org/2001/XMLSchema#dateTime">2025-09-30T12:40:09.786Z</dcterms:modified>
</rdf:Description>

<rdf:Description rdf:about="https://resource.geosphere.at/thes/lith/96">
	<dcterms:modified rdf:datatype="http://www.w3.org/2001/XMLSchema#dateTime">2025-09-30T12:40:18.785Z</dcterms:modified>
</rdf:Description>

<rdf:Description rdf:about="https://resource.geosphere.at/thes/lith/69">
	<dcterms:references rdf:resource="https://resource.geosphere.at/thes/citation/665"/>
	<dcterms:modified rdf:datatype="http://www.w3.org/2001/XMLSchema#dateTime">2025-09-30T12:41:03.988Z</dcterms:modified>
</rdf:Description>

<rdf:Description rdf:about="https://resource.geosphere.at/thes/lith/288">
	<dcterms:references rdf:resource="https://resource.geosphere.at/thes/citation/477"/>
	<dcterms:modified rdf:datatype="http://www.w3.org/2001/XMLSchema#dateTime">2025-09-30T12:41:28.397Z</dcterms:modified>
</rdf:Description>

<rdf:Description rdf:about="https://resource.geosphere.at/thes/lith/92">
	<dcterms:references rdf:resource="https://resource.geosphere.at/thes/citation/901"/>
	<dcterms:modified rdf:datatype="http://www.w3.org/2001/XMLSchema#dateTime">2025-09-30T12:41:42.884Z</dcterms:modified>
</rdf:Description>

<rdf:Description rdf:about="https://resource.geosphere.at/thes/lith/90">
	<dcterms:modified rdf:datatype="http://www.w3.org/2001/XMLSchema#dateTime">2025-09-30T12:41:51.357Z</dcterms:modified>
</rdf:Description>

<rdf:Description rdf:about="https://resource.geosphere.at/thes/lith/91">
	<dcterms:modified rdf:datatype="http://www.w3.org/2001/XMLSchema#dateTime">2025-09-30T12:41:58.770Z</dcterms:modified>
</rdf:Description>

<rdf:Description rdf:about="https://resource.geosphere.at/thes/lith/289">
	<dcterms:references rdf:resource="https://resource.geosphere.at/thes/citation/477"/>
	<dcterms:modified rdf:datatype="http://www.w3.org/2001/XMLSchema#dateTime">2025-09-30T12:42:08.036Z</dcterms:modified>
</rdf:Description>

<rdf:Description rdf:about="https://resource.geosphere.at/thes/lith/95">
	<dcterms:modified rdf:datatype="http://www.w3.org/2001/XMLSchema#dateTime">2025-09-30T12:42:20.552Z</dcterms:modified>
</rdf:Description>

<rdf:Description rdf:about="https://resource.geosphere.at/thes/lith/290">
	<dcterms:references rdf:resource="https://resource.geosphere.at/thes/citation/477"/>
	<dcterms:modified rdf:datatype="http://www.w3.org/2001/XMLSchema#dateTime">2025-09-30T12:42:57.910Z</dcterms:modified>
</rdf:Description>

<rdf:Description rdf:about="https://resource.geosphere.at/thes/lith/291">
	<dcterms:references rdf:resource="https://resource.geosphere.at/thes/citation/477"/>
	<dcterms:modified rdf:datatype="http://www.w3.org/2001/XMLSchema#dateTime">2025-09-30T12:42:59.903Z</dcterms:modified>
</rdf:Description>

<rdf:Description rdf:about="https://resource.geosphere.at/thes/lith/292">
	<dcterms:references rdf:resource="https://resource.geosphere.at/thes/citation/477"/>
	<dcterms:modified rdf:datatype="http://www.w3.org/2001/XMLSchema#dateTime">2025-09-30T12:43:07.037Z</dcterms:modified>
</rdf:Description>

<rdf:Description rdf:about="https://resource.geosphere.at/thes/lith/293">
	<dcterms:references rdf:resource="https://resource.geosphere.at/thes/citation/477"/>
</rdf:Description>

<rdf:Description rdf:about="https://resource.geosphere.at/thes/lith/294">
	<dcterms:references rdf:resource="https://resource.geosphere.at/thes/citation/477"/>
	<dcterms:modified rdf:datatype="http://www.w3.org/2001/XMLSchema#dateTime">2025-09-30T12:43:12.117Z</dcterms:modified>
</rdf:Description>

<rdf:Description rdf:about="https://resource.geosphere.at/thes/lith/295">
	<dcterms:references rdf:resource="https://resource.geosphere.at/thes/citation/477"/>
	<dcterms:modified rdf:datatype="http://www.w3.org/2001/XMLSchema#dateTime">2025-09-30T12:43:14.623Z</dcterms:modified>
</rdf:Description>

<rdf:Description rdf:about="https://resource.geosphere.at/thes/lith/296">
	<dcterms:references rdf:resource="https://resource.geosphere.at/thes/citation/477"/>
	<dcterms:modified rdf:datatype="http://www.w3.org/2001/XMLSchema#dateTime">2025-09-30T12:43:16.928Z</dcterms:modified>
</rdf:Description>

<rdf:Description rdf:about="https://resource.geosphere.at/thes/lith/297">
	<dcterms:references rdf:resource="https://resource.geosphere.at/thes/citation/665"/>
	<dcterms:modified rdf:datatype="http://www.w3.org/2001/XMLSchema#dateTime">2025-09-30T12:43:30.279Z</dcterms:modified>
</rdf:Description>

<rdf:Description rdf:about="https://resource.geosphere.at/thes/lith/67">
	<dcterms:references rdf:resource="https://resource.geosphere.at/thes/citation/665"/>
	<dcterms:modified rdf:datatype="http://www.w3.org/2001/XMLSchema#dateTime">2025-09-30T12:44:15.204Z</dcterms:modified>
</rdf:Description>

<rdf:Description rdf:about="https://resource.geosphere.at/thes/lith/84">
	<dcterms:modified rdf:datatype="http://www.w3.org/2001/XMLSchema#dateTime">2025-09-30T12:44:26.102Z</dcterms:modified>
</rdf:Description>

<rdf:Description rdf:about="https://resource.geosphere.at/thes/lith/85">
	<dcterms:modified rdf:datatype="http://www.w3.org/2001/XMLSchema#dateTime">2025-09-30T12:44:28.924Z</dcterms:modified>
</rdf:Description>

<rdf:Description rdf:about="https://resource.geosphere.at/thes/lith/62">
	<dcterms:references rdf:resource="https://resource.geosphere.at/thes/citation/665"/>
</rdf:Description>

<rdf:Description rdf:about="https://resource.geosphere.at/thes/lith/71">
	<skos:altLabel xml:lang="de">Rhyolit (TAS)</skos:altLabel>
	<skos:altLabel xml:lang="en">Rhyolite (TAS)</skos:altLabel>
	<skos:scopeNote xml:lang="de">Zur Klassifikation von feinkörnigen oder glasigen Vulkaniten, deren Bestimmung des modalen Mineralbestandes nicht möglich ist, wird das TAS-Diagramm (Total Alkali vs. Silica) verwendet (Le Bas et al., 1986).</skos:scopeNote>
	<skos:scopeNote xml:lang="en">The TAS-diagram (Total Alkali vs. Silica) is used to classify fine-grained or glassy volcanic rocks with no determinable mineral mode (Le Bas et al., 1986).</skos:scopeNote>
	<skos:definition xml:lang="de">Saures vulkanisches Gestein, welches aus Phenokristallen von Quarz und Alkalifeldspat, oft auch Plagioklas und Biotit, in einer glasigen Grundmasse besteht, die eine chemische Zusammensetzung wie Granit besitzt. Modal definiert in QAPF-Feld 3. Im TAS-Diagramm im Feld R  (Le Bas et al., 1986; Le Maitre et al., 2005).</skos:definition>
	<skos:definition xml:lang="en">A silicic volcanic rock consisting of phenocrysts of quartz and alkali feldspar, often with plagioclase and biotite, in a glassy groundmass having the chemical composition of granite. Defined modally in QAPF-field 3.  Bulk rock composition plotting in field R of the TAS-diagram (Le Bas et al., 1986; Le Maitre et al., 2005).</skos:definition>
</rdf:Description>

<rdf:Description rdf:about="https://resource.geosphere.at/thes/lith/62">
	<dcterms:modified rdf:datatype="http://www.w3.org/2001/XMLSchema#dateTime">2025-09-30T13:24:15.919Z</dcterms:modified>
</rdf:Description>

<rdf:Description rdf:about="https://resource.geosphere.at/thes/lith/70">
	<dcterms:modified rdf:datatype="http://www.w3.org/2001/XMLSchema#dateTime">2025-09-30T13:24:48.836Z</dcterms:modified>
</rdf:Description>

<rdf:Description rdf:about="https://resource.geosphere.at/thes/lith/71">
	<dcterms:references rdf:resource="https://resource.geosphere.at/thes/citation/901"/>
	<dcterms:modified rdf:datatype="http://www.w3.org/2001/XMLSchema#dateTime">2025-09-30T13:25:15.467Z</dcterms:modified>
</rdf:Description>

<rdf:Description rdf:about="https://resource.geosphere.at/thes/lith/68">
	<dcterms:references rdf:resource="https://resource.geosphere.at/thes/citation/665"/>
	<dcterms:modified rdf:datatype="http://www.w3.org/2001/XMLSchema#dateTime">2025-09-30T13:25:54.322Z</dcterms:modified>
</rdf:Description>

<rdf:Description rdf:about="https://resource.geosphere.at/thes/lith/88">
	<dcterms:references rdf:resource="https://resource.geosphere.at/thes/citation/901"/>
	<dcterms:modified rdf:datatype="http://www.w3.org/2001/XMLSchema#dateTime">2025-09-30T13:26:08.629Z</dcterms:modified>
</rdf:Description>

<rdf:Description rdf:about="https://resource.geosphere.at/thes/lith/89">
	<dcterms:references rdf:resource="https://resource.geosphere.at/thes/citation/901"/>
	<dcterms:modified rdf:datatype="http://www.w3.org/2001/XMLSchema#dateTime">2025-09-30T13:26:52.333Z</dcterms:modified>
</rdf:Description>

<rdf:Description rdf:about="https://resource.geosphere.at/thes/lith/64">
	<dcterms:references rdf:resource="https://resource.geosphere.at/thes/citation/665"/>
	<dcterms:modified rdf:datatype="http://www.w3.org/2001/XMLSchema#dateTime">2025-09-30T13:27:11.285Z</dcterms:modified>
</rdf:Description>

<rdf:Description rdf:about="https://resource.geosphere.at/thes/lith/74">
	<dcterms:modified rdf:datatype="http://www.w3.org/2001/XMLSchema#dateTime">2025-09-30T13:28:13.891Z</dcterms:modified>
</rdf:Description>

<rdf:Description rdf:about="https://resource.geosphere.at/thes/lith/75">
	<dcterms:modified rdf:datatype="http://www.w3.org/2001/XMLSchema#dateTime">2025-09-30T13:28:16.254Z</dcterms:modified>
</rdf:Description>

<rdf:Description rdf:about="https://resource.geosphere.at/thes/lith/81">
	<dcterms:modified rdf:datatype="http://www.w3.org/2001/XMLSchema#dateTime">2025-09-30T13:28:18.696Z</dcterms:modified>
</rdf:Description>

<rdf:Description rdf:about="https://resource.geosphere.at/thes/lith/78">
	<dcterms:modified rdf:datatype="http://www.w3.org/2001/XMLSchema#dateTime">2025-09-30T13:28:22.206Z</dcterms:modified>
</rdf:Description>

<rdf:Description rdf:about="https://resource.geosphere.at/thes/lith/80">
	<dcterms:modified rdf:datatype="http://www.w3.org/2001/XMLSchema#dateTime">2025-09-30T13:28:25.064Z</dcterms:modified>
</rdf:Description>

<rdf:Description rdf:about="https://resource.geosphere.at/thes/lith/73">
	<dcterms:modified rdf:datatype="http://www.w3.org/2001/XMLSchema#dateTime">2025-09-30T13:28:27.595Z</dcterms:modified>
</rdf:Description>

<rdf:Description rdf:about="https://resource.geosphere.at/thes/lith/79">
	<dcterms:modified rdf:datatype="http://www.w3.org/2001/XMLSchema#dateTime">2025-09-30T13:28:30.374Z</dcterms:modified>
</rdf:Description>

<rdf:Description rdf:about="https://resource.geosphere.at/thes/lith/76">
	<dcterms:modified rdf:datatype="http://www.w3.org/2001/XMLSchema#dateTime">2025-09-30T13:28:32.982Z</dcterms:modified>
</rdf:Description>

<rdf:Description rdf:about="https://resource.geosphere.at/thes/lith/77">
	<dcterms:references rdf:resource="https://resource.geosphere.at/thes/citation/901"/>
	<dcterms:modified rdf:datatype="http://www.w3.org/2001/XMLSchema#dateTime">2025-09-30T13:28:39.236Z</dcterms:modified>
</rdf:Description>

<rdf:Description rdf:about="https://resource.geosphere.at/thes/lith/97">
	<skos:definition xml:lang="en">Material of undefined consolidation state that records the effects of one or more geologic events subsequent to the primary (sedimentary or igneous) rock-forming process. These events may include burial, heating, ductile or brittle deformation, and/or open system chemical changes (NADM SLTT Appendix B, 2004).</skos:definition>
	<skos:definition xml:lang="de">Material von unbestimmtem Konsolidierungsgrad, das die Auswirkungen eines oder mehrerer geologischer Ereignisse nach dem primären (sedimentären oder magmatischen) Gesteinsbildungsprozess zeigt. Diese umfassen Versenkung, Aufheizung, duktile oder spröde Deformation oder chemische Veränderungen in offenen Systemen (NADM SLTT Appendix B, 2004).</skos:definition>
</rdf:Description>

<rdf:Description rdf:about="https://resource.geosphere.at/thes/lith/256">
	<skos:altLabel xml:lang="de">Locker- und Festgestein</skos:altLabel>
	<skos:altLabel xml:lang="en">Unconsolidated and consolidated rock</skos:altLabel>
</rdf:Description>

<rdf:Description rdf:about="https://resource.geosphere.at/thes/lith/0">
	<skos:hasTopConcept rdf:resource="https://resource.geosphere.at/thes/lith/249"/>
</rdf:Description>

<rdf:Description rdf:about="https://resource.geosphere.at/thes/lith/249">
	<skos:topConceptOf rdf:resource="https://resource.geosphere.at/thes/lith/0"/>
</rdf:Description>

<rdf:Description rdf:about="https://resource.geosphere.at/thes/lith/0">
	<skos:hasTopConcept rdf:resource="https://resource.geosphere.at/thes/lith/1"/>
</rdf:Description>

<rdf:Description rdf:about="https://resource.geosphere.at/thes/lith/1">
	<skos:topConceptOf rdf:resource="https://resource.geosphere.at/thes/lith/0"/>
</rdf:Description>

<rdf:Description rdf:about="https://resource.geosphere.at/thes/lith/0">
	<skos:hasTopConcept rdf:resource="https://resource.geosphere.at/thes/lith/97"/>
</rdf:Description>

<rdf:Description rdf:about="https://resource.geosphere.at/thes/lith/97">
	<skos:topConceptOf rdf:resource="https://resource.geosphere.at/thes/lith/0"/>
</rdf:Description>

<rdf:Description rdf:about="https://resource.geosphere.at/thes/lith/0">
	<dcterms:description xml:lang="en">Comprises lithologiy and rock material (consolidated and unconsolidated), which are classified according to their modal composition and grain size. The classification of igneous and polygenetic (metamorphic and fault-related) rocks follows the recommendations of the IUGS subcommissions on the systematics of igneous and metamorphic rocks. Established international standards are used for sedimentary rocks. Colour code according to the INSPIRE Data Specifications for Geology (http://inspire.jrc.ec.europa.eu/).</dcterms:description>
	<dcterms:description xml:lang="de">Lithologie und Gesteinsmaterial (Locker- und Festgesteine), die nach ihrer modalen Zusammensetzung und deren Korngrößen klassifiziert werden. Die Klassifikation von magmatischen und polygenetischen Gesteinen, Metamorphiten und Störungsgesteinen ist stark an die IUGS-Empfehlungen der Subkommission für die Systematik von magmatischen Gesteinen bzw. metamorphen Gesteinen angepasst; für sedimentäre Locker- und Festgesteine wurde auf gängige internationale Standards zurückgegriffen. Farbschema entsprechend der INSPIRE Datenspezifikation für Geologie (http://inspire.jrc.ec.europa.eu/).</dcterms:description>
	<skos:hasTopConcept rdf:resource="https://resource.geosphere.at/thes/lith/158"/>
</rdf:Description>

<rdf:Description rdf:about="https://resource.geosphere.at/thes/lith/158">
	<skos:topConceptOf rdf:resource="https://resource.geosphere.at/thes/lith/0"/>
</rdf:Description>

<rdf:Description rdf:about="https://resource.geosphere.at/thes/lith/0">
	<dcterms:modified rdf:datatype="http://www.w3.org/2001/XMLSchema#dateTime">2025-09-30T14:49:59.039Z</dcterms:modified>
</rdf:Description>

<rdf:Description rdf:about="https://resource.geosphere.at/thes/lith/249">
	<dcterms:modified rdf:datatype="http://www.w3.org/2001/XMLSchema#dateTime">2025-09-30T14:50:12.294Z</dcterms:modified>
</rdf:Description>

<rdf:Description rdf:about="https://resource.geosphere.at/thes/lith/1">
	<dcterms:modified rdf:datatype="http://www.w3.org/2001/XMLSchema#dateTime">2025-09-30T14:50:20.579Z</dcterms:modified>
</rdf:Description>

<rdf:Description rdf:about="https://resource.geosphere.at/thes/lith/97">
	<dcterms:modified rdf:datatype="http://www.w3.org/2001/XMLSchema#dateTime">2025-09-30T14:50:25.498Z</dcterms:modified>
</rdf:Description>

<rdf:Description rdf:about="https://resource.geosphere.at/thes/lith/2">
	<dcterms:modified rdf:datatype="http://www.w3.org/2001/XMLSchema#dateTime">2025-10-06T13:03:40.552Z</dcterms:modified>
</rdf:Description>

<rdf:Description rdf:about="https://resource.geosphere.at/thes/lith/4">
	<dcterms:modified rdf:datatype="http://www.w3.org/2001/XMLSchema#dateTime">2025-10-06T13:05:41.816Z</dcterms:modified>
</rdf:Description>

<rdf:Description rdf:about="https://resource.geosphere.at/thes/lith/237">
	<skos:prefLabel xml:lang="de">Kieselgur</skos:prefLabel>
	<skos:altLabel xml:lang="de">Kieselschlamm</skos:altLabel>
	<skos:prefLabel xml:lang="en">Kieselguhr</skos:prefLabel>
	<skos:altLabel xml:lang="en">Siliceous ooze</skos:altLabel>
</rdf:Description>

<rdf:Description rdf:about="https://resource.geosphere.at/thes/lith/163">
	<skos:narrower rdf:resource="https://resource.geosphere.at/thes/lith/209"/>
</rdf:Description>

<rdf:Description rdf:about="https://resource.geosphere.at/thes/lith/209">
	<skos:broader rdf:resource="https://resource.geosphere.at/thes/lith/163"/>
	<dcterms:modified rdf:datatype="http://www.w3.org/2001/XMLSchema#dateTime">2025-10-06T13:23:44.510Z</dcterms:modified>
</rdf:Description>

<rdf:Description rdf:about="https://resource.geosphere.at/thes/lith/168">
	<skos:prefLabel xml:lang="en">Chemical and biochemical sediment</skos:prefLabel>
</rdf:Description>

<rdf:Description rdf:about="https://resource.geosphere.at/thes/lith/298">
	<skos:broader rdf:resource="https://resource.geosphere.at/thes/lith/160"/>
	<rdf:type rdf:resource="http://www.w3.org/2004/02/skos/core#Concept"/>
</rdf:Description>

<rdf:Description rdf:about="https://resource.geosphere.at/thes/lith/160">
	<skos:narrower rdf:resource="https://resource.geosphere.at/thes/lith/298"/>
</rdf:Description>

<rdf:Description rdf:about="https://resource.geosphere.at/thes/lith/298">
	<dcterms:created rdf:datatype="http://www.w3.org/2001/XMLSchema#dateTime">2025-10-06T13:46:25.680Z</dcterms:created>
	<skos:prefLabel xml:lang="de">Kieseliges Sediment</skos:prefLabel>
	<skos:prefLabel xml:lang="en">Siliceous sediment</skos:prefLabel>
	<skos:scopeNote xml:lang="de">Standard</skos:scopeNote>
	<skos:definition xml:lang="de">Sediment, das aus kieseligen Hartteilen von marinen oder nicht-marinen Organismen oder aus anorganischen kieselsäurehaltigen Ausfällungen besteht (verändert nach Füchtbauer &amp; Valeton, 1988; Neuendorf et al., 2005).</skos:definition>
	<skos:definition xml:lang="en">Sediment composed of siliceous skeletal parts of marine or non-marine siliceous organisms or inorganic siliceous precipitates (modified from Füchtbauer &amp; Valeton, 1988; Neuendorf et al., 2005).</skos:definition>
</rdf:Description>

<rdf:Description rdf:about="https://resource.geosphere.at/thes/lith/165">
	<dcterms:modified rdf:datatype="http://www.w3.org/2001/XMLSchema#dateTime">2025-10-06T13:51:39.902Z</dcterms:modified>
</rdf:Description>

<rdf:Description rdf:about="https://resource.geosphere.at/thes/lith/168">
	<skos:narrower rdf:resource="https://resource.geosphere.at/thes/lith/170"/>
</rdf:Description>

<rdf:Description rdf:about="https://resource.geosphere.at/thes/lith/170">
	<skos:broader rdf:resource="https://resource.geosphere.at/thes/lith/168"/>
	<dcterms:modified rdf:datatype="http://www.w3.org/2001/XMLSchema#dateTime">2025-10-06T13:52:17.800Z</dcterms:modified>
</rdf:Description>

<rdf:Description rdf:about="https://resource.geosphere.at/thes/lith/237">
	<skos:broader rdf:resource="https://resource.geosphere.at/thes/lith/298"/>
</rdf:Description>

<rdf:Description rdf:about="https://resource.geosphere.at/thes/lith/298">
	<skos:narrower rdf:resource="https://resource.geosphere.at/thes/lith/237"/>
</rdf:Description>

<rdf:Description rdf:about="https://resource.geosphere.at/thes/lith/158">
	<skos:scopeNote xml:lang="de">Standard</skos:scopeNote>
	<dcterms:modified rdf:datatype="http://www.w3.org/2001/XMLSchema#dateTime">2025-10-06T13:53:38.622Z</dcterms:modified>
</rdf:Description>

<rdf:Description rdf:about="https://resource.geosphere.at/thes/lith/160">
	<skos:scopeNote xml:lang="de">Standard</skos:scopeNote>
	<dcterms:modified rdf:datatype="http://www.w3.org/2001/XMLSchema#dateTime">2025-10-06T13:53:57.082Z</dcterms:modified>
</rdf:Description>

<rdf:Description rdf:about="https://resource.geosphere.at/thes/lith/163">
	<dcterms:modified rdf:datatype="http://www.w3.org/2001/XMLSchema#dateTime">2025-10-06T13:54:28.836Z</dcterms:modified>
</rdf:Description>

<rdf:Description rdf:about="https://resource.geosphere.at/thes/lith/168">
	<skos:scopeNote xml:lang="de">Standard</skos:scopeNote>
	<dcterms:modified rdf:datatype="http://www.w3.org/2001/XMLSchema#dateTime">2025-10-06T13:55:22.826Z</dcterms:modified>
</rdf:Description>

<rdf:Description rdf:about="https://resource.geosphere.at/thes/lith/298">
	<dcterms:references rdf:resource="https://resource.geosphere.at/thes/citation/545"/>
	<dcterms:modified rdf:datatype="http://www.w3.org/2001/XMLSchema#dateTime">2025-10-06T13:57:01.186Z</dcterms:modified>
</rdf:Description>

<rdf:Description rdf:about="https://resource.geosphere.at/thes/lith/232">
	<dcterms:modified rdf:datatype="http://www.w3.org/2001/XMLSchema#dateTime">2025-10-06T14:21:10.189Z</dcterms:modified>
</rdf:Description>

<rdf:Description rdf:about="https://resource.geosphere.at/thes/lith/230">
	<skos:broader rdf:resource="https://resource.geosphere.at/thes/lith/232"/>
</rdf:Description>

<rdf:Description rdf:about="https://resource.geosphere.at/thes/lith/232">
	<skos:narrower rdf:resource="https://resource.geosphere.at/thes/lith/230"/>
</rdf:Description>

<rdf:Description rdf:about="https://resource.geosphere.at/thes/lith/218">
	<skos:narrower rdf:resource="https://resource.geosphere.at/thes/lith/234"/>
</rdf:Description>

<rdf:Description rdf:about="https://resource.geosphere.at/thes/lith/234">
	<skos:broader rdf:resource="https://resource.geosphere.at/thes/lith/218"/>
	<dcterms:modified rdf:datatype="http://www.w3.org/2001/XMLSchema#dateTime">2025-10-06T14:22:09.623Z</dcterms:modified>
</rdf:Description>

<rdf:Description rdf:about="https://resource.geosphere.at/thes/lith/299">
	<rdf:type rdf:resource="http://www.w3.org/2004/02/skos/core#Concept"/>
	<skos:broader rdf:resource="https://resource.geosphere.at/thes/lith/166"/>
	<dcterms:created rdf:datatype="http://www.w3.org/2001/XMLSchema#dateTime">2025-10-06T14:11:42.860Z</dcterms:created>
	<skos:prefLabel xml:lang="de">Großblöcke</skos:prefLabel>
</rdf:Description>

<rdf:Description rdf:about="https://resource.geosphere.at/thes/lith/166">
	<skos:narrower rdf:resource="https://resource.geosphere.at/thes/lith/299"/>
</rdf:Description>

<rdf:Description rdf:about="https://resource.geosphere.at/thes/lith/299">
	<skos:prefLabel xml:lang="en">Large boulder</skos:prefLabel>
	<skos:notation>Standard</skos:notation>
	<skos:definition xml:lang="de">Klastisches Sediment, bei dem die Kornfraktion größer als 630 mm den größten Massenanteil bildet und der Feinkornanteil (Ton, Silt) das bodenmechanische Verhalten des Sediments nicht prägt. (Linner et al., 2024 und Referenzen darin)</skos:definition>
	<skos:definition xml:lang="en">Clastic sediment composed of components with a grain size larger than 630 mm, which make up the largest portion by weight of the sediment.  Furthermore, the fine grained portion (clay, silt) must not affect the soil mechanical characteristics of the sediment. (Linner et al., 2024; and references therein)</skos:definition>
	<dcterms:references rdf:resource="https://resource.geosphere.at/thes/citation/593"/>
</rdf:Description>

<rdf:Description rdf:about="https://resource.geosphere.at/thes/lith/237">
	<skos:scopeNote xml:lang="de">Standard</skos:scopeNote>
	<dcterms:modified rdf:datatype="http://www.w3.org/2001/XMLSchema#dateTime">2025-10-06T14:19:14.468Z</dcterms:modified>
</rdf:Description>

<rdf:Description rdf:about="https://resource.geosphere.at/thes/lith/166">
	<skos:scopeNote xml:lang="de">Standard</skos:scopeNote>
</rdf:Description>

<rdf:Description rdf:about="https://resource.geosphere.at/thes/lith/228">
	<skos:scopeNote xml:lang="de">Standard</skos:scopeNote>
	<dcterms:modified rdf:datatype="http://www.w3.org/2001/XMLSchema#dateTime">2025-10-06T14:19:51.847Z</dcterms:modified>
</rdf:Description>

<rdf:Description rdf:about="https://resource.geosphere.at/thes/lith/229">
	<dcterms:modified rdf:datatype="http://www.w3.org/2001/XMLSchema#dateTime">2025-10-06T14:19:58.146Z</dcterms:modified>
	<skos:scopeNote xml:lang="de">Standard</skos:scopeNote>
</rdf:Description>

<rdf:Description rdf:about="https://resource.geosphere.at/thes/lith/299">
	<skos:scopeNote xml:lang="de">Standard</skos:scopeNote>
	<dcterms:modified rdf:datatype="http://www.w3.org/2001/XMLSchema#dateTime">2025-10-06T14:20:03.276Z</dcterms:modified>
</rdf:Description>

<rdf:Description rdf:about="https://resource.geosphere.at/thes/lith/222">
	<skos:scopeNote xml:lang="de">Standard</skos:scopeNote>
</rdf:Description>

<rdf:Description rdf:about="https://resource.geosphere.at/thes/lith/240">
	<dcterms:modified rdf:datatype="http://www.w3.org/2001/XMLSchema#dateTime">2025-10-06T14:20:21.989Z</dcterms:modified>
	<skos:scopeNote xml:lang="de">Standard</skos:scopeNote>
</rdf:Description>

<rdf:Description rdf:about="https://resource.geosphere.at/thes/lith/225">
	<skos:scopeNote xml:lang="de">Standard</skos:scopeNote>
	<dcterms:modified rdf:datatype="http://www.w3.org/2001/XMLSchema#dateTime">2025-10-06T14:20:32.760Z</dcterms:modified>
</rdf:Description>

<rdf:Description rdf:about="https://resource.geosphere.at/thes/lith/223">
	<skos:scopeNote xml:lang="de">Standard</skos:scopeNote>
	<dcterms:modified rdf:datatype="http://www.w3.org/2001/XMLSchema#dateTime">2025-10-06T14:20:37.438Z</dcterms:modified>
</rdf:Description>

<rdf:Description rdf:about="https://resource.geosphere.at/thes/lith/224">
	<skos:scopeNote xml:lang="de">Standard</skos:scopeNote>
	<dcterms:modified rdf:datatype="http://www.w3.org/2001/XMLSchema#dateTime">2025-10-06T14:20:42.044Z</dcterms:modified>
</rdf:Description>

<rdf:Description rdf:about="https://resource.geosphere.at/thes/lith/232">
	<skos:scopeNote xml:lang="de">Standard</skos:scopeNote>
</rdf:Description>

<rdf:Description rdf:about="https://resource.geosphere.at/thes/lith/230">
	<skos:scopeNote xml:lang="de">Standard</skos:scopeNote>
	<dcterms:modified rdf:datatype="http://www.w3.org/2001/XMLSchema#dateTime">2025-10-06T14:21:16.839Z</dcterms:modified>
</rdf:Description>

<rdf:Description rdf:about="https://resource.geosphere.at/thes/lith/233">
	<skos:scopeNote xml:lang="de">Standard</skos:scopeNote>
	<dcterms:modified rdf:datatype="http://www.w3.org/2001/XMLSchema#dateTime">2025-10-06T14:21:22.269Z</dcterms:modified>
</rdf:Description>

<rdf:Description rdf:about="https://resource.geosphere.at/thes/lith/231">
	<skos:scopeNote xml:lang="de">Standard</skos:scopeNote>
	<dcterms:modified rdf:datatype="http://www.w3.org/2001/XMLSchema#dateTime">2025-10-06T14:21:27.391Z</dcterms:modified>
</rdf:Description>

<rdf:Description rdf:about="https://resource.geosphere.at/thes/lith/218">
	<skos:scopeNote xml:lang="de">Standard</skos:scopeNote>
	<dcterms:modified rdf:datatype="http://www.w3.org/2001/XMLSchema#dateTime">2025-10-06T14:21:54.568Z</dcterms:modified>
</rdf:Description>

<rdf:Description rdf:about="https://resource.geosphere.at/thes/lith/221">
	<dcterms:modified rdf:datatype="http://www.w3.org/2001/XMLSchema#dateTime">2025-10-06T14:21:59.870Z</dcterms:modified>
	<skos:scopeNote xml:lang="de">Standard</skos:scopeNote>
</rdf:Description>

<rdf:Description rdf:about="https://resource.geosphere.at/thes/lith/219">
	<skos:scopeNote xml:lang="de">Standard</skos:scopeNote>
	<dcterms:modified rdf:datatype="http://www.w3.org/2001/XMLSchema#dateTime">2025-10-06T14:22:04.247Z</dcterms:modified>
</rdf:Description>

<rdf:Description rdf:about="https://resource.geosphere.at/thes/lith/234">
	<skos:scopeNote xml:lang="de">Standard</skos:scopeNote>
</rdf:Description>

<rdf:Description rdf:about="https://resource.geosphere.at/thes/lith/220">
	<skos:scopeNote xml:lang="de">Standard</skos:scopeNote>
	<dcterms:modified rdf:datatype="http://www.w3.org/2001/XMLSchema#dateTime">2025-10-06T14:22:14.542Z</dcterms:modified>
</rdf:Description>

<rdf:Description rdf:about="https://resource.geosphere.at/thes/lith/226">
	<skos:scopeNote xml:lang="de">Standard</skos:scopeNote>
	<dcterms:modified rdf:datatype="http://www.w3.org/2001/XMLSchema#dateTime">2025-10-06T14:22:36.190Z</dcterms:modified>
</rdf:Description>

<rdf:Description rdf:about="https://resource.geosphere.at/thes/lith/214">
	<dcterms:modified rdf:datatype="http://www.w3.org/2001/XMLSchema#dateTime">2025-10-06T14:23:45.272Z</dcterms:modified>
	<skos:scopeNote xml:lang="de">Standard</skos:scopeNote>
</rdf:Description>

<rdf:Description rdf:about="https://resource.geosphere.at/thes/lith/217">
	<dcterms:modified rdf:datatype="http://www.w3.org/2001/XMLSchema#dateTime">2025-10-06T14:23:51.059Z</dcterms:modified>
	<skos:scopeNote xml:lang="de">Standard</skos:scopeNote>
</rdf:Description>

<rdf:Description rdf:about="https://resource.geosphere.at/thes/lith/215">
	<skos:scopeNote xml:lang="de">Standard</skos:scopeNote>
	<dcterms:modified rdf:datatype="http://www.w3.org/2001/XMLSchema#dateTime">2025-10-06T14:23:55.625Z</dcterms:modified>
</rdf:Description>

<rdf:Description rdf:about="https://resource.geosphere.at/thes/lith/216">
	<skos:scopeNote xml:lang="de">Standard</skos:scopeNote>
	<dcterms:modified rdf:datatype="http://www.w3.org/2001/XMLSchema#dateTime">2025-10-06T14:24:00.997Z</dcterms:modified>
</rdf:Description>

<rdf:Description rdf:about="https://resource.geosphere.at/thes/lith/227">
	<skos:scopeNote xml:lang="de">Standard</skos:scopeNote>
	<dcterms:modified rdf:datatype="http://www.w3.org/2001/XMLSchema#dateTime">2025-10-06T14:24:43.117Z</dcterms:modified>
</rdf:Description>

<rdf:Description rdf:about="https://resource.geosphere.at/thes/lith/213">
	<dcterms:modified rdf:datatype="http://www.w3.org/2001/XMLSchema#dateTime">2025-10-06T14:25:25.361Z</dcterms:modified>
	<skos:scopeNote xml:lang="de">Standard</skos:scopeNote>
</rdf:Description>

<rdf:Description rdf:about="https://resource.geosphere.at/thes/lith/300">
	<skos:prefLabel xml:lang="de">Schotter</skos:prefLabel>
	<rdf:type rdf:resource="http://www.w3.org/2004/02/skos/core#Concept"/>
	<skos:broader rdf:resource="https://resource.geosphere.at/thes/lith/166"/>
</rdf:Description>

<rdf:Description rdf:about="https://resource.geosphere.at/thes/lith/166">
	<skos:narrower rdf:resource="https://resource.geosphere.at/thes/lith/300"/>
</rdf:Description>

<rdf:Description rdf:about="https://resource.geosphere.at/thes/lith/300">
	<dcterms:created rdf:datatype="http://www.w3.org/2001/XMLSchema#dateTime">2025-11-04T10:18:43.701Z</dcterms:created>
</rdf:Description>

<rdf:Description rdf:about="https://resource.geosphere.at/thes/lith/222">
	<dcterms:modified rdf:datatype="http://www.w3.org/2001/XMLSchema#dateTime">2025-11-04T10:18:54.044Z</dcterms:modified>
</rdf:Description>

<rdf:Description rdf:about="https://resource.geosphere.at/thes/lith/300">
	<skos:prefLabel xml:lang="en">Rounded gravel and pebble</skos:prefLabel>
	<skos:definition xml:lang="de">Schlecht sortiertes klastisches Sediment, welches zu mehr als 50 Gew.-% aus gerundeten Gesteins- oder Mineralbruchstücken (Geröllen) besteht und der überwiegende Anteil der Komponenten eine Korngröße von über 2 mm aufweist. (Linner et al., 2024, S. 123, und darin zitierte Quellen)</skos:definition>
	<dcterms:references rdf:resource="https://resource.geosphere.at/thes/citation/593"/>
</rdf:Description>

<rdf:Description rdf:about="https://resource.geosphere.at/thes/lith/169">
	<skos:prefLabel xml:lang="de">Kohlenstoffreiches Sediment</skos:prefLabel>
	<skos:prefLabel xml:lang="en">Carbon-rich sediment</skos:prefLabel>
	<skos:altLabel xml:lang="de">Organisches Sediment</skos:altLabel>
	<skos:definition xml:lang="de">Nicht- bis moderat konsolidiertes Sediment, das einen signifikanten Anteil an organischem Material enthält, der sich merklich auf die lithologischen Eigenschaften auswirkt. Das organische Material setzt sich überwiegend aus Kohlenstoffverbindungen zusammen, die primär aus Organismenresten abgeleitet und noch als solche erkennbar sind.</skos:definition>
	<skos:definition xml:lang="en">Uconsolidated to moderately consolidated sediment, which contains a significant amount of organic material that noticeably affects lithologic properties. The organic material is predominantly composed of carbon compounds that are primarily derived from still recognizable organism remains.</skos:definition>
</rdf:Description>

<rdf:Description rdf:about="https://resource.geosphere.at/thes/lith/300">
	<skos:definition xml:lang="en">A poorly sorted clastic sediment, which consists of more than 50 % by weight rounded rock or mineral fragments (pebbles) and the majority of components exhibit a grain size of more than 2 mm. (Linner et al., 2024, p. 123, and references therein)</skos:definition>
</rdf:Description>

<rdf:Description rdf:about="https://resource.geosphere.at/thes/lith/169">
	<dcterms:references rdf:resource="https://resource.geosphere.at/thes/citation/593"/>
</rdf:Description>

<rdf:Description rdf:about="https://resource.geosphere.at/thes/lith/301">
	<skos:prefLabel xml:lang="de">Gyttja</skos:prefLabel>
</rdf:Description>

<rdf:Description rdf:about="https://resource.geosphere.at/thes/lith/169">
	<skos:narrower rdf:resource="https://resource.geosphere.at/thes/lith/301"/>
</rdf:Description>

<rdf:Description rdf:about="https://resource.geosphere.at/thes/lith/301">
	<dcterms:created rdf:datatype="http://www.w3.org/2001/XMLSchema#dateTime">2025-11-04T10:41:45.440Z</dcterms:created>
	<skos:broader rdf:resource="https://resource.geosphere.at/thes/lith/169"/>
	<rdf:type rdf:resource="http://www.w3.org/2004/02/skos/core#Concept"/>
	<skos:prefLabel xml:lang="en">Gyttja</skos:prefLabel>
</rdf:Description>

<rdf:Description rdf:about="https://resource.geosphere.at/thes/lith/169">
	<skos:scopeNote xml:lang="de">Standard</skos:scopeNote>
	<dcterms:modified rdf:datatype="http://www.w3.org/2001/XMLSchema#dateTime">2025-11-04T10:42:05.652Z</dcterms:modified>
</rdf:Description>

<rdf:Description rdf:about="https://resource.geosphere.at/thes/lith/300">
	<skos:scopeNote xml:lang="de">Standard</skos:scopeNote>
	<dcterms:modified rdf:datatype="http://www.w3.org/2001/XMLSchema#dateTime">2025-11-04T10:42:14.650Z</dcterms:modified>
</rdf:Description>

<rdf:Description rdf:about="https://resource.geosphere.at/thes/lith/301">
	<skos:scopeNote xml:lang="de">Standard</skos:scopeNote>
</rdf:Description>

<rdf:Description rdf:about="https://resource.geosphere.at/thes/lith/239">
	<skos:scopeNote xml:lang="de">Standard</skos:scopeNote>
	<dcterms:modified rdf:datatype="http://www.w3.org/2001/XMLSchema#dateTime">2025-11-04T10:42:56.074Z</dcterms:modified>
</rdf:Description>

<rdf:Description rdf:about="https://resource.geosphere.at/thes/lith/238">
	<skos:scopeNote xml:lang="de">Standard</skos:scopeNote>
	<dcterms:modified rdf:datatype="http://www.w3.org/2001/XMLSchema#dateTime">2025-11-04T10:43:09.225Z</dcterms:modified>
</rdf:Description>

<rdf:Description rdf:about="https://resource.geosphere.at/thes/lith/301">
	<skos:definition xml:lang="de">Grauschlamm, kalkig-toniger, organogener, meist grünlich-grauer Halbfaulschlamm am Boden nährstoffreicher Seen und brackischer Meeresgebiete. Er entsteht bei eingeschränkter Sauerstoffzufuhr und untergeordneter Beteiligung von Bodenorganismen. Aus dem schwedischen Wort jüttja: Schlamm, Schlick. (Linner et al., 2024, S. 126, und darin zitierte Quellen)</skos:definition>
	<skos:definition xml:lang="en">Gray mud, calcareous-clayey, organogenic, usually greenish-gray semifouling mud at the bottom of nutrient-rich lakes and brackish marine areas. It is formed under limited oxygen supply and subordinate participation of bottom organisms. From the Swedish word jüttja: mud. (Linner et al., 2024, p.126, and references therein)</skos:definition>
</rdf:Description>

<rdf:Description rdf:about="https://resource.geosphere.at/thes/lith/161">
	<dcterms:modified rdf:datatype="http://www.w3.org/2001/XMLSchema#dateTime">2025-11-04T10:48:19.837Z</dcterms:modified>
</rdf:Description>

<rdf:Description rdf:about="https://resource.geosphere.at/thes/lith/166">
	<dcterms:modified rdf:datatype="http://www.w3.org/2001/XMLSchema#dateTime">2025-11-04T10:48:19.836Z</dcterms:modified>
</rdf:Description>

<rdf:Description rdf:about="https://resource.geosphere.at/thes/lith/301">
	<dcterms:modified rdf:datatype="http://www.w3.org/2001/XMLSchema#dateTime">2025-11-04T11:56:51.072Z</dcterms:modified>
	<dcterms:references rdf:resource="https://resource.geosphere.at/thes/citation/593"/>
</rdf:Description>

</rdf:RDF>